\solution{\ref{problemintx^ne^xdx}

\[
\begin{array}{rcl}
\displaystyle\int x^n e^x \diff x &=& \displaystyle \int x^n \diff e^x\\
&=&\displaystyle  x^n e^x- \int  e^x \diff x^n\\
&=&\displaystyle  x^n e^x- n\int  x^{n-1}e^x \diff x\\
&=&\displaystyle x^ne^x- n\left(\int x^{n-1}\diff e^x \right)\\
&=&\displaystyle  x^ne^x - n\left(x^{n-1}e^x- \int (n-1)x^{n-2}e^x \diff x \right) \\
&=&\displaystyle x^{n}e^x-nx^{n-1}xe^x+n(n-1)\int x^{n-2}e^x \diff x \\
&=&\dots \text{(continue above process)}\dots\\
&=&\displaystyle x^ne^{x}- nx^{n-1}e^x + n(n-1 )x^{n-2 } e^x + \dots \\
&&\displaystyle +(-1)^kn(n-1)(n-2)\dots(n-k+1)x^{n-k}e^x\\
&&+\dots +(-1)^n n! e^x+C\\
&=&\displaystyle C+\sum_{k=0}^{n} (-1)^n\frac{n!}{(n-k)!} x^{n-k} e^x \quad .
\end{array}
\]
}