\solution{\ref{problemIntegratex*sin(x)dx}. 
\[
\begin{array}{rcl}
\displaystyle\int x \underbrace{\sin x \diff x}_{=\diff(-\cos x)} = -\int x \diff(\cos x) = -x\cos x + \int \cos x \diff x = -x \cos x +\sin x +C\quad .
\end{array}
\]
}

\solution{\ref{problemIntegratex^2e^xdx}.
\[
\begin{array}{rcl}
\displaystyle\int x^2 \underbrace{e^x \diff x}_{\diff  (e^x)} &=&\displaystyle \int x^2 \diff e^x= x^2e^x - \int e^x2x\diff x=  x^2e^x - \int 2x\diff e^x \\
&=&\displaystyle x^2e^x- 2xe^x+ \int 2e^x \diff x= x^2e^x-2xe^x+2e^x+C\quad .
\end{array}
\]
}

\solution{\ref{problemintx^2e^(-2x)dx}.
\[
\begin{array}{rcll|l}
\displaystyle \int x^2 e^{-2x}\diff x&=&\displaystyle \int x^2 \diff \left( \frac{e^{-2x}}{-2}\right)&&\text{Integrate by parts}\\
&=&\displaystyle -\frac{x^2e^{-2x}}{2}-\int \left(\frac{ e^{-2 x}}{ -2} \right) \diff \left(x^2\right)\\
&=&\displaystyle -\frac{x^2e^{-2x}}{2}+ \int xe^{-2x}\diff x\\
&=&\displaystyle  -\frac{x^2e^{-2x}}{2}+ \int x \diff \left( \frac{e^{ -2 x}}{ -2}\right)&&\text{Integrate by parts}\\
&=&\displaystyle  -\frac{x^2e^{-2x}}{2}-\frac{xe^{-2x}}{2}+ \frac{1}{2} \int e^{ -2x} \diff x\\
&=&\displaystyle -\frac{x^2e^{-2x}}{2}-\frac{xe^{-2x}}{2}- \frac{ e^{-2x }}{ 4}+C\quad .
\end{array}
\]
}