\solution{\ref{problemintxtan^2xdx}
\[
\begin{array}{rcll|l}
\displaystyle\int x \tan^2 x \diff x &=&\displaystyle\int x\left(\sec^2 x-1 \right)\diff x &&\text{use }\sec^2x-1=\tan^2 x\\
&=&\displaystyle\int x\left(\sec^2 x-1 \right)\diff x \\
&=&\displaystyle - \int x\diff x+\int x\sec^2x\diff x&&\text{use }\diff (\tan x)= \sec^2x\diff x\\
&=&\displaystyle - \frac{x^2}{2} +\int x\diff (\tan x)&&\text{integrate by parts}\\
&=&\displaystyle-\frac{x^2}{2} +x\tan x - \int \tan x \diff x \\
&=&\displaystyle-\frac{x^2}{2} +x\tan x - \int \frac{\sin x}{\cos x}\diff x &&\text{use }\sin x\diff x=-\diff (\cos x)\\
&=&\displaystyle -\frac{x^2}{2}+x\tan x+ \int \frac{\diff (\cos x)}{\cos x} &&\text{Set }y=\cos x \\
&=&\displaystyle-\frac{x^2}{2}+x\tan x + \int \frac{1}{y}\diff y\\
&=&\displaystyle-\frac{x^2}{2}+x\tan x + \ln |y|+C&&\text{Substitute back } y=\cos x\\
&=&\displaystyle -\frac{x^2}{2}+x\tan x + \ln |\cos x|+C\quad .

\end{array}
\]

}

\solution{\ref{problemint(e^(-sqrtx)dx)}
\[
\begin{array}{rcll|l}
\displaystyle \int e^{-\sqrt{x}}\diff x&=& \displaystyle \int 2y e^{-y}\diff y&&\text{Subst.: } \begin{array}{rcl} \sqrt{x}&=&y\\
\frac{1}{2\sqrt{x}}\diff x&=&\diff y\\
\diff x&=&2y\diff y
\end{array}
\\
&=&\displaystyle \int 2y \diff \left(-e^{-y}\right) &&\text{int. by parts}\\
&=&-2ye^{-y}+2\int e^{-y}\diff y\\
&=&-2ye^{-y}-2e^{-y}+C\\
&=&-2\sqrt{x}e^{-\sqrt{x}} -2e^{-\sqrt{x}}+C\quad .
\end{array}
\]
}

\solution{\ref{problemintcos^2xdxviaIntByParts}. Later, we shall study general methods for solving trigonometric integrals that will cover this example. Let us however show one way to solve this integral by integration by parts. 
\[
\begin{array}{rcll|l}
\displaystyle \int \cos^2 x \diff x&=&\displaystyle x\cos^2x - \int x\diff (\cos^2 x)\\
&=&\displaystyle x\cos^2 x - \int x2\cos x (-\sin x)\diff x&&\text{Use } \sin (2x)=2\sin x \cos x\\
&=&\displaystyle x \cos^2x +\int x\sin (2x)\diff x\\
&=&\displaystyle x \cos^2x +\int x \diff \left(\frac{-\cos (2x)}{2}\right)\\
&=&\displaystyle x \cos^2x +x\left(\frac{-\cos (2x)}{2}\right) -\int \left(\frac{-\cos (2x)}{2}\right)\diff x\\
&=&\displaystyle \frac{x}{2}\left(2\cos^2 x - \cos (2x)\right)+ \frac{\sin (2x)}{4}+C &&\text{use } \cos (2x)=\cos^2x-\sin^2 x \\
&=&\displaystyle \frac{x}{2}\left(2\cos^2x - (\cos^2x-\sin^2x) \right) + \frac{\sin (2x)}{4}+C&&\text{use }\cos^2x+\sin^2x=1\\
&=&\displaystyle \frac{x}{2} + \frac{\sin (2x)}{4}+C\quad .\\
\end{array}
\]
}

\solution{\ref{problemintarctanxdx}
\[
\begin{array}{rcl}
\displaystyle\int \arctan x \diff x &=& x\displaystyle \arctan x - \int x \diff(\arctan x)\\
&=&\displaystyle x\arctan x - \int \frac{x}{x^2+1}\diff x\\
&=& \displaystyle  x\arctan x - \int \frac{\frac{1}2\diff(x^2)}{x^2+1}\\
&=&\displaystyle  x\arctan x - \int \frac{\frac{1}2\diff(x^2+1)}{x^2+1}\\
&=&\displaystyle  x\arctan x - \frac12\ln (x^2+1) +C\quad .
\end{array}
\]
}

\solution{
\ref{problemintArcsinSquared}. 
\[
\begin{array}{rcll|l}
\displaystyle \int (\Arcsin x)^2 \diff x &=&\displaystyle  \int \left(\Arcsin(\sin y)\right)^2 \diff  (\sin y) &&\text{Set } x= \sin y\\
&=&\displaystyle \int y^2 \cos y \diff y =  \int y^2 \diff (\sin y)  &&\text{Integrate by parts}\\
&=&\displaystyle y^2\sin y - \int 2y\sin y  \diff y\\
&=&\displaystyle y^2\sin y + \int 2y  \diff (\cos y ) & &\text{Integrate by parts}\\
&=&\displaystyle y^2\sin y + 2y \cos y - 2\int \cos y \diff y\\
&=&\displaystyle y^2\sin y+2y \cos y - 2\sin y +C &&\text{Substitute } y=\Arcsin x\\
&=& \displaystyle x(\arcsin x)^2 \\
&&\displaystyle+2\sqrt{1-x^2}\arcsin x - 2x+C\quad .
\end{array}
\]
}

\solution{\ref{problemintsinxe^xdx}
\[
\begin{array}{rcll|l}
\displaystyle\int \sin x \underbrace{e^x \diff x}_{=\diff e^x}&=&\displaystyle\sin x e^x - \int e^x\diff (\sin x)=\sin x e^x - \int \cos x \underbrace{e^x \diff x}_{=\diff e^x}\\
&=& \displaystyle\sin x e^x - e^x\cos x +\int e^x \diff (\cos x) \\
&=& e^x\sin x -e^x\cos x-\int e^x\sin x \diff x &&
\begin{array}{l}
\text{add }\int e^x\sin x \diff x\\
\text{to both sides}
\end{array}\\
\displaystyle 2\int \sin x e^x \diff x& =&\displaystyle \sin x e^x-e^x\cos x\\
\displaystyle \int \sin x e^x \diff x&=&\displaystyle \frac{1}{2} \left(\sin x e^x- e^x\cos x\right)\quad .
\end{array}
\]
}

\solution{\ref{problemintsin(ln x)dx}.

\noindent$
\begin{array}{@{\!\!}r@{~}c@{~}ll|l}
\displaystyle \int \sin (\ln x)\diff x&=&\displaystyle  x\sin (\ln x)-\int x\diff (\sin (\ln x)) &&\text{int. by parts}\\
&=&\displaystyle  x\sin (\ln x ) - \int x \left(\cos (\ln x)\right) \left(\ln x\right)'\diff x\\
&=&\displaystyle x\sin (\ln x)-\int \cos (\ln x)\diff x &&\text{int. by parts}\\
&=&\displaystyle  x\sin (\ln x)- \left( x\cos (\ln x)-\int  x\diff (\cos (\ln x)) \right)\\
&=&\displaystyle x\sin (\ln x)-x\cos (\ln x)+\int x (-\sin (\ln x))(\ln x)'\diff x\\
&=&\displaystyle x\sin (\ln x)-x\cos (\ln x)-\int \sin (\ln x)\diff x &&\begin{array}{l}\text{add } \int \sin (\ln x)\diff x\\ \text{to both sides}\end{array}\\
\displaystyle 2\int \sin (\ln x)\diff x&=&\displaystyle  x\sin (\ln x)-x\cos (\ln x)\\
\displaystyle \int \sin (\ln x)\diff x&=&\displaystyle \frac{x}{2} \left(\sin (\ln x)-\cos (\ln x) \right)\quad .
\end{array}
$
}

\solution{\ref{problemintlnxdx}
\[
\int \ln x \diff x = x\ln x - \int x \diff (\ln x)= x\ln x -\int \frac{x}{x}\diff x= x\ln x -x+C\quad .
\]
}

\solution{\ref{problemintlnx/sqrt(x)dx}
\[
\begin{array}{rcll|l}
\displaystyle \int \frac{\ln x}{\sqrt{x}}\diff x&=&\int \ln x 2\diff \left(\sqrt{x}\right)&&\text{integrate by parts}\\
&=&\displaystyle (\ln x)2\sqrt{x}- \int 2\sqrt{x}\diff (\ln x)\\ 
&=&\displaystyle 2\sqrt{x}\ln x - 2\int \frac{\sqrt{x}}{x}\diff x\\
&=&\displaystyle 2\sqrt{x}\ln x - 2\int x^{-\frac{1}{2}}\diff x\\
&=&\displaystyle 2\sqrt{x}\ln x - 4\sqrt{x}+C\\
&=&\displaystyle 2\sqrt{x}(\ln x -2)+C\quad .
\end{array}
\]
}


