\solution{\ref{problemcos(2arctan t)}
Set $z=\Arctan t$, and so $\tan z= t$. Then
\[
\begin{array}{rcll|l}
\cos (2\Arctan t)&=&\displaystyle \cos (2z) \\
&=&\displaystyle \frac{\cos (2z)}{1}&& \begin{array}{l} \text{use double angle formulas} \\ \text{and } 1=\sin^2z +\cos^2 z\end{array} \\
&=&\displaystyle \frac{\cos^2 z- \sin^2 z}{\cos^2 z +\sin^2 z} && \text{divide top and bottom by } \cos^2z \\
&=&\displaystyle \frac{(\cos^2 z-\sin^2z)\frac{1}{\cos^2 z}}{(\sin^2 z +\cos^2z)\frac{1}{\cos^2 z}}\\
&=&\displaystyle \frac{1-\tan^2z}{1+\tan^2z}\\
&=&\displaystyle \frac{1-t^2}{1+t^2}
\quad .
\end{array}
\]
}
\solution{\ref{problemcot(2arctan t)}
Set $z=\Arctan t$, and so $\tan z= t$. Then
\[
\begin{array}{rcll|l}
\cot (2\Arctan t)&=&\displaystyle \cot (2z) \\
&=&\displaystyle \frac{\cos (2z)}{\sin (2z)}&&\text{use double angle formulas} \\
&=&\displaystyle \frac{\cos^2 z- \sin^2 z}{2\sin z \cos z}\\
&=&\displaystyle \frac{1- \tan^2 z}{2 \tan z}\\
&=&\displaystyle \frac{1-t^2}{2t}\\
&=&\displaystyle \frac{1}{2}\left(\frac{1}{t}-t\right)\quad .
\end{array}
\]
}