Let $x\in (0,1)$. Express the following using $x$ and $\sqrt{1-x^2}$.  
\begin{multicols}{2}
\begin{enumerate}
\item $\sin(\Arcsin (x))$. \answer{$x$}
\pointsii{3} $\sin(2\Arcsin (x))$. \answer{$2x\sqrt{1-x^2} $}
\item $\sin(3\Arcsin (x))$. \answer{$ -4x^3+3x $}
\item $\sin(\Arccos (x))$. \answer{$\sqrt{1-x^2} $}
\item $\sin(2\Arccos (x))$. \answer{$2x \sqrt{1-x^2 }$}
\item $\sin(3\Arccos (x))$. 
\answer{
\begin{tabular}{l}
$\left(4x^2-1\right)\sqrt{1-x^2}$ \\= $-4\left(\sqrt{1-x^2}\right)^3+3\sqrt{1-x^2} $
\end{tabular}
}
\item $\cos(2\Arcsin (x))$. \answer{$ 1-2x^2$}
\item $\cos(3\Arccos (x))$. \answer{$4x^3-3x $}
\end{enumerate}
\end{multicols}

\begin{enumerate}
\setcounter{enumii}{1}
\item  
\solution{%
Let $y = \Arcsin x$.  Then $\sin x = y$, and we can draw a right triangle with opposite side length $x$ and hypotenuse length $1$ to find the other trigonometric ratios of $y$.  

\begin{center}
\psset{xunit=1.0cm,yunit=1.0cm,algebraic=true,dotstyle=o,dotsize=3pt 0,linewidth=0.8pt,arrowsize=3pt 2,arrowinset=0.25}
\begin{pspicture*}(-3.33,-6.11)(14.05,6.58)
\psline(0,0)(4,0)
\psline(0,0)(4,3)
\psline(4,3)(4,0)
\psline(4,0.2)(3.8,0.2)
\psline(3.8,0.2)(3.8,0)
\rput[tl](0.83,0.5){$y$}
\rput[tl](1.56,1.82){$1$}
\rput[tl](4.1,1.4){$x$}
\rput[tl](1.7,-0.05){$\sqrt{1-x^2}$}
\parametricplot{0.0}{0.6435011087932844}{1*0.66*cos(t)+0*0.66*sin(t)+0|0*0.66*cos(t)+1*0.66*sin(t)+0}
\end{pspicture*}
\end{center}

Then $\cos y = \sqrt{1-x^2}/1 = \sqrt{1-x^2}$.  
Now we use the double angle formula to find $\sin(2\Arcsin x)$.  

\begin{align*}
\sin (2 \Arcsin x) & = \sin (2y) \\
& = 2\sin y\cos y \\
& = 2x\sqrt{1-x^2}.
\end{align*}
}%
\item
\solution{%
Use the result of the previous question.  
This also requires the addition formula for sine: 
\[
\sin(A+B) = \sin A \cos B + \sin B\cos A,
\]
and the double angle formula for cosine:
\[
\cos (2y) = \cos^2 y - \sin^2 y.
\]  
\begin{align*}
\sin(3\Arcsin x) & = \sin(3y) \\
& = \sin (2y + y) \\
\text{Addition formula: } \quad & = \sin(2y)\cos y + \sin y \cos (2y) \\
\text{Double angle formulas: } \quad & = (2\sin y \cos y)\cos y + \sin y (\cos^2 y - \sin^2 y) \\
& = 2\sin y \cos^2 y + \sin y \cos^2 y - \sin^3 y \\
& = 3\sin y \cos^2 y - \sin^3 y \\
& = 3x(1-x^2) - x^3 \\
& = 3x - 4x^3.
\end{align*}
}%
\end{enumerate}
