\solution{\ref{problemTangentPlanex^2+y^2-z^2=-3at(2,3,4)}
As studied in the theory, the normal to the tangent plane to a surface given by implicit equation $f=0$ is given by $\nabla f$. Since the tangent plane passes through $(2,3,4)$, this determines the tangent plane. 
\[
\begin{array}{rcll|l}
f=x^2+y^2-z^2-3&=&0&&\text{Equation of the surface}\\
\nabla f&=& (2x,2y,-2z)\\
\nabla f_{|(x,y,z)=(2,3,4)}&=&(4, 6, -8)\\
\nabla f_{|(x,y,z)=(2,3,4)}\cdot (x-2,y-3,z-4)&=&0 &&\text{Equation of plane with normal }\\
4(x-2)+6(y-3)-8(z-4)&=&0\\
2x+3y-4z&=&-3 &&\text{Final answer in simplified form.}\\
\end{array}
\]
}