% begin module substitution-rule-intro
\begin{frame}
\frametitle{The Substitution Rule}
\begin{itemize}
\item  How do we integrate $\displaystyle \int 2x \sqrt{\alertNoH{2}{1+x^2}} \ \diff x$?
\item<2->  Introduce a new variable \alertNoH{2, 3, 8, 14, 17}{$u = 1 + x^2$}.
\item<3->  Then $ \alertNoH{10,24}{\diff \alertNoH{3}{ u}} = \alertNoH{4}{\diff \left(\alertNoH{3}{ 1+x^2} \right)} \uncover<4->{\alertNoH{4}{=\alertNoH{5,6}{ \left(1+x^2 \right)'} \diff x}} \uncover<5->{ \alertNoH{10,24}{=\fcAnswer{6}{ 2x}  \diff x}. }$
\item<7->  Substitute into the integral:
\end{itemize}
\abovedisplayskip=0pt
\belowdisplayskip=0pt
\[
\uncover<7->{%
\int \alertNoH{9,10,24}{2x} \alertNoH{7,8,23}{\sqrt{1 +x^2}} \ \alertNoH{9,10,24}{\diff x}%
 = \int \fcAnswerUncover{7}{8}{ \alertNoH{22,23}{ \sqrt{u}}} \ \fcAnswerUncover{7}{10}{\alertNoH{24}{ \diff u}}}%
\uncover<11->{=\alertNoH{12,13}{\int \alertNoH{22,23}{ u^{\frac{1 }{2}}} \alertNoH{24}{\diff u}}}
\uncover<12->{\alertNoH{12,13}{ =} \fcAnswer{13}{ \alertNoH{21}{\frac{2 }{3 }{\alertNoH{14, 18}{u}}^{\frac{3}{2}}}+C} }%
\uncover<14->{= \alertNoH{16}{ \frac{2}{3 }{\alertNoH{14, 18}{\left(1+ x^2 \right)}}^{{ \frac{3}{2}}}+C} }%
\]
\begin{itemize}
\item<15->  Is this procedure justified?
\item<16->  Take the derivative \uncover<19->{\alertNoH{19}{using the Chain Rule:}}
\end{itemize}
\abovedisplayskip=0pt
\belowdisplayskip=0pt
\[
\uncover<16->{%
\alertNoH{17}{\frac{\diff}{\diff x}} \left(\alertNoH{16}{ \frac{2}{3} \left(\alertNoH{18}{ 1+x^2} \right)^{ \frac{3}{2}}+\alertNoH{17}{C}} \right)
}%
\uncover<17->{%
=\frac{\diff}{\diff x} \left(\alertNoH{21}{ \frac{2}{3}{\alertNoH{18} {u}}^{ \frac{3}{2}}} \right)
}%
\uncover<19->{%
=  \frac{\fcCancel{20}{2}}{ \fcCancel{20}{3}}\cdot \frac{\fcCancel{20}{3} }{\fcCancel{20}{2}} \alertNoH{22,23}{ u^{\frac{1}{2}}} \alertNoH{24}{\frac{\diff u}{\diff x}}%
}%
\uncover<23->{%
 = \alertNoH{23}{\sqrt{1+x^2}} (\alertNoH{24}{2x})%
}%
\]
\end{frame}
% end module substitution-rule-intro
