% begin module substitution-rule-definite-integrals
\begin{frame}
\frametitle{Definite Integrals}
There are two ways to find a definite integral with the Substitution Rule:
\vspace{-.2in}
\begin{enumerate}
\item  First evaluate the indefinite integral, then use the FTC.
\end{enumerate}
\abovedisplayskip=0pt
\belowdisplayskip=0pt
\abovedisplayshortskip=0pt
\belowdisplayshortskip=0pt
\begin{align*}
\uncover<2->{%
\int_{\alert<handout:0| 2>{0}}^{\alert<handout:0| 2>{4}} \sqrt{2x+1} \ \diff x%
}%
 & \uncover<2->{ = } %
\uncover<2->{%
\left[ \int \sqrt{2x+1} \ \diff x \right]_{\alert<handout:0| 2>{0}}^{\alert<handout:0| 2>{4}}%
}%
  \uncover<3->{ = } %
\uncover<3->{%
\left[ \frac{1}{3}(2x+1)^{3/2} \right]_{\alert<handout:0| 2>{0}}^{\alert<handout:0| 2>{4}}%
}\\%
 & \uncover<4->{ = } %
\uncover<4->{%
\frac{1}{3}(2\cdot 4 + 1)^{3/2} - \frac{1}{3}(2\cdot 0 + 1)^{3/2}%
}\\%
 & \uncover<5->{ = } %
\uncover<5->{%
\frac{1}{3}(9)^{3/2} - \frac{1}{3}(1)^{3/2}%
}%
  \uncover<5->{ = } %
\uncover<5->{%
\frac{1}{3}(27 - 1) = \frac{26}{3}%
}%
\end{align*}
\begin{enumerate}
\setcounter{enumi}{1}
\item<6->  Change the limits of integration when the variable is changed.
\end{enumerate}
\uncover<7->{%
\begin{theorem}[The Substitution Rule for Definite Integrals]
%If $g'$ is continuous on $[a,b]$ and $f$ is continuous on the range of $u = g(x)$, then
If $u = g(x)$ and $g$ and $f$ are continuous, then
\abovedisplayskip=0pt
\belowdisplayskip=0pt
\[
\int_{\alert<handout:0| 7>{a}}^{\alert<handout:0| 7>{b}} f(g(x))g'(x) \ \diff x = \int_{\alert<handout:0| 7>{g(a)}}^{\alert<handout:0| 7>{g(b)}} f(u) \ \diff u%
\]
\end{theorem}
}%
\end{frame}
% end module substitution-rule-definite-integrals
