\begin{frame}
Recall that $i^2=-1$, $\sqrt{-1}=i$.
\begin{example}[Polynomial factorizations]
$
\renewcommand{\arraystretch}{2}
\begin{array}{rcl}
2x^2+3x-5&=&(2x+5)(x-1)= 2\left(x-\left(-\frac{5 }{2}\right)\right)(x-1)\\
x^2+1&=&x^2-(-1)=x^2-i^2=(x+i)(x-i)\\
x^4-1&=&(x^2-1)(x^2+1)=(x-1)(x+1)(x^2+1)\\
&=& (x-1)(x+1)(x-i)(x+i) \\
x^4+1&=&(x^2-\sqrt{2}x+1)(x^2+\sqrt{2}x+1)\\
&=&
\left(x-\left(\frac{\sqrt{2}}{2}+\frac{\sqrt{2}}{2}i\right)\right)
\left(x-\left(-\frac{\sqrt{2}}{2}+\frac{\sqrt{2}}{2}i\right)\right)\\&&
\left(x-\left(\frac{\sqrt{2}}{2}-\frac{\sqrt{2}}{2}i\right)\right)
\left(x-\left(-\frac{\sqrt{2}}{2}-\frac{\sqrt{2}}{2}i\right)\right)
\end{array}$
\end{example}

 \end{frame}