\begin{frame}
$\begin{array}{r@{}c@{}l}
a_0 x^{n}+a_1x^{n-1}+\dots + a_n&=& a_0 (x-x_1)\dots (x-x_n)\\
&=&\text{prod. real quadratics no roots \& lin. terms.}
\end{array}
$

\begin{example}

$
\renewcommand{\arraystretch}{2}
\begin{array}{@{\!\!}r@{}c@{}l@{}l@{}|l}
2x^2+3x-5&=&(2x+5)(x-1)= 2\left(x-\left(-\frac{5 }{2}\right)\right)(x-1)&&\text{real roots} \\
x^2+1&=&x^2-(-1)=x^2-i^2=(x+i)(x-i)&&\text{complex roots}\\
x^4-1&=&(x^2-1)(x^2+1)=(x-1)(x+1)(x^2+1)\\
&=& (x-1)(x+1)(x-i)(x+i) &&\text{mixed roots}\\
x^4+1&=&(x^2-\sqrt{2}x+1)(x^2+\sqrt{2}x+1)\\
&=&
\left(x-\left(\frac{\sqrt{2}}{2}+\frac{\sqrt{2}}{2}i\right)\right)
\left(x-\left(-\frac{\sqrt{2}}{2}+\frac{\sqrt{2}}{2}i\right)\right)\\&&
\left(x-\left(\frac{\sqrt{2}}{2}-\frac{\sqrt{2}}{2}i\right)\right)
\left(x-\left(-\frac{\sqrt{2}}{2}-\frac{\sqrt{2}}{2}i\right)\right)&& \text{complex roots}
\end{array}$
\end{example}

 \end{frame}