% begin module chain-rule-ex5
\begin{frame}
\begin{example}[Chain Rule and Quotient Rule]
Find the derivative of
\abovedisplayskip=0pt
\belowdisplayskip=0pt
\abovedisplayshortskip=0pt
\belowdisplayshortskip=0pt
\begin{align*}
g(t) & = \left( \frac{t-2}{2t+1}\right)^9. \\%
&  \uncover<2->{\text{Power Rule and Chain Rule:}}\\%
\uncover<2->{%
g'(t)%
}%
& \uncover<2->{ = } %
\uncover<2->{%
9\left( \frac{t-2}{2t+1}\right)^8 \frac{\diff}{\diff t}\left( \frac{\alertNoH{ 3}{t-2}}{\alertNoH{ 4}{2t+1}}\right)%
}\\%
&  \uncover<3->{\text{Quotient Rule:}}\\%
& \uncover<3->{ = 9\left( \frac{t-2}{2t+1}\right)^8 \frac{\alertNoH{ 5-6}{\frac{\diff}{\diff t}(\alertNoH{ 3}{t-2})} \cdot (\alertNoH{ 4}{2t+1})-(\alertNoH{ 3}{t-2})\alertNoH{ 7-8}{\frac{\diff}{\diff t}(\alertNoH{ 4}{2t+1})}}{(\alertNoH{ 4}{2t+1})^2}%
}\\%
& \uncover<5->{ = 9\left( \frac{t-2}{2t+1}\right)^8 \frac{ \alertNoH{ 5-6}{\fcAnswerUncover{5}{6}{1}}\cdot (2t+1) -(t-2)\cdot \alertNoH{ 7-8}{\fcAnswerUncover{5}{8}{2}}}{(2t+1)^2}%
}\\%
& \uncover<9->{ = 9\left( \frac{t-2}{2t+1}\right)^8 \frac{\fcCancel{10}{2t}+1-\fcCancel{10}{2t}+4}{(2t+1)^2}%
}  \uncover<10->{ = \frac{45(t-2)^8}{(2t+1)^{10}}.%
}%
\end{align*}
\end{example}
\end{frame}
% end module chain-rule-ex5
