% begin module chain-rule-box-ex
\begin{frame}
\begin{example}
Differentiate $y = \sqrt{\alert<handout:0| 7>{\sin (x^2+1)}}$.
\begin{columns}[t]
\column{.3\textwidth}
\begin{itemize}
\item<2-| alert@3-4>  Last operation: \uncover<4->{square root.}
\item<2-| alert@5-7,9>  $\square = \uncover<6->{\sin (x^2+1)}$.
%\vspace{1in}
\item<10-| alert@11-12>  Last operation: \uncover<12->{sine.}
\item<10-| alert@13-15,17>  New $\square = \uncover<14->{x^2+1}$.
\end{itemize}
\column{.7\textwidth}
\abovedisplayskip=0pt
\belowdisplayskip=0pt
\begin{eqnarray*}
\uncover<7->{%
y'%
}%
& \uncover<7->{ = } &%
\uncover<7->{%
\left( \alert<handout:0| 7>{\sqrt{\square}}\right)'%
}  \uncover<8->{ = } \uncover<8->{%
\frac{1}{2\sqrt{\alert<handout:0| 9>{\square}}}\cdot \alert<handout:0| 9>{\square}'%
}\\%
& \uncover<9->{ = } &%
\uncover<9->{%
\frac{1}{2\sqrt{\alert<handout:0| 9>{\sin (x^2+1)}}}\cdot \alert<handout:0| 9-14>{(\sin \alert<handout:0| 15>{(x^2+1)})}\alert<handout:0| 10-14>{'}%
}\\%
& \uncover<15->{ = } &%
\uncover<15->{%
\frac{1}{2\sqrt{\sin (x^2+1)}}\cdot (\sin \alert<handout:0| 15>{\square})'%
}\\%
& \uncover<16->{ = } &%
\uncover<16->{%
\frac{1}{2\sqrt{\sin (x^2+1)}}\cdot (\cos\alert<handout:0| 17>{\square} )\cdot \alert<handout:0| 17>{\square}'%
}\\%
& \uncover<17->{ = } &%
\uncover<17->{%
\frac{\cos\alert<handout:0| 17>{(x^2+1)}}{2\sqrt{\sin (x^2+1)}}\cdot \alert<handout:0| 17>{(x^2+1)}'%
}\\%
& \uncover<18->{ = } &%
\uncover<18->{%
\frac{\cos (x^2+1)}{2\sqrt{\sin (x^2+1)}}\cdot 2x%
} \uncover<19->{ = \frac{x\cos (x^2+1)}{\sqrt{\sin (x^2+1)}}}%
\end{eqnarray*}
\end{columns}
\end{example}
\end{frame}
% end module chain-rule-box-ex
