% begin module chain-rule-power-rule
\begin{frame}
\begin{itemize}
\item  In the example $y = \cos^3 x$, the outer function was a power function: $y = u^3$.
\item<2->  The derivative was $\frac{\diff y}{\diff x} = 3u^2 \frac{\diff u}{\diff x} = (3\cos^2 x) (-\sin x)$.  
\item<3->  We can generalize this:
\end{itemize}

\uncover<3->{%
The Power Rule Combined with the Chain Rule

If $n$ is any real number and $u = g(x)$ is differentiable, then
\[
\frac{\diff}{\diff x} (u^n) = nu^{n-1} \frac{\diff u}{\diff x}
\]
Alternatively,
\[
\frac{\diff}{\diff x}[g(x)]^n = n [g(x)]^{n-1} \cdot g'(x)
\]
}%
\end{frame}
% end module chain-rule-power-rule
