% begin module chain-rule-statement
\begin{frame}
\begin{theorem}[Chain rule]
\alertNoH{17}{$g$-diff. near $a$}, \alertNoH{4}{$f$-diff. near $g(a)$} $\Rightarrow$ $\alertNoH{18}{ \left(f(g(a))\right)'= f'(g(a)) g'(a)}$ .
\end{theorem}
\begin{proof}
\uncover<2->{Define $Q(\alertNoH{8}{y})=\left\{\begin{array}{ll}\alertNoH{4}{\frac{f(\alertNoH{8}{y})-f(g(a))}{\alertNoH{3}{\alertNoH{8}{y}-g(a)}}, }&\alertNoH{4}{\alertNoH{3}{\alertNoH{8}{y}\neq g(a)}} \\\alertNoH{5}{f'(g(a)), } &\alertNoH{5}{\alertNoH{8}{y}=g(a)} \end{array} \right.$.} \uncover<3->{\alertNoH{3,6}{$Q(g(x))$ - defined for all $x$ near $a$.}}
\uncover<4->{Therefore $\alertNoH{4,5,16}{f'(g(a))}\alertNoH{4,5}{=\lim_{y\to a} Q(y)}\alertNoH{6}{= \alertNoH{16}{\lim_{x\to a} Q(g(x))}}$. }
~\\~\\

$\begin{array}{rcl}
\uncover<7->{\alertNoH{14}{ Q(\alertNoH{8}{g(x)})\frac{g(x)-g(a)}{x-a}} &=&}\uncover<8->{ \left\{\begin{array}{ll} \frac{\alertNoH{11}{(f(\alertNoH{8}{g(x)})-f(g(a))) }} {\alertNoH{10}{(\alertNoH{8}{g(x)}-g(a))}} \frac{\alertNoH{10}{(g(x)-g(a))}}{\alertNoH{11}{x-a}} , &\alertNoH{8}{g(x)}\neq g(a) \\ f'(\alertNoH{8}{g(a)})\frac{\alertNoH{9}{\alertNoH{8}{g(a)}-g(a)}}{x-a}\uncover<9->{\alertNoH{9}{=0}}, & \alertNoH{8}{g(x)}=g(a) \end{array} \right. }\\\uncover<10->{ &=&\alertNoH{11,14}{\frac{f(g(x))-f(a)}{x-a}.}}
\end{array}
$
~\\~\\~\\

$\begin{array}{rcl}
\uncover<12->{\alertNoH{18}{ (f \circ g)'(a)} &=&} \uncover<13->{\displaystyle\lim_{x\to a} \alertNoH{14}{\frac{f(g(x)) - f(g(a)) }{x-a}}=} \uncover<14->{\lim_{x\to a} \alertNoH{14}{Q(g(x)) \frac{g(x)-g(a)}{x-a}}}\\
\uncover<15->{&=&\alertNoH{16}{\displaystyle \lim_{x\to a} Q(g(x))}\alertNoH{17}{\lim_{x\to a} \frac{g(x)-g(a)}{x-a}}} \uncover<16->{=\alertNoH{18}{ \alertNoH{16}{f'(g(a))} \alertNoH{17}{g'(a)}}\quad .}
\end{array}
$
\end{proof}
\end{frame}
% end module chain-rule-statement
