% begin module chain-rule-ex6
\begin{frame}
\begin{example}
Find the derivative of $y =\alertNoH{2}{(2x+1)^5}\alertNoH{3}{(x^3- x+1)^4}$.
$
\renewcommand{\arraystretch}{1.5}
\begin{array}{@{}r@{}cl}
&&  \uncover<2->{\text{Product Rule:}}\\%
\uncover<2->{y'& =&\displaystyle  \alertNoH{ 4-5}{\frac{\diff}{\diff x}\left(\alertNoH{2}{(2x+1)^5}\right)}\alertNoH{3}{(x^3-x+1)^4} +\alertNoH{2}{(2x+1)^5} \alertNoH{ 6-7}{\frac{\diff}{\diff x} \left(\alertNoH{3}{(x^3-x+1)^4} \right)}%
}\\%
&&  \uncover<4->{\text{Chain Rule:}}\\%
\uncover<4->{ &  = &\displaystyle 
\alertNoH{ 4-5}{\left(\fcAnswerUncover{4}{5}{5(2x+1)^4\alertNoH{ 10-11}{\frac{\diff}{\diff x}(2x+1)}}\right)} (x^3-x+1)^4%
}\\%
& &\displaystyle 
\uncover<4->{
+(2x+1)^5\alertNoH{ 6-7}{\left(\fcAnswerUncover{4}{7}{4 (x^3-x+1)^3 \alertNoH{ 8-9}{ \frac{\diff}{\diff x}(x^3-x+1)}}\right)}%
}\\%
\uncover<8->{ &=&\displaystyle 5(\alertNoH{12}{2x+1})^4\alertNoH{ 10-11}{\left(\fcAnswerUncover{8}{11}{2}\right)}( \alertNoH{12}{x^3-x+1})^4 +4(\alertNoH{12}{2x +1})^5( \alertNoH{12}{ x^3 -x+1})^3\alertNoH{ 8-9}{(\fcAnswerUncover{8}{9}{3x^2-1})}%
}\\%
&& \uncover<12->{\text{Common factor } 2(\alertNoH{12}{2x+1})^4(\alertNoH{12}{x^3-x+1})^3:}\\%
\uncover<12->{ & = &\displaystyle 2(2x+1)^4(x^3-x+1)^3(\alertNoH{14}{ 2(2x+1)(3x^2-1)+5(x^3-x+1) }) )%
}\\
\uncover<14->{&  = &\displaystyle 2(2x+1)^4(x^3-x+1)^3(\alertNoH{14}{17x^3+6x^2-9x+3})}%
\end{array}
$
\end{example}
\end{frame}
% end module chain-rule-ex6
