\begin{frame}
\begin{example}[Finding maxima, minima]
\begin{columns}
\column{0.3\textwidth}
\psset{xunit=0.5cm, yunit=0.5cm}
\begin{pspicture}(-1, -1)(1, 1)
\tiny
\fcBoundingBox{-3}{-2}{4}{6}
\renewcommand{\fcScreen}{[-4 -0.5 -2] 0}
\fcStartIIIdScene
\only<1>{
\fcSurfaceInScene[iterationsU=25, iterationsV=25, linecolor=black, linewidth=0.6]{-2.1}{-2.1}{2.1}{2.1}{[%
2 dict begin %
/x u def %u v sub 2 sqrt div def
/y v def %u v add 2 sqrt div def
/z x 4 exp  y 4 exp add -4 x mul y mul add def
x y z
end
]}
{
2 dict begin
/x u def %u v sub 2 sqrt div def
/y v def %u v add 2 sqrt div def
/z x 4 exp  y 4 exp add -4 x mul y mul add def
z 3 le %
end %
}
}
\only<2>{
\fcSurfaceInScene[iterationsU=25, iterationsV=25, linecolor=black, linewidth=0.6]{-2.1}{-2.1}{2.1}{2.1}{[%
2 dict begin %
/x u def %u v sub 2 sqrt div def
/y v def %u v add 2 sqrt div def
/z x 4 exp  y 4 exp add -4 x mul y mul add def
x y z
end
]}
{
2 dict begin
/x u def %u v sub 2 sqrt div def
/y v def %u v add 2 sqrt div def
/z x 4 exp  y 4 exp add -4 x mul y mul add def
z 3 le %
0.7 x mul y z add add 1.2 le and %
end %
}
}
\fcAxesIIIdInScene[arrows=->, linecolor=black, linewidth=1]{4}{4}{4.5}
\fcFinishIIIdScene[fastsort=true]
\fcPutIIId[l]{[4 0 0]}{$x$}
\fcPutIIId[l]{[0 4 0]}{$y$}
\fcPutIIId[b]{[0 0 4.5]}{$z$}
\end{pspicture}  
\column{0.7\textwidth}
Find the local and global maxima and minima of $f(x,y) = x^4+y^4-4xy+1$.
\begin{itemize}
  \item $f_{xx} = 12x^2$;
  \item $f_{xy} = -4$;
  \item $f_{yy}=12y^2$;
  \item $D= f_{xx}f_{yy}-f_{xy}^2 = 9x^2y^2-1$
\end{itemize}

Therefore the critical points are the following.
\end{columns}
\begin{tabular}{|c|c|c|c|c|c|}
\hline
$(x_0,y_0)$ & $f_{xx}$ & $f_{yy}$ & $f_{xy}$ & $D$ & Conclusion \\\hline
(0,0) & 0 & 0 & -4 & $-16 <0$ & Saddle point  \\\hline
(1,1) & 12 & 12 & -4 & $144-16 > 0$ & Local min  \\\hline
(-1,-1) & 12 & 12 & -4 & $144-16 > 0$ & Local min \\\hline
\end{tabular}
\pause

In this case it turns out that the two local minimum points are actually global minimum points, because
%
$$f(x,y) = x^4+y^4-4xy = (x^2-1)^2+(y^2-1)^2+2(x-y)^2 -2  \geq -2\; .$$

\end{example}
\end{frame}