\begin{frame}
\vskip -0.1 cm
\begin{proposition}[Product to sum formulas]
\[
\begin{array}{rcl}
\sin \alpha \sin \beta &=&\displaystyle \frac{1}{2}\left(\cos( \alpha -\beta) -\cos(\alpha+\beta) \right)\\
\cos \alpha \cos \beta &=&\displaystyle \frac{1}{2}\left( \cos( \alpha -\beta) +\cos(\alpha+\beta) \right)\\
\sin \alpha \cos \beta &=&\displaystyle \frac{1}{2}\left(\sin( \alpha +\beta) +\sin(\alpha-\beta) \right)\\
\end{array}
\]
\end{proposition}
\begin{proof}
$
\begin{array}{lrcl}
\multirow{2}{*}{$+$}&\cos\alpha\cos\beta+\sin\alpha\sin\beta &=&\cos(\alpha-\beta)\\
&\cos\alpha\cos\beta-\sin\alpha\sin\beta &=&\cos(\alpha+\beta)\\
&2\cos\alpha \cos \beta &=&\cos(\alpha-\beta)+\cos(\alpha+\beta)\\\hline 
\multirow{2}{*}{$-$}&\cos\alpha\cos\beta+\sin\alpha\sin\beta &=&\cos(\alpha-\beta)\\
&\cos\alpha\cos\beta-\sin\alpha\sin\beta &=&\cos(\alpha+\beta)\\
&2\sin\alpha \sin \beta &=&\cos(\alpha-\beta)-\cos(\alpha+\beta)\\\hline 
\multirow{2}{*}{$+$}&\sin\alpha\cos\beta+\cos\alpha\sin\beta &=&\sin(\alpha+\beta)\\
&\sin\alpha\cos\beta-\cos\alpha\sin\beta &=&\sin(\alpha-\beta)\\
&2\sin\alpha \cos \beta &=&\sin(\alpha+\beta)+\sin(\alpha+\beta)\\
\end{array}
$
\end{proof}

\end{frame}
\begin{frame}
\vskip -0.1 cm
\begin{proposition}[Product to sum formulas]
\[
\begin{array}{rcl}
\sin \alpha \sin \beta &=&\displaystyle \frac{1}{2}\left(\cos( \alpha -\beta) -\cos(\alpha+\beta) \right)\\
\cos \alpha \cos \beta &=&\displaystyle \frac{1}{2}\left( \cos( \alpha -\beta) +\cos(\alpha+\beta) \right)\\
\sin \alpha \cos \beta &=&\displaystyle \frac{1}{2}\left(\sin( \alpha +\beta) +\sin(\alpha-\beta) \right)\\
\end{array}
\]
\end{proposition}
\begin{itemize}
\item Product to sum formulas are used when integrating (a topic to be studied later/in another course).
\end{itemize}
\vskip 10cm

\end{frame}