% begin module trig-identities
\begin{frame}
\frametitle{Trigonometric Identities Revisited}
\only<1>{\alert<1>{You are not required to learn the material in this slide. You will not be tested on it.}}
\only<2->{
All trigonometric formulas can be easily derived using
\begin{itemize}
\item<alert@5,7,15,21,23> $e^{ix}=\cos x+i\sin x$  \hfill~ (Euler's Formula).
\item<alert@6,14,22> $e^{ix} e^{iy} = e^{ix+iy}=e^{i(x+y)}$\hfill~ (exponentiation rule: valid for $\mathbb C$).
\item<alert@12> $e^0=1$ \hfill~(exponentiation rule).
\item<alert@16> $\sin (-x) =-\sin x$, $\cos (-x)=\cos x$ \hfill~ (easy to remember).

\end{itemize}
\only<3-10>{ %Example1
\footnotesize
\begin{example}
\[
\begin{array}{rcl}
\alert<9>{\sin (x+y)}&\alert<9>{=}& \alert<9>{\sin x \cos y + \sin y \cos x}\\
\alert<10>{\cos (x+y)}&\alert<10>{=}& \alert<10>{\cos x \cos y - \sin x \sin y} \quad .
\end{array}
\]
\end{example}
\begin{proof}
\uncover<4->{ 
\[
\begin{array}{rcl}
\alert<5,6>{e^{i(x+y)}}&=&\uncover<5->{\alert<5>{\cos (x+y)+i\sin (x+y)}}\\

\uncover<6->{\alert<6,7>{e^{ix} e^{iy}}} &\uncover<6->{=} &\uncover<6->{\cos (x+y)+i\sin (x+y)}\\
 
\uncover<7->{\alert<7>{(\cos x+i\sin x)(\cos y+i\sin y)}} &\uncover<7->{=}&\uncover<7->{\cos (x+y)+i\sin (x+y)}\\

\uncover<8->{{\alert<10>{\cos x\cos y- \sin x \sin y}+i(\alert<9>{\sin x \cos y +\sin y \cos x)}}} &\uncover<8->{=}&\uncover<8->{\alert<10>{\cos (x+y)}+i\alert<9>{\sin (x+y)}}\\
\end{array}
\]
\uncover<9->{\alert<9>{
Compare coefficient in front of $i$ 
} and } 
\uncover<10->{\alert<10>{
remaining terms} to get the desired equalities.
}
}
\uncover<10->{
\end{proof}
}
} %end Example1
\only<11-18>{ %
\begin{example}
\[
\alert<18>{\sin^2 x+\cos^2x=1}
\]
\end{example}
\begin{proof}
\uncover<12->{ %Example2
\[
\begin{array}{rcl}
\alert<12,18>{1}&\alert<12>{=}&\alert<12>{e^{0}}\\
&\uncover<13->{=}&\uncover<13->{\alert<14>{ e^{ix-ix}=}}\uncover<14->{\alert<14,15>{ e^{ix} e^{-ix}}=}\uncover<15->{\alert<15>{ (\cos x+i\sin x)(\alert<16>{\cos (-x)+i\sin (-x)})}} \\
&\uncover<16->{=}&\uncover<16->{(\cos x+i\sin x)(\alert<16>{\cos x-i\sin x})=}\uncover<17->{\cos^2 x -i^2\sin^2x}\\
&\uncover<18->{\alert<18>{=}}&\uncover<18->{\alert<18>{\cos^2x+\sin^2x}}\quad.
\end{array}
\]
}
\uncover<18->{
\end{proof}
}
} %end Example2

\only <19->{ %Example3
\footnotesize
\begin{example}
\[
\begin{array}{rcl}
\alert<25>{\sin 2x}&\alert<25>{=}& \alert<25>{2\sin x \cos x}\\
\alert<26>{\cos 2x}&\alert<26>{=}& \alert<26>{\cos^2 x - \sin^2 x } \quad .
\end{array}
\]
\end{example}
\begin{proof}
\uncover<20->{ 
\[
\begin{array}{rcl}
\alert<21,22>{e^{i(2x)}}&=&\uncover<21->{\alert<21>{\cos 2x+i\sin 2x}}\\

\uncover<22->{\alert<22,23>{e^{ix} e^{ix}}} &\uncover<22->{=} &\uncover<22->{\cos 2x+i\sin 2x}\\
 
\uncover<24->{\alert<24>{(\cos x+i\sin x)^2=}} \uncover<23->{\alert<23>{(\cos x+i\sin x)(\cos x+i\sin x)}} &\uncover<23->{=}&\uncover<23->{\cos 2x+i\sin 2x}\\

\uncover<24->{ \alert<24>{\alert<26>{\cos^2 x- \sin^2 x  }+i(\alert<25>{2\sin x \cos x})} } &\uncover<24->{=}&\uncover<24->{\alert<26>{\cos 2x}+i\alert<25>{\sin 2x}}\\
\end{array}
\]
\uncover<25->{\alert<25>{
Compare coefficient in front of $i$ 
} and } 
\uncover<26->{\alert<26>{
remaining terms} to get the desired equalities.
}
}
\uncover<26->{
\end{proof}
}
} %end Example1


} %end actual slide
\end{frame}
% end module trig-identities
