% begin module trig-identities
\begin{frame}
\frametitle{Trigonometric Identities Revisited}
\begin{itemize}
\item \alertNoH{5,7,15,21,23}{ $e^{ix}=\cos x+i\sin x$  \hfill~ (Euler's Formula).}
\item \alertNoH{6,14,22}{ $e^{ix} e^{iy} = e^{ix+iy}=e^{i(x+y)}$\hfill~ (exponentiation rule: valid for $\mathbb C$).}
\item \alertNoH{12}{ $e^0=1$ \hfill~(exponentiation rule).}
\item<2->\alertNoH{16}{$\sin (-x) =-\sin x$, $\cos (-x)=\cos x$} \hfill~ (easy to remember).
\end{itemize}
\only<handout:0|2>{\alertNoH{2}{ All trigonometric formulas can be easily derived using the above formulas.} }

\footnotesize
\only<handout:0|1-2>{\vspace{10cm}}


\only<handout:1|3-10>{ %Example1
\footnotesize
\begin{example}
\[
\begin{array}{rcl}
\alertNoH{9}{\sin (x+y)}&\alertNoH{9}{=}& \alertNoH{9}{\sin x \cos y + \sin y \cos x}\\
\alertNoH{10}{\cos (x+y)}&\alertNoH{10}{=}& \alertNoH{10}{\cos x \cos y - \sin x \sin y} \quad .
\end{array}
\]
\end{example}
\begin{proof}
\uncover<4->{
\[
\begin{array}{r@{~}c@{~}l}
\alertNoH{5,6}{e^{i(x+y)}}&=&\uncover<5->{\alertNoH{5}{\cos (x+y)+i\sin (x+y)}}\\

\uncover<6->{\alertNoH{6,7}{e^{ix} e^{iy}}} &\uncover<6->{=} &\uncover<6->{\cos (x+y)+i\sin (x+y)}\\

\uncover<7->{\alertNoH{7}{(\cos x+i\sin x)(\cos y+i\sin y)}} &\uncover<7->{=}&\uncover<7->{\cos (x+y)+i\sin (x+y)}\\

\uncover<8->{{\alertNoH{10}{\cos x\cos y- \sin x \sin y}+i(\alertNoH{9}{\sin x \cos y +\sin y \cos x)}}} &\uncover<8->{=}&\uncover<8->{\alertNoH{10}{\cos (x+y)}+i\alertNoH{9}{\sin (x+y)}}\\
\end{array}
\]
\uncover<9->{\alertNoH{9}{
Compare coefficient in front of $i$
} and }
\uncover<10->{\alertNoH{10}{
remaining terms} to get the desired equalities.
}
}
\uncover<10->{
\end{proof}
}
} %end Example1
\only<handout:2|11-18>{
\begin{example}
\[
\alertNoH{18}{\sin^2 x+\cos^2x=1}
\]
\end{example}
\begin{proof}
\uncover<12->{ %Example2
\[
\begin{array}{rcl}
\alertNoH{12,18}{1}&\alertNoH{12}{=}&\alertNoH{12}{e^{0}}\\
&\uncover<13->{=}&\uncover<13->{\alertNoH{14}{ e^{ix-ix}=}}\uncover<14->{\alertNoH{14,15}{ e^{ix} e^{-ix}}=}\uncover<15->{\alertNoH{15}{ (\cos x+i\sin x)(\alertNoH{16}{\cos (-x)+i\sin (-x)})}} \\
&\uncover<16->{=}&\uncover<16->{(\cos x+i\sin x)(\alertNoH{16}{\cos x-i\sin x})=}\uncover<17->{\cos^2 x -i^2\sin^2x}\\
&\uncover<18->{\alertNoH{18}{=}}&\uncover<18->{\alertNoH{18}{\cos^2x+\sin^2x}\quad.}
\end{array}
\]
}
\uncover<18->{
\end{proof}
}
\vspace{3cm}
} %end Example2

\only<handout:3|19->{ %Example3
\footnotesize
\begin{example}
\[
\begin{array}{rcl}
\alertNoH{25}{\sin 2x}&\alertNoH{25}{=}& \alertNoH{25}{2\sin x \cos x}\\
\alertNoH{26}{\cos 2x}&\alertNoH{26}{=}& \alertNoH{26}{\cos^2 x - \sin^2 x } \quad .
\end{array}
\]
\end{example}
\begin{proof}
\uncover<20->{
\[
\begin{array}{rcl}
\alertNoH{21,22}{e^{i(2x)}}&=&\uncover<21->{\alertNoH{21}{\cos 2x+i\sin 2x}}\\

\uncover<22->{\alertNoH{22,23}{e^{ix} e^{ix}}} &\uncover<22->{=} &\uncover<22->{\cos 2x+i\sin 2x}\\

\uncover<24->{\alertNoH{24}{(\cos x+i\sin x)^2=}} \uncover<23->{\alertNoH{23}{(\cos x+i\sin x)(\cos x+i\sin x)}} &\uncover<23->{=}&\uncover<23->{\cos 2x+i\sin 2x}\\

\uncover<24->{ \alertNoH{24}{\alertNoH{26}{\cos^2 x- \sin^2 x  }+i(\alertNoH{25}{2\sin x \cos x})} } &\uncover<24->{=}&\uncover<24->{\alertNoH{26}{\cos 2x}+i\alertNoH{25}{\sin 2x}}\\
\end{array}
\]
\uncover<25->{\alertNoH{25}{
Compare coefficient in front of $i$
} and }
\uncover<26->{\alertNoH{26}{
remaining terms} to get the desired equalities.
}
}
\uncover<26->{
\end{proof}
}
} %end Example1


\end{frame}
% end module trig-identities
