\begin{frame}
\begin{example}
Verify the identity $ \ln (\sec \theta- 1) +\ln (\sec \theta+1) -2\ln (\sec \theta) =2\ln(\sin \theta)$.

\uncover<2->{
We transform the left hand side to the right.
\[\begin{array}{cl}
&\displaystyle \ln (\sec \theta- 1) +\ln (\sec \theta+1) -2\ln (\sec \theta)\\
=& \displaystyle \ln \left((\sec \theta- 1)(\sec \theta+1)\right)-\ln \left(\sec^2 \theta\right) \\
=&\displaystyle \ln\left(\sec^2\theta-1\right) -\ln \left( \sec^2 \theta\right)\\
=&\displaystyle \ln\left(\frac{\sec^2\theta-1}{\sec^2 \theta}\right)\\
=&\displaystyle \ln\left(1- \frac{1}{\sec^2 \theta}\right)\\
=&\displaystyle \ln\left(1- \cos^2\theta\right)\\
=&\displaystyle \ln\left(\sin^2\theta\right)\\
=&\displaystyle 2\ln\left(\sin\theta\right) \\
\end{array}
\]
as desired.
}
\end{example}
\end{frame}
