\begin{frame}[t]
\vskip -0.5cm
\begin{columns}[t]
\column{0.5\textwidth}
\begin{definition}[Exponent, Def. II]
$e^{z}=e(z)=\sum\limits_{n=0}^{\infty}\frac{z^n}{n!}$.
\end{definition}
\column{0.5\textwidth}
\uncover<2->{
\begin{definition}[Polar form]
$|z|=e^{\rho}$, $z=e^{\rho}(\cos \theta+i\sin \theta)$  \vphantom{$\sum\limits_{n=0}^{\infty}\frac{z^n}{n!}$}
\end{definition}
}
\end{columns}
\begin{itemize}
\item<1-> For the duration of this slide, assume Definition II of exponent.
\item<3-> In preceding slides/lectures, by algebraic manipulations of series, we showed that $e(z) e(w)= e^{z} e^{w} = e^{z+w}=e(z+w)$.
\uncover<4->{
\begin{theorem}
$\sin (\alpha+\beta)=\sin \alpha\cos \beta+i\sin \beta \cos \alpha$

$\cos (\alpha+\beta)=\cos\alpha\cos \beta-\sin \alpha\sin \beta$, \quad \quad where $\alpha,\beta\in \mathbb R$
\end{theorem}

\begin{proof}
\small
$\begin{array}{r@{~}c@{~}l}
\uncover<5->{ \alertNoH{10}{\cos (\alpha+\beta)} +i \alertNoH{11}{ \sin (\alpha+\beta)} &=& e^{i(\alpha+ \beta)}} \uncover<6->{ = e^{i\alpha+ i\beta}} \uncover<7->{ =e^{ i \alpha }e^{i\beta}}\\
\uncover<8->{&=&(\cos \alpha +i \sin \alpha)(\cos \beta +i\sin \beta)} \\
\uncover<9->{&=& \alertNoH{10}{(\cos \alpha\cos \beta- \sin\alpha \sin \beta )} \\
&&+ i\alertNoH{11}{( \cos \alpha\sin \beta +\sin\alpha\cos \beta)}.}
\end{array}$

\uncover<10->{Compare \alertNoH{10}{real} and \alertNoH{11}{imaginary} part to get the desired trig identities.}
\end{proof}
}
\end{itemize}
\end{frame}
