\solution{\ref{problemlimxtominusinfty(3x^3+2)/(2x^3-4x+5)}.


\[
\begin{array}{rcll|l}
\displaystyle \lim_{x\to-\infty} \frac{3x^3+2}{2x^3-4x+5}&=&\displaystyle \lim_{x\to-\infty} \frac{\left(3x^3+2\right) \frac{1}{x^3}}{ \left(2x^3-4x +5\right)\frac{1}{ x^3}}&& \begin{array}{l} \text{Divide top}\\ \text{and bottom}\end{array}\\
&=&\displaystyle \lim_{x\to-\infty} \frac{3+\frac{2}{x^3}}{2-\frac{4}{x^2}+\frac{5}{x^3}} && \begin{array}{l} \text{by highest term}\\ \text{in denominator}\end{array}\\
&=&\displaystyle\frac{3+0}{2-0+0}=\frac{3}{2}.
\end{array}
\]
}

\solution{\ref{problemlim(xto-infty)sqrt(x^2+x)-sqrt(x^2-x)}.
\[ \begin{array}{rcl}
\displaystyle\lim_{x\to -\infty} \sqrt{x^2+x}-\sqrt{x^2-x} &=&\displaystyle\lim_{x\to -\infty} \left(\sqrt{x^2+x}-\sqrt{x^2-x}\right) \frac{ \left(\sqrt{x^2+x}+\sqrt{x^2-x}\right) }{\left( \sqrt{x^2+x}+\sqrt{x^2-x}\right)}
\\
&=&\displaystyle \lim_{x\to -\infty} \frac{x^2+x-(x^2-x) }{\sqrt{x^2+x}+\sqrt{x^2-x} } = \lim_{x\to -\infty} \frac{2x \frac{1}{x} }{\left(\sqrt{x^2+x}+\sqrt{x^2-x} \right)\frac{1}{x}} 
\\&=&\displaystyle \lim_{x\to -\infty} \frac{2}{\frac{\sqrt{x^2+x}}x+\frac{\sqrt{x^2-x}}x }= \lim_{x\to -\infty} \frac{2}{ {\color{red}-} \sqrt{\frac{x^2+x}{x^2}} {\color{red}-} \sqrt{\frac{x^2-x}{x^2}} }\\
&=&\displaystyle \lim_{x\to -\infty} \frac{2}{ - \sqrt{1+\frac1x} - \sqrt{1-\frac1x} }=\frac{2}{-\sqrt{1+0}-\sqrt{1-0}}=-1
\end{array}
\]
The sign highlighted in red arises from the fact that, for negative $x$, we have that $ x={\color{red}-}\sqrt{x^2}$.
}