Use implicit differentiation to find an equation of the tangent line to the curve a the given point. The answer key has not been proofread, use with caution.
\begin{multicols}{3}
\begin{enumerate}
\item $y\sin (2x)=x\cos (2y) $, $\left(\frac{\pi}{2}, \frac{\pi}{4}\right)$. 

\answer{$y=\pi^{-1} x+\frac{1}{4} \pi-\frac{1}{4}$}
\item $ \sin (x+y)=2x-2y$, $(\pi,\pi)$ . 

\answer{$\frac{1}{3} x+\frac{2}{3} \pi $}
\item $x^2+x y+y^2=3 $, $(1,2)$ (ellipse). 

\answer{$y=-\frac{4}{5} x+\frac{14}{5} $}
\item $x^2+2x y-y^2+x=2 $, $(1,2)$ (hyperbola). 

\answer{$y= \frac{7}{2} x-\frac{3}{2}$}
\item $x^2+y^2=(2x^2+2y^2-x)^2 $, $(0,\frac{1}{2})$. 

\answer{$y= x+\frac{1}{2}$}
\item $x^{\frac{2}{3}}+y^{\frac{2}{3}}=4$, $(-3\sqrt{3},1)$. 

\answer{$y=\frac{1}{\sqrt{3}}x+4 $}
\item $2(x^2+y^2)^2 =25(x^2-y^2)$, $(3,1)$. 

\answer{$y= -\frac{9}{13} x+\frac{40}{13}$}
\item $y^2(y^2-4)=x^2(x^2-5) $, $(0,-2)$. 

\answer{$y=-2 $}
\end{enumerate}
\end{multicols}
