Express $\frac{\diff y}{\diff x}$ as a function of $x$ and $y$ by implicit differentiation. The answer key has not been proofread, use with caution.
\begin{multicols}{2}
\begin{enumerate}[ref={\fcProblemRef}]
\item $x^3+y^3=1$.

\answer{$\frac{\diff y}{\diff x}=-\frac{x^2}{y^2}$}
\item $ 2\sqrt x+\sqrt y=3$.

\answer{$\frac{\diff y}{\diff x}=-2\sqrt{\frac{ y}{x}}$}
\item $ x^2+x y-y^2=4$.

\answer{$\frac{\diff y}{\diff x}=\frac{-2x-y}{x-2y}$}
\item $ 2x^3+x^2y-x y^3=2$.

\answer{$\frac{\diff y}{\diff x}=\frac{y^{3}-6 x^{2}-2 x y}{-3 x y^{2}+x^{2}}$}
\item $ x^4(x+y)=y^2(3x-y)$.

\answer{$\frac{\diff y}{\diff x}= \frac{ -5x^4 -4x^3y +3y^2}{x^4- 6xy - 3y^2}$}
\item $ y^5+x^2y^3=1+x^4y $.

\answer{$\frac{\diff y}{\diff x}=\frac{ 4x^3y-2xy^3}{5y^4+3x^2y^2- x^4 }$}
\item $ y\cos x=x^2+y^2 $.

\answer{$\frac{\diff y}{\diff x}= \frac{ y\sin x+2x}{\cos x-2y}$}
\item $ \cos (x y)=1+\sin y$.

\answer{$\frac{\diff y}{\diff x}= -\frac{y\sin (xy)}{\cos y+x\sin(xy) }$}
\item $ 4\cos x\sin y=1$.

\answer{$\frac{\diff y}{\diff x}=\tan x \tan y$}
\item $ y\sin \left(x^2\right)=x\sin \left(y^2\right)$.

\answer{$\frac{\diff y}{\diff x}=\frac{-2xy\cos\left(x^2\right)+\sin \left(y^2\right)}{ - 2 x y \cos\left( y^2 \right)+\sin \left(x^2 \right) }$}
\item $ \tan \left(\frac{x}{y}\right)=x+y$.

\answer{$\frac{\diff y}{\diff x}=\frac{-y^2+y\sec^2 \left(\frac{y}{x}\right) }{y^2 + x\sec^2\left(\frac{x}{y}\right) }$}
\item $ \sqrt{x+y}=1+x^2y^2$.

\answer{$\frac{\diff y}{\diff x}= \frac{-\frac{1}{2} (y+x)^{-\frac{1}{2}}+8 x y^{2}}{\frac{1}{2} (y+x)^{-\frac{1}{2}}-8 x^{2} y} $}
\item $ \sqrt{xy}=1+x^2 y$.

\answer{$\frac{\diff y}{\diff x}=\frac{-\frac{1}{2} x^{-\frac{1}{2}} y^{\frac{1}{2}} -2 x y}{\frac{1}{2} x^{\frac12} y^{-\frac{1}{2}} +x^{2}} $}
\item $ x\sin y+y\sin x=1$.

\answer{$\frac{\diff y}{\diff x}=\frac{- y \cos{}x- \sin{}y}{x \cos{}y+\sin{}x}$}
\item $ y\cos x=1+\sin (x y)$.

\answer{$\frac{\diff y}{\diff x}=\frac{\cos{}(x y) y+y \sin{}x}{- \cos{}(x y) x+\cos{}x}$}
\item $ \tan (x-y)=\frac{y}{1+x^2}$.

\answer{$\frac{\diff y}{\diff x}=\frac{- (\sec{}(- y+x))^{2} x^{4}-2 (\sec{}(- y+x))^{2} x^{2}- (\sec{}(- y+x))^{2}-2 y x}{- (\sec{}(- y+x))^{2} x^{4}-2 (\sec{}(- y+x))^{2} x^{2}- (\sec{}(- y+x))^{2}- x^{2}-1}$}

\item  $x^4(x+y)=y^2(3x-y)$.

\answer{ $ \frac{dy}{dx}=\frac{-4 x^{3} y+3 y^{2}-5 x^{4}}{3 y^{2}+x^{4}-6 y x}$}
\item $2x^3+x^2y-xy^3=2$.

\answer{$\frac{dy}{dx}=\frac{y^{3}-6 x^{2}-2 x y}{-3 x y^{2}+x^{2}}$}
\end{enumerate}
\end{multicols}