% begin module diff-eq-ex1
\begin{frame}
\begin{example}[Example 1, p. 606]
Show that every member of the family of functions 
\abovedisplayskip=0pt
\belowdisplayskip=0pt
\[
y = \frac{1 + ce^t}{1-ce^t}
\]
is a solution of the differential equation $\alert<handout:0| 2-4>{y'} = \alert<handout:0| 5->{\frac{1}{2} (y^2 - 1)}$.
\abovedisplayskip=0pt
\belowdisplayskip=0pt
\begin{eqnarray*}
\uncover<2->{%
\textrm{LHS} %
}%
& \uncover<2->{ = } &%
\uncover<2->{%
\frac{(1-ce^t)(ce^t) - (1+ce^t)(-ce^t)}{(1-ce^t)^2}%
}\\%
& \uncover<3->{ = } &%
\uncover<3->{%
\frac{ce^t - c^2 e^{2t} + ce^t + c^2 e^{2t}}{(1-ce^t)^2}%
}  \uncover<4->{ = } \uncover<4->{%
\alert<handout:0| 9>{\frac{2ce^t}{(1-ce^t)^2}}%
}\\%
\end{eqnarray*}
\abovedisplayskip=0pt
\belowdisplayskip=0pt
\begin{eqnarray*}
\uncover<5->{%
\textrm{RHS} %
} 
& \uncover<5->{ = } & 
\uncover<5->{%
\frac{1}{2}\left[ \left( \frac{1+ce^t}{1-ce^t}\right)^2 - 1\right]
} \uncover<6->{ = } \uncover<6->{%
\frac{1}{2}\left[  \frac{(1+ce^t)^2 - (1-ce^t)^2}{(1-ce^t)^2} \right]
}\\ 
& \uncover<7->{ = } &
\uncover<7->{%
\frac{1}{2}\left[  \frac{1+2ce^t +c^2e^{2t} - 1 + 2ce^t - c^2e^{2t}}{(1-ce^t)^2} \right]
}\\
 & \uncover<8->{ = } & %
\uncover<8->{%
\frac{1}{2}  \frac{4ce^t }{(1-ce^t)^2} 
} \uncover<9->{ = } \uncover<9->{%
  \alert<handout:0| 9>{\frac{2ce^t }{(1-ce^t)^2}} \uncover<10->{= \textrm{LHS}}
}\\%
\end{eqnarray*}
\end{example}
\end{frame}
% end module diff-eq-ex1
