% begin module diff-eq-initial-condition-ex2
\begin{frame}
\begin{example} %[Example 2, p. 606]
Find a solution of the differential equation $y' = \frac{1}{2}(y^2 - 1)$ that satisfies the initial condition $y(0) = 2$.

\uncover<2->{%
Substitute $t = 0$ and $y = 2$ into the formula 
\abovedisplayskip=0pt
\belowdisplayskip=0pt
\[
y = \frac{1+ce^t}{1-ce^t}
\]
from Example 1.
}%
\abovedisplayskip=0pt
\belowdisplayskip=0pt
\begin{eqnarray*}
\uncover<3->{%
2 %
}%
& \uncover<3->{ = } &%
\uncover<3->{%
\frac{1+ce^0}{1-ce^0}
} \uncover<4->{ = } \uncover<4->{%
\frac{1+c}{1-c}
}\\%
\uncover<5->{%
2(1-c) %
}%
& \uncover<5->{ = } &%
\uncover<5->{%
1+c%
}\\%
\uncover<6->{%
2-2c %
}%
& \uncover<6->{ = } &%
\uncover<6->{%
1+c%
}\\%
\uncover<7->{%
c %
}%
& \uncover<7->{ = } &%
\uncover<7->{%
1 / 3
}\\%
\end{eqnarray*}

\uncover<8->{%
Therefore the solution to the initial-value problem is
\abovedisplayskip=0pt
\belowdisplayskip=0pt
\[
y = \frac{1+\frac{1}{3}e^t}{1 - \frac{1}{3} e^t} = \frac{3 + e^t}{3 - e^t}.
\]
}%
\end{example}
\end{frame}
% end module diff-eq-initial-condition-ex2
