% begin module logistic-solution
\begin{frame}
\begin{columns}[c]
\column{.6\textwidth}
\abovedisplayskip=0pt
\belowdisplayskip=0pt
\begin{eqnarray*}
\frac{\diff P}{\diff t} & = & kP\left( 1 - \frac{P}{K}\right)\\
\uncover<2->{%
\int \frac{1}{P(1-P/K)}\diff P%
}%
& \uncover<2->{ = } &%
\uncover<2->{%
\int k\diff t%
}\\%
\uncover<3->{%
\int \frac{K}{P(K-P)}\diff P%
}%
& \uncover<3->{ = } &%
\uncover<3->{%
\int k\diff t%
}\\%
\uncover<4->{%
\int \left( \frac{1}{P} + \frac{1}{K-P}\right)\diff P%
}%
& \uncover<4->{ = } &%
\uncover<4->{%
\int k\diff t%
}\\%
\uncover<5->{%
\ln |P| - \ln |K-P|%
}%
& \uncover<5->{ = } &%
\uncover<5->{%
kt + C%
}\\%
\uncover<6->{%
\ln  \left| \frac{K-P}{P}\right|%
}%
& \uncover<6->{ = } &%
\uncover<6->{%
-kt - C%
}\\%
\uncover<7->{%
\alert<handout:0| 11>{ \frac{K-P}{P}}%
}%
& \uncover<7->{ = } &%
\uncover<7->{%
\alert<handout:0| 8>{\pm e^{-C}}e^{-kt}%
}\uncover<8->{\alert<handout:0| 11>{ = \alert<handout:0| 8>{A} e^{-kt}}}\\%
\uncover<9->{%
K%
}%
& \uncover<9->{ = } &%
\uncover<9->{%
P(1+Ae^{-kt})%
}\\%
\uncover<10->{%
P%
}%
& \uncover<10->{ = } &%
\uncover<10->{%
\frac{K}{1+Ae^{-kt}}%
}\\%
\end{eqnarray*}
\column{.4\textwidth}
\uncover<11->{%
Plug in $P(0) = P_0$:
\[
\frac{K - P_0}{P_0} = Ae^{-k\cdot 0} = A.
\]
}%
\end{columns}
\end{frame}


\begin{frame}
The solution to the initial value problem
\[
\frac{\diff P}{\diff t} = kP\left( 1 - \frac{P}{K}\right), \qquad P(0) = P_0
\]
is
\[
P = \frac{K}{1+Ae^{-kt}},\qquad A = \frac{K-P_0}{P_0}.
\]
\end{frame}
% end module logistic-solution
