% begin module natural-growth-solution
\begin{frame}
\[
\frac{\diff P}{\diff t} = kP
\]

This is a separable equation (more on this later), so we can solve it.
\abovedisplayskip=0pt
\belowdisplayskip=0pt
\begin{eqnarray*}
\uncover<2->{%
\int \frac{1}{P}\;\diff P%
}%
& \uncover<2->{ = } &%
\uncover<2->{%
\int k\;\diff t%
}\\%
\uncover<3->{%
\ln |P|%
}%
& \uncover<3->{ = } &%
\uncover<3->{%
kt + C%
}\\%
\uncover<4->{%
 |P|%
}%
& \uncover<4->{ = } &%
\uncover<4->{%
e^Ce^{kt}%
}\\%
\uncover<5->{%
 P%
}%
& \uncover<5->{ = } &%
\uncover<5->{%
\pm e^Ce^{kt}%
}%
\end{eqnarray*}
\begin{itemize}
\item<6->  Let $A = \pm e^C$.  Then the solution is $P = A e^{kt}$.
\item<7->  $A = \pm e^C$ can be any positive or negative number.
\item<8->  The function $P = 0$ is also a solution, so $A$ can be any number.
\item<9->  $P(0) = Ae^{k\cdot 0} = A$.
\end{itemize}
\uncover<10->{%
The solution to the initial value problem
\abovedisplayskip=0pt
\belowdisplayskip=0pt
\[
\frac{\diff P}{\diff t} = kP, \qquad P(0) = P_0
\]
\abovedisplayskip=0pt
\belowdisplayskip=0pt
\[
\textrm{is}\qquad P(t) = P_0e^{kt}.
\]
}%
\end{frame}
% end module natural-growth-solution
