% begin module limit-laws-ex6
\begin{frame}
\begin{example}
\abovedisplayskip=0pt
\belowdisplayskip=0pt
\abovedisplayshortskip=0pt
\belowdisplayshortskip=0pt
\begin{align*}
\text{Find}\quad \lim_{t\to 0} \frac{\sqrt{t^2 + 9}-3}{t^2}%
& \\%
\uncover<2->{%
\text{Plug in 0:}\quad%
\frac%
{\alertNoH{ 2-3}{\sqrt{(0)^2+9}-3}}%
{\alertNoH{ 4-5}{(0)^2}}%
}%
& \uncover<2->{%
= \frac%
{\fcAnswer{3}{0}}%
{\fcAnswerUncover{2}{ 5}{0}}%
}
\end{align*}
\uncover<6->{%
Zero over zero is undefined, so we can't use direct substitution.
}%
\uncover<7->{%
Multiply top \& bottom by (minus) the conjugate radical:
}%
\begin{align*}
\uncover<7->{%
\lim_{t\to 0} \frac%
{\sqrt{t^2+9}-3}%
{t^2}%
}%
& \uncover<7->{%
= \lim_{t\to 0} \frac%
{\alertNoH{ 7-10}{\sqrt{t^2+9}-3}}%
{t^2}%
\cdot \frac%
{\fcAnswer{8}{ \alertNoH{9,10}{\sqrt{t^2+9}+3}}}%
{\fcAnswer{8}{\sqrt{t^2+9}+3}}%
}\\%
& \uncover<9->{ = \lim_{t\to 0} \frac{\fcAnswer{10}{(t^2+\alertNoH{11}{9})\alertNoH{11}{-9}}}{\uncover<9->{\worksheet{ t^2\left(\sqrt{t^2+9}+3\right)}}}}  \uncover<11->{ = \lim_{t\to 0} \frac{\uncover<11->{\worksheet{ \fcCancel{12}{t^2}}}}{\uncover<11->{\worksheet{\fcCancel{12}{t^2}(\sqrt{t^2+9}+3)}}}}\\%
& \uncover<12->{ = \lim_{t\to 0} \frac{\uncover<12->{\worksheet{1}}}{\uncover<12->{\worksheet{\sqrt{\alertNoH{ 13}{t}^2+9}+3}}}}\\%
\uncover<13->{%
\text{Plug in 0:}\quad%
}%
& \uncover<13->{ = }%
\uncover<handout:0| 13->{\frac{1}{\sqrt{(\alertNoH{ 13}{0})^2+9}+3}} \uncover<handout:0| 14->{ = \frac{1}{6}.}
\end{align*}
\end{example}
\end{frame}
% end module limit-laws-ex6
