% begin module sequence-limit-laws
\begin{frame}
The Limit Laws for continuous functions also hold for sequences:

If $\{ a_n\}$ and $\{ b_n\}$ are convergent sequences and $c$ is a constant, then
\begin{enumerate}
\item  $\displaystyle \lim_{n\to\infty}(a_n+b_n) = \lim_{n\to\infty}a_n +\lim_{n\to\infty}b_n$
\item  $\displaystyle \lim_{n\to\infty}(a_n-b_n) = \lim_{n\to\infty}a_n -\lim_{n\to\infty}b_n$
\item  $\displaystyle \lim_{n\to\infty}ca_n = c\lim_{n\to\infty}a_n$
\item  $\displaystyle \lim_{n\to\infty}(a_n b_n) = \lim_{n\to\infty}a_n \cdot \lim_{n\to\infty}b_n$
\item  $\displaystyle \lim_{n\to\infty}\frac{a_n}{ b_n} = \frac{\displaystyle \lim_{n\to\infty}a_n}{\displaystyle  \lim_{n\to\infty}b_n}$ if $\lim_{n\to\infty}b_n\neq 0$
\item  $\displaystyle \lim_{n\to\infty}a_n^p = \left[ \lim_{n\to\infty}a_n\right]^p$ if $p > 0$ and $a_n > 0$.
\end{enumerate}
\end{frame}
% end module sequence-limit-laws
