% begin module inverse-function-calculus
\begin{frame}
\frametitle{The Calculus of Inverse Functions}
We will need the following theorem to compute the derivative of $f^{-1}$.  Its proof can be found in Appendix F.
\begin{theorem}
If $f$ is a one-to-one continuous function, then its inverse $f^{-1}$ is also continuous.
\end{theorem}
\end{frame}

\begin{frame}
\begin{theorem}[The Derivative of $f^{-1}$]
If $f$ is a one-to-one differentiable function with inverse function $f^{-1}$ and $f'(f^{-1}(a)) \neq 0$, then the inverse function is differentiable at $a$ and
\[
(f^{-1})'(a) = \frac{1}{f'(f^{-1}(a))} .
\]
\end{theorem}
\begin{proof}
\begin{itemize}
\item<2->  If $\alert<handout:0| 11>{f(b) = a}$, then $\alert<handout:0| 9,14-15>{f^{-1}(a) = b}$.  
\item<3->  Let $\alert<handout:0| 8>{y = f^{-1}(x)}$, so that $\alert<handout:0| 10>{f(y) = x}$.  
\item<4-| alert@12>  Since $f^{-1}$ is continuous, $y \rightarrow b$ as $x \rightarrow a$.
\end{itemize}
\begin{eqnarray*}
\uncover<5->{(f^{-1})'(a)} & \uncover<5->{=} &%
\uncover<6->{\alert<handout:0| 12>{\lim_{x\rightarrow a}} \frac{\alert<handout:0| 8>{f^{-1}(x)} - \alert<handout:0| 9>{f^{-1}(a)}}{\alert<handout:0| 10>{x} - \alert<handout:0| 11>{a}}}%
\uncover<7->{= \alert<handout:0| 12>{\lim_{y\rightarrow b}} \frac{\alert<handout:0| 8>{y} - \alert<handout:0| 9>{b}}{\alert<handout:0| 10>{f(y)} - \alert<handout:0| 11>{f(b)}}} \\%
& \uncover<13->{=} &%
\uncover<13->{\frac{1}{\lim_{y\rightarrow b} \frac{f(y) - f(b)}{y - b}}}%
\uncover<14->{= \frac{1}{f'(\only<-14>{\alert<handout:0| 14>{b}}\only<handout:0| 15->{\alert<handout:0| 15>{f^{-1}(a)}})}}\qedhere
\end{eqnarray*}
\end{proof}
\end{frame}
% end module inverse-function-calculus
