% begin module inverse-function-solve-for
\begin{frame}
\frametitle{How to Find the Inverse of a One-to-one Function}
\begin{enumerate}
\item<1-| alert@3>  Write $y = f(x)$.
\item<1-| alert@4-5>  Solve this equation for $x$ in terms of $y$ (if possible).
\item<1-| alert@6>  Interchange $x$ and $y$.  The resulting equation is $y = f^{-1}(x)$. 
\end{enumerate}
\uncover<2->{
\begin{example}%[Example 4, p. 388]
If $f(x) = x^3 + 2$, find a formula for $f^{-1}(x)$.
\begin{align*}
\uncover<3->{y} & \uncover<3->{=}  \uncover<3->{x^3 + 2}\\
\uncover<4->{x^3} & \uncover<4->{=}  \uncover<4->{y - 2}\\
\uncover<5->{\alert<handout:0| 6>{x}} & \uncover<5->{=}  \uncover<5->{\sqrt[3]{\alert<handout:0| 6>{y} - 2}}\\% 
\uncover<6->{\alert<handout:0| 6>{y}} & \uncover<6->{=}  \uncover<6->{\sqrt[3]{\alert<handout:0| 6>{x} - 2}} \qquad \uncover<6->{\alert<handout:0| 6>{\text{(New equation.)}}}
\end{align*}
\uncover<7->{
Therefore $f^{-1}(x) = \sqrt[3]{x - 2}$.
}
\end{example}
}
\end{frame}
% end module inverse-function-solve-for
