% begin module inverse-function-solve-for
\begin{frame}
%\frametitle{Inverse of a ne-to-one Function}
\vskip -0.2cm
\begin{example}
\begin{columns}
\column{0.35\textwidth}
Find $f^{-1}(x)$ for $\displaystyle f(x) = \frac{e^x-e^{-x}}{e^x+e^{-x}}  $. 
\uncover<18->{\alertNoH{18}{$f=\tanh$ = hyperbolic tangent function.}}

\psset{xunit=0.6cm, yunit=0.6cm}
\begin{pspicture}(-3.05,-3.1)(3.15,3.2)
\psframe*[linecolor=white](-3.05,-3.1)(3.15,3.2)
\tiny
\psaxes[ticks=none, labels=none]{<->}(0,0)(-3.05,-3.1)(3.05,3.1)
\fcLabels{3.05}{3.1}
%Function formula: (679570457/250000000^{x}- (679570457/250000000^{- (x)}))/(679570457/250000000^{- (x)}+679570457/250000000^{x})
\uncover<1-16>{
\rput(-2,-0.5){$y=f(x)$}
\psplot[linecolor=\fcColorGraph, plotpoints=1000]{-3}{3}{2.71828 x -1 mul exp -1 mul 2.71828 x exp add 2.71828 x exp 2.71828 x -1 mul exp add div }
}
\uncover<17->{
\rput(-2,-0.5){$y=f(x)$}
\psplot[linecolor=gray!50, plotpoints=1000]{-3}{3}{2.71828 x -1 mul exp -1 mul 2.71828 x exp add 2.71828 x exp 2.71828 x -1 mul exp add div }
}
%Function formula: 1/2 (\ln{}((1+x)/(1- (x))))
\uncover<17->{
\psline[linestyle=dashed, linecolor=blue](-3, -3)(3,3)
\rput[tl](1.1,2.5){$y=f^{-1}(x)$}
\psplot[linecolor=\fcColorGraph, plotpoints= 1000]{ -0.994}{ 0.994 }{x 1 add x -1 mul 1 add div ln 0.5 mul }
}
\end{pspicture}
\uncover<17->{Final }\uncover<16->{answer}\uncover<17->{, \alertNoH{17}{relabelled}:}
$\displaystyle 
\uncover<16->{
f^{-1}( \only<handout:0|16>{y}\only<17->{\alertNoH{17}{x}} )=\frac12\ln\left( \frac{1+\only<handout:0|16>{y} \only<17->{ \alertNoH{17}{x}} }{1-\only<handout:0|16>{y} \only< 17->{ \alertNoH{17 }{x}}}\right)
}
$
\column{0.65\textwidth}
$ \begin{array}{@{}r@{~}c@{~}l@{}l|l}
\displaystyle \uncover<2->{ \frac{ \alertNoH{3}{e^x}- \alertNoH{4, 5}{e^{-x} } }{ \alertNoH{3}{e^x}+\alertNoH{4,5}{e^{-x}}} &=&y\uncover<3->{ &&\begin{array}{l} \text{Set } \alertNoH{3, 12}{u=e^x} \\\uncover<4->{ \alertNoH{4, 5}{e^{-x}=} \fcAnswer{5}{\frac{1}{e^x}= \frac{1}{u}}} \end{array}}}  \\
\displaystyle\uncover<3->{ \frac{ \left(\alertNoH{3}{ u} -\fcAnswerUncover{3}{5}{\frac{1}{u}}\right)\uncover<6->{\alertNoH{6}{u}} }{\left( \alertNoH{3}{u}+ \fcAnswerUncover{3}{5}{\frac{1}{u}}\right)\uncover<6->{\alertNoH{6}{u}}}&=&y}\\
\displaystyle\uncover<7->{\frac{u^2-1}{\alertNoH{8}{u^2+1}}&=&y}\\
\displaystyle\uncover<8->{ \alertNoH{9}{u^2}- \alertNoH{10}{1} &=&\alertNoH{9,10}{ y}( \alertNoH{8}{ \alertNoH{9}{u^2} +\alertNoH{10 }{1}})}\\
\displaystyle\uncover<9->{\alertNoH{9}{ u^2(\alertNoH{11}{1-y})}&=&\alertNoH{10} {1+y}}\\
\displaystyle\uncover<11->{ {\alertNoH{12}{u}}^2&=&\displaystyle \frac{1+y}{ \alertNoH{11}{1-y} }}\\
\displaystyle \uncover<12->{\left(\alertNoH{12}{e^{\alertNoH{13}{x}}} \right)^{\alertNoH{13}{2}}&=&\displaystyle \frac{1+y}{1-y}}\\
\uncover<13->{\displaystyle e^{\alertNoH{13}{2x}}&=&\displaystyle \frac{1+y}{1-y}}\uncover<14->{ &&\text{Take }\alertNoH{14}{\ln}} \\
\uncover<14->{\displaystyle \uncover<handout:0|14,15>{ \alertNoH{15}{2}} x&=&\displaystyle \uncover<16->{ \alertNoH{16}{\frac{1}{2}}} \alertNoH{14}{\ln} \left(\frac{1+y}{1-y} \right)}\\
\end{array}
$
\end{columns}
\vskip -0.3cm
\end{example}
\end{frame}
% end module inverse-function-solve-for
