Evaluate the definite integral.
\begin{multicols}{3}
\begin{enumerate}[ref={\fcProblemRef}]
\item $\displaystyle \int\limits_{-2}^{3} \left(x^2-1 \right)  \diff x$.

\answer{$\left[ \frac{1}{3} x^{3}- x \right]_{-2}^3=\frac{20}{3}$}

\item $\displaystyle \int\limits_{1}^{2} \left(4x^3+3x^2+2x+1\right)  \diff x$.

\answer{$\left[ x^{4}+x^{3}+x^{2}+x\right]_{1}^{2}=26$}
\item $\displaystyle \int\limits_{0}^{2}(x-1)(x^2+1)  \diff x$.

\answer{$\left[\frac{1}{4} x^{4}-\frac{1}{3} x^{3}+\frac{1}{2} x^{2}- x \right]_{0}^{2} = \frac{4}{3}$}
\item $\displaystyle \int\limits_{-1}^{1} \left( \frac{x(x+1) }{ 2} \right)^2  \diff x$.

\answer{$\left[\frac{1}{20} x^{5}+\frac{1}{8} x^{4}+\frac{1}{12} x^{3} \right]_{-1}^{1}=\frac{4}{15}$}
\item $\displaystyle \int\limits_{0}^{1}(1+x^2)^3 dx$.

\answer{$\left[\frac{1}{7} x^{7}+\frac{3}{5} x^{5} + x^{3} + x \right]_{0}^{1}=\frac{96}{35}$}
\item $\displaystyle \int \limits_{1}^{2} \left(\frac{1}{x} - \frac{4}{x^2} \right)  \diff x$.

\answer{$\left[ 4 x^{-1}+\ln x\right]_{1}^{2}=\ln 2-2$}
\item $\displaystyle \int\limits_{1}^{4}\sqrt{x}(1+x) \diff x$.

\answer{$\left[\frac{2}{5} x^{\frac{5}{2}}+\frac{2}{3} x^{\frac{3}{2}} \right]_{1}^{4}=\frac{256}{15}$}
\item $\displaystyle \int\limits_{1}^{4} \sqrt{ \frac{6 }{x }} \diff x$.

\answer{$\left[2 \sqrt{6} \sqrt{x} \right]_{1}^{4}=-2 \sqrt{6} + (2)^{\frac{3}{2}}$}
\item $\displaystyle \int \limits_{1}^{4} \frac{ \frac{ 1}{ \sqrt{x}}+1+x}{ \sqrt{x}}  \diff x$.

\answer{$\left[ \right]_{}^{}=$}
\item $\displaystyle \int \limits_{1}^{4} \frac{1+x}{ \sqrt[3]{x}} \diff x$.

\answer{$\left[ \right]_{}^{}=$}
\item $\displaystyle \int\limits_{0}^1 \frac{\frac{1}{ \sqrt[3]{x}} +\sqrt[3]{x}}{ \sqrt{x}}\diff x$.

\answer{$\left[ \right]_{}^{}=$}
\item $\displaystyle \int\limits_0^{1} (\sqrt[5]{x^6} + \sqrt[6]{x^5})\diff x $.

\answer{$\left[ \right]_{}^{}=$}
\item $\displaystyle \int\limits_{1}^{2} \left(x + \frac{1}{x} \right)^2 \diff x$.

\answer{$\left[ \right]_{}^{}=$}
\item $\displaystyle \int\limits_{1}^{2} \left(x + \frac{1}{x} \right)^3 \diff x$.

\answer{$\left[ \right]_{}^{}=$}
\item $\displaystyle \int\limits_{1}^{2} \left(\sqrt{x} + \frac{1}{\sqrt{x}} \right)^2 \diff x$.

\answer{$\left[ \right]_{}^{}=$}
\item $\displaystyle \int\limits_{1}^{2} \left(\sqrt{x} +\frac{1}{\sqrt{x}} \right)^3 \diff x$.

\answer{$\left[ \right]_{}^{}=$}
\item $\displaystyle \int\limits_{0}^{2}|x-1| \diff x$.

\answer{$\left[ \right]_{}^{}=$}
\item \label{problemIntegralAbsoluteValuexminushalf} $\displaystyle \int\limits_{0}^{1} \left|x-\frac{1}{2}\right| \diff x$.

\answer{$\frac{1}{4}$}
\item $\displaystyle \int\limits_{-1}^{1}(x-3|x|) \diff x$.

\answer{$\left[ \right]_{}^{}=$}
\item $\displaystyle \int\limits_{\frac{\pi}{4}}^{\frac{\pi}{2}} \csc^2\theta \diff \theta$.

\answer{$\left[ \right]_{}^{}=$}
\item $\displaystyle \int\limits_{0}^{\frac{\pi}{4}}\frac{1-\cos^2\theta}{\cos^2\theta} \diff \theta$.

\answer{$\left[ \right]_{}^{}=$}
\item $\displaystyle \int\limits_{0}^{\frac{\pi}{4}}\frac{\sin^2\theta}{\cos^2\theta} \diff \theta$.

\answer{$\left[ \right]_{}^{}=$}
\item $\displaystyle \int\limits_{0}^{\frac{\pi}{4}}\tan^2\theta \diff \theta$.

\answer{$\left[ \right]_{}^{}=$}
\item $\displaystyle \int\limits_{0}^{\frac{\pi}{3}} \frac{\sin \theta +\sin \theta \tan^2\theta}{\sec^2\theta}\diff \theta$.

\answer{$\left[ \right]_{}^{}=$}
\item $\displaystyle \int\limits_{0}^{\pi} (\sin \theta -\cos \theta) \diff \theta$.

\answer{$\left[ \right]_{}^{}=$}
\item $\displaystyle \int\limits_{0}^{\pi}|\sin x| \diff x$.
\end{enumerate}
\end{multicols}
