\solution{\ref{problemEulerSub-case1-cos(2arctant)-alternative-exposition-x-via-t}.
\[
\begin{array}{rcll|l}
\sqrt{-x^2+1}&=&(1-x)t&&\text{square both sides}\\
(1-x)(1+x)&=&(1-x)^2t^2&&\text{divide by } (1-x)\\
1+x&=&(1-x)t^2\\
x(1+t^2)&=&t^2-1\\
x&=&\displaystyle \frac{t^2-1}{t^2+1}= 1-\frac{2}{t^2+1}\quad .
\end{array}
\]

}

\solution{\ref{problemEulerSub-case1-cos(2arctant)-alternative-exposition-radical-via-t}.

Use Problem \ref{problemEulerSub-case1-cos(2arctant)-alternative-exposition-x-via-t} to get
\[
\sqrt{-x^2+1}=(1-x)t=\left(1-\left(1-\frac{2t}{t^2+1}\right)\right)t= \frac{ 2t}{ t^2+1}\quad .
\]

}


