\solution{\ref{problemEulerSub-case1-sec(2arctant)-alternative-exposition-x-via-t}.

\[
\begin{array}{rcll|l}
\displaystyle \sqrt{x^2-1}&=&\displaystyle (x+1)t&&\text{square both sides}\\
\displaystyle (x-1)(x+1)&=&\displaystyle (x+1)^2t^2&&\text{divide by } (x+1)\\
\displaystyle x-1&=&\displaystyle (x+1)t^2\\
\displaystyle x(1-t^2)&=&\displaystyle 1+t^2\\
\displaystyle x&=& \displaystyle \frac{1+t^2}{1-t^2}= -1+\frac{2}{1-t^2}
\end{array}
\]
}
\solution{\ref{problemEulerSub-case1-sec(2arctant)-alternative-exposition-radical-via-t}. 

Using \ref{problemEulerSub-case1-sec(2arctant)-alternative-exposition-x-via-t} we get
\[
\sqrt{x^2-1}=(x+1)t=\left(-1+\frac{2}{1-t^2}+1\right)t=\frac{2t}{1-t^2}
\]
}