\solution{\ref{problemIntegrate sqrt(2x^2+2x+1)dx}
\[
\begin{array}{@{}r@{}c@{}l@{}l@{}|l}
\displaystyle \int \sqrt{\left(2x^2+2x+1\right)}\diff x &=&\displaystyle  \int \sqrt{2}\sqrt{\left(\left(x+\frac{1}{2}\right)^2+\frac{1}{4}\right)} \diff x &&\text{complete square}\\
&=&\displaystyle  \frac{\sqrt{2}}{2} \int \sqrt{\left( 4 \left( x + \frac{ 1}{2}\right)^2+1\right)}   \diff {}x\\
&=&\displaystyle  \frac{\sqrt{2}}{2}  \int \sqrt{\left( \left( 2x +1\right)^2+ 1\right)} \frac{1}{2}\diff {}\left(2x+1\right) &&\text{Set }u=2x+1 \\
&=&\displaystyle \frac{\sqrt{2}}{4} \int \sqrt{\left(u^2+1\right)}\diff {}u && \begin{array}{@{}l} \text{Euler subst.: } \\ u = \frac{1}{2}\left(\frac{1}{t}-t\right),\\ t> 0 \\~\\ \diff u = -\frac{1}{2}\left(\frac{1}{t^{2}}+1\right)\diff t \\~\\ \sqrt{u^2+1}= \frac{1}{2}\left(\frac{1}{t}+t\right)\\~\\ t= \sqrt{u^2+1}-u \end{array}\\
&=&\displaystyle - \frac{\sqrt{2} }{16} \int\left(\frac{1}{t}+t\right)\left(\frac{1}{t^2}+1 \right) \diff t\\
&=&\displaystyle - \frac{\sqrt{2} }{16} \int \left( t^{-3}+2t^{-1}+t\right)\diff t\\
&=&\displaystyle - \frac{\sqrt{2} }{16}  \left( -\frac{t^{-2}}{2} + 2\ln |t| + \frac{t^2}{2}\right)+C&& \begin{array}{@{}l}
\text{simplify as} \\
\text{in Problem \ref{problemIntegratesqrt(x^2+1)dx}}
\end{array}
\\
&=&\displaystyle \frac{\sqrt{2}}{8} \left( u\sqrt{u^2+1}+ \ln\left(\sqrt{u^2+1}+u \right) \right) +C \\
&=&\displaystyle \frac{\sqrt{2}}{8} \left( (2x+1)\sqrt{(2x+1)^2+1 }\right.\\
&&\displaystyle ~~~~~~ \left.+\ln \left( \sqrt{(2x+1)^2+1 }+2x+1\right) \right)+C.
\end{array}
\]
}