\begin{solution}
We carry out the Euler substitution $t=\sqrt{x^2+1}-x$ given in \eqref{eqEulerSub1.2}. We plug in $\sqrt{x^2+1}=\frac{1}2\left(\frac 1 t +t\right)$, $\diff x=-\frac12 \left(\frac1{t^2} +1\right)\diff t$ to get
\[
\begin{array}{rcl}
\displaystyle\int \sqrt{(x^2+1)}\diff x&=&\displaystyle-\int  \frac14 \left(\frac1t +t\right)\left(\frac 1 {t^2} +1\right)\diff t\\
&=&\displaystyle -\frac 1 4\int \left( \frac{1}{t^3}+ 2\frac{1}t +t\right)\diff t\\
&=&\displaystyle -\frac{1}4 \left(-\frac{t^{-2}}{2}+2\ln|t|+\frac{t^2}2 \right)+C\\
&=&\displaystyle\frac{1}{8} \left(\frac{1}{(\sqrt{x^2+1} - x )^2 }
- (\sqrt{x^2+1}-x)^2\right)\\
&&\displaystyle -\frac12 \ln (\sqrt{x^2+1}-x)+C
\end{array}
\]
The above expression gives a perfectly good answer to the problem. However, the expression $\frac{1}{(\sqrt{x^2 +1}- x)^2 }- (\sqrt{x^2+1}-x)^2$ can be transformed to a simpler looking expression with a little algebra:
\[\begin{array}{rcl}
\displaystyle\frac{1}{(\sqrt{x^2+1}-x)^2}- (\sqrt{x^2+1}-x)^2&=&\displaystyle
\frac{(\sqrt{x^2+1}+x)^2}{(\sqrt{x^2+1}-x)^2  (\sqrt{x^2+1}+x)^2 } \\
&&\displaystyle - (\sqrt{x^2+1}-x)^2 \\
&=&\displaystyle \frac{(\sqrt{x^2+1}+x)^2}{\underbrace{((\sqrt{x^2+1})^2-x^2)^2}_{=1} }- (\sqrt{x^2+1}-x)^2 \\
&=&\displaystyle 4x\sqrt{x^2+1}
\end{array}
\]
The expression $\ln (\sqrt{x^2+1}-x)$ can be transformed to
\[
\ln \left(\frac{(\sqrt{x^2+1}-x)(\sqrt{x^2+1}+x)}{\sqrt{x^2+1}+x}\right)=\ln \left(\frac{1}{\sqrt{x^2+1}+x}\right)= -\ln (\sqrt{x^2+1}+x)
\]
Finally, we get
\[
\begin{array}{rcl}
\displaystyle \int \sqrt{(x^2+1)}\diff x&=&\frac{1}2\left(x\sqrt{x^2+1}+\ln (\sqrt{x^2+1}+x)+C \right)\quad .
\end{array}
\]
\end{solution}


\solution{\ref{problemIntegrate sqrt(2x^2+2x+1)dx}
\[
\begin{array}{@{}r@{}c@{}l@{}l@{}|l}
\displaystyle \int \sqrt{\left(2x^2+2x+1\right)}\diff x &=&\displaystyle  \int \sqrt{2}\sqrt{\left(\left(x+\frac{1}{2}\right)^2+\frac{1}{4}\right)} \diff x &&\text{complete square}\\
&=&\displaystyle  \frac{\sqrt{2}}{2} \int \sqrt{\left( 4 \left( x + \frac{ 1}{2}\right)^2+1\right)}   \diff {}x\\
&=&\displaystyle  \frac{\sqrt{2}}{2}  \int \sqrt{\left( \left( 2x +1\right)^2+ 1\right)} \frac{1}{2}\diff {}\left(2x+1\right) &&\text{Set }u=2x+1 \\
&=&\displaystyle \frac{\sqrt{2}}{4} \int \sqrt{\left(u^2+1\right)}\diff {}u && \begin{array}{@{}l} \text{Euler subst.: } \\ u = \frac{1}{2}\left(\frac{1}{t}-t\right),\\ t> 0 \\~\\ \diff u = -\frac{1}{2}\left(\frac{1}{t^{2}}+1\right)\diff t \\~\\ \sqrt{u^2+1}= \frac{1}{2}\left(\frac{1}{t}+t\right)\\~\\ t= \sqrt{u^2+1}-u \end{array}\\
&=&\displaystyle - \frac{\sqrt{2} }{16} \int\left(\frac{1}{t}+t\right)\left(\frac{1}{t^2}+1 \right) \diff t\\
&=&\displaystyle - \frac{\sqrt{2} }{16} \int \left( t^{-3}+2t^{-1}+t\right)\diff t\\
&=&\displaystyle - \frac{\sqrt{2} }{16}  \left( -\frac{t^{-2}}{2} + 2\ln |t| + \frac{t^2}{2}\right)+C\\
&=& \displaystyle \frac{\sqrt{2}}{4} \left(-\frac{1}{4}\left( -\frac{\left(\sqrt{u^2+1}-u \right)^{-2} }{2} \right.\right.\\
&&\displaystyle ~~~~~~~  +  2\ln \left(\sqrt{u^2+1}-u \right)\\
&&\displaystyle ~~~~~~~  \left.\left.+ \frac{\left(\sqrt{u^2+1}-u \right)^2 }{2}\right)\right)+C&&\text{simplifies by theory}\\
&=&\displaystyle \frac{\sqrt{2}}{4} \left( \frac{1}{2} u\sqrt{u^2+1}+\frac{1}{2}\ln\left(\sqrt{u^2+1}+u \right) \right) +C \\
&=&\displaystyle \frac{\sqrt{2}}{4} \left( \frac{1}{2} (2x+1)\sqrt{(2x+1)^2+1 }\right.\\
&&\displaystyle ~~~~~~ \left.+ \frac{1}{2}\ln \left( \sqrt{(2x+1)^2+1 }+2x+1\right) \right)+C
\end{array}
\]
}