\solution{\ref{problemcompletesquaresqrt(x^2+x+1)}
\[
\begin{array}{rcl}
\displaystyle \sqrt{x^2+x+1}&=&\displaystyle \sqrt{ x^2+2\frac{1}{2}x +\frac{1}{4}-\frac{1}{4} +1} \\
&=&\displaystyle  \sqrt{ \left(x+\frac{1}{2} \right)^2- }\\
&=&\displaystyle \sqrt{\frac{3}{4}\left( \frac{4}{3} \left(x+\frac{1}{2}\right)^2+1 \right)}\\
&=&\displaystyle \frac{\sqrt{3}}{2} \sqrt{\left( \frac{2}{ \sqrt{3}} \left( x+\frac{1}{2}\right)\right)^2+1}\\
&=&\displaystyle \frac{\sqrt{3}}{2} \sqrt{u^2+1},
\end{array}
\]
where $u=\frac{2}{\sqrt{3}}\left( x+\frac{1}{2}\right) = \frac{2 \sqrt{3}}{3}x+\frac{\sqrt{3}}{3}$.
}

\solution{\ref{problemcompletesquaresqrt(-2x^2+x+1)}
\[
\begin{array}{rcl}
\displaystyle \sqrt{-2x^2+x+1}&=&\displaystyle \sqrt{ -2\left( x^2-\frac{1}{2}x -\frac{1}{2}\right) } \\
&=&\displaystyle \sqrt{ -2\left(x^2-2\frac{1}{4}x +\frac{1}{16}-\frac{1}{16}-\frac{1}{2}\right) }\\
&=&\displaystyle \sqrt{-2\left( \left(x- \frac{1}{16} \right)^2 -\frac{9}{16} \right)}\\
&=&\displaystyle  \sqrt{\frac{9}{8}\left(- \frac{16}{9} \left( x-\frac{1}{16}\right)^2+1 \right)}\\
&=&\displaystyle  \frac{3}{\sqrt{8}} \sqrt{-\left( \frac{4}{3} \left(x-\frac{1}{16}\right)\right)^2+1 }\\
&=&\displaystyle \frac{ 3}{\sqrt{8}} \sqrt{-u^2+1}
\end{array}
\]
where $u=\frac{4}{3}\left(x-\frac{1}{16}\right) = \frac{4}{3}x - \frac{1}{12}$.
}