The trigonometric substitution $x=\sin \theta$ is given by
\[
\begin{array}{rcll|l}
\displaystyle \sqrt{-x^2+1}&=&\displaystyle \sqrt{1-\sin^2\theta}\\
&=&\displaystyle \sqrt{\cos^2\theta} &&\begin{array}{l} \text{when }\theta\in\left[-\frac{\pi}{2}, \frac{\pi}{2} \right] \text{we have}\\
\cos \theta\geq 0 \text{ and so } \sqrt{\cos^2\theta}=\cos \theta
\end{array} \\
&=&\displaystyle \cos \theta\quad .
\end{array}
\]
The differential $\diff x$ can be expressed via $\diff \theta$ from $x=\sin \theta$. The substitution $x=\sin \theta $ can be now summarized as:
\begin{equation*}
\begin{array}{rcl}
x&=&\sin \theta\\
\sqrt{-x^2+1}&=&\sin \theta\\
\diff x&=& \cos \theta \diff \theta\\
\theta&=&\arcsin x \quad .
\end{array}
\end{equation*}