The trigonometric substitution $x=\csc \theta$ is given by
\[
\begin{array}{rcll|l}
\displaystyle \sqrt{x^2-1}&=&\displaystyle \sqrt{\frac{1}{\sin^2\theta}-1}\\
&=&\displaystyle \sqrt{\frac{\cos^2\theta}{\sin^2\theta}}=\sqrt{\cot^2 \theta} &&\begin{array}{l} \text{when }\theta\in \theta \in \left[0, \frac{\pi}{2}\right)\cup \left[\pi, \frac{3\pi}{2}\right) \text{we have}\\
\cot \theta\geq 0 \text{ and so } \sqrt{\cot^2\theta}=\tan \theta
\end{array}  \\
&=&\displaystyle \cot \theta\quad .
\end{array}
\]
The differential $\diff x$ can be expressed via $\diff \theta$ from $x=\csc \theta$. The substitution $x=\csc \theta $ can be now summarized as:
\begin{equation*}
\begin{array}{rcl}
x&=&\displaystyle \csc \theta\\
\sqrt{x^2-1}&=&\displaystyle \cot \theta\\
\diff x&=&\displaystyle  -\frac{\cos \theta }{\sin^2 \theta} \diff \theta = -\csc\theta \cot\theta \diff \theta\\
\theta&=&\displaystyle \Arccsc x \quad .
\end{array}
\end{equation*}