% begin module maclaurin-series-e-ex
\begin{frame}
\begin{example}
Find the sum of the series
\abovedisplayskip=0pt
\belowdisplayskip=0pt
\[
\sum_{n=0}^\infty (-1)^n\frac{1}{2^nn!} = 1 - \frac{1}{2\cdot 1!} + \frac{1}{4\cdot 2!} - \frac{1}{8\cdot 3!} + \cdots
\]
\abovedisplayskip=0pt
\belowdisplayskip=0pt
\begin{eqnarray*}
\uncover<2->{%
\alert<handout:0| 2-3>{%
e^{\alert<handout:0| 7>{x}}%
}%
}%
& \uncover<2->{\alert<handout:0| 2-3>{=}} & %
\uncover<2->{%
\alert<handout:0| 2-3>{%
\sum_{n=0}^\infty \uncover<3->{\frac{1}{n!}\alert<handout:0| 6-7>{x^n}}%
}%
}\\%
& & \\%
\uncover<4->{%
\sum_{n=0}^\infty (-1)^n\frac{1}{2^nn!}%
}%
& \uncover<4->{=} & %
\uncover<4->{%
\sum_{n=0}^\infty \frac{1}{n!}\alert<handout:0| 4-7>{ \left( \uncover<5->{-\frac{1}{2}}\right)^n}%
}\\%
& \uncover<7->{=} & %
\uncover<7->{%
e^{\alert<handout:0| 7>{-1/2}}
}\\%
& \uncover<8->{=} & %
\uncover<8->{%
\frac{1}{\sqrt{e}}
}%
\end{eqnarray*}
\end{example}
\end{frame}
% end module maclaurin-series-e-ex
