% begin module power-series-calculus-ex4
\begin{frame}
\begin{example} %[Example 4, p. 766]
Find the derivative of the Bessel function
\abovedisplayskip=0pt
\belowdisplayskip=0pt
\begin{eqnarray*}
J_0(x) & = & \sum_{n=0}^\infty \frac{(-1)^n x^{2n}}{2^{2n}(n!)^2}\\%
\uncover<2->{%
J_0'(x)%
}%
 & \uncover<2->{ = } &%
\uncover<2->{%
\sum_{n=0}^\infty \frac{\diff}{\diff x}\left( \frac{(-1)^n x^{\alert<handout:0| 3>{ 2n}}}{2^{2n}(n!)^2}\right) %
}\\%
 & \uncover<3->{\  = \ } &%
\uncover<3->{%
\sum_{n=0}^\infty \frac{(-1)^n \alert<handout:0| 3>{2n}x^{\alert<handout:0| 3>{ 2n -1}}}{2^{2n}(n!)^2}%
}%
\end{eqnarray*}
\begin{itemize}
\item<4-| alert@4-5>  $J_0(x)$ is defined \uncover<5->{everywhere.}
\item<6->  Therefore its derivative $J_0'(x)$ is also defined everywhere.
\end{itemize}
\end{example}
\end{frame}
% end module power-series-calculus-ex4
