% begin module taylor-series-ex3
\begin{frame}
\begin{example}
Find the Taylor series for $f(x) = e^x$ at $a = 3$.
\begin{itemize}
\item<2-| alert@2-3>  $f^{(n)}(x) = $ \uncover<3->{$e^x$.}
\item<4-| alert@4-6>  $f^{(n)}(3) = $ \uncover<5->{$e^3$.}
\item<6->  Therefore the Taylor series is
\end{itemize}
\uncover<6->{%
\abovedisplayskip=0pt
\belowdisplayskip=0pt
\[
\sum_{n=0}^\infty \frac{\alertNoH{ 6}{f^{(n)}(3)}}{n!}(x-3)^n = \sum_{n=0}^\infty \frac{\alertNoH{ 6}{e^3}}{n!}(x-3)^n %= e^3 + \frac{e^3}{1!}(x-3) + \frac{e^3}{2!}(x-3)^2 + \frac{e^3}{3!}(x-3)^3 + \cdots%
\]
}%
\begin{itemize}
\item<7->  To find the radius of convergence, let $a_n = \frac{e^3}{n!}(x-3)^n$.
\end{itemize}
\abovedisplayskip=0pt
\belowdisplayskip=0pt
%\begin{eqnarray*}
\[
\uncover<8->{%
\lim_{n\to\infty} \left| \frac{a_{n+1}}{a_n}\right|%
}%
 \uncover<8->{ = } %
\uncover<8->{%
\lim_{n\to\infty} \left| \frac{e^3\alertNoH{ 9-10}{(x-3)^{n+1}}}{\alertNoH{ 11-12}{(n+1)!}}\cdot \frac{\alertNoH{ 11-12}{n!}}{e^3\alertNoH{ 9-10}{(x-3)^n}}\right|%
}%
 \uncover<9->{ = } %
\uncover<9->{%
\alertNoH{ 13-14}{\lim_{n\to\infty} \frac{\uncover<10->{\alertNoH{ 10}{|x-3|}}}{\uncover<12->{\alertNoH{ 12}{n+1}}}}%
}%
 \uncover<13->{\alertNoH{ 13-14}{ = }} %
\uncover<14->{%
\alertNoH{ 14}{0}%
}%
% \uncover<15->{\alertNoH{ 15}{ < 1}} %
%\end{eqnarray*}
\]
\begin{itemize}
\item<15->  Therefore by the Ratio Test the series converges for all $x$.
\item<16->  Therefore $R = \infty$.
\item<17->  Just like the Maclaurin series, this series also represents $e^x$.
\end{itemize}
\end{example}
\end{frame}

\begin{frame}
\begin{example}
Find the Taylor series for $f(x) = e^x$ at $a = 3$.
\[
\begin{array}{rcll|l}
\displaystyle \uncover<2->{e^{x}}&\uncover<2->{=}&\displaystyle \uncover<2->{{\alertNoH{3,4}{e}}^{\alertNoH{4}{x-3} + \alertNoH{3}{ 3}}} \uncover<3->{= \alertNoH{3}{e^{3}}\alertNoH{4,6}{e^{x-3}}} \uncover<5->{&& \begin{array}{l} \text{Recall that } \alertNoH{6}{e^y=\sum\limits_{n=0}^\infty \frac{{y}^n}{n!}} \\ \uncover<6->{\text{Set } \alertNoH{6}{y=x-3} }\end{array}} \\
&\uncover<6->{=}&\displaystyle \uncover<6->{\alertNoH{7}{e^3} \alertNoH{6}{\sum\limits_{n=0}^\infty \frac{(x-3)^n}{n!}}}\\
&\uncover<7->{=}&\displaystyle \uncover<7->{\sum\limits_{n=0}^\infty  \frac{\alertNoH{7}{e^3}}{n!}(x-3)^n}
\end{array}
\]

\uncover<8->{The radius of convergence was already computed to be $R=\infty$.}
\end{example}
\vskip 10 cm
\end{frame}
% end module taylor-series-ex3
