% begin module improper-integral-type1-ex3
\begin{frame}
\begin{example}[Example 3, p. 546]
Evaluate $\int_{-\infty}^\infty \frac{1}{1+x^2}\diff x$.
\abovedisplayskip=0pt
\belowdisplayskip=0pt
\uncover<2->{%
\[
\int_{-\infty}^\infty \frac{1}{1+x^2}\diff x = \alert<handout:0| 4-8>{\int_{-\infty}^0 \frac{1}{1+x^2}\diff x} + \alert<handout:0| 9-12>{\int_0^\infty \frac{1}{1+x^2}\diff x}%
\]
}%
\uncover<3->{Evaluate the two integrals separately:}
\begin{eqnarray*}
\uncover<4->{%
\int_{-\infty}^0 \frac{1}{1+x^2}\diff x%
}%
& \uncover<4->{ = } &%
\uncover<4->{%
\lim_{t\rightarrow -\infty} \int_{t}^0 \frac{1}{1+x^2}\diff x%
}%
\uncover<5->{%
 = \lim_{t\rightarrow -\infty} \left[ \tan^{-1} x\right]_t^0%
}\\%
& \uncover<6->{ = } &%
\uncover<6->{%
\lim_{t\rightarrow -\infty} (\tan^{-1} 0 - \tan^{-1} t)%
}%
\uncover<7->{%
 = \lim_{t\rightarrow -\infty}  (0 -\tan^{-1} t) %
}\\%
& \uncover<8->{ = } &%
\uncover<8->{%
0 - \left( -\frac{\pi}{2}\right) = \frac{\pi}{2}%
}\\%
\uncover<4->{%
\int_0^{\infty} \frac{1}{1+x^2}\diff x%
}%
& \uncover<4->{ = } &%
\uncover<4->{%
\lim_{t\rightarrow \infty} \int_{0}^t \frac{1}{1+x^2}\diff x%
}%
\uncover<9->{%
 = \lim_{t\rightarrow \infty} \left[ \tan^{-1} x\right]_0^t%
}\\%
& \uncover<10->{ = } &%
\uncover<10->{%
\lim_{t\rightarrow \infty} (\tan^{-1} t - \tan^{-1} 0)%
}%
\uncover<11->{%
 = \lim_{t\rightarrow \infty} \tan^{-1} t %
}%
\uncover<12->{%
 = \frac{\pi}{2}
}%
\end{eqnarray*}
\uncover<13->{Therefore $\int_{-\infty}^\infty \frac{1}{1+x^2}\diff x = \frac{\pi}{2} + \frac{\pi}{2} = \pi$.}
\end{example}
\end{frame}
% end module improper-integral-type1-ex3
