% begin module FTC-part1-demo
\begin{frame}
\begin{example}[FTC Part 1]
\abovedisplayskip=0pt
\belowdisplayskip=0pt
\abovedisplayshortskip=0pt
\belowdisplayshortskip=0pt
\begin{align*}
\text{If } g(x) & = \int_0^x (\alert<handout:0| 2-3>{e^t} + \alert<handout:0| 4-5>{2t} )\diff t, \text{ find } g'(x).\\
\uncover<2->{g(x)} & \uncover<2->{= \left[ \alert<handout:0| 2-3>{\uncover<3->{e^t}} + \alert<handout:0| 4-5>{\uncover<5->{t^2}} \right]_1^x}\\
 & \uncover<6->{ = ( e^x + x^2) - (e^1 + 1^2)}\\
 & \uncover<7->{ = e^x + x^2 - e - 1.}\\
& \\
\uncover<8->{g'(x)} & \uncover<8->{ = \frac{\diff}{\diff x} ( \alert<handout:0| 9-10>{e^x} + \alert<handout:0| 11-12>{x^2} - \alert<handout:0| 13-14>{e} - \alert<handout:0| 15-16>{1} )}\\
 & \uncover<9->{ =  \alert<handout:0| 9-10>{\uncover<10->{e^x}} + \alert<handout:0| 11-12>{\uncover<12->{2x}} - \alert<handout:0| 13-14>{\uncover<14->{0}} - \alert<handout:0| 15-16>{\uncover<16->{0}} }\\
 & \uncover<17->{ = e^x + 2x.}
\end{align*}
\end{example}
\end{frame}
% end module FTC-part1-demo
