% begin module net-change-intro
\begin{frame}
\begin{itemize}
\item  Part 2 of the Fundamental Theorem says that, if $f$ is continuous on $[a,b]$, then
\abovedisplayskip=0pt
\belowdisplayskip=0pt
\[
\int_a^b f(x)\diff x = F(b) - F(a),
\]
where $F(x)$ is an antiderivative of $f(x)$.
\item  This means $F' = f$, so
\abovedisplayskip=0pt
\belowdisplayskip=0pt
\[
\int_a^b F'(x)\diff x = F(b) - F(a),
\]
\item<2->  $F'(x)$ is the rate of change of $y = F(x)$ with respect to $x$.
\item<3->  $F(b) - F(a)$ is the net change in $y$ as $x$ changes from $a$ to $b$.
\end{itemize}
\uncover<4->{%
\begin{theorem}[The Net Change Theorem]
The integral of the rate of change is the net change:
\[
\int_a^b F'(x) \diff x = F(b) - F(a).
\]
\end{theorem}
}%
\end{frame}
% end module net-change-intro
