% begin module not-product-rule
\begin{frame}
Now we need a formula for the derivative of the product of two functions.  One might guess that the derivative of a product is the product of the derivatives; however, this is wrong.
\uncover<2->{%
\begin{example}[Not the Product Rule]
Let $f(x) = x$ and $g(x) = x^2$.
\abovedisplayskip=0pt
\belowdisplayskip=0pt
\abovedisplayshortskip=0pt
\belowdisplayshortskip=0pt
\begin{align*}
  \alert<handout:0| 3-4>{f'(x)} & \alert<handout:0| 3-4>{ = \uncover<4->{1.}}  %
& \alert<handout:0| 9-10>{(fg)(x)} & \alert<handout:0| 9-10>{ = \uncover<10->{x^3.}}\\%
  \alert<handout:0| 5-6>{g'(x)} & \alert<handout:0| 5-6>{ = \uncover<6->{2x.}}  %
& \alert<handout:0| 11-12>{(fg)'(x)} & \alert<handout:0| 11-12>{ = \uncover<12->{3x^2.}}\\%
  \alert<handout:0| 7-8>{f'(x)g'(x)} & \alert<handout:0| 7-8>{ = \uncover<8->{2x.}}  %
&  & %
\end{align*}
\uncover<13->{%
Therefore $f'(x)g'(x) \neq (fg)'(x)$.%
}%
\end{example}
}%
\uncover<14->{%
The correct formula is called the Product Rule.
}%
\end{frame}
% end module not-product-rule
