% begin module product-rule
\begin{frame}
\begin{theorem}[The Product Rule]
If \alertNoH{13,19}{$f$} and \alertNoH{15}{$g$} are both \alertNoH{13,15,19}{differentiable}, then
\abovedisplayskip=0pt
\belowdisplayskip=0pt
\[
\alertNoH{20}{ \left(f(x)g(x)\right)' =f'(x) g(x)+ f(x) g'(x)}  .
\]
\end{theorem}
\begin{proof}
\uncover<2->{Let $\alertNoH{ 4,20}{F(x) = f(x)g(x)}$.  Then}
\abovedisplayskip=0pt
\belowdisplayskip=-15pt
\abovedisplayshortskip=0pt
\belowdisplayshortskip=0pt
$
\begin{array}{@{}r@{}c@{}l@{}}
\displaystyle \uncover<2->{\alertNoH{20}{F'(x)}  &  = &\displaystyle \uncover<3->{ \lim_{h \rightarrow 0}\frac{F(x+h)-F(x)}{h}}  \uncover<4->{ = \lim_{ h \rightarrow 0}\frac{f(x+h)g(x+h) - f(x)g(x)}{h}}} \\
\uncover<5->{&  = & \displaystyle \lim_{h\rightarrow 0}\frac{\alertNoH{6}{ f(x + h) }\alertNoH{7}{ g(x+h)} \alertNoH{ 5}{\alertNoH{7}{-} \alertNoH{6}{f ( x+ h )}\alertNoH{7}{g(x)} + \alertNoH{9}{f(x+h)}\alertNoH{8}{ g(x)}} \alertNoH{9}{- f(x)}\alertNoH{8}{g(x)}}{\alertNoH{10}{h}}} \\
\uncover<6->{&  = &\displaystyle \lim_{h\rightarrow 0}\left( \alertNoH{6}{ f(x+h)} \frac{\alertNoH{7}{g (x+h)- g(x)}}{\alertNoH{10}{h}} + \alertNoH{8}{g(x)}\frac{\alertNoH{9}{f(x+h)- f(x)}}{\alertNoH{10}{h}}\right)}\\
\uncover<11->{&  = &\displaystyle \alertNoH{ 12-13}{\lim_{h\rightarrow 0}f(x+h)} \alertNoH{ 14-15}{\cdot \lim_{h\rightarrow 0}\frac{g(x+h) - g(x)}{h}}}\\
&&\displaystyle \uncover<11->{ + \alertNoH{ 16-17}{\lim_{h\rightarrow 0}g(x)}\alertNoH{ 18-19}{\cdot\lim_{h\rightarrow 0}\frac{f(x+h)- f(x)}{h}} } %
\alertNoH{20}{ \uncover<12->{ =   \fcAnswerUncover{12}{13}{f (x) }\fcAnswerUncover{12}{ 15}{g'(x)}  + \fcAnswerUncover{12}{ 17}{g(x)} \fcAnswerUncover{12}{ 19}{f'(x) .} }}  \uncover<20->{\!\!\!\mbox{\qedhere}}
\end{array}
$
\end{proof}
\end{frame}
% end module product-rule
