%begin module Euler-substitution
\begin{frame}
\frametitle{Euler substitution to handle $\sqrt{x^2+1} $}
\begin{itemize}
\item<1-> Suppose we want to integrate 
\[
\int R(x, \sqrt{x^2+1})\diff x\quad .
\]
\only<2-9>{
\item<2-> Substitute $\alert<9>{\sqrt{x^2+1}= x+t }$. 
\item<3-> How is this a substitution of $x$ via t?
\uncover<4->{ Square both sides: 
\[
\begin{array}{rcl}
x^2+1&=&x^2+2xt+t^2\\
\uncover<5->{2xt&=&1-t^2}\\
\uncover<6->{\alert<9>{x}&\alert<9>{=}& \alert<9>{\frac12\left(\frac{1}{t}- t\right)}}
\end{array}
\]
}
\item<7-> Take differentials on both sides:
\[
\alert<9>{\diff x}=\frac12 \diff \left(\left(\frac{1}{t}- t\right)\right)\uncover<8->{\alert<9>{= -\frac12\left(\frac{1}{t^2}+1\right) dt}}
\] 
}
\end{itemize}
\uncover<10->{
\begin{definition}
The Euler substitution for $\sqrt{x^2+1} $ is the substitution given by
\[
\begin{array}{rcl}
\displaystyle\alert<10>{\sqrt{x^2+1}}&\alert<10>{=}&\displaystyle \alert<10>{\frac12 \left(\frac1t +t\right)} \\
\displaystyle\alert<10>{x}&\alert<10>{=}&\displaystyle \alert<10>{ \frac12 \left(\frac{1}{t}- t\right)} \\
\displaystyle \alert<10>{\diff x}&\alert<10>{=}&\displaystyle \alert<10>{ -\frac12\left(\frac{1}{t^2}+1\right) dt}
\quad .
\end{array}
\]
\end{definition}
}
\vspace{10cm}
\end{frame}
\begin{frame}
\frametitle{Euler substitution to handle $\sqrt{-x^2+1} $}
\begin{itemize}
\item<1-> Suppose we want to integrate 
\[
\int R(x, \sqrt{-x^2+1})\diff x\quad .
\]

\item<2-> Substitute $\alert<9>{\sqrt{-x^2+1}=(x-1)t }$. 
\item<3-> How is this a substitution of $x$ via t?
\uncover<4->{
\[
\begin{array}{rcll|l}
-(x-1)(1+x)&=&(x-1)^2t^2&&\text{divide by }x-1\\
\uncover<5->{x&=&1-\frac{2}{t^2+1}\quad .}
\end{array}
\] 
\item 
\[
\diff x=\frac{4t}{(1+t^2)^2}dt
\quad .
\] 
}
\end{itemize}
\begin{definition}
The Euler substitution for $\sqrt{x^2+1}$ is the substitution given by:
\[
\begin{array}{rcl}
\sqrt{-x^2+1}&=&-\frac{2t}{t^2+1}\\
x&=&1-\frac{2}{t^2+1}\\
\diff x&=&\frac{4t}{(t^2+1)^2}dt\quad .
\end{array}
\] 
\end{definition}
\end{frame}
\begin{frame}
Case $\sqrt{x^2-1} $. Substitute $\sqrt{x^2-1}=(x-1)t$. Squaring both sides and dividing out by $(x-1)$ we get $x+1=(x-1)t^2$ or $x=\frac{t^2-1+2}{t^2-1}= 1+\frac{2}{t^2-1}$. Therefore $\diff x=\frac{-4t}{(t^2-1)^2}dt$. To summarize:
\[
\begin{array}{rcl}
\diff x&=&\frac{-4t}{(t^2-1)^2}dt\\
\sqrt{-x^2+1}&=&\frac{2t}{t^2-1} \\
x&=&1+\frac{2}{t^2-1}\quad .
\end{array}
\] 
\end{frame}
%end module Euler-substitution