%begin module Euler-substitution-case-2
\begin{frame}
\frametitle{Euler substitution to handle $\sqrt{-x^2+1} $}
\begin{itemize}
\item<1-> Suppose we want to integrate 
\[
\int R(x, \sqrt{-x^2+1})\diff x\quad .
\]
\only<2-15>{
\item<2-> Substitute $\alert<9,15>{\sqrt{-x^2+1}}=(1-\alert<11>{x})t  \uncover<11->{ =\left( 1 -\alert<11>{ \left(1-\frac{2}{ t^2+1} \right)} \right)t =\alert<15>{\frac{2t}{t^2+1}}}$. 
\item<3-> How is this a substitution of $x$ via t?
\uncover<4->{
\[
\begin{array}{rcll|l}
\sqrt{-x^2+1}&=&(1-x)t&&\text{square}\\
\uncover<5->{(1-x)(1+x)&=&(1-x)^2t^2&&\text{divide by }1-x}\\
\uncover<6->{1+x&=&(1-x)t^2}\\
\uncover<7->{xt^2+x &=&t^2-1}\\
\uncover<8->{x(t^2+1) &=&t^2-1 &&\text{divide by }t^2+1}\\
\uncover<9->{\alert<11,12,15>{x}&\alert<11,15>{=}& \frac{  t^2\uncover<10->{+1-1}-1}{t^2+1} \uncover<10->{ = \alert<11,12,15>{1 -\frac{2}{ t^2+1} }\quad .}}
\end{array}
\] 
\item<12-> 
\[
\alert<12,15>{\diff x =} \alert<12,13,14>{ \diff \left(1-\frac{2}{t^2+1}\right)} \uncover<13->{\alert<13,14,15>{=}}\only<13>{\alert<13>{\textbf{?}}} \uncover<14->{\alert<14,15>{ \frac{4t}{(1+t^2)^2}dt} \quad .}
 {~~~~~~~~~~~~~~~~~~~~~~~~~~~~~~~~~~~~~~~~~~~~~~~~~~~~}
\] 
}
}
\end{itemize}
\uncover<16->{
\begin{definition}
The Euler substitution for $\sqrt{-x^2+1}$ is the substitution given by:
\[
\begin{array}{rcl}
\displaystyle \alert<16>{\sqrt{-x^2+1}}&\alert<16>{=}& \displaystyle  \alert<16>{\frac{2t}{t^2+1}}\\
\displaystyle  \alert<16>{x}&\alert<16>{=}&\displaystyle  \alert<16>{1-\frac{2}{t^2+1}}\\
\displaystyle \alert<16>{\diff x }&\alert<16>{=} & \displaystyle  \alert<16>{\frac{4t}{(t^2+1)^2}dt }\quad .
\end{array}
\] 
\end{definition}
}
\vspace{5cm}
\end{frame}
%end module Euler-substitution-case-2