\begin{frame}
\begin{definition}[Completing the square]
Let $a\neq 0$. \alertNoH{13}{To \emph{complete the square} means} to carry out the following algebraic manipulation.
$
\begin{array}{@{\!\!}r@{}c@{}l@{}l|l}
\displaystyle \alertNoH{13}{ \alertNoH{2}{ax^2}+\alertNoH{3}{b} x+c } \uncover<2->{&\alertNoH{0}{=}&\displaystyle  \alertNoH{2,3}{a}\left( \alertNoH{2}{x^2}+ \alertNoH{3}{\frac{b}{a}}x \right)+c }\\
\uncover<4->{&\alertNoH{0}{=}&\displaystyle  a\! \left(x^{2}+\alertNoH{4}{2}\cdot \alertNoH{6}{\frac{b}{\alertNoH{4}{2}a}} x \right) +c}\\
\uncover<5->{&\alertNoH{0}{=}&\displaystyle  a\left( \! \alertNoH{7}{\alertNoH{8}{x}^{2}+2\alertNoH{9}{ \frac{ b }{ 2 a}} \alertNoH{8}{x} \alertNoH{5}{+{\left( \uncover<6->{\alertNoH{6, 9}{\frac{ b}{2a}}}\right)}^2}}\! \!\alertNoH{5}{- \alertNoH{10}{{\left( \uncover<6->{\alertNoH{6}{\frac{ b}{2 a}}}\right)}^2}} \right)+c} \uncover<5->{&& \begin{array}{@{}l} \text{\alertNoH{5}{Add \& subtract}} \\ {\left( \uncover<6->{\alertNoH{6}{ \frac{ b}{2a}}}\right)}^2\end{array}} \\
\uncover<7->{&\alertNoH{0}{=}&\displaystyle \alertNoH{11}{ a} \left( \alertNoH{7}{\left(\alertNoH{8}{x}+ \alertNoH{9}{\frac{ b}{2 a}}\right)^2} -\alertNoH{10}{\frac{b^2}{4a^2}} \right)+c &&\begin{array}{@{}l} \alertNoH{7}{\text{use }}\\ \alertNoH{7}{(\alertNoH{8}{A}+\alertNoH{9}{B})^2=}\\ \alertNoH{7}{\alertNoH{8}{A}^2+2\alertNoH{8}{A}\alertNoH{9}{B}+\alertNoH{9}{B}^2} \end{array}}\\
\uncover<11->{&\alertNoH{0}{=}&\displaystyle  \alertNoH{11}{a} \left(x +\frac{b}{2a}\right)^2 - \fcCancel{12}{\alertNoH{11}{a}} \cdot \frac{b^2}{4a^{\fcCancel{12}{2}}} +c} \\
\uncover<12->{&\alertNoH{13}{=}&\displaystyle  \alertNoH{13}{a\left(x +\frac{ b}{2a}\right)^2 + c-  \frac{b^2}{4a}}}.
\end{array}
$

\end{definition}

\end{frame}