\begin{frame}
\begin{example}[Completing the square]
Complete the square. 
\[
\begin{array}{rcl}
\displaystyle 3x^2-5x+1\uncover<2->{&=&\displaystyle 3\left(x^2- \fcAnswer{3}{ \frac{5}{3}}x  \right) +1}\\
\uncover<4->{&=&\displaystyle 3\left(x^2- \alertNoH{4}{2}\cdot \frac{5}{ \alertNoH{5}{\alertNoH{4}{2}\cdot 3}}x \right)+1}\\
\uncover<5->{&=&\displaystyle 3\left(\alertNoH{8,9}{ x^2- 2\cdot \frac{5}{\alertNoH{5}{6}} x+ \fcAnswerUncover{5}{7}{\left( \frac{5}{6}\right)^2}} - \fcAnswerUncover{5}{7}{\alertNoH{10,11}{ \left( \frac{5 }{ 6}\right)^2}}  \right)+1}\\
\uncover<8->{&=& \displaystyle \alertNoH{12,13,14}{3} \left(\fcAnswer{9}{\left( x-\frac{5}{ 6}\right)^2} -\fcAnswerUncover{8}{11}{\frac{25}{\alertNoH{13}{36}}} \right)+1} \\
\uncover<12->{&=& \displaystyle \alertNoH{12}{3}\left( x-\frac{5}{ 6}\right)^2 \alertNoH{14,15}{-\frac{25}{\alertNoH{13}{12}} +1 }} \\
\uncover<14->{&=& \displaystyle 3\left( x-\frac{5}{ 6}\right)^2 \fcAnswer{15}{-\frac{13}{12}.}} 
\end{array}
\]
\end{example}
\end{frame}