\begin{frame}
\uncover<6->{
\begin{definition}[Discriminant of quadratic function]
The quantity $\alertNoH{6}{D=b^2-4ac}$ is called the \emph{discriminant} of the quadratic function $ax^2+bx+c$.
\end{definition}
}
Let $a\neq 0$ and let $f(x)=ax^2+bx+c$. Then we have the equality 
\[\begin{array}{rcll|l}
\alertNoH{7}{f(x)}&\alertNoH{0}{=}&\displaystyle \uncover<2->{a\left(x\alertNoH{3}{+} \frac{b}{2 a}\right)^2+ \alertNoH{5}{c} \alertNoH{4}{-} \frac{\alertNoH{4}{b^2 }}{4 a } &&\text{complete the square}}\\
\uncover<3->{&\alertNoH{0}{=}&\displaystyle a\left(x\alertNoH{3}{-} \left( \alertNoH{3}{-} \frac{b}{ 2 a}\right) \right)^2 \alertNoH{4, 5}{-} \frac{ \alertNoH{6}{ \alertNoH{4}{ b^2} \alertNoH{5}{- 4ac}}}{\alertNoH{5}{4a}}} \\
\uncover<6->{&\alertNoH{7}{=}&\displaystyle \alertNoH{7}{ a\left(x- \left( \alertNoH{8}{ - \frac{b }{2a}} \right) \right)^2\alertNoH{9}{ -\frac{\alertNoH{6}{D}}{4a}}}.}
\end{array}
\]
\uncover<7->{
\begin{definition}
The expression $\alertNoH{7}{f(x)=a(x-\alertNoH{8}{h})^2+\alertNoH{9}{k}}$, where $\alertNoH{8}{h=-\frac{b}{2a}}$ and $\alertNoH{9}{ k=- \frac{D}{4a} =-\frac{ b^2- 4a c}{4a}}$ is called the standard form of $ax^2+bx+c$.
\end{definition}
}
\end{frame}