\begin{frame}
\hfil\hfil $ax^2+bx+c=a\left( x- x_1\right)\left(x-x_2\right),\quad\quad\quad\quad \left|\begin{array}{rcl}
x_1x_2&=&\displaystyle \frac{c}{a}\\
x_1+x_2&=&\displaystyle-\frac{b}{a}
\end{array}\right.
$
\vskip -0.05cm
\begin{example}
Factor the quadratic.

\hfil\hfil$
x^2+\alertNoH{9}{3} x+\alertNoH{2,10}{1} \uncover<2->{ = \left(x\uncover<1-12>{+} \alertNoH{2}{ \fcAnswerUncover{2}{13}{- \left(\frac{ -3 + \sqrt{5 }}{2}\right) }} \right) \left( x \uncover<1-12>{+} \alertNoH{2}{ \fcAnswerUncover{2 }{13}{ -\left(\frac{ -3 - \sqrt{5 }}{2}\right) }}\right)}
$
\begin{itemize}
\item<2-> The product of the two roots: $\alertNoH{2,3}{x_1x_2=1}$.
\item<3-> Integer options: $\alertNoH{3,4}{ x_1=1, x_2=1}$ and $\alertNoH{3,5}{x_1=-1,x_2=-1}$.
\item<4-> $\begin{array}{rcl}
(x\alertNoH{4}{-1})(x\alertNoH{4}{-1})\uncover<6->{&=&(x-1)^2=x^2-2x+1}\\
(x+\alertNoH{5}{1})(x+\alertNoH{5}{1})\uncover<6->{&=&(x+1)^2=x^2+2x+1}
\end{array}$ \uncover<6->{both don't work.}
\item<7-> $\Rightarrow$ No easy factorization; must use quadratic formula.
$
\begin{array}{rcl}
\alertNoH{12,13}{x_1,x_2} &=&\displaystyle \frac{-\alertNoH{9}{ b}\pm \sqrt{{\alertNoH{9}{ b}}^2- 4{\alertNoH{8}{a} }\alertNoH{10 }{c}}}{2 {\alertNoH{8}{ a} }} \uncover<8->{ = \frac{- \alertNoH{9}{ 3} \pm \sqrt{\alertNoH{11}{ {\alertNoH{9}{3}}^2 -4 \cdot \alertNoH{8}{1 }\cdot \alertNoH{10}{1}}}}{ 2\cdot \alertNoH{8}{1}}}\\
\uncover<11->{&=&\displaystyle \alertNoH{12,13}{ \frac{ -3 \pm \sqrt{\alertNoH{11}{5 }}}{2}}}
\end{array}
$
\end{itemize}
\end{example}
\end{frame}