%begin module differentials-rules
\begin{frame}
\begin{itemize}
\item All rules for computing with derivatives have analogues for computing with differential forms.
\item<2-> The rules for computing differential forms are a direct consequence of the corresponding derivative rules and the transformation law $\diff (f(x))=f'(x)\diff x$.
\end{itemize}
\end{frame}
\begin{frame}
\uncover<3->{Let $c$ be a constant.} \uncover<handout:0| 1->{Rule name: \phantom{p}}
\only<handout:0|1,2>{\alertNoH{1,2}{product rule. }}
\only<handout:0|3,4>{\alertNoH{3,4}{constant derivative rule. }}
\only<handout:0|7,8>{\alertNoH{7,8}{sum rule. }}
\only<handout:0|9,10>{\alertNoH{9,10}{chain rule. }}
\only<handout:0|11-12>{\alertNoH{11-12}{power rule. }}
\only<handout:0|13-14>{\alertNoH{13-14}{exponent derivative rule. }}
%\only<5,6>{\alertNoH{5,6}{ Constant derivative rule. }}
\only<handout:0|22>{\alertNoH{22}{Integration by parts.}}
\only<handout:0|23>{\alertNoH{23}{Integration is linear.}}
\only<handout:0|24>{\alertNoH{24}{Substitution rule.}}

\uncover<handout:2|21->{Corresponding \alertNoH{21}{integration rules.} \uncover<handout:2|25->{\alertNoH{25}{ Integration rules justified via the Fundamental Theorem of Calculus}}}

\begin{tabular}{ll}
\only<handout:1|1-20>{Differential}\only<handout:2|21->{\alertNoH{21}{Integration}} rule & Derivative rule \\
\uncover<2->{\alertNoH{22}{$\uncover<handout:2|21->{\alertNoH{21}{\int}} \diff (fg)=\uncover<handout:2| 21->{ \alertNoH{21}{ \int }} g \diff f +\uncover<handout:2| 21->{ \alertNoH{21}{ \int }} f \diff g$} }&
\uncover<1->{$ (fg)'=f'g +f g'$} \\
\uncover<4->{$\uncover<handout:2|21->{\alertNoH{21}{\int}}\diff c= 0$} &
\uncover<3->{$(c)'=0$}\\
\uncover<6->{\alertNoH{23}{$\uncover<handout:2|21->{\alertNoH{21}{\int}}\diff (cf)=c \uncover<handout:2|21-> {\alertNoH{21}{\int}}\diff f $}} &
\uncover<5->{$(cf)'=cf'$} \\
\uncover<8->{\alertNoH{23}{$\uncover<handout:2|21->{\alertNoH{21}{\int}}\diff (f+g) = \uncover<handout:2|21->{\alertNoH{21}{\int}}\diff f +\uncover<handout:2|21->{\alertNoH{21}{\int}}\diff g$}} &
\uncover<7->{$(f+g)'=f'+g'$}\\
\uncover<10->{\alertNoH{24}{$\uncover<handout:2|21->{\alertNoH{21}{\int}}\diff f(g(x))=$ $ \uncover<handout:2|21->{\alertNoH{21}{\int}}f'(g(x))\diff g(x) $} }\\
\uncover<10->{\alertNoH{24}{$\phantom{\int \diff f(g(x))}= $  $\uncover<handout:2|21->{\alertNoH{21}{\int}} f'(g(x))g'(x)\diff x$} } &
\uncover<9->{$(f(g(x)))'= f'(g(x))g'(x)$} \\
\uncover<10->{\alertNoH{24}{$\uncover<handout:2|21->{\alertNoH{21}{\int}} \diff f(g)\phantom{(x)}= \uncover<handout:2|21->{\alertNoH{21}{\int}} f'(g) \diff g$} } \\\hline
\uncover<12->{$\diff  x^n= nx^{n-1}\diff x$} &
\uncover<11->{$(x^n)'=nx^{n-1}$}\\
\uncover<14->{$\diff  e^x= e^x \diff x$} &
\uncover<13->{$\left(e^x\right)'=e^x$}\\
\uncover<16->{$\diff \sin x = \cos x \diff x$} &
\uncover<15->{$(\sin x)'= \cos x$}\\
\uncover<18->{$\diff \cos x = -\sin x \diff x$} &
\uncover<17->{$(\cos x)'= -\sin x$}\\
\uncover<20->{$\displaystyle \diff \ln x=\frac{1}{x}\diff x$} &
\uncover<19->{$(\ln x)'=\displaystyle \frac1x$}\\
\end{tabular}


\end{frame}
%end module differentials-rules
