%begin module differentials-rules
\begin{frame}
\begin{itemize}
\item All rules for computing with derivatives have analogues for computing with differential forms.
\item<2-> The rules for computing differential forms are a direct consequence of the corresponding derivative rules and the transformation law $\diff (f(x))=f'(x)\diff x$.
\end{itemize}
\end{frame}
\begin{frame}
\uncover<3->{Let $c$ be a constant.} Rule name: \phantom{p}
\only<1,2>{\alert<1,2>{product rule. }}
\only<3,4>{\alert<3,4>{constant derivative rule. }}
\only<7,8>{\alert<7,8>{sum rule. }}
\only<9,10>{\alert<9,10>{chain rule. }}
\only<11-12>{\alert<11-12>{power rule. }}
\only<13-14>{\alert<13-14>{exponent derivative rule. }}
%\only<5,6>{\alert<5,6>{ Constant derivative rule. }}

\begin{tabular}{lll}
Differential rule & Derivative rule\\
\uncover<2->{$\diff (fg)=g \diff f +f \diff g$} & 
\uncover<1->{$(fg)'=f'g +f g'$} \\
\uncover<4->{$\diff c=0$} &
\uncover<3->{$(c)'=0$} & $c$-const.\\
\uncover<6->{$\diff (cf)=c\diff f $} & 
\uncover<5->{$(cf)'=cf'$} &$c$-const. \\
\uncover<8->{$\diff (f+g)=\diff f +\diff g$} & 
\uncover<7->{$(f+g)'=f'+g'$}\\
\uncover<10->{$\diff f(g(x))=$ $ f'(g(x))\diff g(x) $}\\
\uncover<10->{$\phantom{\diff f(g(x))}=$ $ f'(g(x))g'(x)\diff x$} & 
\uncover<9->{$(f(g(x)))'= f'(g(x))g'(x)$} \\ 
\uncover<10->{$\diff f(g)\phantom{(x)}=f'(g)\diff g$} \\\hline
\uncover<12->{$\diff \left( x^n\right)= nx^{n-1}\diff x$} & 
\uncover<11->{$(x^n)'=nx^{n-1}$}\\
\uncover<14->{$\diff  e^x= e^x \diff x$} & 
\uncover<13->{$\left(e^x\right)'=e^x$}\\
\uncover<16->{$\diff \sin x = \cos x \diff x$} & 
\uncover<15->{$(\sin x)'= \cos x$}\\
\uncover<18->{$\diff \cos x = -\sin x \diff x$} & 
\uncover<17->{$(\cos x)'= -\sin x$}\\
\uncover<20->{$\displaystyle \diff \ln x=\frac{1}{x}\diff x$} & 
\uncover<19->{$\left(\ln x\right)' =\displaystyle \frac1x$}\\
\end{tabular}


\end{frame}
%end module differentials-rules