\begin{frame}
\frametitle{Differentiation Rules}
Component-wise operation $\Longrightarrow$ same rules as for scalar output\\
  \pause Product Rules:
   \begin{align*}
   [f(t) \fcv{r}(t)]' & = f'(t) \fcv{r}(t) + f(t) \fcv{r}'(t) \\
   %
   [\fcv{u}(t)\cdot \fcv{v}(t)]' & = \fcv{u}'(t)\cdot \fcv{v}(t) + \fcv{u}(t)
\cdot \fcv{v}'(t) \\
   %
   [\fcv{u}(t)\times \fcv{v}(t)]' & = \fcv{u}'(t) \times \fcv{v}(t) +
\fcv{u}(t)\times \fcv{v}'(t)
 \end{align*}
  \pause Chain Rule:
  $$[\fcv{r}(f(t))]' = f'(t) \fcv{r}'(f(t))$$
    \pause Example:
    $$\frac{\diff |\fcv{r}(t)|}{\diff t} =
    [\sqrt{\fcv{r}(t)\cdot \fcv{r}(t)}]' = [\sqrt{\Box}]' =
    \frac{1}{2\sqrt{\Box}} \Box' =
    \frac{1}{2\sqrt{\fcv{r}(t)\cdot \fcv{r}(t)}}
    [\fcv{r}(t)\cdot \fcv{r}(t)]' = $$
    $$= \frac{1}{2|\fcv{r}(t)|}
    [\fcv{r}'(t)\cdot \fcv{r}(t) +
    \fcv{r}(t)\cdot \fcv{r}'(t)] = \frac{\fcv{r}(t)\cdot \fcv{r}'(t)}{|\fcv{r}(t)|}$$
\end{frame}