\begin{frame}
Recall $C:\left|\begin{array}{rcl}x&=&\onlyNoH{1}{f}\only<2->{\alertNoH{2}{x}}(t)\\y&=& \onlyNoH{1}{g}\only<2->{\alertNoH{2}{y}}(t)\end{array} \right., t\in [a,b]$, tangent vector at $t$ is $(\onlyNoH{1}{f}\only<2->{\alertNoH{2}{x}}'(t), \onlyNoH{1}{g}\only<2->{\alertNoH{2}{y}}'(t))$. \uncover<2->{We write informally $\alertNoH{2}{x=x(t)}, \alertNoH{2}{y=y(t)}$ to simplify notation.}

\begin{itemize}
\item<3-> Suppose we could eliminate the parameter $t$ and write $y=F(x)$ for some function $F$ near the point $(x,y)=(x(t), y(t))$. 
\item<4-> Suppose in $x'(t)\neq 0$ for some $t$. 
\uncover<5->{
\[
\begin{array}{rcll|l}
\displaystyle y&=&\displaystyle  F(x) &&\text{apply } \frac{\diff }{\diff t}\\
\displaystyle \frac{\diff y}{\diff t}&=&\displaystyle \frac{\diff} {\diff t} \left(F(x)\right)&&\text{use chain rule}\\
&=&\displaystyle  \frac{\diff F}{\diff x} \frac{\diff x}{\diff t}=\frac{\diff y}{\diff  x} \frac{\diff x}{\diff t} &&\text{divide by } x'(t)\\
\displaystyle \frac{\diff y}{\diff x} &=&\displaystyle  \frac{\frac{\diff y}{\diff t} }{\frac{\diff x}{\diff t}}
\end{array}
\] 
}
\end{itemize}
\begin{observation}
If $\frac{\diff x}{\diff t}\neq 0$, we have $\displaystyle \frac{ \diff y}{ \diff x}= \frac{\frac{\diff y}{\diff t}}{\frac{\diff x}{\diff t}}\quad .
$
\end{observation}
\end{frame}
% begin module parametric-tangents-intro-version2
