% begin module parametric-tangents-intro-version2
\begin{frame}
\frametitle{Tangents}
Let $C $ be the curve $C:\left|\begin{array}{rcl}x&=&f(t)\\y&=&g(t)\end{array} \right., t\in [a,b]$.
\begin{definition}
Suppose \alert<4,5>{ $f'(t)$ and $g'(t)$ are not simultaneously equal to $0$.} 
\begin{itemize}
\item  We define $(f'(t), g'(t))$ to be the \emph{tangent vector} to $C$ at $t$.
\item<2->  We define the line passing through $(f(t), g(t))$ with direction vector equal to the tangent vector to be \emph{tangent line} to $C$ at $t$. In other words, the tangent line has equation
\[
(x-f(t))g'(t) =(y-g(t))f'(t)\quad .
\]
\item<3->  We say that the tangent to $C$ at $t$ is vertical if $f'(t)=0$ (\alert<4>{and therefore $g'(t)\neq 0$}).
\end{itemize}
\end{definition}
\uncover<5->{\alert<5->{Note.} When $f'(t)=g'(t)=0$, for curves $C$ with additional properties, natural definition(s) of tangent(s) do exist but are beyond Calc II.}
\end{frame}
\begin{frame}
\begin{example}

\end{example}
\end{frame}

\begin{frame}
Recall $C:\left|\begin{array}{rcl}x&=&\onlyNoH{1}{f}\only<2->{\alertNoH{2}{x}}(t)\\y&=& \onlyNoH{1}{g}\only<2->{\alertNoH{2}{y}}(t)\end{array} \right., t\in [a,b]$, tangent vector at $t$ is $(\onlyNoH{1}{f}\only<2->{\alertNoH{2}{x}}'(t), \onlyNoH{1}{g}\only<2->{\alertNoH{2}{y}}'(t))$. \uncover<2->{We write informally $\alertNoH{2}{x=x(t)}, \alertNoH{2}{y=y(t)}$ to simplify notation.}

\begin{itemize}
\item<3-> Suppose we could eliminate the parameter $t$ and write $y=F(x)$ for some function $F$ near the point $(x,y)=(x(t), y(t))$. 
\item<4-> Suppose in $x'(t)\neq 0$ for some $t$. 
\uncover<5->{
\[
\begin{array}{rcll|l}
\displaystyle y&=&\displaystyle  F(x) &&\text{apply } \frac{\diff }{\diff t}\\
\displaystyle \frac{\diff y}{\diff t}&=&\displaystyle \frac{\diff} {\diff t} \left(F(x)\right)&&\text{use chain rule}\\
&=&\displaystyle  \frac{\diff F}{\diff x} \frac{\diff x}{\diff t}=\frac{\diff y}{\diff  x} \frac{\diff x}{\diff t} &&\text{divide by } x'(t)\\
\displaystyle \frac{\diff y}{\diff x} &=&\displaystyle  \frac{\frac{\diff y}{\diff t} }{\frac{\diff x}{\diff t}}
\end{array}
\] 
}
\end{itemize}
\begin{observation}
If $\frac{\diff x}{\diff t}\neq 0$, we have $\displaystyle \frac{ \diff y}{ \diff x}= \frac{\frac{\diff y}{\diff t}}{\frac{\diff x}{\diff t}}\quad .
$
\end{observation}
\end{frame}
% begin module parametric-tangents-intro-version2
