\begin{frame}[t]
\vskip -0.4cm
\begin{columns}[T]
\column{0.2\textwidth}
\psset{xunit=0.4cm, yunit=0.4cm}
\begin{pspicture}(-2,-4.4)(4.4,4.45)%
\tiny%
\newcommand{\tangentWidth}{1pt}%
\newcommand{\tangentColor}{black}%
\fcAxesStandard{-2}{-4.4}{4.4}{4.4}%
\pstVerb{%
40 dict begin /stickingCoeffOne 1.2 def /stickingCoeffTwo -0.2 def  /coeffA 0.2 def /coeffB 1.2 def /theFun {x x x mul mul x coeffA mul coeffB add add sqrt} def%
}%
\pstVerb{%
/xOne -1 def %
/xTwo 0 def %
}%
\pstVerb{%
%Input: xA yA xB yB. Let (xA, yA) * (xB, yB) = (xC, yC). 
%This function outputs xC, and the next function outputs yC.
/xNew {
20 dict begin /a coeffA def /b coeffB def
/yB exch def /xB exch def /yA exch def /xA exch def 
b 2 1 div mul xA a mul add xB a mul add yB yA mul -2 1 div mul add xB 2 1 div exp xA mul add xB xA 2 1 div exp mul add xB xA mul -2 1 div mul xA 2 1 div exp add xB 2 1 div exp add div
end
} def %
/yNew {
20 dict begin /a coeffA def /b coeffB def
/yB exch def /xB exch def /yA exch def /xA exch def 
yA b mul 2 1 div mul yB b mul -4 1 div mul add b yA mul 2 1 div mul add yA xA mul a mul add yB xA mul a mul -3 1 div mul add yA xB mul a mul add yB xB mul a mul -1 1 div mul add xB a mul yA mul 2 1 div mul add xB 3 1 div exp yA mul 2 1 div mul add yB xA 3 1 div exp mul -1 1 div mul add yA xB 3 1 div exp mul -1 1 div mul add yA xB 2 1 div exp mul xA mul 3 1 div mul add yB xB mul xA 2 1 div exp mul -3 1 div mul add xA 3 1 div exp -1 1 div mul xB 3 1 div exp add xB 2 1 div exp xA mul -3 1 div mul add xB xA 2 1 div exp mul 3 1 div mul add div
end
} def %
/yOne 1 dict begin /x xOne def theFun end def%
/yTwo 1 dict begin /x xTwo def theFun end def%
}%
\psplot[linecolor=\fcColorGraph, plotpoints = 300]{-1}{2.5}{theFun}%
\psplot[linecolor=\fcColorGraph, plotpoints = 300]{-1}{2.5}{theFun -1 mul}%
\pstVerb{%
/xThree xOne yOne xTwo yTwo xNew def%
/yThree xOne yOne xTwo yTwo yNew def%
}%
\psline[linewidth=\tangentWidth, linecolor=\tangentColor](!%
xOne stickingCoeffOne mul xThree stickingCoeffTwo mul add %
yOne stickingCoeffOne mul yThree -1 mul stickingCoeffTwo mul add %
)(!%
xOne stickingCoeffTwo mul xThree stickingCoeffOne mul add %
yOne stickingCoeffTwo mul yThree -1 mul stickingCoeffOne mul add %
)%
\rput[tl](! xThree yThree -1 mul){$C'$}%

\fcFullDot[linecolor=green]{xThree}{yThree -1 mul}%
\fcFullDot{xThree}{yThree}%
\fcPerpendicular[linestyle=dotted]{[xThree yThree -1 mul]}{[1 0]}{0.2}%
\psline[linestyle=dotted](! xThree yThree)(! xThree 0)%
\rput[bl](! xThree yThree){$C$}%
\fcFullDot{xOne}{yOne}%
\fcFullDot{xTwo}{yTwo}%
\rput[tl](! xOne yOne){$A$}%
\rput[br](! xTwo yTwo){$B$}%
\rput[lb](-1.9,-2.5){$y^2=x^3+ax+b$}
\pstVerb{end}%
\end{pspicture}
\column{0.8\textwidth}
Let $A=\left(x_A, y_A\right), B=\left(x_B, y_B\right)$. Let $s$ be the slope of line $AB$. Let $x_C,y_C$ be the unknown coordinates of $C$.

$
\begin{array}{r@{~}c@{~}l@{}l|l}
s&=&\displaystyle \text{line slope}\\
\uncover<-2>{
\displaystyle \frac{-y - y_A}{x-x_A}&=& s \\
-y&=& s\left(x-x_A\right) + y_A  && (*) %\begin{array}{l}x=x_C, y=y_C\\ \text{solves this} \end{array}
\\
x^3+a x +b  &=& (-y)^2  && (**)
%\begin{array}{l}x=x_C, y=y_C\\ \text{solves this} \end{array}
\\
x^3 + a x + b &=& \left(s\left(x-x_A\right) + y_A\right)^2}
\end{array}
$
\end{columns}
\only<handout:1|1>{
$
\begin{array}{rcl}
x^3+ax+b - \left(s^2 (x-x_A)^2 + 2s y_A(x-x_A) +y_A^2\right)&=&0\\
x^3 - s^2x^2+2s^2xx_A +s^2x_A^2-2sy_Ax + 2sy_Ax_A -y_A^2+ax+b &=&0\\
x^3 - x^2s^2 + x(2s^2 x_A-2sy_A+a) + s^2x_A^2+2sy_Ax_A-y_A^2+b &=& 0\\
\end{array}
$

Setting  $x=x_A$ solves $(*), (**)$. Similarly setting $x=x_B$ solves $(*),(**)$. Since $(**)$ is cubic $\Rightarrow$ its unknown $3^{rd}$ root is $x_C$. By Vieta's formulas, 
}
$
\begin{array}{rcll|l}
\uncover<-2>{x_A + x_B + x_C &=& s^2} \\
\alertNoH{3}{x_C} &\alertNoH{3}{{=}}& \alertNoH{3}{s^2 - x_A-x_B} \\
\alertNoH{3}{y_C} &\alertNoH{3}{{=}}& \alertNoH{3}{- s\left(x_C-x_A\right)-y_A}\\
\only<handout:2|2->{
\alertNoH{3}{s} &\alertNoH{3}{{=}}& \displaystyle \alertNoH{3}{\frac{y_B-y_A}{x_B-x_A}}&& \alertNoH{3}{\text{if } x_A\neq x_B} \\
\alertNoH{3}{s} &\alertNoH{3}{{=}}& \uncover<-2>{\displaystyle \frac{\diff y}{\diff x} =} \alertNoH{3}{\frac{3x_A^2+a}{2y_A}} && \alertNoH{3}{\text{if } x_A =x_B, y_A=y_B}\\
\uncover<-2>{
y^2 &=& x^3 + ax +b &&\text{apply }\diff \\
2y\diff y &=& 3x^2\diff x + a \diff x\\
\displaystyle \frac{\diff y}{\diff x}& =&\displaystyle \frac{3x^2+a}{2y}
}}
\end{array}
$

\vskip 10cm
\end{frame}

\begin{frame}
\begin{emptyTheorem}[Elliptic curve group law, algebraic definition]
Let $\left(x_A, y_A\right), \left(x_B, y_B\right)$ be two points on the elliptic curve. 
\begin{itemize}
\item Suppose $y_A\neq -y_B$. Define:

$\begin{array}{rcl|l}
s&=& \left\{ \begin{array}{ll}\displaystyle\frac{y_B-y_A}{x_B-x_A} &\displaystyle\text{if } x_A\neq x_B \\\displaystyle \frac{3x_A^2+a}{2y_A}&\text{if }x_A=x_B, y_A=y_B \end{array} \right.\\
x_C &=& s^2 - x_A-x_B &\text{if } y_A\neq -y_B\\
y_C &=& -s(x_C-x_A)-y_A&\text{if } y_A\neq -y_B 
\end{array}
$
\item If $y_A= -y_B$, define $(x_C, y_C) = \mathbf 1$.
\item Define $\mathbf 1\cdot \left(x_A, y_A\right) = \left(x_A,y_A\right)$.
\item Define $\mathbf 1\cdot \mathbf 1 = \mathbf 1$.

\end{itemize}
\end{emptyTheorem}

\begin{itemize}
\item<2-> When we derived the formulas above, we assumed working over $\mathbb C$ or $\mathbb R$.
\item<3-> However, the formulas are well-defined over an arbitrary field (a field is a set of elements where the operations $+, -, *, /$ are well defined and obey the basic rules of arithmetic we expect numbers to have. Full definition of field: outside of our scope.
\end{itemize}
\end{frame}