\begin{frame}
\vskip -0.2cm
\begin{example}
Guess a rational root of $\alertNoH{6}{6} {\alertNoH{11}{x}}^{3}-19 {\alertNoH{11}{x}}^{2}+17 {\alertNoH{11}{x}} \alertNoH{4}{-3}$.

\uncover<2->{
By the rational root theorem, a rational root $\displaystyle \frac{\alertNoH{3, 4}{p }}{ \alertNoH{5,6}{ q}}$ has that 

\begin{itemize}
\item \alertNoH{3,4}{ $p$ is \alertNoH{7}{a divisor of $\fcAnswer{4}{-3}$},}\uncover<7->{ so $p$ is one of: $\alertNoH{7}{\pm 1, \pm 3}$.}
\item \alertNoH{5,6}{ $q$ is \alertNoH{8}{a divisor of $\fcAnswer{6}{6}$},}\uncover<8->{ so $q$ is one of: $\alertNoH{8}{\pm 1, \pm 2, \pm 3, \pm 6}$.}
\end{itemize}
}
\uncover<9->{ Therefore $\frac{p}{q}$ is one of $12$ possibilities: $\pm 1, \pm \frac{1}{3}, \pm \frac{1}{2}, \pm \frac{1}{6}, \pm 3, \pm \frac{3}{2}$. Try all:
}

\uncover<10->{
$
\begin{array}{rclcl}
f(1)&=& 6\cdot{\alertNoH{11} {1}}^3-19\cdot {\alertNoH{11} {1}}^2+17\cdot {\alertNoH{11} {1}}-3&=&1 \\
\uncover<12->{
f(-1)&=&6 \left(-1\right)^{3}-19 \left(-1\right)^{2}+17 \left(-1\right)-3&=&-45\\
f{}\left(3\right)&=&6\cdot 3^{3}-19\cdot 3^{2}+17\cdot 3-3&=&39\\
f{}\left(-3\right)&=&6 \left(-3\right)^{3}-19 \left(-3\right)^{2}+17 \left(-3\right)-3&=&-387\\
f{}\left(\frac{1}{3}\right)&=&6 \left(\frac{1}{3}\right)^{3}-19 \left(\frac{1}{3}\right)^{2}+17\cdot \frac{1}{3}-3&=&\frac{7}{9}\\
\vdots \\ 
f{}\left(\alertNoH{13}{\frac{3}{2}}\right)&=&6 \left(\frac{3}{2}\right)^{3}-19 \left(\frac{3}{2}\right)^{2}+17\cdot \frac{3}{2}-3&=&\alertNoH{13}{0}\\
}
\end{array}$

\uncover<13->{Answer: $\alertNoH{13}{x=\frac{3}{2}}$ is the only rational root.}
}


\end{example}
\end{frame}