\begin{frame}
$\begin{array}{r@{}c@{}l}
a_0 x^{n}+a_1x^{n-1}+\dots + a_n&=& a_0 (x-x_1)\dots (x-x_n)\\
&=&\text{prod. real quadratics no roots \& lin. terms.}
\end{array}
$

\begin{example}

$
\renewcommand{\arraystretch}{2}
\begin{array}{@{\!\!}r@{}c@{}l@{}l@{}|l}
\alertNoH{2}{2x^2+3x-5}&\alertNoH{2}{=} &(2x+5)(x-1)= \alertNoH{2}{ 2\left(x- \alertNoH{3}{ \left(-\frac{5 }{2}\right)} \right)(x-\alertNoH{3}{1})} \uncover<2->{&&} \uncoverAlert{2}{ \alertNoH{3}{\text{real roots}}} \\
\alertNoH{4}{x^2+1}&\alertNoH{4}{=} &x^2-(-1)=x^2-i^2= \alertNoH{4}{(x-(\alertNoH{5}{-i}) )(x-\alertNoH{5}{i})} \uncover<4->{&&} \uncoverAlert{4}{\alertNoH{5}{ \text{complex roots}}} \\
\alertNoH{6}{x^4-1} &\alertNoH{6}{=}&(x^2-1)(x^2+1)=(x-1)(x+1)(x^2+1)\\
&\alertNoH{0}{=}& \alertNoH{6}{(x-\alertNoH{7}{1})(x-\alertNoH{7}{(-1)})(x-\alertNoH{7}{i})(x-(\alertNoH{7}{-i}))} \uncover<6->{&&} \uncoverAlert{6}{\alertNoH{7}{\text{mixed roots}}}\\
\alertNoH{8}{x^4+1}&\alertNoH{8}{=}&(x^2-\sqrt{2}x+1)(x^2+\sqrt{2}x+1)\\
&\alertNoH{0}{=}&
\alertNoH{8}{
\! \left(x-\alertNoH{9}{\left(\frac{\sqrt{2}}{2}+\frac{\sqrt{2}}{2}i\right)}\right)
\left(x-\alertNoH{9}{\left(\frac{\sqrt{2}}{2}-\frac{\sqrt{2}}{2}i\right)}\right)
}
\\&&
\alertNoH{8}{
\! \left(x-\alertNoH{9}{\left(-\frac{\sqrt{2}}{2}+\frac{\sqrt{2}}{2}i\right)}\right)\!\!
\left(x-\alertNoH{9}{\left(-\frac{\sqrt{2}}{2}-\frac{\sqrt{2}}{2}i\right)}\right)
}
\uncover<8->{&&} \uncoverAlert{8}{ \alertNoH{9}{\text{complex roots}}}
\end{array}$
\end{example}

 \end{frame}