\begin{frame}
Recall that $i^2=-1$, $\sqrt{-1}=i$.
\begin{example}[Polynomial factorizations]
$
\renewcommand{\arraystretch}{2}
\begin{array}{rcl}
\alertNoH{2,3}{2x^2+3x-5}&\alertNoH{2,3}{=}& \uncover<2->{ (\fcAnswer{3}{ \alertNoH{4 }{2}x +5})( \fcAnswer{3}{x -1}) \uncover<4->{= \alertNoH{4}{2} \left(x- \left(- \frac{5 }{ \alertNoH{4}{2} }\right)\right)(x-1)} }\\
\alertNoH{18}{x^2 \alertNoH{5}{+} 1} &\alertNoH{18}{=}& \uncover<5->{ x^2 \alertNoH{5}{-}(\alertNoH{6}{\alertNoH{5}{-}1} ) \uncover<6->{= {\alertNoH{7}{x}}^{\alertNoH{9}{2}} {\alertNoH{9}{-}} \alertNoH{6}{ {\alertNoH{8}{i}}^{\alertNoH{9}{2}}}} \uncover<7->{=\alertNoH{18}{ ({\alertNoH{7}{x}}{\alertNoH{9}{+}}{\alertNoH{8}{i}})({\alertNoH{7}{x}}{\alertNoH{9}{-}}{\alertNoH{8}{i}})}}} \\
\alertNoH{10}{{\alertNoH{11}{x}}^{\alertNoH{13}{4}} \alertNoH{13}{-} \alertNoH{12}{ 1}}&\alertNoH{10}{ =}&\uncover<10->{ \alertNoH{10}{ \alertNoH{14}{ ({ \alertNoH{11,15}{x }}^{ \alertNoH{13,17}{2} } \alertNoH{13,17}{-} \alertNoH{12,16}{ 1}) } ({\alertNoH{11}{x}}^{ \alertNoH{13}{2} } { \alertNoH{13}{+} } \alertNoH{12}{1 })}\uncover<14->{ =\alertNoH{14} {( \alertNoH{15}{x} \alertNoH{17}{-} \alertNoH{16}{ 1} )( \alertNoH{15}{x} \alertNoH{17}{+} \alertNoH{16}{ 1})} (\alertNoH{18}{ x^2+1} )} }\\
\uncover<18->{&\alertNoH{0}{ =} & (x-1)(x+1) \alertNoH{18}{(x-i)(x+i)}} \\
\alertNoH{19}{x^4+1}&\alertNoH{19}{=}&\uncover<19->{ \alertNoH{19}{ \left(\alertNoH{20}{ x^2- \sqrt{2}x+1} \right)\left( \alertNoH{21}{x^2+\sqrt{2}x+1} \right)}}\\
\uncover<20->{&\alertNoH{0}{=}&
\alertNoH{20}{
\left(x-\left(\frac{\sqrt{2}}{2}+\frac{\sqrt{2}}{2}i\right)\right)
\left(x-\left(\frac{\sqrt{2}}{2}-\frac{\sqrt{2}}{2}i\right)\right)
}
\\&&
\alertNoH{21}{
\left(x-\left(-\frac{\sqrt{2}}{2}+\frac{\sqrt{2}}{2}i\right)\right)
\left(x-\left(-\frac{\sqrt{2}}{2}-\frac{\sqrt{2}}{2}i\right)\right)
}
}
\end{array}$
\end{example}

 \end{frame}