\begin{frame}
\vskip -0.1cm
\begin{example}
Demonstrate that $6 x^{3}-19 x^{2}+17 x-3$ is divisible by $(2x-3)$ using polynomial long division. \alertNoH{25,33}{Use your work to factor the cubic.} \alertNoH{34}{Solve the equation $6 x^{3}-19 x^{2}+17 x-3=0$}.

\vskip -0.2cm
\only<1-25| handout:1>
{\renewcommand{\arraystretch}{1.2}\begin{longtable}{@{}c@{}c@{}c@{}c@{}c@{}c@{}c@{}c@{}c}\uncover<23->{\alertNoH{23}{\textbf{Quotient: }}}&\multicolumn{8}{c}{ \fcAnswer{5}{\alertNoH{6, 7, 23, 5}{$3x^{2}$}} \uncover<11->{\alertNoH{12, 13, 23, 11}{$-$}} \fcAnswer{11}{\alertNoH{12, 13, 23, 11}{$5x $}} \uncover<17->{\alertNoH{18, 19, 23, 17}{$+$}} \fcAnswer{17}{\alertNoH{18, 19, 23, 17}{$1$}} }\\ \cline{2-9} \cline{2-9}\multicolumn{1}{c|}{ \alertNoH{3, 4, 5, 6, 7, 10, 11, 12, 13, 16, 17, 18, 19}{$2x $} \alertNoH{3, 6, 7, 12, 13, 18, 19}{$-$} \alertNoH{3, 6, 7, 12, 13, 18, 19}{$3$} }&&\alertNoH{2, 4, 5, 8, 9}{$6x^{3}$}&\alertNoH{2, 8, 9}{$-$}&\alertNoH{2, 8, 9}{$19x^{2}$}&\alertNoH{2, 8, 9}{$+$}&\alertNoH{2, 8, 9}{$17x $}&\alertNoH{2, 8, 9}{$-$}&\alertNoH{2, 8, 9}{$3$}\\\uncover<6->{\uncover<8->{\alertNoH{8, 9}{$\overline{\phantom{A}}$}}&&\fcAnswer{7}{\alertNoH{8, 9, 7}{$6x^{3}$}}&\uncover<7->{\alertNoH{8, 9, 7}{$-$}}&\fcAnswer{7}{\alertNoH{8, 9, 7}{$9x^{2}$}}&&&\\\cline{2-9}}\uncover<8->{&&&\uncover<9->{\alertNoH{10, 11, 14, 15, 9}{$-$}}&\fcAnswer{9}{\alertNoH{10, 11, 14, 15, 9}{$10x^{2}$}}&\uncover<9->{\alertNoH{14, 15, 9}{$+$}}&\fcAnswer{9}{\alertNoH{14, 15, 9}{$17x $}}&\uncover<9->{\alertNoH{14, 15, 9}{$-$}}&\fcAnswer{9}{\alertNoH{14, 15, 9}{$3$}}\\\uncover<12->{\uncover<14->{\alertNoH{14, 15}{$\overline{\phantom{A}}$}}&&&\uncover<13->{\alertNoH{14, 15, 13}{$-$}}&\fcAnswer{13}{\alertNoH{14, 15, 13}{$10x^{2}$}}&\uncover<13->{\alertNoH{14, 15, 13}{$+$}}&\fcAnswer{13}{\alertNoH{14, 15, 13}{$15x $}}&\\\cline{4-9}}}\uncover<14->{&&&&&&\fcAnswer{15}{\alertNoH{16, 17, 20, 21, 15}{$2x $}}&\uncover<15->{\alertNoH{20, 21, 15}{$-$}}&\fcAnswer{15}{\alertNoH{20, 21, 15}{$3$}}\\\uncover<18->{\uncover<20->{\alertNoH{20, 21}{$\overline{\phantom{A}}$}}&&&&&&\fcAnswer{19}{\alertNoH{20, 21, 19}{$2x $}}&\uncover<19->{\alertNoH{20, 21, 19}{$-$}}&\fcAnswer{19}{\alertNoH{20, 21, 19}{$3$}}\\\cline{6-9}}}\uncover<20->{\uncover<24->{\textbf{\color{orange}Remainder: }}&&&&&&&&$ { \only<22->{\color{orange}}\fcAnswer{21}{0}}$}\end{longtable} $\vphantom{\frac{x^1}{x^1}}$\only<4,5|handout:0>{Divide \alertNoH{4,5}{$6x^{3}$ } by \alertNoH{4,5}{$2x $}.}\only<6, 7| handout:0>{Multiply \alertNoH{6, 7}{$3x^{2}$} by divisor. }\only<8, 9| handout:0>{Subtract last two polynomials.}\only<10,11| handout:0>{Divide \alertNoH{10,11}{$-10x^{2}$ } by \alertNoH{10,11}{$2x $}.}\only<12, 13| handout:0>{Multiply \alertNoH{12, 13}{$-5x $} by divisor. }\only<14, 15| handout:0>{Subtract last two polynomials.}\only<16,17| handout:0>{Divide \alertNoH{16,17}{$2x $ } by \alertNoH{16,17}{$2x $}.}\only<18, 19| handout:0>{Multiply \alertNoH{18, 19}{$1$} by divisor. }\only<20, 21| handout:0>{Subtract last two polynomials.}}\uncover<23->{
$\begin{array}{@{}r@{}c@{}l}
\uncover<1-25| handout:1>{\textbf{(Divident)}&\alertNoH{0}{=}&  \textbf{(\alertNoH{23}{Quotient})} \cdot \textbf{(Divisor)}+ \textbf{(\alertNoH{24}{Remainder})}}\\
\alertNoH{25,26,33,35}{( 6x^3-19x^2+17x-3)}&\alertNoH{25,26}{=}&\alertNoH{25,26}{ (\alertNoH{23}{\alertNoH{29}{3}x^2\alertNoH{30}{-5} x+\alertNoH{31}{1} }) \cdot(2x-3)}\\
\only<26-|handout:2>{\uncover<27->{&\alertNoH{0}{=}&\alertNoH{33,35}{ \left(x- \fcAnswerUncover{27}{32}{\left(\frac{5+ \sqrt{13}}{6}\right)} \right)\left(x- \fcAnswerUncover{27}{32}{\left(\frac{5- \sqrt{13}}{6}\right)}\right)(2x-3)} }}
\end{array}
$
\only<26-|handout:2>{
\uncover<27->{
No easy factorization of quadratic, so use formula:

\hfil\hfil$
\alertNoH{32}{x_1,x_2}=\fcAnswer{28}{\frac{-b\pm\sqrt{b^2-4ac}}{2a}}\uncover<29->{=\frac{-(\alertNoH{30}{-5})\pm\sqrt{(\alertNoH{30}{-5})^2-4\cdot \alertNoH{29}{ 3}\cdot \alertNoH{31}{1} } }{2\cdot\alertNoH{29}{ 3} }}\uncoverAlert{32}{ =\frac{ 5\pm\sqrt{13}}{6}}
$
\uncover<34->{
We are ready to solve the equation.

\hfil\hfil $\begin{array}{rcl}
\alertNoH{34}{ 6x^3-19x^2+17x-3}&=&0\\
\uncover<35->{\alertNoH{35}{\left(\alertNoH{37}{ x- \left(\frac{5+ \sqrt{13} }{6} \right)}\right)\left(\alertNoH{38}{x- \left(\frac{5- \sqrt{13} }{6}\right)} \right) (\alertNoH{36}{2x-3})} &=&0}\\
\end{array}
$
}

\uncover<36->{
$\begin{array}{rclcrclcrcl}
\alertNoH{36}{\alertNoH{40}{2}x\alertNoH{39}{-3}}&\alertNoH{36}{=}&\alertNoH{36}{0}&\quad \alertNoH{41}{\textbf{or}} \quad &\alertNoH{37,41}{x}&\alertNoH{37,41}{=}& \alertNoH{37,41}{\left(\frac{5+ \sqrt{13}}{6}\right)}&\quad \alertNoH{41}{ \textbf{or} } \quad &\alertNoH{38, 41}{x} &\alertNoH{38, 41}{=} & \alertNoH{38, 41}{ \left(\frac{5- \sqrt{13}}{6}\right)} \\
\uncover<39->{ \alertNoH{41}{x}&\alertNoH{41}{=}&\alertNoH{41}{ \frac{ \alertNoH{39 }{3}}{ \alertNoH{40}{2}}}}
\end{array}
$
}
}
}
}

\end{example}
\vskip 10cm
\end{frame}

