\begin{frame}
\begin{example}
Rewrite  $\cos (3\Arccos (x))$ as an algebraic expression of $x$ and $\sqrt{1-x^2}$.

\uncover<2->{
Our only means of simplifying $\Arccos x$ away is to exploit $\cos (\Arccos x) =x $. Therefore our aim is to rewrite the expression only using the $\cos $ function.
\[
\displaystyle \begin{array}{@{}r@{}c@{}l@{}l|l}
\cos (3\Arccos (x))&=&\displaystyle  \cos (3y)=\cos(2y+y)&&y=\Arccos x\\
&=&\displaystyle \cos(2y)\cos y - \sin (2y)\sin y\\
&=&\displaystyle  (\cos^2y -\sin^2y)\cos y &&\text{Express via }\\
&&- 2\sin y \cos y\sin y  &&\sin y, \cos y\\
&=&\cos^3y -\sin^2y\cos y-2\sin^2y\cos y\\
&=&\cos^3y - 3\sin^2y \cos y&& \begin{array}{l}\text{Express }\sin y \\\text{ via } \cos y\end{array}\\
&=&\cos^3y -3(1-\cos^2y)\cos y\\
&=& 4\cos^3y-3\cos y\\
&=&4x^3-3x &&x=\cos y
\end{array}
\]
}
\end{example}

\end{frame}