Find all antiderivatives of the functions.
\begin{multicols}{3}
\begin{enumerate}
\item $\displaystyle f(x)=\sqrt {3}+\pi^2$.

\answer{$\displaystyle x\left(\pi^{2} +\sqrt{3}\right)+C$}
\item $\displaystyle f(x)=x-5$.

\answer{$\displaystyle \frac{x}{2}-5x+C$}

\item $\displaystyle f(x)= x^2-2x+6$.

\answer{ $\frac{x^3}{3} -x^2+6x+C$ }

\item $\displaystyle f(x)=\frac{x(x+1)}{2} $.

\answer{$\frac{1}{6} x^{3}+\frac{1}{4} x^{2}+C$}
\item $\displaystyle f(x)=x(x+1)(2x+1)$.

\answer{$\frac{1}{2} x^{4}+x^{3}+\frac{1}{2} x^{2}+C$}
\item $\displaystyle f(x)=7x^{\frac{2}{7}}+x^{-\frac{4}{7}}$.

\answer{$\frac{49}{9} x^{\frac{9}{7}}+\frac{7}{3} x^{\frac{3}{7}}+ C$}
\item $\displaystyle f(x)=x^{2.4}-2x^{\sqrt{3}-1}$.

\answer{$\frac{5}{17} x^{\frac{17}{5}}-\frac{2\sqrt{3} x^{\sqrt{3}}}{3} +C$}
\item $\displaystyle f(x)=\frac{8}{x^7}$.

\answer{$-\frac{4}{3} x^{-6}+C$}
\item $\displaystyle f(x)=\frac{x+1}{x^3}$.

\answer{$- x^{-1}-\frac{1}{2} x^{-2}+C$}
\item $\displaystyle f(x)=\frac{1}{x}$.

\answer{$\ln |x|+C$}
\item $\displaystyle f(x)=\frac{x^2+1}{x}$.

\answer{$\frac{1}{2} x^{2}+\ln|x|+C $}
\item $\displaystyle f(x)=\frac{5-4x^3+2x^6}{x^4}$.

\answer{$\frac{2}{3} x^{3}-\frac{5}{3} x^{-3}-4 \ln|x|+C $}
\item $\displaystyle g(x)=\frac{1+\sqrt{x}+x}{\sqrt{x^3}}$.

\answer{$2 x^{\frac{1}{2}}-2 x^{-\frac{1}{2}}+\ln|x|+C $}
\item $\displaystyle f(x)=3\sin t-4\cos t$.

\answer{$-3\cos t -4\sin t +C $}
\item $\displaystyle f(\theta)=\sec^2\theta$.

\answer{$\tan \theta +C $}
\item $\displaystyle f(\theta)=\csc^2\theta$.

\answer{$\tan \theta +C $}

\item $\displaystyle f(t)=\sec t \tan t +\csc t \cot t$.

\answer{$\sec t-\csc t +C $}
\item $\displaystyle f(x)=\frac{2+x\cos x}{x}$.

\answer{$2\ln |x|+\sin x $}
\end{enumerate}
\end{multicols}