\solution{\ref{problemd/dx(ln(sec x)+ln(cot x))}

\[\begin{array}{rcll|l}
\displaystyle \frac{\diff }{\diff x}(\ln(\sec x)+\ln(\cot x))&=&\displaystyle  \frac{\diff }{\diff x}\left(\ln\left(\frac{1}{\cos x}\right)+\ln\left(\frac{\cos x}{\sin x}\right)\right)\\
&=&\displaystyle  \frac{\diff }{\diff x}\left( \cancel{- \ln\left(\cos x\right)}+\cancel{\ln\left(\cos x\right)}-\ln (\sin x) \right)\\
&=&\displaystyle -\frac{\diff }{\diff x}(\ln (\sin x))&&\text{chain rule}\\
~\\
&=&\displaystyle -\frac{1}{\sin x}\frac{\diff }{\diff x}(\sin x)\\
~\\
&=&\displaystyle -\frac{\cos x}{\sin x}\\
~\\
&=&\displaystyle -\cot x
\end{array}\]
}