

\solution{\ref{problemlimxtoinfty((x-2)/x)^x}.

\noindent\textbf{Variant I.}
\[
\begin{array}{rcll|l}
\displaystyle \lim_{x\to \infty }\left( \frac{x-2}{x}\right)^x&=& \displaystyle \lim\limits_{ x \to \infty }\left( 1- \frac{2}{x}\right)^x &&\text{use } \lim\limits_{x\to\infty} \left( 1+ \frac{k}{x}\right)^x=e^k\\
&=&e^{-2}\quad .
\end{array}
\]

\noindent\textbf{Variant II.}
\[
\begin{array}{rcll|l}
\displaystyle \lim_{x\to \infty }\left( \frac{x-2}{x}\right)^x&=& \displaystyle \lim_{ x \to \infty } e^{\ln \left( \left( \frac{x-2}{x}\right)^x\right)} \\
\displaystyle \lim_{x\to \infty} \ln \left( \left( \frac{x-2}{x}\right)^x\right)&=&\displaystyle  \lim_{x\to \infty} x\left( \ln (x-2) -\ln (x) \right)\\
&=&\displaystyle \lim_{x\to\infty } \frac{ \ln (x-2) -\ln (x)}{\frac{1}{x}} &&\text{L'Hospital rule}\\
&=&\displaystyle \lim_{x\to\infty } \frac{ \frac{1}{ x-2} -\frac{1}{x}}{- \frac{ 1}{ x^2 }}\\
&=&\displaystyle \lim_{x\to \infty }\frac{-2x^2}{x^2-2x}=-2 &&\text{Therefore}\\
\displaystyle \lim_{x\to \infty }\left( \frac{x-2}{x}\right)^x&=& \displaystyle \lim_{ x \to \infty } e^{\ln \left( \left( \frac{x-2}{x}\right)^x\right)} \\
&=&e^{\lim\limits_{x\to \infty} \ln \left( \left( \frac{x-2}{x}\right)^x\right) }\\
&=&e^{-2}\quad .
\end{array}
\]
}