\solution{\ref{problem2ln(2)-3ln(3)+4ln(4)}.
\begin{align*}
2\ln 2 - 3\ln 3 + 4\ln 4 & = \ln 2^2 - \ln 3^3 + \ln 4^4 \\
 & = \ln 4 - \ln 27 + \ln 256 \\
 & = \ln \Big( \frac{4}{27}\Big) + \ln 256 \\
 & = \ln \Big( \frac{4\cdot 256}{27}\Big) \\
 & = \ln \Big( \frac{1024}{27}\Big).
\end{align*}

$\frac{1024}{27}$ is not a rational power of $e$, therefore $ \ln \left( \frac{1024}{27}\right)$ is not a rational number and there are no further simplifications of the answer (except possibly a numerical approximation with a calculator or equivalent). 
}%

\solution{\ref{problemlog_7(24)+log_(1/7)3-log_(49)64}

\[
\renewcommand{\arraystretch}{2}
\begin{array}{@{}r@{}c@{}l@{}l|l}
\displaystyle \log_{7}{(24)}+\log_{\frac{1}{7}}{(3)}-\log_{49}{(64)}&=&\displaystyle  \log_{7}{(24)}+ \frac{\log_{7}{(3)}}{ \log_{7}{\left(\frac{1}{7}\right)}}- \frac{\log_{7}{ (64)}}{\log_{7}{(49)}} && \text{common base}\\
&=&\displaystyle \log_{7}{(24)}+ \frac{\log_{7}{(3)}}{-1} -\frac{\log_{7}{(64)}}{2}&&\text{simplify logarithms}\\
&=&\displaystyle \log_{7}{(24)}-\log_{7}{(3)}-\frac{1}{2}\log_{7}{(64)}\\
&=&\displaystyle \log_{7}{\left(\frac{24}{3}\right)}- \log_{7}{ \left(64^{ \frac{ 1}{2}}\right) }&&\renewcommand{\arraystretch}{1.2} \begin{array}{@{}l}\text{rule: } \log_ax-\log_ay=\log_a\left( \frac{x}{y}\right)  \\ \text{rule: } \log_ax^r=r\log_ax \end{array} \\
&=&\displaystyle \log_{7}{\left(8\right)}-\log_{7}\left(\sqrt{64} \right)\\
&=&\displaystyle \log_78-\log_78 =0 &&\text{alternatively: }\\
&=&\displaystyle \log_7\left(\frac{8}{8}\right)\\
&=&\displaystyle \log_7(1)\\
&=&0.
\end{array}
\]
}