
\solution{\ref{problem2^(x-3)=5}
\[\begin{array}{rcll|l}
\displaystyle 2^{x-3} &=& 5 &&\displaystyle  \text{take } \log_2 \\
x-3&=&\displaystyle  \log_2(5) &&\text{add } 3 \text{ to both sides}\\
x&=&\displaystyle \log_2(5)+3 &&\text{answer is complete} \\
&=&\displaystyle \frac{\ln 5}{\ln 2}+3 && \text{optional step: convert to }\ln\\
&\approx &5.321928095 &&\text{calculator}
\end{array}
\]
}

\solution{ \ref{probleme-e^(-2x)=1}

\[
\begin{array}{rcll|l}
\displaystyle e-e^{-2x}&=&1\\
\displaystyle e^{-2x}&=&e-1&& \text{apply }\ln\\
\displaystyle \ln e^{-2x}&=&\displaystyle \ln(e-1)\\
-2x&=&\displaystyle\ln(e-1)\\
x&=&\displaystyle-\frac{1}{2}\ln(e-1)\\
&\approx& -0.270662427&&\text{calculator}
\end{array}
\]

}

\solution{\ref{problemlnx+ln(x-1)=1} %
\[
\begin{array}{rcl}
\displaystyle \ln x + \ln (x-1) & =& 1 \\
\displaystyle \ln \left(x^2-x\right) & =& 1 \\
\displaystyle e^{\ln (x^2-x)} & =& e^1 \\
\displaystyle x^2-x & =& e \\
\displaystyle x^2-x-e & =& 0 \\
\text{Quadratic formula:}\quad x & = &\displaystyle \frac{-(-1)\pm \sqrt{(-1)^2-4(1)(-e)}}{2(1)} \\
& =&\displaystyle  \frac{1\pm \sqrt{1+4e}}{2}.
\end{array}
\]
However $\frac{1-\sqrt{1+4e}}{2}$ is negative, so $\ln\left( \frac{1-\sqrt{1 + 4e}}{2} \right)$ is undefined.  
Hence the only solution is $x = \frac{1+\sqrt{1+4e}}{2}\approx 2.2229$.  
}%

\input{../../modules/logarithms/homework/logarithms-equations-subproblem-16-solution}

\input{../../modules/logarithms/homework/logarithms-equations-subproblem-17-solution}
