\solution{\ref{problemSolve4^(3x)-2^(3x+2)-5}

\[
\begin{array}{rcll|l}
\displaystyle 4^{3x}-2^{3x+2}-5&=&0 \\
\displaystyle 4^{3x}-4\cdot 2^{3x}-5&=&0&&\text{Set } \begin{array}{rcl}\displaystyle 2^{3x}&=&u\\ \displaystyle 4^{3x}&=&u^2\end{array} \\
\displaystyle u^2-4u-5&=&0\\
\displaystyle (u-5)(u+1)&=&0\\
\displaystyle u=5&\text{or}& u=-1\\
\displaystyle 2^{3x}=5&&\displaystyle 2^{3x}=-1\\
\displaystyle 3x=\log_2(5)&&\text{no real solution}\\
\displaystyle x=\frac{\log_2 5}{3}\\
\text{Calculator: }x\approx 0.773976
\end{array}
\]
}