\solution{\ref{problemintsqrt(1-x^2)dx} 

\textbf{Variant I.} This integral can quickly be solved using a trig substitution. The Euler substitution results in a slightly longer solution, shown in the next solution variant.

\noindent $
\begin{array}{rcl@{}l@{}|l}
\displaystyle \int \sqrt{1-x^2}\diff x &=&\displaystyle  \int \sqrt{1-\cos^2\theta}\diff (\cos \theta) &&\text{Set }x=\cos \theta, \theta\in[0,\pi]\\
&=&\displaystyle \int \sqrt{\sin^2\theta } (-\sin \theta)\diff \theta &&\theta\in [0,\pi]\Rightarrow \sin \theta\geq 0\\
&=&\displaystyle -\int \sin^2\theta \diff \theta && \sin^2\theta= \frac{1-\cos (2\theta) }{2}\\
&=&\displaystyle-\int \frac{1-\cos (2\theta)}{2}\diff \theta\\
&=&\displaystyle - \frac{\theta}{2}+\frac{ \sin (2\theta)}{4}+C\\
&=&\displaystyle - \frac{\theta}{2}+\frac{ 2\sin \theta\cos \theta }{4}+C
&&
\begin{array}{@{}r@{}c@{}l}
x &=&\cos \theta\\
\theta &=&\Arccos x\\
\sin \theta&=&\sin \left(\Arccos x\right)\\
&=&\sqrt{1-x^2}
\end{array}
\\
&=&\displaystyle -\frac{\Arccos x}{2}+ \frac{x\sqrt{1-x^2} }{2} + C\\
&=&\displaystyle \frac{\Arcsin x}{2}+\frac{x\sqrt{1- x^2} }{2} + K\quad ,
\end{array}
$
where for the last equality we recall that the derivative of $\Arcsin x$ is minus the derivative of $\Arccos x$.



\textbf{Variant II.} We show how to do this integral via the Euler substitution $x=\cos (2\Arctan t)$.

$
\begin{array}{rcl@{}l@{}|l}
\displaystyle \int \sqrt{1-x^2}\diff x &=&\displaystyle  \int \sqrt{1-\cos^2\theta}\diff (\cos \theta) &&\begin{array}{@{}r@{}c@{}l} &&\text{Set }\\
x&=&\cos(2\Arctan t)\\
\frac{1}{2}\Arccos x&=&\Arctan t\\ 
x&=&\frac{1-t^2}{1+t^2}\\
&=& \frac{2}{1+t^2}-1\\
\sqrt{1-x^2}&=&\frac{2t}{1+t^2}\\
\end{array}\\
&=&\displaystyle \int \frac{2t}{1+t^2}\diff \left(\frac{1-t^2}{1+t^2} \right) \\
&=&\displaystyle \int \frac{2t}{1+t^2} \left(\frac{-4t}{\left(1+t^2\right)^2}\right)\diff t &&\begin{array}{l}
\text{Integral rational}\\
\text{function}\\
\text{we skip details}
\end{array} \\
&=&\displaystyle \frac{-t}{t^{2}+1}+\frac{2 t}{ \left(t^{2}+1\right)^{2}}\\
&&\displaystyle - \Arctan{}t+C \\
&=&\displaystyle -\frac{1}{2}\sqrt{1-x^2} +\frac{\sqrt{1-x^2}}{t^2+1} \\
&&- \Arctan t+C\\
&=&\displaystyle \frac{1}{2} \sqrt{1-x^2} \left(\frac{ 2}{ t^2 +1} -1\right)\\
&&-\Arctan t+C\\
&=&\displaystyle \frac{x\sqrt{1-x^2}}{2}-\frac{1}{2}\arccos x+C\\
&=&\displaystyle \frac{x\sqrt{1-x^2}}{2}+\frac{1}{2}\arcsin x+K,
\end{array}
$
where for the very last equality we used the fact that the derivatives of $\arcsin x$ and $\arccos x$ are negatives of one another.

\textbf{Variant III. } We show how to do this integral geometrically, provided already know the area of a sector of circle. Of course, here we assume we have already derived the formula for an area of a circle. We warn the reader that most methods for deriving the formula of a sector area rely on integrals, so it is possible we are making a circular reasoning argument. Since we already did the integral purely algebraically in the preceding solution variants, we can safely ignore the danger of the aforementioned circular reasoning argument. In other words, the present solution Variant is a geometric interpretation of the problem which relies on the formula for sector area of a circle (which we assumed proved elsewhere, possibly using similar integration techniques to the ones presented in Variant I and II).

By the Fundamental Theorem of Calculus, the indefinite integral measures up to a constant the area locked under the graph of $\sqrt{1-x^2}$. This graph is a part of a circle. Therefore, up to a constant, $\int\sqrt{1-t^2}\diff t$ equals $\int_{0}^{x}\sqrt{1-t^2}\diff t$. In turn $\int_{0}^{x}\sqrt{1-t^2}\diff t$ is given by the area highlighted in the picture below.

\psset{xunit=2cm, yunit=2cm}
\begin{pspicture}(-0.3,-0.4)(1.3,1.3)
\tiny
\pscustom*[linecolor=\fcColorAreaUnderGraph]{
\psplot[linecolor=\fcColorGraph]{0}{0.75}{1 x x mul sub sqrt}
\psline(! 0.75 1 0.75 0.75 mul sub sqrt)(0.75, 0)
\psline(0.75, 0)(0,0)
}
\fcAxesStandardNoFrame{-0.3}{-0.3}{1.2}{1.2}

\psplot[linecolor=\fcColorGraph, linewidth=1.5pt]{0}{0.75}{1 x x mul sub sqrt}
\psplot{0.75}{1}{1 x x mul sub sqrt}
\rput[t](0.75,-0.05){$P$}
\fcFullDot{0.75}{0}
\rput(0.375, -0.1){$x$}
\psline(0,0)(! 0.75 1 0.75 dup mul sub sqrt)(0.75, 0)
\rput[l](0.2, 0.5){$A$}
\rput[b](0.5, 0.2){$B$}
\rput[lb](0.45, 0.9){$\Arcsin x $}
\fcFullDot{0}{1}
\rput[r](-0.1, 1){$P$}
\rput[l](0.8, 0.3){$\sqrt{1-x^2}$} 
\rput[l](0.8, 0.65){$Q$}
\fcFullDot{0.75}{1 0.75 0.75 mul sub sqrt}
\rput[tr](-0.05, -0.05){$O$}
\end{pspicture}
\[
\begin{array}{rcll|l}
\text{Area}(A)&=&\displaystyle  \frac{\text{length }\left( \stackrel{\frown}{ PQ}
\right) }{2\pi } \pi= \frac{\text{length }\left(
\stackrel{\frown}{ PQ}
\right)}{2} = \frac{\Arcsin x}{2}\\
\text{Area}(B)&=&\displaystyle \text{Area}(\triangle OPQ)= \frac{x \sqrt{1-x^2} }{2}\\
\displaystyle \int_{0}^x\sqrt{1-t^2}\diff t&=&\displaystyle  \text{Area}(A)+\text{Area}(B)\\
&=&\displaystyle \frac{\Arcsin x}{2}+\frac{x\sqrt{1-x^2}}{2}\\
&\Rightarrow\\
\displaystyle\int\sqrt{1-x^2}\diff x&=&  \displaystyle \frac{\Arcsin x}{2} + \frac{x\sqrt{1-x^2}}{2}+C\quad .
\end{array}
\] 
}

\solution{\ref{problemintsqrt(1-x^2)/(1+x)dx} In this problem solution we use the standard Euler substitution $x=\cos (2\Arctan t)$. We recall \refBad{\ref{eqEulerSubx=cos(2arctant)}}{that}{from \eqref{eqEulerSubx=cos(2arctant)} that}

\noindent $\begin{array}{rcl}
\displaystyle x& =&\displaystyle \cos(2\Arctan t)= \frac{1-t^2}{1+t^2}\\
\Arccos (x)&=& 2 \Arctan t\\
\displaystyle \diff x &=&\displaystyle  -\frac{4t}{(1+t^2)^2}\diff t\\
\displaystyle \sqrt{1-x^2}&=&\displaystyle \sin (2\Arctan t)= \frac{2t}{1+t^2}\\
t&=&\displaystyle \frac{\sqrt{1-x^2}}{x+1}\quad .
\end{array}
$

\noindent $
\begin{array}{@{}r@{}c@{}l@{}l@{}|l}
\displaystyle \int  \frac{\sqrt{1-x^2}}{1+x}\diff x&=& \displaystyle \int t \left(-\frac{4t}{\left(1+t^2\right)^2} \right)\diff t&&\begin{array}{l} \text{Set }x=\frac{1-t^2}{1+t^2}\\
\text{Use f-las above}
\end{array}
\\
&=&\displaystyle -4\int\frac{t^2}{\left(1+t^2\right)^2}\diff t\\
&=&\displaystyle -4\int\frac{1+t^2-1}{\left(1+t^2\right)^2 }\diff t\\
&=&\displaystyle -4\int\left(\frac{1}{1+t^2} -\frac{1}{\left(1+t^2\right)^2}\right)\diff t\\
&=&\displaystyle -4\left(\Arctan t - \frac{1}{2}\left(\Arctan t+ \frac{t}{1+t^2} \right) \right)+C\\
&=&\displaystyle -2\left(\Arctan {}t - \frac{t}{1+t^2} \right) +C\\
&=&\displaystyle -2\left( \Arctan {}\left(\frac{\sqrt{1-x^2}}{1+x} \right) - \frac{1}{2}\sqrt{1-x^2} \right) +C\\
&=&\displaystyle -2 \Arctan {}t  +\sqrt{1-x^2} +C &&\text{Use f-las above}
\\
&=&\displaystyle -\Arccos x+ \sqrt{1-x^2}  +C\\
&=&\displaystyle \Arcsin x +\sqrt{1-x^2}+K\quad .
\end{array}
$

We have included the last equality to remind the student that derivatives of $\Arcsin(x)$ and $\Arccos x$ are negatives of one another.


}