\solution{\ref{probleminte^x(sqrt(e^x+1))dx}.
\[
\begin{array}{rcll|l}
\displaystyle\int e^x\sqrt{e^x+1} ~ \diff x&=& \displaystyle \int \sqrt{e^x+1} ~ \diff \left(e^x\right)\\
&=&\displaystyle \int \sqrt{e^x+1}~ \diff \left(e^x+1\right)
\displaystyle &&\text{Set }u=e^x+1\\
&=&\displaystyle \int \sqrt{u}~ \diff u\\
&=&\displaystyle \frac{2}{3}u^{\frac{3}{2}}+C\\
&=&\displaystyle \frac{2}{3}\left(e^x+1\right)^{\frac{3}{2}}+C
\end{array}
\]
}

\solution{\ref{problemintsin(2x)/(2+cos^2x)dx}
\[
\begin{array}{rcll|l}
\displaystyle\int \frac{\sin (2x)}{2+\cos^2x}\diff x&=&\displaystyle\int \frac{2\cos x \sin x  \diff x }{2+\cos^2x}&&\text{use } \sin (2x)=2\sin x \cos x\\
&=& \displaystyle\int \frac{2\cos x   \diff(-\cos x) }{2+\cos^2x}&&\text{use }\diff (\cos x)=-\sin x \diff x\\
&=&\displaystyle-\int \frac{2 u   \diff(u) }{2+u^2} &&\text{set }u=\cos x\\
&=&\displaystyle-\int \frac{   \diff\left(2+u^2\right) }{2+u^2}&&\text{use }\diff (u^2+2)=2u\diff u\\
&=&\displaystyle -\int \frac{   \diff z }{z}&&\text{set }z= 2+u^2\\
&=&\displaystyle -\ln |z| +C &&\text{Substitute back }z=u^2+2\\
&=&\displaystyle -\ln (u^2+2) +C &&\begin{array}{l} u^2+2\text{ is positive}\\\Rightarrow \text{omit the abs. value}\\ \text{Substitute back }u=\cos x \end{array}\\
&=&\displaystyle -\ln (\cos^2x+2) +C .
\end{array}
\]

}

\input{../../modules/substitution-rule/homework/substitution-rule-2-problem-13-solution}
