% begin module MVT-corollary2
\begin{frame}
\begin{corollary}
If $f'(x) = g'(x)$ for all $x$ in an interval $(a,b)$, then $f-g$ is constant on $(a,b)$; that is, $f(x) = g(x) + c$ where $c$ is constant.
\end{corollary}
\begin{proof}
\begin{itemize}
\item<2->  Let $F(x) = f(x) - g(x)$.
\item<3->  Then $F'(x) = f'(x) - g'(x) = 0$ for all $x$ in $(a,b)$.
\item<4->  By the previous theorem, $F$ is constant, so $f - g$ is constant.\qedhere
\end{itemize}
\end{proof}
\end{frame}
% end module MVT-corollary2
