% begin homework chain-rule1
Compute the derivative using the chain rule.
\begin{enumerate}[ref={\fcProblemRef}]
\item   $\displaystyle f(x)=\sqrt{1+x^2}$

\answer{$x (x^{2}+1)^{-\frac{1}{2}}  $}
\item\label{problemDifferentialtexDivsqrt(1+2divx^2)}  $\displaystyle  f(x)=\frac{x }{\sqrt{1+\frac{2}{x^2}}}$.

\answer{$\frac{\pm x^2}{\sqrt{x^2+2}} $}
\pointsii{3} \label{problemd/dx((cosx)^(1/2))} $y = (\cos x)^{\frac{1}{2}}$

\answer{$\frac{1}{2} x^{-\frac{1}{2}} \cos{}\left(\sqrt{x}\right)  = \frac{\cos \left(\sqrt{x}\right)}{2\sqrt{x}}$}

\item $\displaystyle f(x)=\sin^3 x$.

\answer{$ 3 \cos{}x \sin^{2}{}x$}
\pointsii{3} \label{problemd/dx((1+cosx)^2)}  $y = (1+\cos x)^2$.


\answer{$ -2 \cos{}x \sin{}x-2 \sin{}x =-\sin(2x)-2\sin x$}
\item   $\displaystyle f(x)=\frac{1}{\sin^3x}$.

\answer{$  -\frac{3 \cos{}x}{\sin^{4}{}x} $}
\item  $\displaystyle f(x)= \sqrt[3]{4+3\tan x}$.

\answer{$  (4+3\tan x)^{-\frac{2}{3}}\sec^2x $}
\item  $f(x)=(\cos x + 3\sin x)^4$.

\answer{$4(\cos x + 3\sin x)^3 (3\cos x-\sin x) $}

\pointsii{4} \label{problemd/dx(sin(sqrt(x)))}  $\displaystyle y = \sin \left( \sqrt{x}\right)$

\answer{$\frac{\cos\sqrt{x}}{2\sqrt{x}}$}
\item  $y = \cos\left( 4x\right)$

\answer{$-4 \sin{}\left(4 x\right)  $}

\item $\sec^2 (3x^2)$. 

\answer{$12 \frac{x\sin{}(3 x^{2}) }{\left(\cos{}\left(3 x^{2}\right)\right)^{3}}$}

\item $\csc^2 (3x^2)$. 

\answer{$-12 \frac{ x  \cos{}\left(3 x^{2}\right) }{\left(\sin{}\left(3 x^{2}\right)\right)^{3}}$}
\item $2^{3^x}$.

\answer{$2^{3^{x}} 3^{x} (\ln{}2)  (\ln{}3) $}
\item $3^{2^x}$.

\answer{$ 3^{2^{x}} 2^{x}(\ln{}2)(\ln{}3)$}
\pointsii{5} \label{problemd/dx(sqrt(sec(4x)))}  $y = \sqrt{\sec (4x)}$

\answer{ $  2\sqrt{\sec (4x)}\tan (4x) =  2(\sec (4x))^{\frac{3}{2}}\sin (4x). $}
\item \label{problemd/dx(x^2tan(5x))} $y = x^2\tan (5x)$

\answer{$2x\tan (5x) - 5x^2\sec^2 (5x)$}
\pointsii{5} \label{problemd/dx((1+sin(x^2))/(1+cos(x^2)))}  $\displaystyle y = \frac{1+\sin \left(x^2\right)}{1+\cos \left(x^2\right)}$.

\answer{ $ \frac{2x(1 + \cos \left(x^2\right) + \sin \left(x^2\right))}{(1+\cos \left(x^2\right))^2}$}

\end{enumerate}
% end homework chain-rule1
