(Textbook, page 154, problems 7-46) Compute the derivative.
\begin{multicols}{2}
\begin{enumerate}
\item $\displaystyle f(x)= (x^4+3x^2-2)^5$.

\answer{$ (30 x +20 x^{3}) (-2+3 x^{2}+x^{4})^{4}$}
\item $\displaystyle f(x)= (4x-x^2)^{100}$.

\answer{$(-200 x+400) (4 x- x^{2})^{99}$}
\item $\displaystyle f(x)= \sqrt{1-2x}$.

\answer{$- (1-2 x)^{-\frac{1}{2}}$}
\item $\displaystyle f(x)= \frac{1}{(1+\sec x)^2}$.

\answer{$\frac{-2 \cos{}(x) \sin{}(x)}{(1+\cos{}(x))^{3}} =\frac{- \sin{}(2x)} {(1+\cos{}(x))^{3}} $}
\item $\displaystyle f(z)=\frac{1}{1+z^2} $.

\answer{$\frac{-2 z}{(1+z^{2})^{2}} $}
\item $\displaystyle f(t)= \sqrt[3]{1+\tan t}$.

\answer{$\frac{\frac{1}{3}}{(\cos{}(t))^{2}} \left( \frac{\cos{}(t) +\sin{}(t)}{\cos{}(t)} \right)^{-\frac{2}{3}} $}
\item $\displaystyle f(x)=\cos (a^3+x^3) $.

\answer{$ -3 x^{2}\sin{}(a^{3}+x^{3}) $}
\item $\displaystyle f(x)= a^3+\cos^3 x$.

\answer{$ -3 \sin{}(x) (\cos{}(x))^{2}$}
\item $\displaystyle f(x)= x\sec (k x) $.

\answer{$\frac{\cos{}(k x)+k x \sin{}(k x) }{(\cos{}(k x))^{2}} $}
\item $\displaystyle f(\theta)= 3\cot (n\theta)$.

\answer{$ \frac{-3 n}{(\sin{}(n \theta))^{2}}$}
\item $\displaystyle f(x)= (2x - 3)^4 (x^2 + x + 1)^5$.

\answer{$ (-7-12 x+28 x^{2})(-3+2 x)^{3} (1+x+x^{2})^{4}$}
\item $\displaystyle f(x)= (x^2+1)^3(x^2+2)^6$.

\answer{$\left(24 x+18 x^{3}\right)\left(1+x^{2}\right)^{2} \left(2+x^{2}\right)^{5} $}
\item $\displaystyle f(t)= (t+1)^{\frac{2}{3}}(2t^2-1)^3$.

\answer{$ \left(\frac{40}{3} t^{2}+12 t-\frac{2}{3}\right)\left(2 t^{2}-1\right)^{2}\left(t+1\right)^{-\frac{1}{3}}$}
\item $\displaystyle f(t)= (3t-1)^4(2t+1)^{-3}$.

\answer{$(3 t-1)^{3}\frac{6 t+18}{(2 t+1)^{4}}$}
\item $\displaystyle f(x)=\left(\frac{x^2+1}{x^2-1} \right)^3 $.

\answer{$\frac{-12 x}{\left(x^{2}-1\right)^{2}} \left(\frac{x^{2}+1}{x^{2}-1}\right)^{2} $}
\item $\displaystyle f(s)= \sqrt{\frac{s^2+1}{s^2+4}}$.

\answer{$\frac{3 s}{\left(s^{2}+4\right)^{2}} \left(\frac{s^{2}+1}{s^{2}+4}\right)^{-\frac{1}{2}} $}
\item $\displaystyle f(x)=\sin (x\cos x) $.

\answer{$\cos{}(x) \cos{}(x \cos{}(x))- x \cos{}(x \cos{}(x)) \sin{}(x) $}
\item $\displaystyle f(x)=\frac{x}{\sqrt{7-3x}} $.

\answer{$ \frac{-\frac{3}{2} x+7}{(-3 x+7)^{\frac{3}{2}}}$}
\item $\displaystyle f(z)=\sqrt{\frac{z-1}{z+1}} $.

\answer{$\frac{1}{(z+1)^{2}} \left(\frac{z-1}{z+1}\right)^{ -\frac{1}{2}} $}
\item $\displaystyle f(y)= \frac{(y-1)^4 }{(y^2+2y)^5}$.

\answer{$(y-1)^{3}\frac{-6y^{2}+8y +10}{(y^{2}+2 y)^{6}} $}
\item $\displaystyle f(r)=\frac{r}{\sqrt{r^2+1}} $.

\answer{$ \frac{1}{\left(r^{2}+1\right)^{\frac{3}{2}}}$}
\item $\displaystyle f(x)=\frac{\cos (\pi x)}{\sin (\pi x)+\cos (\pi x) } $.

\answer{$ \frac{- \pi}{(\sin{}(\pi x)+\cos{}(\pi x))^{2}}$}
\item $\displaystyle f(x)=\sin \left(\sqrt{1+x^2}\right) $.

\answer{$x \cos{}\left(\left(x^{2}+1\right)^{\frac{1}{2}}\right) \left(x^{2}+1\right)^{-\frac{1}{2}}$}
\item $\displaystyle f(v)=\left(\frac{v}{v^3+1}\right)^6 $.

\answer{$\frac{-12 v^{3}+6}{\left(v^{3}+1\right)^{2}} \left(\frac{v}{v^{3}+1}\right)^{5} $}
\end{enumerate}
\end{multicols}

