\begin{problem}(Textbook, page 154, problems 7-46) Compute the derivative.
\begin{multicols}{2}
\begin{enumerate}
\item $\displaystyle f(x)= (x^4+3x^2-2)^5$.

\answer{$ (30 x +20 x^{3}) (-2+3 x^{2}+x^{4})^{4}$}
\item $\displaystyle f(x)= (4x-x^2)^{100}$.

\answer{$(-200 x+400) (4 x- x^{2})^{99}$}
\item $\displaystyle f(x)= \sqrt{1-2x}$.

\answer{$- (1-2 x)^{-\frac{1}{2}}$}
\item $\displaystyle f(x)= \frac{1}{(1+\sec x)^2}$.

\answer{$\frac{-2 \cos{}(x) \sin{}(x)}{(1+\cos{}(x))^{3}} =\frac{- \sin{}(2x)} {(1+\cos{}(x))^{3}} $}
\item $\displaystyle f(z)=\frac{1}{1+z^2} $.

\answer{$\frac{-2 z}{(1+z^{2})^{2}} $}
\item $\displaystyle f(t)= \sqrt[3]{1+\tan t}$.

\answer{$\frac{\frac{1}{3}}{(\cos{}(t))^{2}} \left( \frac{\cos{}(t) +\sin{}(t)}{\cos{}(t)} \right)^{-\frac{2}{3}} $}
\item $\displaystyle f(x)=\cos (a^3+x^3) $.

\answer{$ -3 x^{2}\sin{}(a^{3}+x^{3}) $}
\item $\displaystyle f(x)= a^3+\cos^3 x$.

\answer{$ -3 \sin{}(x) (\cos{}(x))^{2}$}
\item $\displaystyle f(x)= x\sec (k x) $.

\answer{$\frac{\cos{}(k x)+k x \sin{}(k x) }{(\cos{}(k x))^{2}} $}
\item $\displaystyle f(\theta)= 3\cot (n\theta)$.

\answer{$ \frac{-3 n}{(\sin{}(n \theta))^{2}}$}
\item $\displaystyle f(x)= (2x - 3)^4 (x^2 + x + 1)^5$.

\answer{$ (-7-12 x+28 x^{2})(-3+2 x)^{3} (1+x+x^{2})^{4}$}
\item $\displaystyle f(x)= (x^2+1)^3(x^2+2)^6$.

\answer{$\left(24 x+18 x^{3}\right)\left(1+x^{2}\right)^{2} \left(2+x^{2}\right)^{5} $}
\item $\displaystyle f(t)= (t+1)^{\frac{2}{3}}(2t^2-1)^3$.

\answer{$ \left(\frac{40}{3} t^{2}+12 t-\frac{2}{3}\right)\left(2 t^{2}-1\right)^{2}\left(t+1\right)^{-\frac{1}{3}}$}
\item $\displaystyle f(t)= (3t-1)^4(2t+1)^{-3}$.

\answer{$(3 t-1)^{3}\frac{6 t+18}{(2 t+1)^{4}}$}
\item $\displaystyle f(x)=\left(\frac{x^2+1}{x^2-1} \right)^3 $.

\answer{$\frac{-12 x}{\left(x^{2}-1\right)^{2}} \left(\frac{x^{2}+1}{x^{2}-1}\right)^{2} $}
\item $\displaystyle f(s)= \sqrt{\frac{s^2+1}{s^2+4}}$.

\answer{$\frac{3 s}{\left(s^{2}+4\right)^{2}} \left(\frac{s^{2}+1}{s^{2}+4}\right)^{-\frac{1}{2}} $}
\item $\displaystyle f(x)=\sin (x\cos x) $.

\answer{$\cos{}(x) \cos{}(x \cos{}(x))- x \cos{}(x \cos{}(x)) \sin{}(x) $}
\item $\displaystyle f(x)=\frac{x}{\sqrt{7-3x}} $.

\answer{$ \frac{-\frac{3}{2} x+7}{(-3 x+7)^{\frac{3}{2}}}$}
\item $\displaystyle f(z)=\sqrt{\frac{z-1}{z+1}} $.

\answer{$\frac{1}{(z+1)^{2}} \left(\frac{z-1}{z+1}\right)^{ -\frac{1}{2}} $}
\item $\displaystyle f(y)= \frac{(y-1)^4 }{(y^2+2y)^5}$.

\answer{$(y-1)^{3}\frac{-6y^{2}+8y +10}{(y^{2}+2 y)^{6}} $}
\item $\displaystyle f(r)=\frac{r}{\sqrt{r^2+1}} $.

\answer{$ \frac{1}{\left(r^{2}+1\right)^{\frac{3}{2}}}$}
\item $\displaystyle f(x)=\frac{\cos (\pi x)}{\sin (\pi x)+\cos (\pi x) } $.

\answer{$ \frac{- \pi}{(\sin{}(\pi x)+\cos{}(\pi x))^{2}}$}
\item $\displaystyle f(x)=\sin \left(\sqrt{1+x^2}\right) $.

\answer{$x \cos{}\left(\left(x^{2}+1\right)^{\frac{1}{2}}\right) \left(x^{2}+1\right)^{-\frac{1}{2}}$}
\item $\displaystyle f(v)=\left(\frac{v}{v^3+1}\right)^6 $.

\answer{$\frac{-12 v^{3}+6}{\left(v^{3}+1\right)^{2}} \left(\frac{v}{v^{3}+1}\right)^{5} $}
\item $\displaystyle f(x)=\sin (\tan (2x)) $.

\answer{$2\sec^2(2x) \cos (\tan 2x) $}
\item $\displaystyle f(x)=\sec^2(m x) $.

\answer{$ \frac{2 m \sin{}(m x) }{(\cos{}(m x))^{3}} $}
\item $\displaystyle f(x)= \sec^2 x+\tan^2 x$.

\answer{$\frac{4 \sin{}x}{\cos^{3}{}x} $}
\item $\displaystyle f(x)=x\sin \frac{1}{x} $.

\answer{$- x^{-1}\cos{}(x^{-1}) +\sin{}(x^{-1})$}
\item $\displaystyle f(x)= \left(\frac{1-\cos (2x)}{1+\cos (2x)}\right)^4$.

\answer{$\frac{16 \sin{}(2 x)}{(\cos{}(2 x)+1)^{2}} \left(\frac{- \cos{}(2 x)+1}{\cos{}(2 x)+1}\right)^{3} $}
\item $\displaystyle f(t)=\sqrt{\frac{t}{t^2+4}} $.

\answer{$ \frac{-\frac{1}{2} t^{2}+2}{(t^{2}+4)^{2}} \left(\frac{t}{t^{2}+4}\right)^{-\frac{1}{2}}$}
\item $\displaystyle f(t)= \cot^2(\sin t)$.

\answer{$ \frac{-2 \cos{}t \cos{}(\sin{}t)}{\sin^{3}{}(\sin{}t)}$}
\item $\displaystyle f(x)= (a x+\sqrt{x^2+b^2})^{-2}$.

\answer{$\frac{-2 x\left(x^{2}+b^{2}\right)^{-\frac{1}{2}} -2 a}{\left(\left(x^{2}+b^{2}\right)^{\frac{1}{2}}+a x\right)^{3}} $}
\item $\displaystyle f(x)= \left(x^2+(1-3x)^5\right)^3$.

\answer{
\begin{tabular}{l}
$\left(-45 (-3 x+1)^{4} +6 x \right) \left((-3 x+1)^{5}+x^{2}\right)^{2}$
\\
Using computer algebra:
\\
$(-3645x^{4}+4860x^{3}-2430x^{2}+546x -45)\left((-3 x+1)^{5}+x^{2}\right)^{2}$ \\
Using computer algebra full expansion:
\\
$\begin{array}{l}
-215233605x^{14}+1004423490x^{13}-2176250895x^{12}\\
+2903793624x^{11} -2666357595x^{10}+1782098820x^{9}\\
-893713176x^{8} +341444160x^{7} -99805041x^{6} \\ +22199676x^{5}-3697470x^{4}  +447132x^{3}\\
-37125x^{2}+1896x -45
\end{array}
$
\end{tabular} 
}
\item $\displaystyle f(x)=\sin (\sin (\sin x))$.

\answer{$\cos{}x \cos{}(\sin{}x) \cos{}(\sin{}(\sin{}x)) $}
\item $\displaystyle f(x)= \sqrt{x+\sqrt{x}}$.

\answer{$ \left(\frac{1}{2} +\frac{1}{4} x^{-\frac{1}{2}}\right) \left(x^{\frac{1}{2}}+x\right)^{-\frac{1}{2}}$}
\item $\displaystyle f(x)= \sqrt{x+\sqrt{x+\sqrt{x}}}$.

\answer{$\frac{1}{2} \left(\left(x^{\frac{1}{2}}+x\right)^{\frac{1}{2}}+x\right)^{-\frac{1}{2}} \left(\frac{1}{2} \left(x^{\frac{1}{2}}+x\right)^{-\frac{1}{2}} \left(\frac{1}{2} x^{-\frac{1}{2}}+1\right)+1\right) $}
\item $\displaystyle f(x)=(2r \sin (r x)+n)^p $.

\answer{$ p r(2 r \sin{}(r x)+n)^{p-1} \cos{}(r x) $}
\item $\displaystyle f(x)=\cos^4(\sin^3 x) $.

\answer{$-12 \cos{}x \sin^{2}{}x \sin{}(\sin^{3}{}x) \cos^{3}{}(\sin^{3}{}x) $}
\item $\displaystyle f(x)=\cos \sqrt{\sin (\tan (\pi x))} $.

\answer{$ \frac{-\frac{1}{2} \pi \cos{}(\tan{}(\pi x)) \sin^{-\frac{1}{2}}{}(\tan{}(\pi x)) \sin{}(\sin^{\frac{1}{2}}{}(\tan{}(\pi x)))}{\cos^{2}{}(\pi x)}$}
\item $\displaystyle f(x)=\left(x+(x+\sin^2 x)^3 \right)^4 $.

\answer{$4 ((\sin^{2}{}x+x)^{3}+x)^{3} (3 (\sin^{2}{}x+x)^{2} (2 \sin{}x \cos{}x+1)+1) $}
\end{enumerate}
\end{multicols}
\end{problem}
\begin{problem}Compute the second derivative.
\begin{multicols}{3}
\begin{enumerate}
\item $\displaystyle f(x)=\sin (-5x)$. 

\answer{$ 25 \sin{}(5 x)$}
\item $\displaystyle f(x)=e^{-3x}$. 

\answer{$9 e^{-3 x} $}
\item $\displaystyle f(x)=e^{\frac{1}x}$. 

\answer{$ 2 e^{x^{-1}} x^{-3}+e^{x^{-1}} x^{-4}$}
\item $\displaystyle f(x)=e^{\sqrt{x}}$. 

\answer{$ e^{x^{\frac{1}{2}}} x^{-\frac{3}{2}}+\frac{1}{4} e^{x^{\frac{1}{2}}} x^{-1}$}
\item $\displaystyle f(x)=\frac{e^{x}-e^{-x}}{e^x+e^{-x}} $

\answer{$\frac{-8 \left(- e^{- x}+e^{x}\right)}{\left(e^{- x}+e^{x}\right)^{3}} $}
\item $\displaystyle f(x)=\frac{1}2\ln \left(\frac{1+x}{1-x}\right) $

\answer{$\frac12\left(-\frac{1}{(x+1)^{2}}+\frac{1}{(- x+1)^{2}}\right)= \frac{ 2x}{\left(1-x^2\right)^2} $}
\end{enumerate}
\end{multicols}
\end{problem}