% begin homework chain-rule6
Differentiate the following functions with respect to $x$.  
Simplify your answers.  

\begin{enumerate}
\pointsii{5}  $y = \sqrt{\sec (4x)}$
\solution{%
\begin{align*}
\text{Chain Rule: } \quad \frac{\diff y}{\diff x} & = \big( \frac{1}{2}(\sec (4x))^{-\frac{1}{2}}\big) \frac{\diff}{\diff x}(\sec (4x)) \\
\text{Chain Rule: } \quad \frac{\diff y}{\diff x} & = \Big( \frac{1}{2\sqrt{\sec (4x)}}\Big) (\sec (4x) \tan (4x))\frac{\diff}{\diff x}(4x) \\
 & = \Big( \frac{1}{2\sqrt{\sec (4x)}}\Big) (\sec (4x) \tan (4x))(4) \\
 & =  \frac{2\sec (4x)\tan (4x)}{\sqrt{\sec (4x)}} \\
\intertext{There are many ways to simplify this answer, including both of the following.}
 & =  2\sqrt{\sec (4x)}\tan (4x). \\
 & =  2(\sec (4x))^{\frac{3}{2}}\sin (4x). 
\end{align*}
}%

\item  $y = x^2\tan (5x)$
%\solution{%
%\begin{align*}
%\text{Product Rule: } \quad \frac{\diff y}{\diff x} & = (x^2)\frac{\diff}{\diff x}(\tan 5x) + (\tan 5x)\frac{\diff}{\diff x}(x^2) \\
%\intertext{Use the Chain Rule to differentiate $\tan 5x$ in the first term.}
%\frac{\diff y}{\diff x} & = (x^2)(-5\sec^2 5x) + (\tan 5x)(2x) \\
% & = 2x\tan 5x - 5x^2\sec^2 5x.
%\end{align*}
%}%

\pointsii{5}  $y = \frac{1+\sin \left(x^2\right)}{1+\cos \left(x^2\right)}$
\solution{%
\begin{align*}
\text{Quotient Rule: } \quad \frac{\diff y}{\diff x} & = \frac{(1+ \cos \left(x^2\right))\frac{\diff}{\diff y}(1+\sin \left(x^2\right)) - (1+\sin \left(x^2\right))\frac{\diff}{\diff x}(1+\cos \left(x^2\right))}{(1+\cos \left(x^2\right))^2} \\
\intertext{By the Chain Rule, $\frac{\diff}{\diff x}(1+\cos \left(x^2\right)) = -2x\sin \left(x^2\right)$ and $\frac{\diff}{\diff x}(1+\sin \left(x^2\right)) = 2x\cos \left(x^2\right)$.}
\frac{\diff y}{\diff x} & = \frac{(1+\cos \left(x^2\right))(2x\cos \left(x^2\right)) - (1+\sin \left(x^2\right))(-2x\sin \left(x^2\right))}{(1+\cos \left(x^2\right))^2} \\
 & = \frac{2x\cos \left(x^2\right) + 2x\cos^2 \left(x^2\right) + 2x\sin \left(x^2\right) + 2x\sin^2 \left(x^2\right)}{(1+\cos \left(x^2\right))^2} \\
 & = \frac{2x(\cos^2 \left(x^2\right) + \sin^2 \left(x^2\right)) + 2x(\cos \left(x^2\right) + \sin \left(x^2\right))}{(1+\cos \left(x^2\right))^2} \\
\intertext{By the Pythagorean Identity, $\cos^2 \left(x^2\right) + \sin^2 \left(x^2\right) = 1$.}
\frac{\diff y}{\diff x} & = \frac{2x + 2x(\cos \left(x^2\right) + \sin \left(x^2\right))}{(1+\cos \left(x^2\right))^2} \\
 & = \frac{2x(1 + \cos \left(x^2\right) + \sin \left(x^2\right))}{(1+\cos \left(x^2\right))^2}.
\end{align*}
}%

\end{enumerate}
% end homework chain-rule6
