% begin module alternating-estimate-ex4
\begin{frame}
\begin{example} %[Example 4, p. 749]
Find the sum of $\sum_{n=0}^\infty \frac{(-1)^n}{n!}$ correct to three decimal places.  (\alert<handout:0| 10>{$0! = 1$}.)
\begin{enumerate}
\item<2->  $\displaystyle b_{n+1} = \frac{1}{(n+1)!} \uncover<3->{ = \frac{1}{n!(n+1)} } \uncover<4->{ < \frac{1}{n!} = b_n.}$
\item<5->  $\displaystyle 0 < \frac{1}{n!} \uncover<6->{ < \frac{1}{n} }\uncover<7->{ \to 0 }$\uncover<7->{, so } \uncover<7->{$\displaystyle b_n \to 0$ as $n\to \infty$.}
\end{enumerate}
\begin{itemize}
\item<8->  Therefore the series converges by the Alternating Series Test.
%\item<9->  Compute the first few terms:
\end{itemize}
\abovedisplayskip=0pt
\belowdisplayskip=0pt
\begin{eqnarray*}
\uncover<9->{s} & \uncover<9->{=} & \uncover<9->{\alert<handout:0| 12>{\alert<handout:0| 10>{\frac{1}{0!}} - \frac{1}{1!} + \frac{1}{2!} - \frac{1}{3!} + \frac{1}{4!} - \frac{1}{5!} + \frac{1}{6!}} - \alert<handout:0| 11>{\frac{1}{7!}} + \cdots}\\
 & \uncover<10->{=} & \uncover<10->{\alert<handout:0| 12>{\alert<handout:0| 10>{1} - 1 + \frac{1}{2} - \frac{1}{6} + \frac{1}{24} - \frac{1}{120} + \frac{1}{720}} - \alert<handout:0| 11>{\frac{1}{5040}} + \cdots}
\end{eqnarray*}
\begin{itemize}
\item<11-| alert@11,13>  $|s - s_6| \leq b_7 = \frac{1}{5040} < 0.0002$.
\item<12-| alert@12>  $s_6 = 1 - 1 + \frac{1}{2} - \frac{1}{6} + \frac{1}{24} - \frac{1}{120} + \frac{1}{720} \approx 0.36\alert<handout:0| 13>{80}56$.
\item<13->  The error of less than $0.0002$ doesn't affect the third decimal place\uncover<14->{, so $s \approx s_6 \approx 0.368$.}
\end{itemize}
\end{example}
\end{frame}
% end module alternating-estimate-ex4
