% begin module alternating-estimate
\begin{frame}
\frametitle{Estimating Sums}
This theorem allows us to estimate the size of the remainder $R_n = s - s_n$ in an alternating series.
\begin{theorem}[Alternating Series Estimation Theorem]
Let $\displaystyle \sum (-1)^{n-1} b_n$ be the sum of an alternating series that satisfies
\begin{enumerate}
\item  $0\leq b_{n+1}\leq b_n$ and
\item  $\displaystyle \lim_{n\to\infty} b_n = 0$.
\end{enumerate}
Then the size of the error is less than the first omitted term; that is,
\[
|R_n| = |s - s_n| \leq b_{n+1}.
\]
\end{theorem}
\end{frame}
% end module alternating-estimate
