% begin module alternating-ex1
\begin{frame}
\begin{example} %[Example 1, p. 747]
The alternating harmonic series
\abovedisplayskip=0pt
\belowdisplayskip=0pt
\[
1 - \frac{1}{2} + \frac{1}{3} - \frac{1}{4} + \cdots = \sum_{n=1}^\infty \frac{(-1)^{n-1}}{n}
\]
satisfies
\begin{enumerate}
\item  $b_{n+1} < b_n$ because $\frac{1}{n+1} < \frac{1}{n}$.
\item  $\lim_{n\to\infty} b_n = $\alert<handout:0| 2-3>{$\lim_{n\to\infty} \frac{1}{n}$ \uncover<2->{$ = $} \uncover<3->{\alert<handout:0| 4>{$0$}.}}
\end{enumerate}
\uncover<4->{Therefore the series is \alert<handout:0| 4>{convergent} by the Alternating Series Test.}
\end{example}
\end{frame}
% end module alternating-ex1
