% begin module geometric-sum-example
\begin{frame}
\begin{example}[The sum of a geometric series]
Find the sum of the geometric series
\abovedisplayskip=0pt
\belowdisplayskip=0pt
\[
\sum_{n=1}^{12} 6(-2)^{n-1}.
\]
\uncover<2->{%
\begin{align*}
\alert<handout:0| 2-3>{\text{The first term is } a} & \alert<handout:0| 2-3>{= \uncover<3-| handout:0>{6.}} \\
\alert<handout:0| 4-5>{\text{The ratio is } r} & \alert<handout:0| 4-5>{= \uncover<5-| handout:0>{-2.}} \\
\alert<handout:0| 6-7>{\text{The number of terms is } M} & \alert<handout:0| 6-7>{= \uncover<7-| handout:0>{12.}} \\
\alert<handout:0| 8-9>{\text{The sum is } s} & \alert<handout:0| 8-9>{= \uncover<9-| handout:0>{6\frac{1-(-2)^{12}}{1-(-2)} = -8190.}} 
\end{align*}
}%
\end{example}

\end{frame}
% end module geometric-sum-example
