% begin module ratio-test-ex4
\begin{frame}
\begin{example} %[Example 4, p. 753]
Test the series $\displaystyle \sum_{n=1}^\infty (-1)^n \frac{n^3}{3^n}$ for absolute convergence.
\abovedisplayskip=0pt
\belowdisplayskip=0pt
\begin{eqnarray*}
\uncover<2->{%
\left| \frac{a_{n+1}}{a_n}\right| %
}%
 & \uncover<2->{=} & %
\uncover<2->{%
\left| \frac{(-1)^{n+1}\frac{(n+1)^3}{3^{n+1}}}{(-1)^n\frac{n^3}{3^n}}\right| %
}\\%
 & \uncover<3->{=} & %
\uncover<3->{%
\frac{(n+1)^3}{3^{n+1}}\cdot \frac{3^n}{n^3}%
}\\%
 & \uncover<4->{=} & %
\uncover<4->{%
\frac{1}{3} \left( \frac{n+1}{n}\right)^3%
}\\%
 & \uncover<5->{=} & %
\uncover<5->{%
\alert<handout:0| 6-7>{%
\frac{1}{3} \left( 1 + \frac{1}{n}\right)^3%
}%
}\\%
 & \uncover<6->{\alert<handout:0| 6-7>{\to}} & %
\uncover<7->{%
\alert<handout:0| 6-7,9>{%
\frac{1}{3} \uncover<9->{ < 1 }
}%
}%
\end{eqnarray*}
\uncover<8->{%
Therefore the series is \uncover<9->{\alert<handout:0| 9>{absolutely convergent}} by the Ratio Test.%
}%
\end{example}
\end{frame}
% end module ratio-test-ex4
