% begin module series-divergence-test
\begin{frame}[t]
\begin{theorem}
If the series $\sum_{n=1}^\infty a_n$ is convergent, then $\lim_{n\to\infty}a_n = 0$.
\end{theorem}
\begin{proof}
\begin{itemize}
\item<2->  Let $s_n = a_1 + a_2 + \cdots + a_n$.
\item<3->  Then \alert<handout:0| 8>{$a_n = s_n - s_{n-1}$}.
\item<4->  Since $\sum_{n=1}^\infty a_n$ is convergent, the sequence $\{ s_n\}$ is convergent.
\item<5->  Let \alert<handout:0| 9>{$\lim_{n\to\infty} s_n = s$.}
\item<6->  Then \alert<handout:0| 6-7,9>{$\lim_{n\to\infty} s_{n-1} =$ \uncover<7->{$s$.}}
\item<8->  Therefore
\end{itemize}
\[
\uncover<8->{\lim_{n\to\infty}\alert<handout:0| 8>{a_n}} %
\uncover<8->{= \lim_{n\to\infty}\alert<handout:0| 8>{(\alert<handout:0| 9>{s_n}-\alert<handout:0| 9>{s_{n-1}})}} %
\uncover<9->{= \alert<handout:0| 9>{s} - \alert<handout:0| 9>{s}} %
\uncover<10->{= 0\qedhere}%
\]
\end{proof}
\end{frame}


\begin{frame}[t]
\begin{theorem}
If the series $\sum_{n=1}^\infty a_n$ is convergent, then $\lim_{n\to\infty}a_n = 0$.
\end{theorem}
This is just a restatement of the previous theorem:
\begin{theorem}[The Divergence Test]
If $\lim_{n\to\infty} a_n$ doesn't exist or if $\lim_{n\to\infty}a_n \neq 0$, then the series $\sum_{n=1}^\infty a_n$ is divergent.
\end{theorem}
\end{frame}
% end module series-divergence-test
