% begin module series-telescoping-ex6
\begin{frame}
\begin{example}[Example 6, p. 727]
Show that the series $\sum_{n=1}^\infty \frac{1}{n(n+1)}$ is convergent and find its sum.
\begin{itemize}
\item<2-| alert@2-3>  Is this a geometric series?  \uncover<3->{No.}%
\item<4->  Use partial fractions:
\end{itemize}
\uncover<4->{%
\abovedisplayskip=0pt
\belowdisplayskip=0pt
\[
a_n = \alert<handout:0| 7>{\frac{1}{n(n+1)} \uncover<5->{ = \frac{1}{n} - \frac{1}{n+1}}}%
\]
}%
\abovedisplayskip=0pt
\belowdisplayskip=0pt
\begin{eqnarray*}
\uncover<6->{%
\alert<handout:0| 15>{s_n}%
}%
& \uncover<6->{ = } &%
\uncover<6->{%
\sum_{i=1}^n \alert<handout:0| 7>{\frac{1}{i(i+1)}}%
}  \uncover<7->{ = } \uncover<7->{%
\sum_{i=1}^n \alert<handout:0| 7>{\left( \frac{1}{i} - \frac{1}{i+1}\right)}%
}\\%
& \uncover<8->{ = } &%
\uncover<8->{%
\left( \alert<handout:0| 13>{1} - \alert<handout:0| 9>{\frac{1}{2}}\right) %
+ \left( \alert<handout:0| 9>{\frac{1}{2}} - \alert<handout:0| 10>{\frac{1}{3}}\right) %
+ \left( \alert<handout:0| 10>{\frac{1}{3}} - \alert<handout:0| 11>{\frac{1}{4}}\right) %
+ \alert<handout:0| 11-12>{\cdots} %
+ \left( \alert<handout:0| 12>{\frac{1}{n}} \alert<handout:0| 13>{- \frac{1}{n+ 1}}\right) %
}\\%
& \uncover<13->{\alert<handout:0| 15>{ = }} &%
\uncover<13->{%
\alert<handout:0| 13,15>{1 - \frac{1}{n+1}}%
}%
\end{eqnarray*}
\uncover<14->{%
\abovedisplayskip=0pt
\belowdisplayskip=0pt
\[
\textrm{Therefore}\quad \sum_{i=1}^\infty \frac{1}{i(i+1)} = \lim_{n\to\infty} \alert<handout:0| 15>{s_n} \uncover<15->{= \lim_{n\to\infty} \alert<handout:0| 15>{\left( 1 - \frac{1}{n+1}\right)}} \uncover<16>{= 1}%
\]
}%
\vspace{-.1in}
\end{example}
\end{frame}
% end module series-telescoping-ex6
