% begin module natural-growth-solution
\begin{frame}
\frametitle{Newton's Law of Cooling}
Newton's Law of Cooling states that the rate of cooling of an object is 
proportional to the temperature difference between the object and its 
surroundings, provided that this difference is not too large.\\
 (This law also applies to warming.) \\
  If we let $T (t)$ be the temperature of the object at time $t$ and $T_s$ 
be the temperature of the surroundings, 
then we can formulate Newton's Law of Cooling as a differential equation: 
\[
\frac{dT}{dt}=k(T-T_s)
\]
where $ k $ is a constant of proportionality.\\ 
This equation is not quite the same as $ y'=ky$, 
so we make the change of variable $y = T - T_s$.\\ \pause

 Because $T_s$ is constant, we have $y'(t) = T '(t)=k(T=T_s)=ky$, so the equation  becomes \[ y'=ky\] 
 which we can solve for $ y $ and then for $ T $.

\end{frame}

\begin{frame}
$\frac{dT}{dt}=k(T-T_s)$ and $y = T - T_s$ give  $y'=ky$, which has solution \[ y=y_0e^{kt} \]
\onslide<2->{
so
\[ T-T_s=y_0e^{kt} \]
 where $ y_0=T_0-T_s$,}
 \onslide<3->{ so
\[
T=y_0e^{kt}+T_s=(T_0-T_s)e^{kt}+T_s
\]}
\end{frame}

% end module natural-growth-solution
