\begin{frame}
\begin{example}
Find the directional derivative of $f(x,y,z) = \ln{ (x^2+ 2y^2- z^2 )}$ at $P(2,1,-1)$ in the direction $\fcv{v}=( -1,2,1)$.

\uncover<2->{
A unit vector in the direction of $\fcv{v}$ is
\[
\fcv{u} = \frac{1}{|\fcv{v}|} \fcv{v} = \frac{1}{\sqrt{6}} ( -1, 2, 1 )\; .
\]
}
%\begin{overlayarea}{\textheight}{5cm}
\only<handout:1|3-6>{The partial derivatives are
\[
\begin{array}{rcllrcl}
\alert<3,4>{\frac{\partial f}{\partial x}}&\alert<3,4>{=}&  \uncover<4->{\alert<4>{ \frac{ 2 x}{x^2+2y^2-z^2} }}&&  \uncover<5->{\alert<5,6>{ \frac{\partial f}{\partial x}( 2, 1, -1 )}} &\uncover<5->{\alert<5,6>{=}}& \uncover<6->{\alert<6>{ \frac{ 4}{5} }} \\
\alert<3,4>{\frac{\partial f}{\partial y}} &\alert<3,4>{=}& \uncover<4->{\alert<4>{\frac{ 4 y}{x^2+2y^2-z^2} }}&& \uncover<5->{ \alert<5,6>{ \frac{\partial f}{\partial y}( 2, 1, -1 )}} &\uncover<5->{\alert<5,6>{=}}& \uncover<6->{\alert<6>{ \frac{ 4}{5}}} \\
\alert<3,4>{\frac{\partial f}{\partial z}} &\alert<3,4>{ =}& \uncover<4->{\alert<4>{\frac{ - 2z }{x^2+2y^2-z^2}}} && \uncover<5->{ \alert<5,6>{ \frac{\partial f}{\partial z}(2,1,-1)}} &\uncover<5->{\alert<5,6>{=}}& \uncover<6->{ \alert<6>{ \frac{2}{5}}}
\end{array}
\]
\[
\uncover<6->{\alert<6>{\nabla f _{|(x,y,z)=(2,1,-1)} = \left( \frac{4}{5}, \frac{4}{5}, \frac{2}{5} \right ) }}
\]
}
\only<handout:2|7->{
\[
\nabla f_{|(x,y,z)=(2,1,-1)} = ( f_x, f_y, f_z )_{|(x,y,z)= (2,1,-1) } = \left( \frac{4}{5}, \frac{4}{5}, \frac{2}{5}\right)
\]
\[
\alert<7>{(D_{\fcv{u}}f)_{|(x,y,z)=(2,1,-1)} = \nabla f_{|(x,y,z)=(2,1,-1)} \cdot \fcv{u} =} \uncover<8->{\alert<8>{ \frac{ \sqrt{6}}{5}}}
\]

\uncover<9->{
$(D_{\fcv{u}}f)(2,1,-1)>0 $ implies that if we start at $(2, 1, -1)$ and move in the direction $\fcv{u}$, then $f$ is increasing.
}
}
%\end{overlayarea}
\end{example}
\vskip 5cm
\end{frame}
