\begin{frame}
  \frametitle{Chain Rule}
Differentials
%
\[
\diff w=w_x(x,y,z){\color{red}{\diff x}} +
w_y(x,y,z){\color{blue}{\diff y}}+
w_z(x,y,z){\color{green}{\diff z}}
\]
%
and
%
\[
{\color{red}{\diff x=x'(t)\diff t}} \qquad
{\color{blue}{\diff y = y'(t)\diff t}} \qquad
{\color{green}{\diff z=z'(t)\diff t}} \; .
\]
%
\pause Then
%
\[
\diff \left(w(x(t), y(t), z(t)) \right)= \left( w_x(x,y,z) x'(t) + w_y(x,y,z) y'(t) +
w_z(x,y,z) z'(t) \right) \diff t
\]
%
\pause
Therefore

\[\!\!\displaystyle
\frac{\diff }{\diff t}(w(x(t), y(t), z(t))) = \frac{\partial w}{\partial x}(x,y,z) \frac{\diff x}{\diff t} +
\frac{\partial w}{\partial y}(x,y,z) \frac{\diff y}{\diff t} +
\frac{\partial w}{\partial z}(x,y,z) \frac{\diff z}{\diff t}
\]

\pause
Derivative of composition of functions $\Longrightarrow$ \alert<1->{Chain Rule}
\end{frame}