\begin{frame}
  \frametitle{More General Chain Rule}

More general formula:
%
\begin{itemize}
\item $w=F(x,y,z)$;
\item $x=f(u,v)$, $y=g(u,v)$, $z=h(u,v)$.
\end{itemize}
%
$$w = F(f(u,v), g(u,v), h(u,v)) = G(u,v)$$
%
To compute $\frac{\partial w}{\partial u} = \frac{\partial G}{\partial u}$:

\begin{itemize}
  \item arrange variables in a tree diagram:
  $$\xymatrix{ & & & & w &  & & \\ & x  \ar[urrr]^F & & & y \ar[u]^F & & &  z \ar[ulll]_F & \\ u \ar[ur]^f & & v\ar[ul]_f & u \ar[ur]^g & & v \ar[ul]_g & u \ar[ur]^h & & v \ar[ul]_h  }$$
\end{itemize}

\end{frame}
