

\begin{frame}
\begin{example}[Partial Derivatives in Polar Coordinates]
Express $\frac{\partial }{\partial x}$ and $\frac{\partial}{ \partial y}$ via $\frac{\partial }{\partial r}$ and $\frac{\partial}{\partial \theta}$, where $\alert<handout:0|5,13,21>{ x=r\cos \theta}, \alert<handout:0|4,14,20>{y=r\sin \theta}$.

\begin{columns}
\column{0.55\textwidth}
\uncover<6->{\alert<handout:0|6>{Suppose $ \theta\in \left(-\frac{\pi}{2}, \frac{\pi}{2}\right)$.}} \uncover<2->{Recall that}
\[
\begin{array}{rcl}
\uncover<2->{\alert<handout:0|6>{ \tan \theta} &\alert<handout:0|6>{=}& \frac{ \alert<handout:0|4>{\uncover<3->{\alert<handout:0|3>{r} } \sin \theta}}{ \alert<handout:0|5>{ \uncover<3->{\alert<handout:0|3>{r}}\cos \theta}} } \uncover<4->{ = \alert<handout:0|6>{ \frac{\alert<handout:0|4>{y}}{\alert<handout:0|5>{x}}}} \\
\uncover<6->{\alert<handout:0|6,11,12,18,19>{ \theta} &\alert<handout:0|6,11,12,18,19>{=}& \alert<handout:0|6,11,12,18,19>{\arctan \left(\frac{y}{x}\right)}}\\
\uncover<7->{\alert<handout:0|9,10,13,14,16,17,20,21>{r}}&\uncover<7->{\alert<handout:0|9,10,13,14,16,17,20,21>{=}}&\uncover<7->{\alert<handout:0|9,10,13,14,16,17,20,21>{\sqrt{x^2+y^2}}}\\
\end{array}
\]
\column{0.45\textwidth}
\uncover<8->{ 
$\xymatrix@R=1em@C=0.5em{
& & & z &    &   & \\
 & r \ar[urr] &        &   &    & \theta \ar[ull] & \\
x\ar[ur]&   & y \ar[ul]&   &  x\ar[ur] &   & y \ar[ul]
}$
}
\end{columns}
$ 
\renewcommand{\arraystretch}{1.8}
\begin{array}{rcl}
\displaystyle \uncover<8->{\frac{\alert<handout:0|23>{ \partial} \alert<handout:0|22>{z}}{\alert<handout:0|23>{\partial x}} &=& \displaystyle \frac{\partial z}{\partial r} \alert<handout:0|9,10>{ \frac{ \partial r}{\partial x}} +\frac{\partial z}{\partial \theta} \alert<handout:0|11,12>{ \frac{\partial \theta}{\partial x}}} 
\uncover<9->{ = \displaystyle \frac{\partial z}{\partial r} \uncover<handout:0|9>{ \alert<handout:0|9>{ \textbf{?}}}\uncover<10->{\alert<handout:0|10,13>{ \frac{x}{\sqrt{x^2+y^2}} }}  + \frac{\partial z}{\partial \theta} \uncover<handout:0|11>{\alert<handout:0|11>{\textbf{?}}}\uncover<12->{\left(\alert<handout:0|12>{\alert<handout:0|14>{ \frac{-y}{x^2+y^2}} }\right) }}\\
\uncover<13->{&=&\displaystyle \alert<handout:0|13,23>{ \cos\theta} \frac{ \alert<handout:0|23>{\partial} \alert<handout:0|22>{z}}{\alert<handout:0|23>{\partial r}}  \alert<handout:0|14,23>{- \frac{ \sin\theta }{ r}} \frac{ \alert<handout:0|23>{\partial} \alert<handout:0|22>{z}}{\alert<handout:0|23>{\partial \theta}}} \\
\uncover<15->{\displaystyle \frac{ \alert<handout:0|23>{\partial} \alert<handout:0|22>{z}}{\alert<handout:0|23>{\partial y}} } &\uncover<15->{=}&\uncover<15->{ \displaystyle \frac{\partial z}{\partial r} \alert<handout:0|16,17>{ \frac{ \partial r}{\partial y}} +\frac{\partial z}{\partial \theta} \alert<handout:0|18,19>{ \frac{\partial \theta}{\partial x}}}      \uncover<16->{=\displaystyle \frac{\partial z}{\partial r} \uncover<handout:0|16>{ \alert<handout:0|16>{ \textbf{?}}}\uncover<17->{\alert<handout:0|17,20>{ \frac{y}{\sqrt{x^2+y^2}} }}  + \frac{\partial z}{\partial \theta} \uncover<handout:0|16-18>{\alert<handout:0|18>{\textbf{?}}}\uncover<19->{\alert<handout:0|19,21>{ \frac{x}{x^2+y^2}} }}\\
&\uncover<20->{=}&\uncover<20->{\displaystyle \alert<handout:0|20,23>{ \sin\theta} \frac{ \alert<handout:0|23>{\partial} \alert<handout:0|22>{z}}{\alert<handout:0|23>{\partial r}} +  \alert<handout:0|21,23>{\frac{ \cos\theta }{ r}} \frac{ \alert<handout:0|23>{\partial} \alert<handout:0|22>{z}}{\alert<handout:0|23>{\partial \theta}}}
\end{array}
$

\uncover<22->{ The above hold for all $z$, \uncover<23->{ therefore \alert<handout:0|23>{$\begin{array}{rcl}
\frac{\partial}{\partial x} &=&   \cos\theta \frac{ \partial }{\partial r} - \frac{ 1 }{ r}\sin\theta \frac{ \partial }{\partial \theta}\\
\frac{\partial}{\partial y} &=& \sin \theta \frac{\partial }{\partial r} +\frac{1}{r}\cos \theta\frac{\partial}{\partial\theta}
\end{array}
$}.  }}

\end{example}

\vskip 8cm
\end{frame}


