Prove the trigonometry identities.
\begin{multicols}{3}
\begin{enumerate}
\item $\displaystyle \sin \theta\cot \theta =\cos \theta$.
\item $\displaystyle (\sin \theta +\cos \theta)^2=1+\sin(2\theta)$.
\item $\displaystyle \sec \theta - \cos \theta= \tan \theta \sin \theta$.
\item $\displaystyle \tan^2 \theta-\sin^2 \theta=\tan^2\theta\sin^2\theta$.
\item $\displaystyle \cot^2\theta+\sec^2\theta=\tan^2\theta+\csc^2\theta$.
\item $\displaystyle 2\csc (2\theta)= \sec \theta \csc \theta$.
\item $\displaystyle \tan (2\theta) =\frac{2\tan \theta}{1-\tan^2\theta} $.
\item $\displaystyle \frac{1}{1-\sin \theta}+ \frac{1}{1+\sin \theta}=2\sec^2\theta$.
\item $\displaystyle \tan \alpha + \tan \beta = \frac{\sin (\alpha+\beta)}{\cos \alpha \cos \beta}$.
\item $\displaystyle \tan (\alpha+\beta)= \frac{\tan \alpha +\tan \beta}{1-\tan \alpha\tan \beta}$.
\item $\displaystyle \sin (3\theta) +\sin \theta = 2 \sin (2\theta ) \cos \theta $.
\item $\displaystyle \cos (3\theta) = 4\cos^3\theta-3\cos \theta $.
\item $\displaystyle 1+\tan^2\theta = \sec^2\theta$.
\item $\displaystyle 1+\csc^2\theta = \cot^2\theta$.
\item $\displaystyle \frac{1+\tan \left(\frac{\theta}{2} \right) } {1 -\tan \left(\frac{\theta}{2}\right)}= \tan \theta +\sec \theta$.
\end{enumerate} 
\end{multicols}
