
\begin{frame}
\frametitle{Parametric Equations}
    \begin{itemize}
    \item Parametric vectorial equation of $L$:
    %
    $$\textbf{r} = \textbf{r}_0 +  t\textbf{u},  \quad t \text{ real number.}$$
    %
  $$\textbf{r} = \textbf{r}_0 + t(\textbf{r}_1-\textbf{r}_0), \quad t \text{ real number.}$$
  %
  $$\textbf{r} = (1-t)\textbf{r}_0 + t\textbf{r}_1, \quad t \text{ real number.}$$
  %
  \item Parametric scalar equations:
%
$$\left\{ \begin{array}{l}
           x  = x_0 + tu_1 \\
	   y  = y_0 + tu_2 \\
           z  = z_0 + tu_3
          \end{array}
\right. \leftrightarrow \left\{ \begin{array}{l}
           x  = x_0 + t(x_1-x_0) \\
	   y  = y_0 + t(y_1-y_0) \\
           z  = z_0 + t(z_1-z_0)
          \end{array}
\right. \leftrightarrow \left\{ \begin{array}{l}
           x  = (1-t)x_0 + tx_1 \\
	   y  = (1-t)y_0 + ty_1 \\
           z  = (1-t)z_0 + tz_1
          \end{array}
\right. $$
  \item Segment with endpoints $P_0(\textbf{r}_0)$ and $P_1(\textbf{r}_1)$:
%
$$\textbf{r} = (1-t)\textbf{r}_0 + t\textbf{r}_1, \quad 0 \leqslant t \leqslant 1$$

  \end{itemize}

\end{frame}


\begin{frame}
\frametitle{Examples}

\begin{enumerate}
  \item Line with direction $\textbf{u} = \langle 4,5,6\rangle$ through $P_0(1,2,3)$:
\begin{itemize}
 \item Parametric vectorial equation:
%
$$\textbf{r} = \langle 1,2,3\rangle + t \langle 4,5,6\rangle \leftrightarrow
\textbf{r} = \langle 1+4t, 2+5t, 3+6t\rangle$$
%
\item Parametric scalar equations:
%
$$\left\{ \begin{array}{ll}
           x & = 1 + 4t \\
	   y & = 2+5t \\
           z & = 3+6t
          \end{array}
\right. , \quad t \text{ real number.}$$
\end{itemize}
%
\item Line $L$ through $P_0(1,2,3)$ and $P_1(5,2,1)$.

\begin{itemize}
 \item Direction of $L$: $\textbf{u} = \textbf{r}_1-\textbf{r}_0 = \langle 4, 0, -2\rangle$.
\item Parametric vectorial equation:
%
$$\textbf{r} = \langle 1,2,3\rangle + t \langle 4, 0 -2\rangle \leftrightarrow \textbf{r} = \langle 1+4t, 2, 3-2t\rangle\; .$$
%
\item Parametric scalar equations:
$$\left\{ \begin{array}{ll}
           x & = 1+4t \\
	   y & = 2 \\
           z & = 3-2t
          \end{array}
\right. , \quad t \text{ real number.}$$
\end{itemize}
\end{enumerate}

\end{frame}


\begin{frame}
 \frametitle{Parametrized Curves}
    \begin{itemize}
    \item Functions $f: [a,b] \to \RR^2$, $g: [a,b] \to \RR^3$
      \item Scalar input (parameter)
      \item Vectorial output (position vector)
      \item Images: parametrized curves
      \item $\textbf{r} \colon [a,b] \to \RR^2$ plane curve
      \item $\textbf{r} \colon [a,b] \to \RR^3$ space curve\pause
      \item Function $\textbf{r}$: parametrization\pause
      \item $t$: parameter
      \item $\textbf{r}(t) = \langle x(t), y(t), z(t)\rangle$,
      $a \leqslant t \leqslant b$
      \item $x,y,z \colon [a,b] \to \RR$, coordinate functions
    \end{itemize}
\end{frame}

\begin{frame}
  \frametitle{Example}

    \begin{itemize}
    \item $\textbf{r} \colon \RR \to \RR^3$,
    %
    $$\textbf{r}(t) = \textbf{r}_0 +t\textbf{u}$$
    \item Line through $P(1,4,3)$\\
    direction $\textbf{u}=\langle -1,2,0\rangle$:\pause
    %
    $$\textbf{r}(t) = \langle 1-t,4+2t,3\rangle$$\pause
    \item Parametrization of a curve: not unique!
    \item $t=1-s=\varphi(s)$: reparametrization
    \item $\textbf{p}(s) = \textbf{r}(\varphi(s))$
    \item $\textbf{p}(s) = \langle s, 6-2s, 3\rangle$
    \end{itemize}
\end{frame}

\begin{frame}
  \frametitle{}

    Describe the curve:
    \begin{align*}
      x(t) & = 3t\cos{(2t)}\\
      y(t) & = 3t\sin{(2t)}\\
      z(t) & = t^2
    \end{align*}
    \pause Cylindrical coordinates:
    \begin{align*}
      r(t) & = 3t\\
      \theta(t) & = 2t \\
      z(t) & = t^2
    \end{align*}
    \pause Tornado!
\end{frame}

\begin{frame}
    \frametitle{Limits}
    $$\lim_{t\to a} \textbf{r}(t) = \textbf{u}$$
    we can keep $\textbf{r}(t)$ as close to $\textbf{u}$ as we want by
    keeping $t$ close enough to $a$.

    \bigskip \pause

    Close in Euclidean distance $\Longleftrightarrow$ close in postman distance

    $$\textbf{r}(t) = \langle x(t), y(t), z(t) \rangle \quad , \quad \textbf{u}=\langle u_1,u_2,u_3\rangle$$

    $$\lim_{t\to a} \textbf{r}(t) = \textbf{u} \Longleftrightarrow
    \left\{
    \begin{array}{l}
      \lim_{t\to a} x(t) = u_1\\
      \lim_{t\to a} y(t) = u_2\\
      \lim_{t\to a} z(t) = u_3\\
    \end{array}
    \right.$$
\end{frame}

\begin{frame}
  \frametitle{Continuity}
  $\textbf{r} \colon [a,b] \to \RR^3$ is continuous at $t_0$ if
  $$\lim_{t\to t_0} \textbf{r}(t) = \textbf{r}(t_0)$$
  Conditions:\pause
  \begin{itemize}
    \item $\textbf{r}$ is defined at $t_0$
    \item $\lim_{t\to t_0} \textbf{r}(t)$ exists.
    \item Expected value (limit) = Actual value
  \end{itemize}
  \pause
  Component-wise:

  $\textbf{r}(t) = \langle x(t), y(t), z(t) \rangle$ is continuous at $t_0$ $\Longleftrightarrow$\\
  $x, y, z \colon [a,b] \to \RR$ are ALL continuous at $t_0$.

\end{frame}

\begin{frame}
  \frametitle{Derivatives}
  $$\textbf{f}\colon [a,b]\to \RR^3\quad , \quad \textbf{f}(t) = \langle x(t), y(t), z(t)\rangle$$
 \begin{itemize}
   \item  Average rate of change:
  $$\frac{\textbf{f}(t)-\textbf{f}(t_0)}{t-t_0} = \frac{\text{Displacement}}{\text{Time}} =
  \text{Average Velocity}$$
  %
  \item Instantaneous rate of change:
  $$\textbf{f}\,'(t_0) = \lim_{t\to t_0} \frac{\textbf{f}(t)-\textbf{f}(t_0)}{t-t_0} =
  \lim_{h\to 0}\frac{\textbf{f}(t_0+h)-\textbf{f}(t_0)}{h}$$
  %
  \item $\textbf{f}(t)$ vector $\Longrightarrow$ $\textbf{f}\,'(t)$ vector
  %
  \item Higher order derivatives: $\textbf{f}'(t)$, $\textbf{f}\,''(t) = (\textbf{f}\,'(t))'$ (acceleration), ...
  \item Component-wise operation:
  $$\textbf{f}\,'(t) = \langle x'(t), y'(t), z'(t)\rangle$$
 \end{itemize}

\end{frame}

\begin{frame}
  \frametitle{Tangent Lines}
  $$\textbf{f}\colon [a,b]\to \RR^3\quad , \quad \textbf{f}(t) = \langle x(t), y(t), z(t)\rangle$$
  \begin{itemize}
    \item $\textbf{f}\,'(t_0)$: direction of tangent line
  \item Equation of tangent line at $\textbf{f}(t_0)$:
  %
  $$\textbf{r}(t) = \textbf{f}(t_0) + t \textbf{f}\,'(t_0)$$

  \item Linear approximation:
  %
  $$\textbf{f}(t) \simeq L_{\textbf{f},t_0} (t) = \textbf{f}(t_0) + t \textbf{f}\,'(t_0)$$
  %
  \item Good approximation:
  %
  $$\lim_{t\to 0} \left|\frac{\textbf{f}(t) - L_{\textbf{f},t_0}(t)}{t} \right| =0$$
  %
  \item Differentials:
  %
  $$d\textbf{f} = \textbf{f}\, ' \, dt \Rightarrow d\textbf{f} = dt\, \langle x',y',z' \rangle$$
  \end{itemize}
\end{frame}

\begin{frame}
  \frametitle{Example}
  Coordinate curves for spherical coordinates:\\
  Fix $\rho = \rho_0$ and $\phi = \phi_0$.
  $$\textbf{r}(t) = \langle \rho_0\sin\phi_0 \cos{t}, \rho_0\sin\phi_0 \sin{t}, \rho_0\cos\phi_0\rangle$$
  \pause Then
  $$\textbf{r}'(t) = \langle -\rho_0\sin\phi_0 \sin{t}, \rho_0\sin\phi_0 \cos{t}, 0\rangle$$
  Define
  $$\widehat{\textbf{e}}_\theta (\rho_0,\phi_0,\theta_0) = \frac{1}{|\textbf{r}'(\theta_0)|}\,\textbf{r}'(\theta_0) = \langle -\sin{\theta_0},\cos{\theta_0},0\rangle$$
  Similar constructions for $\widehat{\textbf{e}}_\rho (\rho_0,\phi_0,\theta_0)$ and
  $\widehat{\textbf{e}}_\phi (\rho_0,\phi_0,\theta_0)$
  %
  $$\text{Compute}\qquad
  (\widehat{\textbf{e}}_{\rho} \times
  \widehat{\textbf{e}}_{\theta})\cdot
  \widehat{\textbf{e}}_{\phi}$$
\end{frame}

\begin{frame}
  \frametitle{Differentiation Rules}
  Component-wise operation $\Longrightarrow$ same rules as for scalar output\\
  \pause Product Rules:
   \begin{align*}
   [f(t) \textbf{r}(t)]' & = f'(t) \textbf{r}(t) + f(t) \textbf{r}'(t) \\
   %
   [\textbf{u}(t)\cdot \textbf{v}(t)]' & = \textbf{u}'(t)\cdot \textbf{v}(t) + \textbf{u}(t)
\cdot \textbf{v}'(t) \\
   %
   [\textbf{u}(t)\times \textbf{v}(t)]' & = \textbf{u}'(t) \times \textbf{v}(t) +
\textbf{u}(t)\times \textbf{v}'(t)
 \end{align*}
  \pause Chain Rule:
  $$[\textbf{r}(f(t))]' = f'(t) \textbf{r}'(f(t))$$
    \pause Example:
    $$\frac{d |\textbf{r}(t)|}{dt} =
    [\sqrt{\textbf{r}(t)\cdot \textbf{r}(t)}]' = [\sqrt{\Box}]' =
    \frac{1}{2\sqrt{\Box}} \Box' =
    \frac{1}{2\sqrt{\textbf{r}(t)\cdot \textbf{r}(t)}}
    [\textbf{r}(t)\cdot \textbf{r}(t)]' = $$
    $$= \frac{1}{2|\textbf{r}(t)|}
    [\textbf{r}'(t)\cdot \textbf{r}(t) +
    \textbf{r}(t)\cdot \textbf{r}'(t)] = \frac{\textbf{r}(t)\cdot \textbf{r}'(t)}{|\textbf{r}(t)|}$$
\end{frame}

\begin{frame}
  \frametitle{Application}
  $$|\textbf{r}|' = \frac{\textbf{r} \cdot \textbf{r}'}{|\textbf{r}|}$$

  Trajectory on a sphere with center at origin $\Longleftrightarrow$ $|\textbf{r}(t)| = $constant \pause $\Longleftrightarrow$

  $$|\textbf{r}(t)|'\equiv0 \Longleftrightarrow$$
  %
  $$\textbf{r}(t)\cdot \textbf{r}'(t)\equiv 0 \Longleftrightarrow$$
  %
  $$\textbf{r}(t) \bot \textbf{r}'(t) \Longleftrightarrow$$

  \pause Velocity  $\bot$ Position  $\Longleftrightarrow$ Velocity vector $\textbf{r}'(t)$ tangent to sphere.

  \bigskip

  How about the acceleration?\pause
  %
  $$\textbf{r}\cdot \textbf{r}'\equiv 0 \Longrightarrow [\textbf{r}\cdot \textbf{r}']'\equiv 0 \Longleftrightarrow
  \textbf{r}'\cdot \textbf{r}'+\textbf{r}\cdot \textbf{r}'' \equiv 0 \Longrightarrow \textbf{r}\cdot \textbf{r}'' = -|\textbf{r}'|^2 \leqslant 0$$
  %
  Acceleration vector $\textbf{r}''$ points inside the sphere.
\end{frame}

\begin{frame}
  \frametitle{Definite Integrals}
  $\textbf{r} \colon [a,b] \to \RR^3$

  \begin{itemize}
    \item Division $a =t_0 < t_1 <t_2 < \dotsb < t_k < t_{k+1} < \dotsb < t_n = b$
    \item Sample points $t_k \leqslant s_k \leqslant t_{k+1}$
    \item Riemann sum:
    $$\sum_{k=0}^{n-1} (t_{k+1}-t_k) \textbf{r}(s_k)$$
    \item Definite integral:
    $$\int_{t=a}^{t=b} \textbf{r}(t) \; dt = \lim \sum_{k=0}^{n-1} (t_{k+1}-t_k) \textbf{r}(s_k)$$
    \item Result: \pause a vector.
  \end{itemize}
\end{frame}

\begin{frame}
  \frametitle{Properties}
  \begin{itemize}
    \item\uncover<1->{ Component-wise: if $\textbf{r}(t) = \langle x(t), y(t), z(t) \rangle$, then
    %
    $$\int_{a}^{b} \textbf{r}(t) \; dt = \langle \int_{a}^{b} x(t) \; dt, \int_{a}^{b} y(t) \; dt,\int_{a}^{b} z(t) \; dt \rangle$$}
    \item\uncover<2->{ Substitution Rule:
    $$\int_{a}^b f'(t) \textbf{r}(f(t)) \; dt = \int_{f(a)}^{f(b)} \textbf{r}(\tau) \; d\tau$$}
    \item\uncover<3->{ Fundamental Theorem of Calculus: If $\textbf{u}'(t)\equiv \textbf{r}(t)$, then
    %
    $$\int_{t=a}^{t=b} \textbf{r}(t) \; dt = \textbf{u}(b) - \textbf{u}(a)$$}
    \item\uncover<4->{ Derivative $\Longrightarrow$ Total change
    %
    $$\textbf{r}(t) = \textbf{r}(t_0) + \int_{t_0}^t \textbf{r}'(\tau) \; d\tau$$}
  \end{itemize}
\end{frame}

\begin{frame}
  \frametitle{Application}

  Object thrown from initial position $\textbf{r}_0$ with initial velocity $\textbf{v}_0$.

  Describe trajectory (ignore air resistance).\pause

  Total force: Gravity.
%
$$m\textbf{a} = \textbf{F} =  -mg \textbf{k} \Longrightarrow \textbf{a} =
-g \textbf{k} \Longrightarrow \textbf{r}''(t) = -g \textbf{k}$$
\pause
%
$$\textbf{r}'(t) = \textbf{r}'(0) + \int_{0}^t -g \textbf{k} \; d\tau = \textbf{v}_0 + \left(\int_{0}^t -g\; d\tau \right) \textbf{k} = \textbf{v}_0 -gt \textbf{k}$$
%
\pause
$$\textbf{r}(t) = \textbf{r}(0) + \int_{0}^t (\textbf{v}_0-g\tau \textbf{k}) \; d\tau = \textbf{r}_0 + \left( \int_0^t d\tau \right) \textbf{v}_0 - \left( \int_0^t g\tau \; d\tau \right) \textbf{k} \Longrightarrow$$
%
$$\boxed{\textbf{r}(t) = \textbf{r}_0  +t  \textbf{v}_0 - \frac{1}{2}gt^2 \textbf{k}}$$
\pause
Parabola in the plane determined by $\textbf{v}_0$ and $\textbf{k}$.
\end{frame}

\begin{frame}
  \frametitle{Arclength}

  \begin{itemize}
    \item $\textbf{r}\colon [a,b] \to \RR^3$: piecewise smooth function
    %
    \item Distance traveled:
    %
    $$\text{Distance} = \text{Speed} \cdot \text{Time}$$
    %
    $$dL = |\textbf{r}'(t)| \, dt \Longrightarrow L = \int_{t=a}^{t=b} |\textbf{r}'(t)| \, dt$$

    \item $\Delta s$: distance along the curve
    %
    $$\Delta s \simeq \sqrt{(\Delta x)^2 + (\Delta y)^2 +
(\Delta z)^2} = \sqrt{\left(\frac{\Delta x}{\Delta t}
\right)^2 + \left(\frac{\Delta y}{\Delta t}\right)^2 +
\left(\frac{\Delta z}{\Delta t}\right)^2} \; \Delta t
\; .$$
%
\item Element of arclength ($\Delta t \to 0$):
%
$$ds = \sqrt{(x'(t))^2 + (y'(t))^2 + (z'(t))^2} \;
dt = |\textbf{r}'(t)| \, dt$$
%
\item Length of parametrized curve:
%
$$L = \int_{t=a}^{t=b} ds = \int_a^b |\textbf{r}'(t)| \, dt\; .$$
  \end{itemize}
\end{frame}

\begin{frame}
  \frametitle{Arclength Function}

  \begin{itemize}
    \item Fix the point $a$ as starting point. For $t \geqslant a$, let
\item $L(t) = $ distance traveled between $a$ and $t$ = \\
length of the piece of the curve corresponding
to values of the parameter between $a$ and $t$.
%
$$L(t) =  \int_{a}^t |\textbf{r}'(\tau)| \, d\tau $$
%
\item The function $L\colon [a,b]\to \RR$ is called the
\emph{arclength function}.
%
\item \underline{Example}: $\textbf{r}(t) = \langle \cos{t}, \sin{t}, t\rangle$.
Then
%
$$\textbf{r}'(t) = \langle -\sin{t}, \cos{t}, 1 \rangle
\Longrightarrow |\textbf{r}'(t)| = \sqrt{2}\; $$
%
and the arclength function is
%
$$L(t) = \int_0^t |\textbf{r}'(\tau)| \; d\tau = t\sqrt{2} \; .$$
  \end{itemize}

\end{frame}

\begin{frame}
  \frametitle{Parametrization by Arclength}

  \begin{itemize}
    \item $C$: piecewise smooth parametrized curve joining points $A$ and $B$;
    \item $\textbf{r} \colon I \to C$: parametrization of $C$,
    %
    $$\textbf{r}(t) = \text{position at time }t$$
    %
    Not canonically defined. Depends who is driving.
    %
    \item $\textbf{p} \colon [0,L] \to C$:
    %
    $$\textbf{p}(s) = \text{position at distance } s \text{ from }A \text{ along } C$$
    %
    Canonically defined. Markers along the road.
    %
    \item $\textbf{p}$: parametrization by arclength
    $$s=L(s) = \int_{\sigma=a}^{\sigma=s} |\textbf{p}'(\sigma)| \, d\sigma \Longrightarrow 1 = L'(s) = |\textbf{p}'(s)|\; .$$
    %

  \end{itemize}
\end{frame}

\begin{frame}
  \frametitle{Reparametrizations}

  \begin{itemize}
    \item $C$: piecewise smooth curve joining points $A$ and $B$;
    \item $\textbf{r} \colon [a,b] \to C$: parametrization of $C$;
    \item $\textbf{p} \colon [0,L] \to C$: arclength parametrization;
    \item \underline{Question}: How do we get $\textbf{p}$ from $\textbf{r}$?
    \item $Q = \textbf{r}(t) = \textbf{p}(s)$: point on curve $C$;
    $$s = \text{distance from } A \text{ to } Q \text{ along } C = \int_{\tau=a}^{\tau=t} |\textbf{r}'(\tau)| \, d\tau = \varphi(t)$$
    \item $\varphi$ invertible and $\varphi^{-1}$ smooth $\Longleftarrow \varphi'(t) \neq 0 \Longleftrightarrow \textbf{r}'(t)\neq \textbf{0}$.
     \item Regular parametrization: $\textbf{r}'(t) \neq 0$ for all $t$
    \item $t=\varphi^{-1}(s) \Longrightarrow \textbf{p}(s) = \textbf{r}(\varphi^{-1}(s))$.
  \end{itemize}
\end{frame}

\begin{frame}
  \frametitle{Example}

  \begin{itemize}
    \item $\textbf{r}(t) = \langle \cos{t}, \sin{t}, t\rangle$;
    \item $|\textbf{r}'(t)| = \sqrt{2} \Longrightarrow $
    $$\varphi(t) = \int_{\tau=0}^{\tau=t}|\textbf{r}'(\tau)|\, d\tau =  t\sqrt{2}$$
    \item $\varphi^{-1}(s) = \frac{s}{\sqrt{2}}$
    %
    $$\textbf{p}(s) = \langle \cos{\left( \frac{s}{\sqrt{2}} \right)}, \sin{\left( \frac{s}{\sqrt{2}} \right)}, \left( \frac{s}{\sqrt{2}} \right) \rangle$$
    %
    is a parametrization by arclength.
  \end{itemize}
\end{frame}

\begin{frame}
  \frametitle{Curvature}
  
  \begin{itemize}
    \item \underline{Question}: How can we \emph{measure} how bent a curve is?
    \item \underline{Solution}: Measure change in tangent
direction with respect to arclength.
  \end{itemize}
  
  \begin{itemize}
    \item $\textbf{p}=\textbf{p}(s)$: parametrization by arclength of smooth curve $C$;
    \item $\textbf{v}$: fixed direction (unit vector);
    \item $\textbf{T}(s)$: unit tangent vector;
    \item $\alpha(s)$: angle between $\textbf{T}(s)$ and $\textbf{v}$;
    \item We define the \emph{curvature} of $C$ at $\textbf{p}(s)$ to be
        %
        $$\kappa(s) = \left| \alpha'(s) \right|\; .$$
    \item Simpler formulas:
    $$\kappa(s) = | \textbf{T}'(s) | = \left| \frac{d\textbf{T}}{ds}\right| \; .$$
    \item $\textbf{r}=\textbf{r}(t)$: smooth parametrization, not necessary by arclength.
    $$\kappa(t) = \frac{|\textbf{T}'(t)|}{|\textbf{r}'(t)|} = \frac{|\textbf{r}''(t) \times \textbf{r}'(t)|}
{|\textbf{r}'(t)|^3}\; .$$
  \end{itemize}
  
\end{frame}

\begin{frame}
  \frametitle{Example}
  
  \begin{itemize}
    \item $\textbf{r}(t) = \langle \cos{t}, \sin{t}, t\rangle \Longrightarrow \textbf{r}'(t) = \langle -\sin{t}, \cos{t}, 1 \rangle \Longrightarrow|\textbf{r}'(t)| = \sqrt{2}$;
%
$$\textbf{T}(t) = \frac{1}{\sqrt{2}}
\langle -\sin{t}, \cos{t}, 1 \rangle
\Longrightarrow
\textbf{T}'(t) = \frac{1}{\sqrt{2}}
\langle -\cos{t}, -\sin{t}, 0 \rangle
\Longrightarrow $$
$$|\textbf{T}'|=\frac{1}{\sqrt{2}}$$
 %
 \item Curvature:
%
$$\kappa(t) = \frac{|\textbf{T}'(t)|}{|\textbf{r}'(t)|} =
\frac{1}{2}\; .$$ 
  \end{itemize}

Alternatively: $\textbf{r}''= \langle -\cos{t}, -\sin{t}, 0 \rangle$,
%
$$\textbf{r}'' \times \textbf{r}' = \left|
\begin{array}{ccc}
\textbf{i} & \textbf{j} & \textbf{k} \\
-\cos{t}&  -\sin{t}&  0 \\
-\sin{t}& \cos{t}& 1
\end{array}
\right| = -\sin{t} \, \textbf{i} +
\cos{t}\, \textbf{j} -\textbf{k} $$
%
$$\kappa(t) =
\frac{|\textbf{r}''(t) \times \textbf{r}'(t)|}
{|\textbf{r}'(t)|^3} =
\frac{\sqrt{2}}{(\sqrt{2})^3} = \frac{1}{2}\; .$$

\end{frame}

\begin{frame}
  \frametitle{Components of Acceleration}
  
  \begin{itemize}
    \item Object moves through space, $\textbf{r}=\textbf{r}(t)$ position vector at time $t$;
    \item Velocity vector $\textbf{v}(t) = \textbf{r}'(t)$; 
    \item Tangent direction: $\textbf{T}(t) = \frac{\textbf{v}(t)}{|\textbf{v}(t)|}$;
    \item Speed is $v(t) = |\textbf{v}(t)|$;
    \item Acceleration $\textbf{a}(t) = \textbf{r}''(t)$;
    \item Tangential component $\textbf{a}_T(t)$:
%
$$\textbf{a}_T(t) =
\textbf{\text{proj}}_{\bm{T}(t)} \textbf{a}(t) =
\frac{\textbf{a}\cdot \textbf{T}}{|\textbf{T}|}
\textbf{T} = \frac{\textbf{v}'\cdot \textbf{v}}
{|\textbf{v}|} \textbf{T} =
|\textbf{v}|' \textbf{T} = v' \textbf{T}\;,$$
%
$$a_T(t) = |\textbf{a}_T(t)| = |v'(t)|\; .$$

\item Normal component $\textbf{a}_N(t)=\textbf{\text{orth}}_{\bm{T}(t)} \textbf{a}(t)$,
%
$$a_N(t) = |\textbf{a}_N(t)| = |\textbf{\text{orth}}_{\bm{T}} \textbf{a}| =
|\textbf{a} \times \textbf{T}| =
\frac{|\textbf{r}'' \times \textbf{r}'|}
{|\textbf{r}'|} = \kappa |\textbf{r}'|^2 =
\kappa(t) v^2(t)  \; .$$
  \end{itemize}

\end{frame}

