\begin{frame}
\vskip -0.2cm
\begin{example}
Give simplified f-las for $f\circ g$, $f\circ f$, $g\circ f$, $g\circ g$. \alertNoH{2,3,4,5,21,22,31,32}{Find the implied domains.}
$
\begin{array}{@{}r@{}c@{}l@{}l|l}
\displaystyle \alertNoH{26}{ \alertNoH{8,27}{f(} \alertNoH{9,28}{x} \alertNoH{8,27}{)} }& \alertNoH{26}{=} &\displaystyle  \alertNoH{26}{ \only<handout:0|8,27>{\color{red}} \frac{2 \only<handout:0|8,27>{\color{black}} \alertNoH{9,28}{x} \only<handout:0|8,27>{\color{red}} -1}{\alertNoH{3,34}{\only<handout:0|8,27>{\color{black}}  \alertNoH{9,28}{x} \only<handout:0|8,27>{\color{red}} +2}}} && \uncover<2->{\alertNoH{2,3}{x \neq}  \fcAnswer{3}{-2}}\\
\displaystyle \alertNoH{7}{ g(x)}& \alertNoH{7}{=} &\displaystyle \alertNoH{7}{ \frac{2x+ 3}{\alertNoH{5,24}{5x-7}}} && \uncover<4->{\alertNoH{4,5,24}{x \neq}} \fcAnswer{5}{ \alertNoH{24}{\frac{7}{5}}}\\
\uncover<6->{% 
\displaystyle (f\circ g)(x)&\alertNoH{0}{=} &\displaystyle f(\alertNoH{7}{g(x)}) \uncover<7->{ = \only<handout:0|8>{\color{red}} f\left( \only<handout:0|8>{\color{black}} \alertNoH{7,9}{ \frac{2x+3}{ \alertNoH{24}{5x-7} }} \only<handout:0|8>{\color{red}}\right)\only<handout:0|8>{\color{black}}}
\uncover<8->{ = \only<handout:0|8>{\color{red}} \frac{ \alertNoH{10}{2} \only<handout:0|8>{\color{black}} \left( \alertNoH{9}{\frac{2x +3}{5x -7}} \right) \only<handout:0|8>{ \color{red}} -\alertNoH{11}{ 1} }{ \only<handout:0|8>{ \color{black}} \alertNoH{9}{\frac{2 x+3}{ 5x -7}} \only<handout:0|8>{\color{red}}+\alertNoH{12}{2 }}}
}%uncover<6-> 
\\
\uncover<10->{
&\alertNoH{0}{=}&\displaystyle \frac{ \frac{\alertNoH{10}{2} (2x+3)}{\alertNoH{13}{ 5x-7} }\alertNoH{14}{-} \alertNoH{11}{\frac{5x- 7}{ \alertNoH{13}{ 5x-7}}} }{\frac{2x+3}{ \alertNoH{13}{ 5x-7}}+ \alertNoH{12}{\frac{\alertNoH{15}{ 2( 5x-7) }}{\alertNoH{13}{ 5x-7}}}} \uncover<13->{= \frac{\frac{ \alertNoH{17}{ 4x} +\alertNoH{18}{6} \alertNoH{14 }{\alertNoH{17, 18}{-}(}\alertNoH{17}{5x}\alertNoH{18}{ - 7}\alertNoH{14}{)}}{\fcCancel{16}{ \alertNoH{13}{5 x-7} }}}{ \frac{\alertNoH{19}{2x} +\alertNoH{20}{3}+ (\alertNoH{15}{\alertNoH{19}{10x} \alertNoH{20}{ -14}}) }{\fcCancel{16}{ \alertNoH{13}{5x -7} }} }} \uncover<17->{= \frac{ \alertNoH{17}{-x} +\alertNoH{18}{ 13} }{\alertNoH{23}{ \alertNoH{19}{12x} \alertNoH{20}{-11}} } \uncover<21->{ && \alertNoH{21-24} {x\neq} \fcAnswer{22}{ \alertNoH{23}{ \frac{11}{12}} , \alertNoH{24}{\frac{7}{5}}}}}
}%uncover<10->
\\
\uncover<25->{
(f\circ f)(x)&\alertNoH{0}{=}& \displaystyle f(\alertNoH{26}{f(x)})\uncover<26->{ =\only<handout:0|27>{\color{red}} f\left(\only<handout:0|27>{\color{black}} \alertNoH{26,28}{ \frac{ 2x- 1}{\alertNoH{34}{x+2} }} \only<handout:0|27>{ \color{red}} \right) \only<handout:0|27>{\color{black}} } \uncover<27->{ = \alertNoH{29,30}{ \only<handout:0|27>{ \color{red}} \frac{  2  \only<handout:0|27>{ \color{black}} \left( \alertNoH{28}{\frac{ 2x- 1}{x+2}} \right)\only<handout:0|27>{\color{red}} -1 }{\only<handout:0|27>{\color{black}} \alertNoH{28}{\frac{ 2x- 1}{x+2}} \only<handout:0|27>{\color{red}}+2 }}
}}%uncover<25->
\\
\uncover<29->{ & \alertNoH{29,30}{=} &\displaystyle  \fcAnswer{30}{\frac{3 x-4}{ \alertNoH{33}{4 x+3} }} \uncover<31->{ && \alertNoH{31-34}{x\neq} \!\! \fcAnswer{32}{ \alertNoH{34}{-2}, \! \alertNoH{33}{ -\frac{3}{4}}} }
}%uncover<29->
 \\
\uncover<35->{ \alertNoH{35,36}{(g\circ f)(x)} &\alertNoH{35,36}{=}& \fcAnswer{36}{ \frac{7 x+4}{3 x-19}} && \alertNoH{35,36}{x\neq}  \fcAnswer{36}{ -2,\frac{19}{3}}} \\
\uncover<35->{\alertNoH{35,36}{ (g\circ g)(x)}&\alertNoH{35,36}{=} &\fcAnswer{36}{ \frac{19 x-15}{-25 x+64}} && \alertNoH{35,36}{ x \neq } \fcAnswer{36}{ \frac{7}{5},  \frac{64}{25} }}
\end{array}
$

\end{example}
\end{frame}