% begin module limit-laws-ex6
\begin{frame}
\begin{example} %[Example 6, p. 108]
\abovedisplayskip=0pt
\belowdisplayskip=-15pt
\abovedisplayshortskip=0pt
\belowdisplayshortskip=0pt
\begin{align*}
\text{Find}\quad \lim_{t\to 0} \frac{\sqrt{t^2 + 9}-3}{t^2}%
& \\%
\uncover<2->{%
\text{Plug in 0:}\quad%
\frac%
{\alert<handout:0| 2-3>{\sqrt{(0)^2+9}-3}}%
{\alert<handout:0| 4-5>{(0)^2}}%
}%
& \uncover<2->{%
= \frac%
{\uncover<3->{\alert<handout:0| 3>{0}}}%
{\uncover<5->{\alert<handout:0| 5>{0}}}%
}\\%
\uncover<6->{%
\intertext{Zero over zero is undefined, so we can't use direct substitution.}
}%
\uncover<7->{%
\intertext{Use minus the conjugate radical:}%
}%
\uncover<7->{%
\lim_{t\to 0} \frac%
{\sqrt{t^2+9}-3}%
{t^2}%
}%
& \uncover<7->{%
= \lim_{t\to 0} \frac%
{\alert<handout:0| 7-10>{\sqrt{t^2+9}-3}}%
{t^2}%
\cdot \frac%
{\uncover<handout:0| 8->{\alert<handout:0| 8-10>{\sqrt{t^2+9}+3}}}%
{\uncover<handout:0| 8->{\alert<handout:0| 8>{\sqrt{t^2+9}+3}}}%
}\\%
& \uncover<9->{ = \lim_{t\to 0} \frac{\uncover<10->{\uncover<handout:0| 10->{\alert<handout:0| 10>{(t^2+9)-9}}}}{\uncover<handout:0| 9->{t^2(\sqrt{t^2+9}+3)}}}  \uncover<11->{ = \lim_{t\to 0} \frac{\uncover<handout:0| 11->{\alert<handout:0| 12>{t^2}}}{\uncover<handout:0| 11->{\alert<handout:0| 12>{t^2}(\sqrt{t^2+9}+3)}}}\\%
& \uncover<12->{ = \lim_{t\to 0} \frac{\uncover<handout:0| 12->{1}}{\uncover<handout:0| 12->{\sqrt{\alert<handout:0| 13>{t}^2+9}+3}}}\\%
\uncover<13->{%
\text{Plug in 0:}\quad%
}%
& \uncover<13->{ = }%
\uncover<handout:0| 13->{\frac{1}{\sqrt{(\alert<handout:0| 13>{0})^2+9}+3}} \uncover<handout:0| 14->{ = \frac{1}{6}.}
\end{align*}
\end{example}
\end{frame}
% end module limit-laws-ex6
