% begin module limit-denominator-ex
\begin{frame}
\begin{example}[Example 6, p. 81]
\abovedisplayskip=0pt
\belowdisplayskip=-15pt
\abovedisplayshortskip=0pt
\belowdisplayshortskip=0pt
\begin{align*}
\text{Find}\quad \lim_{t\to 0} \frac{\sqrt{t^2 + 9}-3}{t^2}%
& \\%
\uncover<2->{%
\text{Plug in 0:}\quad%
\frac%
{\alertNoH{ 2-3}{\sqrt{(0)^2+9}-3}}%
{\alertNoH{ 4-5}{(0)^2}}%
}%
& \uncover<2->{%
= \frac%
{\uncover<3->{\alertNoH{ 3}{0}}}%
{\uncover<5->{\alertNoH{ 5}{0}}}%
}\\%
\uncover<6->{%
\intertext{Zero over zero is undefined, so we can't use direct substitution.}
}%
\uncover<7->{%
\intertext{Use a conjugate radical:}%
}%
\uncover<7->{%
\lim_{t\to 0} \frac%
{\sqrt{t^2+9}-3}%
{t^2}%
}%
& \uncover<7->{%
= \lim_{t\to 0} \frac%
{\alertNoH{ 7-10}{\sqrt{t^2+9}-3}}%
{t^2}%
\cdot \frac%
{\uncover<handout:0| 8->{\alertNoH{ 8-10}{\sqrt{t^2+9}+3}}}%
{\uncover<handout:0| 8->{\alertNoH{ 8}{\sqrt{t^2+9}+3}}}%
}\\%
& \uncover<9->{ = \lim_{t\to 0} \frac{\uncover<10->{\uncover<handout:0| 10->{\alertNoH{ 10}{(t^2+9)-9}}}}{\uncover<handout:0| 10->{t^2(\sqrt{t^2+9}+3)}}}  \uncover<11->{ = \lim_{t\to 0} \frac{\uncover<handout:0| 11->{\alertNoH{ 12}{t^2}}}{\uncover<handout:0| 11->{\alertNoH{ 12}{t^2}(\sqrt{t^2+9}+3)}}}\\%
& \uncover<12->{ = \lim_{t\to 0} \frac{\uncover<handout:0| 12->{1}}{\uncover<handout:0| 12->{\sqrt{\alertNoH{ 13}{t}^2+9}+3}}}\\%
\uncover<13->{%
\text{Plug in 0:}\quad%
}%
& \uncover<13->{ = }%
\uncover<handout:0| 13->{\frac{1}{\sqrt{(\alertNoH{ 13}{0})^2+9}+3}} \uncover<handout:0| 14->{ = \frac{1}{6}.}
\end{align*}
\end{example}
\end{frame}
% end module limit-denominator-ex
