% begin module integration-by-parts-intro
\begin{frame}
\frametitle{Integration by Parts}
Every \alertNoH{2}{differentiation rule} \uncover<3->{corresponds to a \alertNoH{3}{differential form rule}} \uncover<4->{which in turn corresponds to an integration rule.}
\[
\begin{array}{rcll|l}
\uncover<2->{\displaystyle (uv)'&=&\displaystyle  u' v + u v' &&\text{Product Rule}}\\
\uncover<3->{\displaystyle \diff (uv)&=&\displaystyle  v\diff u + u \diff v &&\text{Differential Prod. Rule} }\\
\uncover<4->{\displaystyle \alertNoH{5}{\int \diff (uv)}&=&\displaystyle  \int v\diff u + \int u \diff v&&\text{integration of the above}}\\
\uncover<5->{\displaystyle \alertNoH{5,6}{uv}&=&\displaystyle \alertNoH{8}{ \int v \diff u} + \alertNoH{7,9}{\int u \diff v}} \uncover<6->{ &&\text{rearrange}}\\
\displaystyle  \uncover<6->{\alertNoH{7,9}{ \int u \diff v}&\alertNoH{9}{=}&\displaystyle \alertNoH{9}{\alertNoH{6}{uv}- \alertNoH{8}{\int v \diff u}}}
\end{array}
\]
\uncover<9->{
We just proved the following.
\begin{proposition}[(Rule of) Integration by Parts]
$\displaystyle \alertNoH{9}{ \int u \diff v = uv- \int v \diff u}$
\end{proposition}
}
\end{frame}
% end module integration-by-parts-intro
