% begin module integration-by-parts-ex3
\begin{frame}
\alert<4,5,12,13>{Integration by parts:} $\displaystyle \int \alert<6,14>{u} \diff \alert<7,15>{v} = \alert<6 ,14>{ u} \alert<7,15>{v} - \int \alert<7,15>{v} \diff \alert<6,14>{u}.$

\begin{example}

$\begin{array}{rcll|l}
\displaystyle \int t^2\alert<2,3>{ e^t \diff t} \uncover<2->{ &\alert<0>{=}&\displaystyle \int \alert<6>{ t^2} \alert<2,3>{ \diff \left(\fcAnswer{3}{\alert<7>{e^t}}\right) }} \uncover<4->{&& \alert<4,5>{\text{integrate by parts}}}\\
\uncover<4->{&\alert<4>{=}&\displaystyle \fcAnswer{5}{  \alert<6>{t^2}\alert<7>{ e^t} - \int\alert<7>{ e^t} \alert<8,9>{\diff \left(\alert<6>{t^2}\right) }}}\\
\uncover<8->{ &\alert<0>{=}&\displaystyle t^2e^t- \int \alert<10,11>{e^t} \fcAnswer{9}{2t} \alert<8,9,10,11>{ \diff t}}\\
\uncover<10->{&\alert<0>{=}&\displaystyle t^2 e^t - 2 \alert<12,13>{ \int \alert<14>{t} \alert<10,11>{ \diff (\fcAnswer{11}{ \alert<15>{e^t} })}}} \uncover<12->{&&\alert<12,13>{\text{integrate by parts}}}\\
\uncover<12->{&\alert<0>{=}&\displaystyle t^2e^t\alert<17>{-2}\fcAnswer{13}{\left(\alert<14>{t} \alert<15>{e^t}\alert<17>{-} \alert<16>{\int \alert<15>{e^t} \diff \alert<14>{t}} \right)}}\\
\uncover<16->{&\alert<0>{=}&\displaystyle t^2e^t-2te^t\alert<17>{+2}\alert<16>{e^t}+C}
\end{array}
$
\end{example}
\end{frame}
% end module integration-by-parts-ex3
