\begin{frame}
\begin{example}
Compute $f_x$, $f_y$, where $f(x,y) = y^2\ln{(2x+y)}- e^y$.

\[
\renewcommand{\arraystretch}{1.5}
\begin{array}{r@{~}c@{~}l}
\uncover<2->{f_x &=&\displaystyle \frac{\partial f}{\partial x} = } \uncover<3->{\frac{\partial}{\partial x}\left(y^2\ln{(2x+y)}- e^y\right) =} \uncover<4->{\frac{\partial}{\partial x}\left( y^2\ln{(2x+y)}\right) - \frac{\partial}{\partial x}\left(e^y\right) } \\
\uncover<5->{&= &\displaystyle y^2 \frac{\partial}{\partial x}\left(\ln{(2x+y)}\right) - 0 =}\uncover<6->{ y^2 \cdot \frac{1}{2x+y} \cdot \frac{\partial}{\partial x}(2x+y) =}\uncover<7->{ \frac{2y^2}{2x+y}\; .}\\~\\
\uncover<8->{ f_y &=&\displaystyle \frac{\partial f}{\partial y} =}\uncover<9->{ \frac{\partial}{\partial y}\left(y^2\ln{(2x+y)}- e^y\right) =} \uncover<10->{ \frac{\partial}{\partial y}\left(y^2\ln{(2x+y)}\right) - \frac{\partial}{\partial y}\left(e^y\right) } \\
\uncover<11->{&  = &\displaystyle y^2 \frac{\partial}{\partial y}\left(\ln{(2x+y)}\right) +\frac{\partial}{\partial y}\left(y^2\right) \ln{(2x+y)}
- e^y } \\
\uncover<12->{&  = &\displaystyle 2y\ln{(2x+y)}+ y^2 \cdot \frac{1}{2x+y} \cdot \frac{\partial}{\partial y}(2x+y) - e^y } \\
\uncover<13->{& = &\displaystyle \frac{y^2}{2x+y} +2y\ln{(2x+y)} - e^y\; .} 
\end{array}
\]
\end{example}
\end{frame}