For each of the items below, do the following.
\begin{itemize}
\item Find the Maclaurin series of the function (i.e., the power series representation of the function around $a=0$).
\item Find the radius of convergence of the series you found in the preceding point. 
\end{itemize}
You are not asked to find the entire interval of convergence, but just the radius. In other words, you only need to find the inside of the interval of convergence but do not need to worry for the endpoints. Nevertheless in the answer key we indicate the entire interval of convergence - including the endpoints. 

The fact that the value of the series at the endpoints, whenever convergent, coincides with the value of the function has not been demonstrated so far. Nevertheless that is true - but we shall not show it here.

Please post on piazza if you discover errors in the answer key.
\begin{multicols}{2}
\begin{enumerate}[ref={\fcProblemRef}]
\item $\displaystyle \frac{1}{3-x}$.

\answer{$
\begin{array}{l}
\displaystyle \sum\limits_{n=0}^{\infty} \frac{x^n}{3^{n+1}}\\
R=3 \\
\text{converges for }x\in \left(-3,3 \right) 
\end{array}
$}
\item $\displaystyle \frac{1}{3-2x}$.

\answer{$
\begin{array}{l}
\displaystyle \sum\limits_{n=0}^{\infty} \frac{ 2^n}{3^{n+1}}x^n \\
R=\frac{3}{2}\\
\displaystyle \text{converges for }x\in \left(-\frac{3}{2},\frac{3}{2} \right) 
\end{array}
$}
\item $\displaystyle \frac{1}{2x+3}$.

\answer{ $\begin{array}{l}
\displaystyle \frac{1}{3}\left(1- \frac{2x}{3} +\left(\frac{2 x}{ 3} \right)^2 -\left(\frac{2x}{3}\right)^3+\dots\right) \\
\displaystyle = \sum\limits_{0}^{ \infty} \frac{(-1)^n}{3}\left(\frac{2}{3}\right)^n x^n  \\
R=\frac{3}{2}\\
\displaystyle \text{converges for }x\in \left(-\frac{3}{2}, \frac{3}{2} \right) 
 \end{array}
 $}
\item $\displaystyle \frac{1}{1+x^2}$.

\answer{$\begin{array}{l} 
\displaystyle \sum\limits_{n=0}^{\infty } (-1)^nx^{2n} \\
R=1\\
\text{converges for }x\in \left(-1,1 \right) 
\end{array}
$ }
\item $\displaystyle \frac{1}{1-2x^2}$.

\answer{ $ \begin{array}{l} 
\displaystyle \sum\limits_{n=0}^{\infty } 2^n x^{2n} \\
\displaystyle R=\frac{1}{2}\\
\displaystyle \text{converges for }x\in \left(-\frac{1}{2}, \frac{1}{2}\right)
\end{array}
$ }
\item \label{problemMaclaurin(1/(x^2-1))} $\displaystyle \frac{1}{x^2-1}$. 

\answer{$\begin{array}{l}
\displaystyle - \sum\limits_{n=0}^\infty x^{2n}\\
\displaystyle R=1\\
\text{converges for } x\in (-1,1)
\end{array}
$}
\item $\displaystyle\frac{\frac12}{x-1}-\frac{\frac12}{x+1}$.

\answer{same as \ref{problemMaclaurin(1/(x^2-1))}}
\item \label{problemMaclaurin(1/(1-x)^2)} $\displaystyle \frac{1}{(1-x)^2}$.

\answer{ $
\begin{array}{l}
1+2x+3x^2+4x^3+\dots\\
=\sum\limits_{n=0}^{\infty} (n+1) x^n \\
R=1\\
\text{converges for }x\in \left(-1,1 \right) 
\end{array}
$}
\item $\displaystyle \frac{1}{(1-x)^3}$.

\answer{ $
\begin{array}{l}
\frac{1}{2}\left( 2+6x+12x+\dots+n(n-1)x^{n-2}+\dots \right) \\
=\sum\limits_{n=0}^{\infty} \frac{(n+1)(n+2)}{2} x^n \\
R=1\\
\text{converges for }x\in \left(-1, 1  \right) 
\end{array}
$
}
\item $\displaystyle\ln (1+x)$.

\answer{ $
\begin{array}{l}
\displaystyle \sum\limits_{n=1}^\infty (-1)^{n+1} \frac{x^n}{n} \\
R=1\\
\text{converges for } x\in \left(-1,1\right]
\end{array}
$}
\item \label{problemMaclaurinSeriesln(1-x)} $\ln (1-x)$.

\answer{ $
\begin{array}{l}
\displaystyle -\sum\limits_{n=1}^\infty \frac{x^n}{n} \\
R=1\\
\text{converges for } x\in \left[-1,1\right)
\end{array}
$}
\item $\ln (1-3x)$.

\answer{ $
\begin{array}{l}
\displaystyle -\sum\limits_{n=0}^\infty \frac{3^n x^n}{n} \\
\displaystyle R=\frac{1}{3}\\
\displaystyle \text{converges for }x\in\left( - \frac{ 1}{ 3}, \frac{1}{3} \right] 
\end{array}
$}
\item $\ln (1-3x^2)$.

\answer{ $\begin{array}{l}
\displaystyle -\sum\limits_{n=1}^\infty \frac{3^nx^{2n }}{n} \\
\displaystyle R= \frac{1}{\sqrt{3}}\\
\displaystyle \text{converges for }x\in \left(- \frac{ 1}{ \sqrt{3}}, \frac{1}{\sqrt{3}}\right)
\end{array}
$}

\item \label{problemMaclaurin(ln(3-2x^2))} $\ln (3-2x^2)$.

\answer{ $\begin{array}{l}
\displaystyle \ln 3-\sum\limits_{n=1}^\infty \left( \frac{ 2}{3}\right)^n \frac{x^{2n }}{n} \\
\displaystyle R=\sqrt{\frac{2}{3}}\\
\displaystyle \text{converges for }x\in \left(-\sqrt{\frac{2}{3}}, \sqrt{\frac{2}{3}} \right)
\end{array}
$}
\item $x\ln (3-2x^2)$.

\answer{ $
\begin{array}{l}
\displaystyle x\ln 3-\sum\limits_{n=1}^\infty \left( \frac{ 2 }{3}\right)^n \frac{x^{2n+1 }}{n} \\
\displaystyle R=\sqrt{\frac{2}{3}}\\
\displaystyle \text{converges for }x\in \left(-\sqrt{\frac{2}{3}}, \sqrt{\frac{2}{3}} \right)
\end{array}
$}

\item $\displaystyle\arctan x$.

\answer{$
\begin{array}{l}
\displaystyle \sum\limits_{n=0}^\infty (-1)^n \frac{x^{2 n+1 }}{2n+1}\\
R=1\\
\text{converges for } x\in\left(-1 ,1 \right]
\end{array}
$ }
\item $\displaystyle\arctan (2x)$.

\answer{$
\begin{array}{l}
\displaystyle \sum\limits_{n=0}^\infty \frac{(-1)^n 2^{ 2n +1} x^{2n+1}}{2n+1}\\
\displaystyle R=\frac{1}{2}\\
\displaystyle \text{converges for }x\in \left( -\frac{ 1}{ 2}, \frac{1}{2} \right] 
\end{array}
$ }
\item $\displaystyle\arctan \left(2x^2\right)$.

\answer{$
\begin{array}{l}
\displaystyle \sum\limits_{n=0}^\infty (-1)^n \frac{ 2^{ 2n +1} x^{4n+2}}{2n+1}\\
\displaystyle R=\frac{1}{\sqrt{2}}\\
\displaystyle \text{converges for } x \in \left( -\frac{ 1}{ \sqrt{2}}, \frac{1}{\sqrt{2}} \right] 
\end{array}
$ }

\end{enumerate}
\end{multicols}