\solution{\ref{problemMaclaurin(ln(3-2x^2))}. 
We solve this problem by reducing it to Problem \ref{problemMaclaurinSeriesln(1-x)}, which asserts the power series expansion $\displaystyle \ln (1-y) = -\sum\limits_{n=1}^\infty \frac{y^n}{n}$ for $|y|<1$.
\[
\begin{array}{rcll|l}
\ln \left(3-2x^2\right)&=& \displaystyle \ln \left(3 \left(1 -\frac{2}{3} x^2\right)\right)\\
&=&\displaystyle \ln 3+ \ln  \left(1 -\frac{2}{3} x^2\right)&&\text{Set } y=\frac{2}{3}x^2\\
&=&\displaystyle \ln 3+\ln (1-y)\\
&=&\displaystyle \ln 3-\sum\limits_{n=1}^\infty \frac{y^n}{n}&& \begin{array}{l}
\ln (1-y)= -\sum\limits_{n=1}^\infty \frac{y^n}{n} \text{ for } |y|<1\\
\text{above does not hold for } |y|>1\\
\text{above may (not) hold for } y=\pm 1
\end{array}
\\
&=&\displaystyle \ln 3-\sum\limits_{n=1}^\infty \left(\frac{2}{3}\right)^n\frac{x^{2n}}{n}\quad . &&\text{Substituted back } y=\frac{2}{3}x^2\quad .
\end{array}
\]
As indicated above, the equality $\ln (1-y)= -\sum\limits_{n=1}^\infty \frac{y^n}{n}$ holds for $|y|<1$ and fails for $|y|>1$ (for $|y|>1$ the series $\sum\limits_{ n=1}^\infty \frac{y^n}{n}$ diverges). Therefore interval of convergence is given by 

\[\begin{array}{rcll|l}
|y|&<&1 &&\text{use }y=\frac{2}{3}x^2\\
\left|\frac{2}{3 }x^2\right|&<&1\\
|x^2|&<&\frac{3}{2}\\
|x|&<&\sqrt{\frac{3}{2}},
\end{array}
\]
i.e., the radius of convergence is $R=\sqrt{\frac{3}{2}}$.
}