\solution{\ref{problemIntervalConvergence_sum(x-2)^n/(3sqrt(n+1))}.
We apply the Ratio Test to get that $\lim\limits_{n\to \infty }\left| \frac{ a_{n+1} }{a_n }\right| = |x-2|$. Therefore the power series converges at least on the interval $(1, 3)$. When $x = 3$, the series becomes $\sum\limits_{n=1}^{\infty} \frac{1}{3\sqrt{n+1}}$, which diverges - this can be seen, for example, by comparing to the $p$-series $\frac{1}{\sqrt{n}}$. When $x = 1$, the series becomes $\sum\limits_{n=1}^{\infty} \frac{(-1)^n}{3\sqrt{n+1}}$, which converges by the Alternating Series Test. Our final answer $x\in [1, 3)$.
}