\solution{ \ref{problemIntegral x^4/((x^2+2)(x+1)^2)}
We are trying to integrate a rational function; we aim to decompose into partial fractions the following function. 
\[
\frac{x^{4}}{x^{4}+2x^{3}+3x^{2}+4x +2}=\frac{x^{4}}{ \left(x +1\right)^2 \left(x^{2}+2\right)}
\]

Since the numerator of the function is of degree greater than or equal to the denominator, we start the partial fraction decomposition by polynomial division.
\renewcommand{\arraystretch}{1.2}\begin{longtable}{|cccccc|} \hline&\multicolumn{5}{|c|}{\textbf{Remainder}}\\\multicolumn{1}{|c|}{} & &$\color{red}{-2x^{3}}\color{black}$ & $\color{red}{-3x^{2}}\color{black}$ & $\color{red}{-4x }\color{black}$ & $\color{red}{-2}\color{black}$ \\\hline\textbf{Divisor(s)} &\multicolumn{5}{|c|}{\textbf{Quotient(s)}}\\$x^{4}+2x^{3}+3x^{2}+4x +2$& \multicolumn{5}{|l|}{$1$}\\\hline& \multicolumn{5}{|c|}{\textbf{Dividend}}\\\multicolumn{1}{|c|}{$\underline{~}$} &$x^{4}$ & &&&\\&$x^{4}$ & $+2x^{3}$ & $+3x^{2}$ & $+4x $ & $+2$ \\\cline{2-6}&&$\color{red}{-2x^{3}}\color{black}$ & $\color{red}{-3x^{2}}\color{black}$ & $\color{red}{-4x }\color{black}$ & $\color{red}{-2}\color{black}$ \\\hline\end{longtable}
Therefore we have
\[
\begin{array}{rcl}
\displaystyle \frac{x^{4}}{x^{4}+2x^{3}+3x^{2}+4x +2}&=&\displaystyle 1+ \frac{-2x^3-3x ^2-4x-2}{x^{4}+2x^{3} +3x^{2} +4x +2}\\
\displaystyle \frac{-2x^3-3x^2-4x-2}{x^{4}+2x^{3}+3x^{2}+4x +2} & =&\displaystyle  \frac{-2x^3-3x^2-4x-2 }{\left(x +1\right)^2\left(x^{2}+2\right)}\\
&=&\displaystyle  \frac{A_1}{(x+1)}+\frac{A_2}{(x+1)^2}+\frac{A_3+A_4x}{(x^2+2)}
\end{array}
\]
We seek to find $A_i$'s that turn the above expression into an identity. Just as in the solution of Problem \ref{problemIntegrate x/(2x^2+x-1)dx}, we will use the method of coefficient comparison (see the solution of Problem \ref{problemint(3x^2+2x-1)/((x-1)(x^2+1))dx} for a shortcut method).


After clearing denominators, we get the following equality. 

\noindent$\begin{array}{@{}rcl@{}}
-2x^{3}-3x^{2}-4x -2 &=& A_{1} (x +1)(x^{2}+2)+A_{2} (x^{2}+2)\\
&&+(A_{3} + A_{4} x)(x +1)^{2}\\
0&=&(A_{4} +A_{1} +2)x^{3}\\
&&+(2A_{4} +A_{3} +A_{2} +A_{1} +3)x^{2}\\
&&+(A_{4} +2A_{3} +2A_{1} +4)x \\
&&+(A_{3} +2A_{2} +2A_{1} +2)\quad .
\end{array}
$

\noindent In order to turn the above into an identity we need to select $A_i$'s such that the coefficients of all powers of $x$ become zero. In other words, we need to solve the following system. 
\[
\begin{array}{llllll} & A_{1} & & & +A_{4} & =-2\\ & A_{1} & +A_{2} & +A_{3} & +2A_{4} & =-3\\ & 2A_{1} & & +2A_{3} & +A_{4} & =-4\\ & 2A_{1} & +2A_{2} & +A_{3} & & =-2\quad .\\
\end{array}
\] 
This is a system of linear equations. There exists a standard method for solving system of linear equations called Gaussian Elimination (also known as Row-Echelon Form Reduction Method). This method is very well suited for computer implementation. We illustrate it on this particular example; for a description of the method in full generality we direct the reader to a standard course in Linear algebra. 

\begin{longtable}{cc} System status & Action \\\hline $\begin{array}{llllll} & A_{1} & & & +A_{4} & =-2\\ & A_{1} & +A_{2} & +A_{3} & +2A_{4} & =-3\\ & 2A_{1} & & +2A_{3} & +A_{4} & =-4\\ & 2A_{1} & +2A_{2} & +A_{3} & & =-2\\\end{array}$& Sel. pivot column 2. Eliminate non-pivot entries. \\\hline $\begin{array}{llllll} & A_{1} & & & +A_{4} & =-2\\ & & A_{2} & +A_{3} & +A_{4} & =-1\\ & & & 2A_{3} & -A_{4} & =0\\ & & 2A_{2} & +A_{3} & -2A_{4} & =2\\\end{array}$& Sel. pivot column 3. Eliminate non-pivot entries. \\\hline $\begin{array}{llllll} & A_{1} & & & +A_{4} & =-2\\ & & A_{2} & +A_{3} & +A_{4} & =-1\\ & & & 2A_{3} & -A_{4} & =0\\ & & & -A_{3} & -4A_{4} & =4\\\end{array}$& Sel. pivot column 4. Eliminate non-pivot entries. \\\hline $\begin{array}{llllll} & A_{1} & & & +A_{4} & =-2\\ & & A_{2} & & +\frac{3}{2}A_{4} & =-1\\ & & & A_{3} & -\frac{A_{4} }{2} & =0\\ & & & & -\frac{9}{2}A_{4} & =4\\\end{array}$& Sel. pivot column 5. Eliminate non-pivot entries. \\\hline $\begin{array}{llllll} & A_{1} & & & & =-\frac{10}{9}\\ & & A_{2} & & & =\frac{1}{3}\\ & & & A_{3} & & =-\frac{4}{9}\\ & & & & A_{4} & =-\frac{8}{9}\\\end{array}$& Final result.\\ \end{longtable}

Therefore, the final partial fraction decomposition is the following. 
\[\begin{array}{rcl}
\displaystyle \frac{x^{4}}{x^{4}+2x^{3}+3x^{2}+4x +2}&=&\displaystyle 1+ \frac{-2x^{3}- 3x^{2}-4x -2}{x^{4}+2x^{3}+3x^{2}+4x +2}\\
&=&\displaystyle 1+ \frac{-\frac{10}{9}}{(x +1)}+\frac{\frac{1}{3}}{(x +1)^{2}}+\frac{-\frac{8}{9}x -\frac{4}{9}}{(x^{2}+2)}
\end{array}
\]

Therefore we can integrate as follows.
\[
\begin{array}{rcl}
\displaystyle \int \frac{x^4}{(x^2+2)(x+1)^2} \diff x &=&\displaystyle \int \left( 1+ \frac{-\frac{10}{9}}{(x +1)}+\frac{\frac{1}{3}}{(x +1)^{2}}+\frac{-\frac{8}{9}x -\frac{4}{9}}{(x^{2}+2)}\right)\diff x\\
&=&\displaystyle \int \diff x-\frac{10}{9}\int \frac{1}{(x +1)}\diff x + \frac{ 1}{3}\int \frac{ 1}{(x +1)^{2}}\diff x \\
&&\displaystyle -\frac{8}{9} \int \frac{x}{x^{2}+2}\diff x-\frac{4}{9} \int \frac{ 1}{x^{2}+2}\diff x \\
&=&\displaystyle x -\frac{1}{3} (x+1)^{-1}-\frac{10}{9} \log{}\left(x+1\right)\\
&&\displaystyle -\frac{4}{9} \log{}\left(x^{2} +2\right) -\frac{ 2}{ 9} \sqrt{ 2} \arctan{}\left(\frac{\sqrt{2}}{2} x\right)+C
\end{array}
\]
}

\solution{\ref{problemintx^5/(x^3-1)dx}
This problem can be solved directly with a substitution shortcut, or by the standard method. 

\textbf{Variant I (standard method).}

\noindent$\begin{array}{@{}r@{}c@{}l@{}l@{}|l}
\displaystyle \int \frac{x^5}{x^3-1}\diff x&=&\displaystyle \int\left( x^2+\frac{x^2}{x^3-1}\right)\diff x  &&\text{Polyn. long div. }\\
&=&\displaystyle\frac{x^3}{3}+\int \frac{x^2}{(x-1)(x^2+x+1)}\diff x&&\text{part. frac.}\\
&=&\displaystyle\frac{x^3}{3}+\int \left(\frac{\frac{1}{3}}{x -1}+\frac{\frac{2}{3}x +\frac{1}{3}}{x^{2}+x +1}\right)\diff x &&\text{complete square}\\
&=&\displaystyle \frac{x^3}{3}+\frac{1}{3}\ln |x-1|+\frac{2}{3}\int \frac{x+\frac{1}{2}}{\left(x+\frac{1}{2}\right)^2+ \frac{3}{4}}\diff x &&\text{Set } \begin{array}{rcl} u&=&\left(x+\frac{1}{2}\right)^2+ \frac{3}{4}\\\frac{1}{2}\diff u&= &\left(x+\frac{1}{2}\right) \diff x\end{array}\\
&=&\displaystyle \frac{x^3}{3}+\frac{1}{3}\ln |x-1|+\frac{1}{3} \int \frac{\diff u}{u}\\
&=&\displaystyle \frac{x^3}{3}+\frac{1}{3}\ln |x-1|+\frac{1}{3}\ln |u|+C\\
&=&\displaystyle \frac{x^3}{3}+\frac{1}{3}\ln |x-1|+\frac{1}{3}\ln |x^2+x+1|+C\\
\end{array}
$

\textbf{Variant II (shortcut method).}
\[
\begin{array}{rcll|l}
\displaystyle \int \frac{x^5}{x^3-1}\diff x&=&\displaystyle \int \frac{x^5-x^2+x^2}{x^3-1}\diff x\\
&=&\displaystyle \int \frac{x^2(x^3-1)+x^2}{x^3-1}\diff x\\
&=&\displaystyle\int x^2\diff x+ \int \frac{x^2}{x^3-1}\diff x\\
&=&\displaystyle \frac{x^3}{3}+\int \frac{\diff \left(\frac{x^3}{3}\right)}{x^3-1}\\
&=& \displaystyle \frac{x^3}{3}+\frac{1}{3} \int \frac{\diff \left(x^3-1\right)}{x^3-1}&&\text{Set }u=x^3-1\\
&=&\displaystyle \frac{x^3}{3}+\frac{1}{3}\int \frac{\diff u}{u}\\
&=&\displaystyle\frac{x^3}{3}+\frac{1}{3}\ln |u|+C\\
&=&\displaystyle \frac{x^3}{3}+\frac{1}{3} \ln \left|x^3-1\right|+C\quad .
\end{array}
\]
The answers obtained in the two solution variants are of course equal since 
\[
\ln |x-1|+\ln |x^2+x+1|= \ln \left|\left(x-1\right)\left(x^2+x+1\right)\right|=\ln \left|x^3-1\right|\quad .
\]
}

\solution{\ref{problemint(3x^2+2x-1)/((x-1)(x^2+1))dx}. 
This is a concise solution written in a form suitable for exam taking. We set up the partial fraction decomposition as follows.
\[
\displaystyle \frac{3x^2 + 2x - 1}{(x-1)(x^2+1)} = \frac{A}{x-1} + \frac{Bx+C}{x^2+1}\quad .
\]
Therefore $3x^2 + 2x - 1 = A(x^2+1) + (Bx+C)(x-1)$. 
\begin{itemize}
\item We set $x = 1$ to get $4 = 2A$, so $A = 2$.
\item We set $x = 0$ to get $-1=A-C$, so $C=3$.
\item Finally, set $x = 2$ to get $15=5A+2B+C$, so $B=1$.
\end{itemize}
We can now compute the integral as follows.
\[
\displaystyle \int\left( \frac{2}{x-1} + \frac{x+3}{x^2+1} \right) \diff x = 2 \ln(|x-1|) + \frac{1}{2} \ln(x^2+1) + 3 \Arctan x+K\quad .
\]
}
