% begin module differentiation-laws-constant
\begin{frame}
\begin{theorem}[The Constant Multiple Rule]
If $c$ is a constant and $f$ is a differentiable function, then
\abovedisplayskip=0pt
\belowdisplayskip=0pt
\[
\frac{\diff}{\diff x} [cf(x)] = c\frac{\diff}{\diff x}f(x).
\]
\end{theorem}
\begin{proof}
\abovedisplayskip=0pt
\belowdisplayskip=-15pt
\abovedisplayshortskip=0pt
\belowdisplayshortskip=0pt
\begin{align*}
\uncover<2->{%
\text{Let}\quad \alert<handout:0| 4>{g(x)} %
}%
 & \uncover<2->{%
 \alert<handout:0| 4>{= cf(x)}.  %
}\\%
\uncover<3->{%
\text{Then}\quad g'(x)%
}%
 & \uncover<3->{%
 = \lim_{h\rightarrow 0}\frac{g(x+h)-g(x)}{h}%
}\\%
 & \uncover<4->{%
 = \lim_{h\rightarrow 0}\frac{cf(x+h)-cf(x)}{h}%
}\\%
 & \uncover<5->{%
 = \lim_{h\rightarrow 0}\frac{\alert<handout:0| 6>{c}(f(x+h)-f(x))}{h}%
}\\%
\uncover<6->{%
\text{Limit Law 3:}\quad %
}%
 & \uncover<6->{%
 = \alert<handout:0| 6>{c}\alert<handout:0| 7-8>{\lim_{h\rightarrow 0}\frac{f(x+h)-f(x)}{h}}%
}\\%
 & \uncover<7->{%
 = c\alert<handout:0| 7-8>{\uncover<8->{f'(x).}}%
}%
\uncover<8->{\qedhere}
\end{align*}
\end{proof}
\end{frame}
% end module differentiation-laws-constant
