% begin module differentiation-laws-ex2
\begin{frame}
\begin{example}[Example 2, p. 137]
\begin{columns}[t]
\column{.5\textwidth}
\begin{eqnarray*}
& & \frac{\diff}{\diff x} (\alert<handout:0| 2>{3}x^4)\\
& \uncover<2->{ = } & %
\uncover<2->{\alert<handout:0| 2>{3}\frac{\diff}{\diff x}(x^4)}\\
& \uncover<3->{ = } & %
\uncover<3->{3(4x^3)}\\
& \uncover<4->{ = } & %
\uncover<4->{12x^3}\\
\end{eqnarray*}
\column{.5\textwidth}
\begin{eqnarray*}
& & \frac{\diff}{\diff x} (-x)\\
& \uncover<5->{ = } & %
\uncover<5->{\frac{\diff}{\diff x}[\alert<handout:0| 6>{(-1)}x]}\\
& \uncover<6->{ = } & %
\uncover<6->{\alert<handout:0| 6>{(-1)}\frac{\diff}{\diff x}(x)}\\
& \uncover<7->{ = } & %
\uncover<7->{(-1)(1)}\\
& \uncover<8->{ = } & %
\uncover<8->{-1}\\
\end{eqnarray*}
\end{columns}
\end{example}
\end{frame}
% end module differentiation-laws-ex2
