% begin module differentiation-laws-sum
\begin{frame}
\begin{theorem}[The Sum Rule]
If $f$ and $g$ are both differentiable, then
\abovedisplayskip=0pt
\belowdisplayskip=0pt
\[
\frac{\diff}{\diff x} [f(x) + g(x)] = \frac{\diff}{\diff x} f(x) + \frac{\diff}{\diff x}g(x).
\]
\end{theorem}
\begin{proof}
\abovedisplayskip=0pt
\belowdisplayskip=-15pt
\abovedisplayshortskip=0pt
\belowdisplayshortskip=0pt
\begin{align*}
\uncover<2->{%
\text{Let}\quad \alert<handout:0| 4>{F(x)}
}%
 &  \uncover<2->{%
\alert<handout:0| 4>{= f(x) + g(x)}.%
}\\%
\uncover<3->{%
\text{Then}\quad F'(x)%
}%
 & \uncover<3->{%
 = \lim_{h\rightarrow 0}\frac{F(x+h)-F(x)}{h}%
}\\%
& \uncover<4->{%
 = \lim_{h\rightarrow 0}\frac{[\alert<handout:0| 6>{f(x+h)}+\alert<handout:0| 7>{g(x+h)}]-[\alert<handout:0| 6>{f(x)}+\alert<handout:0| 7>{g(x)}]}{h}%
}\\%
& \uncover<5->{%
 = \lim_{h\rightarrow 0}\left[ \frac{\alert<handout:0| 6>{f(x+h) - f(x)}}{h} + \frac{\alert<handout:0| 7>{g(x+h)-\alert<handout:0| 7>{g(x)}}}{h}\right]%
}\\%
\uncover<8->{%
\text{Limit Law 1:}\quad %
}%
& \uncover<8->{%
 = \lim_{h\rightarrow 0} \frac{f(x+h) - f(x)}{h} + \lim_{h\rightarrow 0}\frac{g(x+h)-g(x)}{h}%
}\\%
& \uncover<9->{%
 = f'(x)+g'(x)%
}\uncover<9->{\qedhere}
\end{align*}
\end{proof}
\end{frame}
% end module differentiation-laws-sum
