% begin module differentiation-laws-polynomial
\begin{frame}
The \alert<handout:0| 4>{Constant Multiple Rule}, the \alert<handout:0| 3>{Sum Rule}, the \alert<handout:0| 3>{Difference Rule}, and the \alert<handout:0| 5-14>{Power Rule} can be combined to differentiate any polynomial.
\begin{example}[Derivative of a Polynomial]
\begin{align*}
\text{If}\quad y  & = x^{16} + 2\sqrt{3}x^7 - 4x^3 + \frac{x}{8} - 5,\\%
\uncover<1->{%
\text{Then}\quad \frac{\diff y}{\diff x}%
}% 
& = \uncover<2->{%
 \frac{\diff}{\diff x}\left( x^{16} + 2\sqrt{3}x^7 - 4x^3 + \frac{x}{8} - 5 \right) %
}\\%
& \uncover<3->{%
 = \frac{\diff}{\diff x}\left( x^{16}\right)%
 + \frac{\diff}{\diff x}\left( 2\sqrt{3}x^7 \right)%
 - \frac{\diff}{\diff x}\left( 4x^3 \right)%
 + \frac{\diff}{\diff x}\left( \frac{x}{8} \right)%
 - \frac{\diff}{\diff x}\left( 5 \right) %
}\\%
& \uncover<4->{%
 = \alert<handout:0| 5-6>{\frac{\diff}{\diff x}\left( x^{16}\right)}%
 + 2\sqrt{3}\alert<handout:0| 7-8>{\frac{\diff}{\diff x}\left( x^7 \right)}%
 - 4\alert<handout:0| 9-10>{\frac{\diff}{\diff x}\left( x^3 \right)}%
 + \frac{1}{8}\alert<handout:0| 11-12>{\frac{\diff}{\diff x}\left( x \right)}%
 - \alert<handout:0| 13-14>{\frac{\diff}{\diff x}\left( 5 \right)} %
}\\%
& \uncover<5->{%
 = \alert<handout:0| 5-6>{(\uncover<6->{16x^{15}})}%
 + 2\sqrt{3}\alert<handout:0| 7-8>{\left( \uncover<8->{7x^6} \right)}%
 - 4\alert<handout:0| 9-10>{\left( \uncover<10->{3x^2} \right)}%
 + \frac{1}{8}\alert<handout:0| 11-12>{\left( \uncover<12->{1} \right)}%
 - \alert<handout:0| 13-14>{\left( \uncover<14->{0} \right)} %
}\\%
& \uncover<15->{%
 = 16x^{15} + 14\sqrt{3}x^6 - 12x^2 + \frac{1}{8}.
}%
\end{align*}
\end{example}
\end{frame}
% end module differentiation-laws-polynomial
