% begin module differentiation-formulas-power
\begin{frame}
\begin{theorem}[The Power Rule]
\abovedisplayskip=0pt
\belowdisplayskip=0pt
\[
\text{If $n$ is a positive integer, then}\qquad \frac{\diff}{\diff x} (x^n) = nx^{n - 1}.
\]
\belowdisplayskip=0pt
\end{theorem}
\begin{proof}
\abovedisplayskip=0pt
\belowdisplayskip=-15pt
\abovedisplayshortskip=0pt
\belowdisplayshortskip=0pt
\begin{align*}
\uncover<2->{%
\intertext{Use this formula (which you can verify):}
}%
\uncover<2->{%
\alert<handout:0| 6>{x^n - a^n} %
}%
 & \uncover<2->{%
\alert<handout:0| 6>{= (x-a)(x^{n-1} + x^{n-2}a + \cdots + xa^{n-2} + a^{n-1})}.
}\\%
\uncover<3->{%
\intertext{Let $f(x) = x^n$.  Then}
}%
\uncover<3->{f'(a)} & \uncover<3->{ = }  %
\uncover<4->{\lim_{x\rightarrow a}\frac{f(x) - f(a)}{x-a}} \uncover<5->{ = } \uncover<5->{\lim_{x\rightarrow a}\frac{\alert<handout:0| 6>{x^n - a^n}}{x-a}}\\
& \uncover<6->{ = }  %
\uncover<6->{\lim_{x\rightarrow a}\frac{\alert<handout:0| 6>{\alert<handout:0| 7>{(x-a)}(x^{n-1} + x^{n-2}a + \cdots + xa^{n-2} + a^{n-1})}}{\alert<handout:0| 7>{x-a}}}\\
& \uncover<7->{ = }  %
\uncover<7->{\lim_{\alert<handout:0| 8>{x\rightarrow a}}(\alert<handout:0| 8>{x^{n-1}} + \alert<handout:0| 8>{x^{n-2}}a + \cdots + \alert<handout:0| 8>{x}a^{n-2} + a^{n-1})}\\
& \uncover<8->{ = }  %
\uncover<8->{\alert<handout:0| 8>{a^{n-1}} + \alert<handout:0| 8>{a^{n-2}}a + \cdots + \alert<handout:0| 8>{a}a^{n-2} + a^{n-1}} \uncover<9->{ = na^{n-1}.\qedhere}
\end{align*}
\end{proof}
\end{frame}
% end module differentiation-formulas-power
