% begin module negative-exponents
\begin{frame}[t]
\begin{theorem}[The Power Rule for Negative Exponents]
If $n$ is a positive integer, then %
\[
\frac{\diff}{\diff x}(x^{-n}) = -nx^{-n-1}.
\]
\end{theorem}
\begin{proof}
\abovedisplayskip=0pt
\belowdisplayskip=-15pt
\abovedisplayshortskip=0pt
\belowdisplayshortskip=0pt
\begin{align*}
\uncover<2->{%
\text{Let}\quad y = \alertNoH{ 2-3}{x^{-n}} %
}%
& \uncover<2->{\alertNoH{ 2-3}{ = \uncover<3->{\frac{1}{x^n}.}}%
}\\%
\uncover<4->{%
\text{Quotient Rule:}\quad%
}%
\uncover<4->{%
\frac{\diff y}{\diff x}%
}%
& \uncover<4->{%
 = \frac%
{\left( x^{n} \right) \alertNoH{ 5-6}{\frac{\diff}{\diff x}\left( 1 \right)} - \left( 1 \right) \alertNoH{ 7-8}{\frac{\diff}{\diff x}\left( x^n \right)}}%
{\left( x^n\right)^2}%
}\\%
& \uncover<5->{%
 = \frac%
{\left( x^n \right) \alertNoH{ 5-6}{\left(\uncover<6->{ 0 }\right)} - \left( 1 \right) \alertNoH{ 7-8}{\left( \uncover<8->{nx^{n-1}} \right)}}%
{ x^{2n}}%
}\\%
& \uncover<9->{%
 = -n\alertNoH{ 10-11}{\frac{x^{n-1}}{x^{2n}}}%
}\\%
& \uncover<10->{%
 = -n\alertNoH{ 10-11}{\uncover<11->{x^{-n-1}.}}%
}%
\end{align*}
\end{proof}
\end{frame}
% end module negative-exponents
