% begin module product-rule
\begin{frame}
Now we need a formula for the derivative of the product of two functions.  One might guess that the derivative of a product is the product of the derivatives; however, this is wrong.
\uncover<2->{%
\begin{example}[Incorrect Product Rule]
Let $f(x) = x$ and $g(x) = x^2$.
\begin{itemize}
\item<3-| alert@4-5>  $f'(x) = \uncover<5->{1.}$
\item<3-| alert@6-7>  $g'(x) = \uncover<7->{2x.}$
\item<8-| alert@9-10>  $(fg)(x) = \uncover<10->{x^3.}$
\item<8-| alert@11-12>  $(fg)'(x) = \uncover<12->{3x^2.}$
\item<13->  $(fg)'(x) = 3x^2 \neq 1\cdot 2x = f'(x)g'(x).$
\end{itemize}
\end{example}
}%
\uncover<14->{%
The correct formula is called the Product Rule.
}%
\end{frame}

\begin{frame}
\begin{theorem}[The Product Rule]
If $f$ and $g$ are both differentiable, then
\abovedisplayskip=0pt
\belowdisplayskip=0pt
\[
\frac{\diff}{\diff x} [f(x)g(x)] = f(x)\frac{\diff}{\diff x} [g(x)] + g(x)\frac{\diff}{\diff x} [f(x)] .
\]
\end{theorem}
\begin{proof}
\uncover<2->{Let $\alert<handout:0| 4>{F(x) = f(x)g(x)}$.  Then}
\abovedisplayskip=0pt
\belowdisplayskip=0pt
\[
 \uncover<2->{F'(x)}  \uncover<2->{ = } \uncover<3->{\lim_{h\rightarrow 0}\frac{F(x+h)-F(x)}{h}}  \uncover<4->{ = } \uncover<4->{\lim_{h\rightarrow 0}\frac{f(x+h)g(x+h) - f(x)g(x)}{h}}
\]
\abovedisplayskip=0pt
\belowdisplayskip=0pt
\begin{eqnarray*}
& \uncover<5->{ = } & %
\uncover<5->{\lim_{h\rightarrow 0}\frac{f(x+h)g(x+h) \alert<handout:0| 5>{- f(x+h)g(x) + f(x+h)g(x)} - f(x)g(x)}{h}}\\
& \uncover<6->{ = } & %
\uncover<6->{\lim_{h\rightarrow 0}\left[f(x+h) \frac{g(x+h)- g(x)}{h} + g(x)\frac{f(x+h)- f(x)}{h}\right]}\\
& \uncover<7->{ = } & %
\uncover<7->{\alert<handout:0| 8-9>{\lim_{h\rightarrow 0}f(x+h)}\alert<handout:0| 10-11>{\cdot \lim_{h\rightarrow 0}\frac{g(x+h) - g(x)}{h}}}\\
& & \ \uncover<7->{ + \alert<handout:0| 12-13>{\lim_{h\rightarrow 0}g(x)}\alert<handout:0| 14-15>{\cdot\lim_{h\rightarrow 0}\frac{f(x+h)- f(x)}{h}} = }\uncover<9->{\alert<handout:0| 9>{f(x)}}\uncover<11->{\alert<handout:0| 11>{g'(x)}} \uncover<13->{ + \alert<handout:0| 13>{g(x)}}\uncover<15->{\alert<handout:0| 15>{f'(x)}\qedhere}
\end{eqnarray*}
\end{proof}
\end{frame}
% end module product-rule
