% begin module sum-rule-with-algebra
\begin{frame}
\begin{example}[Difference Rule, Negative Fractional Exponents]
\abovedisplayskip=0pt
\belowdisplayskip=0pt
\abovedisplayshortskip=0pt
\belowdisplayshortskip=0pt
\begin{align*}
\text{Differentiate}\quad v & = \frac{3\sqrt{x} - \sqrt[3]{x}}{x}.\\%
\uncover<2->{%
v %
}%
& \uncover<2->{%
 = 3 \alert<handout:0| 3-4>{\frac{\sqrt{x}}{x}} - \alert<handout:0| 5-6>{\frac{\sqrt[3]{x}}{x}}
}\\%
\uncover<3->{%
v %
}%
& \uncover<3->{%
 = 3 \alert<handout:0| 3-4>{\uncover<4->{x^{-1/2}}} - \alert<handout:0| 5-6>{\uncover<6->{x^{-2/3}.}}
}\\%
\uncover<7->{%
\text{Difference Rule:}\quad %
\frac{\diff v}{\diff x} %
}%
& \uncover<7->{%
 = \frac{\diff}{\diff x}(\alert<handout:0| 8>{3}x^{-1/2}) - \frac{\diff}{\diff x}(x^{-2/3})
}\\%
\uncover<8->{%
\text{Constant Multiple Rule:}\quad %
}%
& \uncover<8->{%
 = \alert<handout:0| 8>{3}\alert<handout:0| 9-10>{\frac{\diff}{\diff x}(x^{-1/2})} - \alert<handout:0| 11-12>{\frac{\diff}{\diff x}(x^{-2/3})}
}\\%
\uncover<9->{%
\text{Power Rule:}\quad %
}%
& \uncover<9->{%
 = 3\alert<handout:0| 9-10>{\left( \uncover<10->{-\frac{1}{2}x^{-3/2}}\right)} - \alert<handout:0| 11-12>{\left( \uncover<12->{-\frac{2}{3}x^{-5/3}} \right)}
}\\%
& \uncover<13->{%
 = \frac{2}{3}x^{-5/3} - \frac{3}{2}x^{-3/2}.
}%
\end{align*}
\end{example}
\end{frame}
% end module sum-rule-with-algebra
