% begin module infinite-limit-at-infinity-ex9
\begin{frame}
\begin{example}[Example 9, p. 132]
Find $\lim_{x\rightarrow \infty}(x^2-x)$.
\begin{itemize}
\item<2-| alert@2->  WRONG: $\lim_{x\to\infty} (x^2-x) = \lim_{x\to\infty}x^2-\lim_{x\to\infty} x = \infty-\infty = 0$.
\item<3->  We can't use the limit laws in this way with $\infty$ because $\infty$ isn't a number.
\item<4->  Instead: $\lim_{x\to \infty} (x^2-x) = \lim_{x\to\infty}x(x-1) = \infty$.
\item<5->  This is because $x$ and $x-1$ both become arbitrarily large as $x\to\infty$.
\end{itemize}
\end{example}
\end{frame}
% end module infinite-limit-at-infinity-ex9
