% begin module limit-at-infinity-ex5
\begin{frame}
\begin{example}[Example 6, p. 131]
\begin{columns}[c]
\column{.45\textwidth}
Evaluate $\lim_{x\to \infty} \sqrt{x^2+1}-x$.

\ \only<handout:0| -8>{%
\includegraphics[width=5cm]{curve-sketching/pictures/04-04-ex5a.pdf}%
}%
\only<9->{%
\includegraphics[width=5cm]{curve-sketching/pictures/04-04-ex5b.pdf}%
}%
\begin{itemize}
\item<2->  $\sqrt{x^2+1}\to \infty$ and $x\to \infty$ as $x\to \infty$.
\item<2->  It isn't clear what happens to the difference.
\item<7-| alert@7>  Divide top and bottom by $x$.
\end{itemize}
\column{.55\textwidth}
\begin{itemize}
\item<3-| alert@3-4>  Standard approach: multiply top and bottom by conjugate radical.
\end{itemize}
\abovedisplayskip=0pt
\belowdisplayskip=0pt
\begin{eqnarray*}
&&%
\uncover<2->{%
\lim_{x\to \infty} \left( \sqrt{x^2+1}-x\right) \uncover<4->{\alert<handout:0| 4>{\frac{\sqrt{x^2+1}+x}{\sqrt{x^2+1}+x}}}%
}%
\\%
&&%
\uncover<5->{%
 = \lim_{x\to \infty} \frac{(x^2+1)-x^2}{\sqrt{x^2+1}+x}%
}%
\\%
&&%
\uncover<6->{%
 = \lim_{x\to \infty} \frac{1}{\sqrt{x^2+1}+x}\uncover<7->{\alert<handout:0| 7>{\cdot \frac{\frac{1}{x}}{\frac{1}{x}}}}%
}%
\\%
&&%
\uncover<8->{%
 = \lim_{x\to \infty} \frac{\frac{1}{x}}{\sqrt{1+\frac{1}{x^2}}+1}%
}%
\\%
&&%
\uncover<9->{%
 = \frac{0}{\sqrt{1+0}+1} = 0%
}%
\end{eqnarray*}
\end{columns}
\end{example}
\end{frame}
% end module limit-at-infinity-ex5
