\begin{frame}
\vskip -0.1 cm
\begin{proposition}[Product to sum formulas]
\[
\begin{array}{rcl}
\alertNoH{13}{\sin \alpha \sin \beta} &\alertNoH{13}{{=}}&\displaystyle \alertNoH{13}{\frac{1}{2}\left(\cos( \alpha -\beta) -\cos(\alpha+\beta) \right)}\\
\alertNoH{11}{\cos \alpha \cos \beta} &\alertNoH{11}{{=}}&\displaystyle \alertNoH{11}{ \frac{1}{\alertNoH{12}{2}} \left( \cos( \alpha -\beta) +\cos(\alpha+\beta) \right)} \\
\alertNoH{14}{\sin \alpha \cos \beta} &\alertNoH{14}{{=}}&\displaystyle \alertNoH{14}{\frac{1}{2}\left(\sin( \alpha +\beta) +\sin(\alpha-\beta) \right)}\\
\end{array}
\]
\end{proposition}
\begin{proof}
$
\begin{array}{lrcl}
\multirow{2}{*}{$\uncover<6->{\alertNoH{6,7,8,9,10}{+}}$}& \uncover<4->{ \fcAnswer{5}{ \alertNoH{6,8,9}{\alertNoH{10}{\cos\alpha\cos\beta} + \fcCancel{9}{ \sin\alpha\sin\beta}} } &\alertNoH{4,5,6}{{=}}& \uncover<4->{\alertNoH{4,5,6,7}{{\cos(\alpha-\beta)}}}}\\
\uncover<2->{& \fcAnswer{3}{\alertNoH{6,8,9}{ \alertNoH{10}{\cos\alpha\cos\beta} - \fcCancel{9}{\sin\alpha \sin\beta}}} &\alertNoH{2,3,6}{{=}}& \uncover<2->{\alertNoH{2,3,6,7}{{ \cos(\alpha+\beta)}}}}\\
\uncover<7->{&\fcAnswerUncover{7}{9}{\alertNoH{10,11}{ \alertNoH{12}{2}\cos\alpha \cos \beta}} &\alertNoH{11}{{=}}& \alertNoH{7,11}{{ \cos(\alpha-\beta)+\cos(\alpha+\beta)}}} \uncover<13->{\\\hline} \uncover<13->{  
\multirow{2}{*}{$\alertNoH{13}{-}$} &\cos\alpha\cos\beta+\sin\alpha\sin\beta &=&\alertNoH{13}{{\cos(\alpha-\beta)}}} \\
\uncover<13->{&\cos\alpha\cos\beta-\sin\alpha\sin\beta &=&\alertNoH{13}{{\cos(\alpha+\beta)}}}\\
\uncover<13->{&2\sin\alpha \sin \beta &=&\cos(\alpha-\beta)-\cos(\alpha+\beta)} \uncover<14->{\\\hline} \uncover<14->{ 
\multirow{2}{*}{$\alertNoH{14}{+}$}&\sin\alpha\cos\beta+\cos\alpha\sin\beta &=&\alertNoH{14}{{\sin(\alpha+\beta)}}}\\
\uncover<14->{&\sin\alpha\cos\beta-\cos\alpha\sin\beta &=&\alertNoH{14}{{\sin(\alpha-\beta)}}} \\
\uncover<14->{&2\sin\alpha \cos \beta &=&\sin(\alpha+\beta)+\sin(\alpha+\beta)}\\
\end{array}
$
\end{proof}

\end{frame}
\begin{frame}
\vskip -0.1 cm
\begin{proposition}[Product to sum formulas]
\[
\begin{array}{rcl}
\sin \alpha \sin \beta &=&\displaystyle \frac{1}{2}\left(\cos( \alpha -\beta) -\cos(\alpha+\beta) \right)\\
\cos \alpha \cos \beta &=&\displaystyle \frac{1}{2}\left( \cos( \alpha -\beta) +\cos(\alpha+\beta) \right)\\
\sin \alpha \cos \beta &=&\displaystyle \frac{1}{2}\left(\sin( \alpha +\beta) +\sin(\alpha-\beta) \right)\\
\end{array}
\]
\end{proposition}
\begin{itemize}
\item Product to sum formulas are used when integrating (a topic to be studied later/in another course).
\end{itemize}
\vskip 10cm

\end{frame}