\begin{frame}[t]
The integral $\int \sec \theta \diff \theta$ appears often in practice. A quicker solution will be shown later, but first we show the standard method.
\begin{example}
Set $\displaystyle \alert<9>{\theta=2\Arctan t}$, $\displaystyle \alert<3>{ \cos \theta =} \frac{1-\tan^2(\frac{\theta}{2}) }{1+\tan^2\left(\frac{\theta}{2}\right)}= \alert<3>{\frac{1-t^2}{1+t^2}}$, $\displaystyle  \alert<4>{\diff \theta = 2 \frac{1 }{ 1+t^2}\diff t}$.
$
\begin{array}{rclll}
\displaystyle \int \sec \theta\diff\theta &=& \displaystyle
\vphantom{ %phantom to align formulas
\ln \left|\frac{1+\tan \left(\frac{\theta}{2}\right)}{1-\tan \left(\frac{\theta}{2}\right)}\right|
} 
\displaystyle 
\only<1-10>{
\uncover<2->{ \int \frac{1}{\alert<3>{ \cos \theta}} \alert<4>{\diff \theta}}\uncover<3->{ = \int \frac{1}{ \left( \alert<3>{ \frac{1- t^2 }{ \alert<5>{1+t^2}}} \right)} \alert<4>{\frac{2}{(\alert<5>{ 1+t^2})} \diff t} } \\
\uncover<5->{ &=&\displaystyle \int \alert<6>{\frac{2}{1-t^2}}\diff t}\uncover<6->{ =\int \left(\alert<6>{ \frac{1}{1 -t}+ \frac{1}{ 1 +t}} \right)\diff t} \uncover<6->{&&\alert<6>{ \text{part. fractions}}}\\
\uncover<7->{&=&\displaystyle - \ln |1-t|+\ln |1+t| +C}\\
\uncover<8->{&=&\displaystyle \ln \left|\frac{1+\alert<9>{t}}{1-\alert<9>{t}}\right|+C}\\

\uncover<9->{&=&}
}
\only<1-21>{
\displaystyle \uncover<9->{ \alert<10,11>{\alert<21>{ \ln \left|\frac{1+\tan \left(\alert<9>{ \frac{\theta}{2}} \right)}{1-\tan \left(\alert<9>{\frac{\theta}{2}}\right)}\right|}+C} }
}
\only<22->{
\uncover<22->{\displaystyle  \alert<22>{\ln \left|\tan \theta +\sec \theta\right|} +C}
}
\end{array}
$

\only<11->{
\uncover<12->{
\noindent This is a perfectly good answer, however there's a simplification:}

$ 
\begin{array}{rcl} 
\uncover<12->{\alert<21,22>{\tan \theta+\sec \theta}&=&}\displaystyle\uncover<13->{ \frac{\alert<14>{ \sin \theta} +\alert<15>{1} }{\alert<16>{\cos \theta}}}\uncover<14->{ =\frac{\alert<17>{ \alert<14>{2\sin \frac{\theta}{2}\cos \frac{\theta}{2}} +\alert<15>{ \sin^2\frac{\theta}{2} + \cos^2\frac{\theta}{2}} }}{ \alert<16,18>{ \cos^2\frac{\theta}{2} -\sin^2\frac{\theta}{2}}} } \\
\uncover<17->{ &=&\displaystyle \frac{\alert<17>{ \left(\alert<19>{ \sin \frac{\theta}{2}+ \cos\frac{\theta}{2}} \right)^2 } }{ \alert<18>{ \left(\cos\frac{\theta}{2}-\sin \frac{\theta}{2}\right) \alert<19>{\left(\cos \frac{\theta}{2}+\sin \frac{\theta}{2}\right)} }}} \uncover<19->{ = \displaystyle \frac{\sin \frac{\theta}{2} +\cos\frac{\theta}{2}}{\cos\frac{\theta}{2} - \sin \frac{\theta}{2}}}\\
\uncover<20->{&\alert<21,22>{=}& \displaystyle\alert<21,22>{ \frac{1+\tan\frac{\theta}{2}}{1-\tan\frac{\theta}{2}}}\quad .}
\end{array}
$
}

\end{example}

\vspace{5cm}
\end{frame}