% begin module trig-integrals-ex2
\begin{frame}
\begin{example} %[Example 2, p. 496]
Evaluate $\int \sin^5 x \cos^2 x \diff x$.
\begin{itemize}
\item<2->  We could convert $\cos^2 x$ to $1 - \sin^2 x$, but then we'd have an expression involving $\sin x$ without any $\cos x$.
\item<3->  Instead split off one $\sin x$ and express the remaining $\sin^4 x$ in terms of $\cos x$:
\item<4-| alert@10>  $\sin^5 x = (\sin^2 x)^2\sin x = (1 - \cos^2 x)^2\sin x$.
\item<5->  Now let \alert<handout:0| 6-7,11>{$u = \uncover<7->{\cos x}$}, so \alert<handout:0| 8-9,12>{$\diff u = \uncover<9->{-\sin x \diff x}$}.
\end{itemize}
\abovedisplayskip=0pt
\belowdisplayskip=0pt
\begin{eqnarray*}
\uncover<10->{%
\int \alert<handout:0| 10>{\sin^5 x}\cos^2 x \diff x 
}%
& \uncover<10->{ = } &%
\uncover<10->{%
\int \alert<handout:0| 10>{(1-\alert<handout:0| 11>{\cos^2 x})^2}\alert<handout:0| 11>{\cos^2 x}\alert<handout:0| 10,12>{\sin x}\alert<handout:0| 12>{\diff x}
}\\%
& \uncover<11->{ = } &%
\uncover<11->{%
\int (1-\alert<handout:0| 11>{u^2})^2\alert<handout:0| 11>{u^2}\alert<handout:0| 12>{(-\diff u)}
}  \uncover<13->{ = } \uncover<13->{%
-\int (u^2 - 2u^4 + u^6)\diff u
}\\%
& \uncover<14->{ = } &%
\uncover<14->{%
-\left( \frac{u^3}{3} - 2\frac{u^5}{5} +\frac{u^7}{7}\right) + C
}\\%
& \uncover<15->{ = } &%
\uncover<15->{%
-\frac{1}{3}\cos^3 x + \frac{2}{5}\cos^5 x - \frac{1}{7}\cos^7 x + C
}%
\end{eqnarray*}
\end{example}
\end{frame}
% end module trig-integrals-ex2
