\solution{\ref{sum_n=0^infty(2^(n+1)+(-3)^(n-1))/5^n}.
\[
\begin{array}{rcll|l}
\displaystyle \sum\limits_{n=0}^{\infty} \frac{2^{n+1}+ (-3)^{ n-1}}{5^n} &=& \displaystyle \sum \limits_{n=0}^{ \infty} \left(2\cdot \frac{2^{n}}{5^n}-\frac{ 1 }{3}\cdot  \frac{ (-3)^n }{5^n}\right)\\
&=&\displaystyle 2 \sum_{n=0}^{ \infty}\left(\frac{2}{5 } \right)^n -\frac{1}{3} \sum_{ n=0}^{\infty}\left(-\frac{3}{5 } \right) ^n &&\text{use }\sum_{n= 0 }^\infty r^n=\frac{1}{1-r}, |r|<1\\
&=&\displaystyle 2\cdot  \frac{1}{ \left(1 -\frac{ 2}{5} \right)}- \frac{ 1}{3}\cdot  \frac{1 }{ \left(1-\left(-\frac{3}{ 5}\right) \right)} \\
&=&\displaystyle \frac{25}{8} \quad .
\end{array}
\]

}