Establish whether the series is convergent or divergent. Use the ratio or root tests. Show all your work. The answer key has not been proofread, use with caution.
\begin{enumerate}[ref={\fcProblemRef}]
\item \label{problemConvergenceSum n=0 ^ infty (-1)^n n^2 3^(-n)}
$\displaystyle \sum_{n=0}^\infty (-1)^n n^2 3^{-n}$
\answer{convergent, straightforward with ratio test}
\item $\displaystyle \sum \limits_{n=1}^{\infty} \left( \frac{ n+1 }{4n}\right)^n$
\answer{convergent, straightforward with root test}
\item $\displaystyle \sum\limits_{n=1}^{\infty}\left(\frac{4n+1 }{n}\right)^n$
\answer{divergent, straightforward with root test}
\item $\displaystyle \sum\limits_{n=1}^{\infty} \frac{n^n }{4^n n!}$
\answer{convergent, use ratio test}
\item \label{problemConvergenceSum_n=1^infty(4n)^n/nfactorial} $\displaystyle \sum\limits_{n=1}^{\infty} \frac{(4n)^n }{ n!}$
\answer{divergent, use ratio test}
\end{enumerate}