\solution{\ref{problemConvergenceSum n=0 ^ infty (-1)^n n^2 3^(-n)}
We proceed with the ratio test; the alternating series test works too, however that approach is a lot less straightforward and we leave it to the reader.

Let the $n^{th}$ term of the series be $a_n= (-1)^n n^2 3^{-n}$. The ratio test states that if the limit $\lim_{n\to \infty} \left|\frac{ a_{n+1}}{ a_n} \right|$ exists and is less than $1$, then the series is convergent, and if the limit exists and is greater than $1$, then then the series is divergent. 
\[
\begin{array}{rcl}
\displaystyle \lim\limits_{n\to \infty} \left|\frac{a_{n+1}}{a_n}\right|&=&\displaystyle \lim\limits_{n\to \infty} \left|\frac{(-1)^{n+1} 3^{-n-1} (n+1)^2}{(-1)^n 3^{-n}n^2}\right|\\
&=&\displaystyle \lim\limits_{n\to \infty} \left|\frac{ 1}{3 } \left(1+\frac{1}{n} \right)^2\right|\\
&=&\frac{1}{3} <1\quad .
\end{array}
\]
Therefore the series is convergent by the ratio test.
}

\solution{\ref{problemConvergenceSum_n=1^infty(4n)^n/nfactorial} 
The series can quickly be shown to be divergent by showing that $\lim_{n\to \infty}\frac{( 4n)^n}{n!}=\infty $. Nonetheless we will use the ratio test, as it provides insight to what happens when we replace the constant $4$ with another constant. In order to establish the divergence of 
\[ 
\sum_{n=1}^{\infty }\frac{(4n)^{n}}{n!}\quad ,
\]
we shall use the ratio test. We recall that the ratio test states that if $\displaystyle \lim\limits_{n\to \infty} \frac{a_{n+1}}{a_{n}} $ exists and is equal to $L$, then if $L>1$ the series is divergent and if $L<1$ the series is convergent (if $L=1$ the test is inconclusive). 

We compute:
\[
\begin{array}{rcl}
\displaystyle\lim\limits_{n\to \infty} \frac{a_{n+1}}{a_{n}}&=&\displaystyle \lim \limits_{ n \to\infty} \left|\frac{(4n+4)^{n+1}n !}{ (n+ 1)! ( 4n )^{ n}} \right|\\
&=&\displaystyle
\lim\limits_{n\to\infty} \left| \frac{ (4n+4)(4n+4 )^{n}}{(n+1)(4n)^{n}}\right|\\
&=&\displaystyle \left(\lim\limits_{n\to\infty} \frac{4n+4}{n+1} \right) \left(\lim\limits_{n\to \infty} \left( \frac{n+1}{n}\right)^{n}\right)=4e> 1\quad,
\end{array}
\]
and therefore the series is divergent.
}

