\solution{\ref{problemsum_(n=3)^(infty)(n^2+n+2)/(n^4-5n^2+4)}

The partial fractions decomposition algorithm shows that 
\[
\frac{n^{2}+n +2}{n^{4}-5n^{2}+4}=\frac{1}{3} \left( \frac{2}{n -2}-\frac{2}{n -1}+\frac{1}{n +1}-\frac{1}{n +2}\right)\quad .
\]
We omit the details of the partial fraction decomposition as it is quite laborious, but otherwise straightforward. Therefore 
\[
\begin{array}{rc@{}ll|l}
\displaystyle \sum\limits_{n=3}^{\infty}\frac{n^{2}+n +2}{n^{4}-5n^{2}+4}&=&\displaystyle \phantom{+} \frac{1}{3} \sum\limits_{n=3}^{\infty} \left( \frac{2}{n -2}-\frac{2}{n -1}+\frac{1}{n +1}-\frac{1}{n +2}\right)\\
&=&\displaystyle\phantom{+}  \frac{2}{3} \sum\limits_{ n=3}^{ \infty} \left( \frac{1}{n -2}-\frac{1}{n -1}\right)\\
&&\displaystyle +\frac{1}{3}\sum\limits_{n=3}^{\infty} \left(\frac{1}{n +1}-\frac{1}{n +2}\right)\\
&=& \displaystyle\phantom{+} \frac{2}{3} \left( \left(1- \cancel{ \frac{1}{2}} \right) + \left(\cancel{\frac{1}{2}}-\cancel{ \frac{2}{3}}\right)+\cancel{\dots} +\left(\cancel{\frac{1}{n-2}}-\frac{1}{n-1}\right)+\dots  \right)\\
&&\displaystyle+\frac{1}{3}\left( \left(\frac{1}{4} - \cancel{ \frac{1}{5}} \right) +\left(\cancel{ \frac{1}{5}}- \cancel{ \frac{1}{6}} \right)+\cancel{\dots} +\left( \cancel{ \frac{1 }{n+1}} -\frac{1}{n+2} \right)+\dots \right)\\
&=&\displaystyle \phantom{+}\lim\limits_{n\to \infty}  \frac{2}{3}\left(1-\frac{1}{n-1} \right)+\lim\limits_{n\to \infty}  \frac{1}{3}\left( \frac{1}{4} - \frac{1}{n+2} \right)\\
&=&\displaystyle \phantom{+}\frac{2}{3}+ \frac{1}{3} \cdot \frac{1}{4}\\
&=&\displaystyle \phantom{+}\frac{3}{4}


\quad .

\end{array}
\]


}