Use partial fractions to split the summand of each sum into two. Sum the telescoping series (a sum is ``telescoping'' if it can be broken into summands so that consecutive terms cancel). The answer key has not been proofread, use with caution.
\begin{enumerate}[ref={\fcProblemRef}]
\item $\displaystyle \sum\limits_{n=0}^{\infty} \frac{-6}{9 n^{2}+3 n-2}$\quad.
\answer{$ 2$}
\item \label{probelmSum_n=3^infty 3/(n^2-3n+2) }  $\displaystyle \sum \limits_{n=3}^{\infty} \frac{3}{n^{2}-3 n+2} $\quad.
\answer{$3$}

\item \label{problemsumn=2^inftyln(1-1/n^2)} $\displaystyle\sum_{n=2}^{\infty} \ln \left(1-\frac{1}{n^2}\right).$ (Hint: Use the properties of the logarithm to aim for a telescoping series).

\answer{$-\ln 2$}

\end{enumerate}