Use partial fractions to sum the telescoping series (a sum is ``telescoping'' if it can be broken into summands so that consecutive terms cancel).
\begin{multicols}{2}
\begin{enumerate}
\item $\displaystyle \sum\limits_{n=1}^\infty \frac{1}{n^{2}+n}$

\answer{$1$}
\item $\displaystyle \sum\limits_{n=2}^\infty\frac{2 n+1}{n^{4}+2 n^{3}- n^{2}-2 n}$

\answer{$\frac{1}{3}$}

\item $\displaystyle \sum\limits_{n=1}^\infty \frac{2 n}{n^{4}-3 n^{2}+1}$

\answer{$-1$}

\item \label{problemsum_(n=3)^(infty)(n^2+n+2)/(n^4-5n^2+4)} $\displaystyle \sum\limits_{n=3}^\infty \frac{n^{2}+n+2}{ n^{4}- 5  n^{2}+4}$
\answer{$\frac{3}{4}$}

\end{enumerate}
\end{multicols}