%begin module partial-fractions-building-block-1b
\begin{frame}
\frametitle{Building block Ib}
Building block Ib: $\displaystyle \int \frac{1}{x^n }\diff x=\int x^{-n}\diff x$, $n\neq 1$. 
\begin{example} Integrate the building block integral Ib
\[
\int \frac{1}{x^n }\diff x\quad , n\neq 1.
\]

\[
\int \frac{1}{x^n}\diff x \uncover<2->{\alert<2,3>{= \int x^{-n}\diff x}}\uncover<3->{\alert<3>{=}} \uncover<4->{\alert<4>{\frac{x^{-n+1}}{-n+1} +C}}
\]
\end{example}
\end{frame}
\begin{frame}
\frametitle{Linear substitutions leading to building block Ib}
Building block Ib: $\displaystyle \int \frac{1}{x^n }\diff x=\int x^{-n}\diff x= \frac{x^{-n+1}}{-n+1} +C$, $n\neq 1$. 
\begin{example} Integrate 
\[
\begin{array}{rcll|l}
\alert<8>{\displaystyle \int \frac{1}{(3x+5)^3 }\diff x} \uncover<2->{&=&\displaystyle \int \frac{1}{(3x+5)^3 }\frac{\alert<3>{ \diff (\alert<2>{3} x)}}{\alert<2>{3}}} \\
\uncover<3->{&=&\displaystyle \int \frac{1}{(\alert<4>{3x+5})^3 }\frac{\alert<3>{\diff ( \alert<4>{3 x+5})}}{3}} \uncover<4->{&&\text{Set }\alert<4,7>{ u=3x+5}{~~~~~~~~~~~~~~~~~~~} } \\
\uncover<4->{&=&\displaystyle \int\alert<5>{ \frac{1}{{\alert<4>{u}}^3} } \frac{\diff \alert<4>{u}}{3}}\\
\uncover<5->{ &=&\displaystyle \frac{1}{3} \alert<6>{\int \alert<5>{ u^{-3}} \diff u}} \uncover<6->{ =\frac{1}{3} \alert<6>{ \frac{{\alert<7>{u}}^{-2}}{(-2)}}+C}\\
\uncover<7->{&=&\displaystyle \alert<8>{-\frac{1}{6(\alert<7>{3x+5})^2}+C}\quad .}
\end{array}
\]

\end{example}
\end{frame}
\begin{frame}
\frametitle{Lin. subst. leading to building block Ib: general case}
Building block Ib: $\displaystyle \int \frac{1}{x^n }\diff x=\int x^{-n}\diff x= \frac{x^{-n+1}}{-n+1} +C$, $n\neq 1$. 
\begin{example} Let $n\neq 1$. Integrate 
\[
\begin{array}{rcll|l}
\displaystyle \alert<1>{\int \frac{1}{(ax+b)^n }\diff x} &=&\displaystyle \int \frac{1}{(ax+b)^n }\frac{\diff (a x)}{a} \\
&=&\displaystyle \int \frac{1}{(ax+b)^n }\frac{\diff (a x+b)}{a} &&\text{Set }u=ax+b\\
&=&\displaystyle \int\frac{1}{u^3}\frac{\diff u}{a}\\
&=&\displaystyle \frac{1}{a}\int u^{-n} \diff u =-\frac{1}{a} \frac{u^{-n+1}}{(n-1)}+C\\
&=&\displaystyle \alert<1>{-\frac{1}{ a(n-1)(ax+b)^{n-1}}+C}\quad .
\end{array}
\]

\end{example}
\end{frame}

%end module partial-fractions-building-block-1b