%begin module Building block IIIb
\begin{frame}
\frametitle{Building block IIIb}
\begin{itemize}
\item<1-> Building block IIIa:
\[
\uncover<6->{\alertNoH{6}{J(1)=}} \int \frac{1}{(x^2+1)}\diff x=\alertNoH{6}{\arctan x+C}\quad .
\]
\item<2-> Block IIIb:
\[
\uncover<4->{\alertNoH{4}{J(n)=}} \alertNoH{4}{\int \frac{1}{(x^2+1)^n}\diff x}
\]
\item<3-> Unlike other cases, IIIb is much harder than IIIa.
\item<4-> Set $\alertNoH{4}{J(n)=\int \frac{1}{(x^2+1)^n}\diff x}$. \uncover<5->{We are looking for a formula for $J(n)$.} \uncover<6->{We know $\alertNoH{6}{J(1)=\arctan x+C}$ (this is block IIIa).}
\item<7-> We start by $J(n-1) =\int \frac{1}{(x^2+1)^{n-1}} \diff x$ and integrate by parts.
\item<8-> In this way we end up expressing $J(n)$ via $J(n-1)$.
\item<9-> We work our way from $J(n)$ to $J(n-1)$, from $J(n-1)$ to $J(n-2)$, and so on, until we get to $J(1)$.
\end{itemize}
\end{frame}

\begin{frame}
\begin{example}
Recall that $\alertNoH{11,12}{J(n)=\int \frac{1}{(x^2+1)^{n}}\diff x}$. %\uncover<3->{Set $\alertNoH{3}{u=\frac{1}{(1+x^2)^{n-1}}}$.}
\uncover<2->{We have that:}
\[
\begin{array}{rcl}
\uncover<2->{\alertNoH{13,14,16}{J(n-1)}}
\only<handout:1|1-13>{\uncover<2->{&\alertNoH{13}{=} &
\displaystyle \int \alertNoH{3}{\frac{1}{(x^2+1)^{n-1 }}} \diff \alertNoH{4}{x} } \\
\uncover<3->{&=&\displaystyle  \alertNoH{3}{\frac{1}{(x^2+1)^{n-1}} } \alertNoH{4}{x}-\int  \alertNoH{4}{x} \alertNoH{5,6}{ \diff \left(\alertNoH{3}{ \frac{1}{ (1+x^2)^{ n-1}}}\right)}}\\
\uncover<5->{&=&\displaystyle  \frac{x}{(x^2+1)^{n-1}} \alertNoH{ 7}{-} \int \alertNoH{7}{ x} \left(\fcAnswer{6}{
\frac{ \alertNoH{7}{(-n+1) 2 x}}{ (1+x^2 )^{n}} }\right) \alertNoH{5, 6}{ \diff x}} \\
\uncover<7->{ &=&\displaystyle  \frac{x}{(x^2+1)^{n-1}} \alertNoH{7}{+ 2(n-1)} \int \frac{\uncover<8->{ \alertNoH{8,9}{1+}} \alertNoH{7,9}{x^2} \uncover<8->{\alertNoH{8,10}{-1}}}{ \alertNoH{9,10}{ (1+x^2)^n} }\diff x}\\
\uncover<9->{ &=&\displaystyle  \frac{x}{(x^2+1)^{n-1}}+ 2(n-1)\alertNoH{11}{ \int \alertNoH{9}{\frac{1}{(1+x^2)^{n-1}}} \diff x}} \\
\uncover<9->{&&\displaystyle \alertNoH{10}{-} 2(n-1)\alertNoH{12}{ \int \alertNoH{10}{\frac{1}{(1+x^2)^n}}\diff x} }\\
} %only<1-13>
\uncover<11->{&\alertNoH{13,14}{=}&\displaystyle \alertNoH{13,14}{ \frac{x}{(x^2+1)^{n-1}}+\alertNoH{16}{ 2(n-1)\alertNoH{11}{ J(n-1)}}  \alertNoH{15}{ -2(n-1)\alertNoH{12}{J(n)}}}\quad .}
\end{array}
\]

\only<handout:2|14->{
\uncover<15->{
Rearrange to get:
\[
\begin{array}{rcl}
\alertNoH{15}{ \alertNoH{17}{2(n-1)}J(n) } &=& \displaystyle \frac{x}{(x^2+1)^{n-1}}+\alertNoH{16}{(2n-3) J(n-1)} \\
\uncover<17->{ \alertNoH{19,20,21}{J (n ) }&\alertNoH{19, 20, 21 }{ =}&\displaystyle \alertNoH{19,20,21}{ \frac{x}{ \alertNoH{ 17}{(2n-2)} (x^2+ 1)^{ n-1}}+ \frac{2n-3}{ \alertNoH{ 17}{ 2n-2 }} J(n-1)} \quad .}
\end{array}
\]

\uncover<18->{In this way we expressed $J(n)$ using $J(n-1)$.} \uncover<19->{We apply the above formula consecutively:

$
\alertNoH{19}{ J(n)=  \frac{x}{ (2n-2) (x^2+ 1)^{ n-1}}+   \frac{ 2n-3}{ 2n-2}\only<handout:0|19,20>{ \alertNoH{20}{ J (n-1)}  \phantom{\left(\frac{x}{(2n-4)(x^2+1)^{n-2}}\right)}
}} \only<21->{\alertNoH{21}{\left(\frac{x}{(2n-4)(x^2+1)^{n-2}}+\frac{2n-5 }{2n-4} \alertNoH{22,23}{ J(n-2)} \right)}}  \uncover<22->{\alertNoH{22}{=\dots}}
$
}

\noindent \uncover<22->{\alertNoH{22}{and so on.}} \uncover<23->{The above can be used to write a formula for the final result, but that is as complicated as the process above.}

} %uncover15
} %uncover14
\end{example}


\vspace{8cm}
\end{frame}
%end module Building block IIIb
