
\begin{frame}
  \frametitle{Example}

  Let $\textbf{F}(u,v) = (u\cos{v}, u\sin{v}, e^{2u-4})$ and $P=\textbf{F}(2, \pi/3)$. \pause
%
\begin{align*}
  \textbf{F}_u(u,v) =  \langle \cos{v}, \sin{v}, 2e^{2u-4}\rangle & \Longrightarrow \textbf{F}_u(1,\pi/3) = \langle \frac{1}{2}, \frac{\sqrt{3}}{2}, 2\rangle \\
  %
  \textbf{F}_v(u,v) = \pause \langle -u\sin{v}, u\cos{v}, 0 \rangle & \Longrightarrow \textbf{F}_v(1,\pi/3) = \langle -\sqrt{3}, 1, 0 \rangle
\end{align*}
%
\pause
%
$$\textbf{N}(2,\pi/3) = \pause \textbf{F}_u(2,\pi/3) \times \textbf{F}_v(2,\pi/3)  \Longrightarrow \textbf{N}(2,\pi/3) = -2 \, \textbf{i} - 2\sqrt{3}\, \textbf{j} + 2\,\textbf{k}$$
%
and since $\textbf{F}(2,\pi/3) = \langle 1, \sqrt{3},1\rangle$, an equation for the tangent plane is\pause
%
$$(\langle x,y,z\rangle - \langle 1, \sqrt{3},1\rangle) \cdot \langle -2, -2\sqrt{3}, 2\rangle = 0$$
%
$$-2(x-1) -2\sqrt{3}(y-\sqrt{3}) +2(z-1) = 0 \Longleftrightarrow x + \sqrt{3} y -z = 3\; .$$
\pause
Parametric equations for the normal line are\pause
%
$$x= 1-2t, \quad y=\sqrt{3} -2\sqrt{3} t,\quad z = 1+2t\; .$$
\end{frame}