\begin{frame}
\frametitle{Tangent Plane to a Graph Surface}
\begin{columns}
\column{0.4\textwidth}
\psset{xunit=0.7cm, yunit=0.7cm}
\begin{pspicture}(-2.2,-2)(2,2)%
\tiny%
\fcBoundingBox{-2.2}{-1.4}{2.1}{2.2}%
\pstVerb{%
5 dict begin%
/theEllipsoidTop {[u v u 2 div dup mul v 1.5 div dup mul add 1 exch sub sqrt]} def%
/basePoint 2 dict begin /u 1 def /v 0 def theEllipsoidTop end def%
/tangent1 [0 1 0] def%
/tangent2 [1 0 3 sqrt 6 div -1 mul] def% 
}%
\fcStartIIIdScene%
\fcSurfaceInScene[forceForeground=false, linecolor=red,iterationsU=7,iterationsV=8,colorUV={1 0.5 0.5}, colorVU={0.7 0.2 0.2}]{-1.4}{-1}{1.4}{1}{theEllipsoidTop}%
\only<14->{%
\fcSurfaceInScene[linecolor=orange,iterationsU=2,iterationsV=2,colorVU=cyan,colorUV=cyan,forceForeground=true]{-2}{-2}{2}{2}{%
3 dict begin %
basePoint tangent1 u \fcVectorTimesScalar tangent2 v \fcVectorTimesScalar \fcVectorPlusVector \fcVectorPlusVector end%
}%
}%
\fcFinishIIIdScene%
\uncover<2->{\fcCurveIIId[linecolor=blue, linewidth=2pt]{-1.4}{1.4}{2 dict begin /u {t} def /v 0 def theEllipsoidTop end} }
\uncover<3->{\fcCurveIIId[linecolor=blue, linewidth=2pt]{-1}{1}{2 dict begin /u 1 def /v {t} def theEllipsoidTop end} }
\fcAxesIIId{3}{3}{3}%
\fcDotIIId[linecolor=blue]{basePoint}%
\uncover<5->{\fcLineIIId[arrows=->, linewidth =2pt, linecolor=brown]{basePoint}{basePoint tangent2 \fcVectorPlusVector}}%
\uncover<7->{\fcLineIIId[arrows=->, linewidth =2pt, linecolor=brown]{basePoint}{basePoint tangent1 \fcVectorPlusVector}}%
\uncover<13->{%
\fcLineIIId[arrows=->, linewidth =2pt, linecolor=orange]{basePoint}{basePoint tangent2  tangent1 \fcVectorCrossVector \fcVectorPlusVector}%
}%
\pstVerb{end}%
\end{pspicture}
\column{0.6\textwidth}
\begin{itemize}
\item Graph surface $z=f(x,y)$, point $P(x_0,y_0,z_0)$ on the surface.
\item<2-> Call $\fcv p(x)$ the curve given by $f(x,y)$ by keeping $y=y_0$ constant; \uncover<3->{call $\fcv q(y)$ the curve given by $f(x,y)$ by keeping $x=x_0$ constant.} 
\end{itemize}
\end{columns}
\begin{itemize}
\item<4-> $\begin{array}{rclllrcl}
\alert<4,5>{\fcv{p}(x)}&\alert<4,5>{=}& \alert<4,5>{\langle x,y_0, f(x,y_0) \rangle} &&&
\uncover<5->{\alert<5>{\fcv p'(x_0)}}& \uncover<5->{ \alert<5>{ =}}& \uncover<5->{\alert<5>{ \langle 1,0,f_x(x_0,y_0)\rangle}} \\
\alert<6,7>{\fcv q(y)}&\alert<6,7>{=}& \alert<6,7>{ \langle x_0,y, f(x_0,y) \rangle } &&&
\uncover<7->{\alert<7>{ \fcv q'(y_0)}}&\uncover<7->{\alert<7>{=}}& \uncover<7->{\alert<7>{\langle 0,1,f_y(x_0,y_0)\rangle}} \; .
\end{array}
$
\item<8-> Normal to tangent plane at $P$:
$\alert<13>{ \fcv{n} =} \alert<9>{ \fcv{p}'(x_0) }\times \alert<10>{ \fcv q'(y_0)} =  \uncover<9->{\alert<11,12>{ \alert<9>{\langle 1,0,f_x(x_0,y_0)\rangle} \times \alert<10>{\langle 0,1,f_y(x_0,y_0)\rangle }} } \uncover<11->{ \alert<11,12>{ =}} 
\uncover<12->{\alert<12,13,16>{\langle -f_x(x_0,y_0), -f_y(x_0,y_0), 1 \rangle}} \; .
$
\item<14-> Equation of tangent plane at $P(x_0,y_0,f(x_0,y_0))$:
$\alert<14>{ \alert<16>{ \fcv{n}} \cdot (\alert<15>{ \fcv{r}-\fcv{r}_0}) = 0 }$
\uncover<15->{
$ \alert<16>{ -f_x(x_0,y_0)}\alert<15>{ (x-x_0)}  \alert<16>{ -f_y(x_0,y_0)}\alert<15>{ (y-y_0)} + \alert<15>{ (z-f(x_0,y_0))} = 0  $
}
\uncover<17->{
$\boxed{ \; z= f(x_0,y_0) + f_x(x_0,y_0) (x-x_0) + f_y(x_0,y_0)(y-y_0) \; }\; .$
}
\end{itemize}
\end{frame}