% begin module IVT-ex9
\begin{frame}
\begin{example}
Show that there is a root of the equation
\[
4x^3 - 6x^2 + 3x - 2 = 0
\]
between 1 and 2.
\begin{itemize}
\item<2->  Let $f(x) = 4x^3 - 6x^2 + 3x - 2$.
\item<3->  Use the intermediate value theorem with $a = 1$, $b = 2$, and $N = 0$.
\item<4->  $f(1) = 4\cdot 1^3 - 6\cdot 1^2 + 3\cdot 1 - 2 = -1 < 0$.
\item<5->  $f(2) = 4\cdot 2^3 - 6\cdot 2^2 + 3\cdot 2 - 2 = 12 > 0$.
\item<6->  $N = 0$ is a number between $f(1) = -1$ and $f(2) = 12$.
\item<7->  Therefore there is a $c$ between $1$ and $2$ such that $f(c) = 0$.
\end{itemize}
\end{example}
\end{frame}
% end module IVT-ex9
