

\begin{frame}\frametitle{Difference of vectors}
\begin{columns}
\column{0.4\textwidth}
\psset{xunit=1cm, yunit=1cm}
\begin{pspicture}(-0.5,-2.5)(4.1,3.1)%
\fcBoundingBox{-0.5}{-2.5}{4.1}{3.1}
\uncover<1,2,6>{\rput[b](1, 0.6){$\bm u$}}
\uncover<1,2,6>{\psline[arrows=->](0,0)(2,1)}
\uncover<3>{\psline[arrows=->, linecolor=red](0,0)(2,1)}

\uncover<3-4,7->{\psline[arrows=->, linecolor=red](2,1)(0,0)}
\uncover<5>{\psline[arrows=->](2,1)(0,0)}
\uncover<3>{\rput[lt](1,0.5){$\alert<3>{-\bm u=\bm{BA}}$}}
\uncover<4-5,7->{\rput[lt](1,0.5){$\alert<4,7>{-\bm u}$}}
\uncover<3>{\fcFullDot{0}{0}}
\uncover<6>{\psline[arrows=->](0,0)(1,-2)}
\uncover<7>{\psline[arrows=->, linecolor=red](0,0)(1,-2)}
\uncover<6->{\rput[tr](0.5, -1){$\alert<7>{\bm v}~$}}

\uncover<1-5>{
\rput[tl](0,-0.1){$A$}
\rput[tl](2,0.9){$B$}
}
\end{pspicture}
\column{0.6\textwidth}
\begin{itemize}
\item Let $\bm u=\bm{AB}$. 
\item<2-> We define $-\bm u$ to be \uncover<5->{\alert<5>{the}} \uncover<1-4>{a} vector for which $\bm u +(-\bm u)=\bm 0 $. 
\item<3-> Since $\bm{AB} + \bm{BA} = \bm{0}$, it follows $\alert<3>{-\bm u=\bm {BA}}$.
\item<4-> In other words $-\bm{u}$ is depicted using the arrow opposite to $\bm u$.
\item<5-> From picture, it's evident \alert<5>{$-\bm u $ can be chosen in a only one way}.
\item<6-> We define the difference of vectors $\bm v, \bm u$ via \uncover<7->{$\alert<7>{\bm{v}-\bm{u}= (-\bm{u})+ \bm{v} } $ (triangle rule)}.
\end{itemize}
\end{columns}
\end{frame}