\begin{problem} (Textbook, page 136, 1-44).
Compute the derivative.
\begin{multicols}{2}
\begin{enumerate}
\item $f(x)=2^{40}$.

\answer{$0$}
\item $f(x)=\pi^2$.

\answer{$0$}
\item $f(t)=2-\frac{2}{3}t$.

\answer{$-\frac{2}{3}$}
\item $F(x)=\frac{3}{4}x^8$.

\answer{$6 x^{7}$}
\item $f(x)=x^3-4x+6$.

\answer{$-4+3 x^{2} $}
\item $f(t)=\frac{1}{2}t^6-3t^4+t$.

\answer{$ 3 t^{5}-12 t^{3}+1$}
\item $g(x)=x^2(1-2x)$. 

\answer{$ 2 x-6 x^{2}$}
\item $h(x)=(x-2)(2x+3)$.

\answer{$ 4x-1$}
\item $g(t)=2t^{-3/4}$.

\answer{$-\frac{3}{2} t^{-\frac{7}{4}} $}
\item $B(y)=c y^{-6}$.

\answer{$-6 c y^{-7} $}
\item $A(s)=-\frac{12}{s^5}$.

\answer{$60 s^{-6}$}
\item $y=x^{\frac53}-x^{\frac23}$.

\answer{$ \frac53 x^{\frac23}-2/3 x^{-\frac13}$}
\item $S(p)=\sqrt{p}-p$.

\answer{$-1+\frac{1}{2} p^{-\frac{1}{2}} $}
\item $y=\sqrt{x}(x-1)$.

\answer{$ \frac{3}{2} x^{\frac{1}{2}}- \frac{1}{2}  x^{-\frac{1}{2}}$}
\item $R(a)=(3a+1)^2$.

\answer{$6+18 a $}
\item $S(R)=4\pi R^2$.

\answer{$8 \pi R$}
\item $y=\frac{ x^2+4x+3}{\sqrt{x}}$.

\answer{$ 2 x^{-\frac{1}{2}}+\frac{3}{2} x^{\frac{1}{2}}-\frac{3}{2} x^{-\frac{3}{2}}$}
\item $y=\frac{\sqrt{x}+x}{x^2}$.

\answer{$- x^{-2}-\frac{3}{2} x^{-\frac{5}{2}} $}
\item $H(x)=(x+x^{-1})^3$.

\answer{$3x^{2}+3-3x^{-2}-3x^{-4} $}
\item $g(u)=\sqrt 2 u +\sqrt{3u}$.

\answer{$ \sqrt{2}+\frac{\sqrt3}{2}  u^{-\frac{1}{2}}$}
\item $u=\sqrt[5]t+4\sqrt{t^5}$.

\answer{$10 t^{\frac{3}{2}}+\frac{1}{5} t^{-\frac{4}{5}} $}
\item $v=\left(\sqrt{x}+\frac{1}{\sqrt[3]{x}}\right)^2$.


\answer{$1+\frac{1}{3} x^{-\frac{5}{6}}-\frac{2}{3} x^{-\frac{5}{3}} $}
\item $f(x)=(1+2x^2)(x-x^2)$.

\answer{$1-2 x+6 x^{2}-8 x^{3}$}
\item $f(x)=\frac{x^4-5x^3+\sqrt{x}}{x^2}$.

\answer{$-5+2 x-\frac{3}{2} x^{-\frac{5}{2}} $}
\item $V(x)=(2x^3+3)(x^4-2x)$.

\answer{$-6-4 x^{3}+14 x^{6}$}
\item $L(x)=(1+x+x^2)(2-x^4)$.

\answer{$ 2+4 x-4 x^{3}-5 x^{4}-6 x^{5}$}
\item $F(y)=\left(\frac{1}{y^2}-\frac{3}{y^4} \right)(y+5y^3)$.

\answer{$5+9 y^{-4}+14 y^{-2} $}
\item $J(v)=(v^3-2v)(v^{-4}+v^{-2})$.

\answer{$1+6 v^{-4}+v^{-2}$}
\item $g(x)=\frac{1+2x}{3-4x}$.

\answer{$ 10 (3-4 x)^{-2}$}
\item $f(x)=\frac{x-3}{x+3}$.

\answer{$6 (3+x)^{-2} $}
\item $y=\frac{x^3}{1-x^2}$.

\answer{$ \frac{3 x^{2}- x^{4}}{(1- x^{2})^{2}}$}
\item $y=\frac{x+1}{x^3+x-2}$.

\answer{$\frac{-3-3 x^{2}-2 x^{3}}{(-2+x+x^{3})^{2}} $}
\item $y=\frac{v^3-2v\sqrt{v}}{v}$.

\answer{$2 v- v^{-\frac{1}{2}}$}
\item $y=\frac{t}{(t-1)^2}$.

\answer{$-\frac{t +1}{(t-1)^3} $}
\item $y=\frac{t^2+2}{t^4-3t^2+1}$.

\answer{$\frac{14 t-8 t^{3}-2 t^{5}}{(1-3 t^{2}+t^{4})^{2}} $}
\item $g(t)=\frac{t-\sqrt{t}}{t^{1/3}}$.

\answer{$-\frac{1}{6} t^{-\frac{5}{6}}+\frac{2}{3} t^{-\frac{1}{3}} $}
\item $y=a x^2+b x + c$.

\answer{$ b+2 a x$}
\item $y=A+\frac{B}x +\frac{C}{x^2}$.

\answer{$\frac{- B-2 C x^{-1}}{x^{2}}$}
\item $f(t)=\frac{2t}{2+\sqrt{t}}$.

\answer{$\frac{4+t^{\frac{1}{2}}}{(2+t^{\frac{1}{2}})^{2}} $}
\item $y=\frac{c x}{1+c x}$.

\answer{$ c (1+c x)^{-2}$}
\item $y=\sqrt[3]{t}(t^2+t+t^{-1}) $.

\answer{$-\frac{2}{3} t^{-\frac{5}{3}}+\frac{4}{3} t^{\frac{1}{3}}+\frac{7}{3} t^{\frac{4}{3}} $}
\item $y=\frac{u^6-2u^3+5}{u^2}$.

\answer{$-2-10 u^{-3}+4 u^{3} $}
\item $f(x)=\frac{x}{x+\frac{c}{x}}$.

\answer{$ \frac{2 x c}{(c+x^{2})^{2}}$}
\item $f(x)=\frac{a x+b}{c x+ d}$.

\answer{$\frac{a d- b c}{(d+c x)^{2}}$}
\end{enumerate}
\end{multicols}
\end{problem}