Compute the derivative.
\begin{multicols}{2}
\begin{enumerate}[ref={\fcProblemRef}]

\item $\displaystyle f(x)=\frac{x-3}{x+3}$.

\answer{$6 (3+x)^{-2} $}
\item $\displaystyle y=\frac{x^3}{1-x^2}$.

\answer{$ \frac{3 x^{2}- x^{4}}{(1- x^{2})^{2}}$}
\item $\displaystyle y=\frac{x+1}{x^3+x-2}$.

\answer{$\frac{-3-3 x^{2}-2 x^{3}}{(-2+x+x^{3})^{2}} $}
\item $\displaystyle y=\frac{x^3-2x\sqrt{x}}{x}$.

\answer{$2 x- x^{-\frac{1}{2}}$}
\item \label{problemd/dt(t/(t-1)^2)}  $\displaystyle y=\frac{t}{(t-1)^2}$.

\answer{$-\frac{t +1}{(t-1)^3} $}
\item $\displaystyle y=\frac{t^2+2}{t^4-3t^2+1}$.

\answer{$\frac{14 t-8 t^{3}-2 t^{5}}{(1-3 t^{2}+t^{4})^{2}} $}
\item $\displaystyle g(t)=\frac{t-\sqrt{t}}{t^{\frac{1}{3}}}$.

\answer{$-\frac{1}{6} t^{-\frac{5}{6}}+\frac{2}{3} t^{-\frac{1}{3}} $}
\item $\displaystyle y=a x^2+b x + c$.

\answer{$ b+2 a x$}
\item $\displaystyle y=A+\frac{B}x +\frac{C}{x^2}$.

\answer{$\frac{- Bx-2 C }{x^{3}}$}
\item $\displaystyle f(t)=\frac{2t}{2+\sqrt{t}}$.

\answer{$\frac{4+t^{\frac{1}{2}}}{\left( 2+t^{\frac{1 }{ 2}} \right)^{2}} $}
\item $\displaystyle y=\frac{c x}{1+c x}$.

\answer{$ c (1+c x)^{-2}$}
\item $\displaystyle y=\sqrt[3]{t}(t^2+t+t^{-1}) $.

\answer{$-\frac{2}{3} t^{-\frac{5}{3}}+\frac{4}{3} t^{\frac{1}{3}}+\frac{7}{3} t^{\frac{4}{3}} $}
\item $\displaystyle y=\frac{u^6-2u^3+5}{u^2}$.

\answer{$-2-10 u^{-3}+4 u^{3} $}
\item $\displaystyle f(x)=\frac{a x+b}{c x+ d}$.

\answer{$\frac{a d- b c}{(d+c x)^{2}}$}
\item $\displaystyle f(x)=\frac{1+x }{1+\frac{2}x}$. 

\answer{$\frac{x^{2}+4 x+2}{(2+x)^{2}}$}
\item $\displaystyle f(x)=\frac{1+x }{1+\frac{3}x}$. 

\answer{$\frac{x^{2}+6 x+3}{(3+x)^{2}}$}
\item $\displaystyle f(x)=\frac{x}{x+\frac{c}{x}}$.

\answer{$ \frac{2 x c}{(c+x^{2})^{2}}$}
\end{enumerate}
\end{multicols}
