Compute the derivative.
\begin{multicols}{2}
\begin{enumerate}[ref={\fcProblemRef}]
\item $\displaystyle y=x^{\frac53}-x^{\frac23}$.

\answer{$ \frac53 x^{\frac23}-2/3 x^{-\frac13}$}
\item $\displaystyle f(x)=\sqrt{x}-x$.

\answer{$-1+\frac{1}{2} x^{-\frac{1}{2}} $}
\item $\displaystyle y=\sqrt{x}(x-1)$.

\answer{$ \frac{3}{2} x^{\frac{1}{2}}- \frac{1}{2}  x^{-\frac{1}{2}}$}
\item $\displaystyle f(x)=(2x+1)^2$.

\answer{$4+8 x $}
\item $\displaystyle f(x)=4\pi x^2$.

\answer{$8 \pi x$}
\item $\displaystyle y=\frac{ x^2+4x+3}{\sqrt{x}}$.

\answer{$ 2 x^{-\frac{1}{2}}+\frac{3}{2} x^{\frac{1}{2}}-\frac{3}{2} x^{-\frac{3}{2}}$}
\item $\displaystyle y=\frac{\sqrt{x}+x}{x^2}$.

\answer{$- x^{-2}-\frac{3}{2} x^{-\frac{5}{2}} $}
\item $\displaystyle f(x)=\left(x+x^{-1}\right)^3$.

\answer{$3x^{2}+3-3x^{-2}-3x^{-4} $}
\item $\displaystyle f(x)=\sqrt 2 x +\sqrt{5x}$.

\answer{$ \sqrt{2}+\frac{\sqrt5}{2}  x^{-\frac{1}{2}}=\sqrt{2}+\frac{\sqrt5}{2\sqrt{x}}$}
\item $\displaystyle y=\sqrt[5]x+4\sqrt{x^5}$.

\answer{$10 x^{\frac{3}{2}}+\frac{1}{5} x^{-\frac{4 }{5}} $}
\item \label{problemd/dx((sqrt(x)+1/sqrt[3](x))^2)} $\displaystyle y=\left(\sqrt{x}+ \frac{1}{ \sqrt[3]{x}}\right)^2$.


\answer{$1+\frac{1}{3} x^{-\frac{5}{6}}-\frac{2}{3} x^{-\frac{5}{3}} $}
\item $\displaystyle f(x)=(1+2x^2)(x-x^2)$.

\answer{$1-2 x+6 x^{2}-8 x^{3}$}
\item $\displaystyle f(x)=\frac{x^4-5x^3+ \sqrt{x}}{x^2}$.

\answer{$-5+2 x-\frac{3}{2} x^{-\frac{5}{2}} $}
\item $\displaystyle f(x)=(2x^3+3)(x^4-2x)$.

\answer{$-6-4 x^{3}+14 x^{6}$}
\item $\displaystyle f(x)=(1+x+x^2)(2-x^4)$.

\answer{$ 2+4 x-4 x^{3}-5 x^{4}-6 x^{5}$}
\item $\displaystyle g(y)= \left(\frac{1}{y^2}- \frac{3}{y^4} \right)(y+5y^3)$.

\answer{$5+9 y^{-4}+14 y^{-2} $}
\item $\displaystyle f(x)=(x^3-2x)(x^{-4}+x^{-2})$.

\answer{$1+6 x^{-4}+x^{-2}$}
\item $\displaystyle f(x)=\frac{1+2x}{3-4x}$.

\answer{$ 10 (3-4 x)^{-2}$}
\end{enumerate}
\end{multicols}