\solution{\ref{problemConvergencex^2/(x^4+2)from-inftyto+infty}
The integrand is a rational function and therefore we can solve this problem by finding the indefinite integral and then computing the limit. We would need to start by factoring $x^4+2$ into irreducible quadratic factors - that is already quite laborious:
\[
x^4+2= \left(x^2+\sqrt[4]{8}x+\sqrt{2} \right)\left(x^2-\sqrt[4]{8}x+\sqrt{2}\right)\quad.
\]
The problem asks us only to establish the convergence of the integral; it does not ask us to compute its actual numerical value. Therefore we can give a much simpler solution. The function is even and therefore it suffices to establish whether $\displaystyle \int\limits_0^\infty \frac{x^2}{x^4+2}\diff x$ is convergent.

We have that 
\[
\int\limits_{0}^\infty \frac{x^2}{x^4+2}\diff x= \int\limits_{0}^1 \frac{x^2}{ x^4 +2 }\diff x+\int\limits_{1}^\infty \frac{x^2}{x^4+2}\diff x\quad.
\]
The function $ \frac{x^2}{x^4+2}$ is continuous so $\int\limits_{0}^1 \frac{x^2}{x^4+2}\diff x$ integrates to a number, which does not affect the convergence of the above expression. Therefore the convergence of our integral is governed by the convergence of $\int\limits_{1}^\infty \frac{x^2}{x^4+2}\diff x$. To establish that that integral is convergent, we use the comparison theorem as follows.
\[
\begin{array}{rcll|l}
\displaystyle
\int\limits_{1}^\infty \frac{x^2}{x^4+2}\diff x&\leq & \displaystyle \int \limits_{ 1}^\infty \frac{x^2}{x^4}\diff x && \begin{array}{l} \text{we have that } x^4+2>x^4\\ \text{and therefore }\displaystyle \frac{x^2}{x^4+2}\leq \frac{x^2}{x^4}\end{array}\\
&=&\displaystyle \int_1^{\infty} x^{-2}\diff x\\
&=&\displaystyle \lim\limits_{t\to \infty} \left[ -\frac{1}{x}\right]_{1}^{t}\\
&=&\displaystyle  \lim\limits_{t\to\infty} 1- \frac{1}{t}\\
&=&\displaystyle  1\quad .
\end{array}
\]
In this way we showed $ \displaystyle\int_{1}^\infty \frac{x^2}{x^4+2} \diff x \leq 1$. Therefore, as $\displaystyle \frac{x^2 }{ x^4 + 2}\geq 0 $ is positive, we can apply the comparison theorem to get that $\displaystyle\int_{1}^\infty \frac{ x^2}{x^4+2} \diff x $ is convergent.
}

\solution{\ref{problemConvergencesqrt(x)e^-sqrt(x)zerotoinfty}
It is possible to show that this integral is convergent by using the comparison theorem. However, we shall use direct integration instead. First, we solve the indefinite integral:

\[
\begin{array}{rcll|l}
\displaystyle \int \sqrt{x} e^{-\sqrt{x}} \diff x&=& \displaystyle \int \sqrt{x} e^{-\sqrt{x}} \frac{2\sqrt{x} \diff x}{2\sqrt{x}} &&\text{use }  \diff \sqrt{x} = \frac{\diff x}{2\sqrt{x}} \\
&=& \displaystyle \int \sqrt{x} e^{-\sqrt{x}} \left(2 \sqrt{x} \diff \sqrt{x}\right) &&\text{Set } \sqrt{x}=u\\
&=& \displaystyle 2\int u^2 e^{-u}\diff u\\
&=& \displaystyle 2\left( -\int u^2 \diff \left( e^{-u} \right) \right) &&\text{integrate by parts} \\
&=& \displaystyle 2\left(- u^2e^{-u}+\int e^{-u}\diff \left(u^2\right) \right) \\
&=&\displaystyle 2\left(- u^2e^{-u}+\int 2 u e^{-u}\diff u \right)\\
&=&\displaystyle 2\left(- u^2e^{-u}-\int 2 u \diff e^{ -u} \right) &&\text{integrate by parts again}\\
&=&\displaystyle 2\left(- u^2e^{-u}- 2 u  e^{-u}+ \int 2e^{-u}\diff u \right) \\
&=&\displaystyle 2\left( - u^2e^{-u} -2ue^{-u} -2e^{ -u} \right)+C\\
&=&\displaystyle 2\left( - xe^{-\sqrt{x}} -2\sqrt{x } e^{ -\sqrt{x}} -2e^{-\sqrt{x}}\right)+C
\end{array}
\]
Therefore 
\[
\begin{array}{rcll|l}
\displaystyle \int \sqrt{x} e^{-\sqrt{x}} \diff x&=& \displaystyle \lim\limits_{t\to \infty} 2\left[ - xe^{- \sqrt{ x} } -2\sqrt{x}e^{-\sqrt{x}} -2e^{- \sqrt{x}} \right]_{ 0}^{\infty}\\
&=&\displaystyle 4+ \lim\limits_{t\to \infty} 4\left( -te^{ -\sqrt{t}} -\sqrt{t}e^{-\sqrt{t}}- e^{-\sqrt{t}} \right) && \text{Set }u=\sqrt{t}\\
&=&\displaystyle 4- 4\lim\limits_{u\to \infty} \left( u^2 e^{-u} + ue^{-u}+e^{-u}\right)\\
&=& \displaystyle 4- 4\lim\limits_{u\to \infty} \frac{ u^2 + u+1}{e^u} &&\text{use L'Hospital's rule for limit, see below}\\
&=& 4\quad ,
\end{array}
\]
and the integral converges to $4$. In the above computation we used the following limit computation
\[
\begin{array}{rcll|l}
\displaystyle \lim\limits_{u\to \infty}\frac{u^2+u+1}{e^u}&=&\displaystyle  \lim\limits_{u\to \infty} \frac{2u+1}{e^u}&&\text{Apply L'Hospital's rule}\\
&=&\displaystyle \lim\limits_{u\to \infty} \frac{2}{e^u}\\
&=&\displaystyle 0\quad .
\end{array}
\]

}