% begin module implicit-differentiation-ex4
\begin{frame}
\begin{example}
%\uncover<2->{Differentiate implicitly:}%
\abovedisplayskip=0pt
\belowdisplayskip=0pt
\abovedisplayshortskip=0pt
\belowdisplayshortskip=0pt
\begin{align*}
\text{Let ~~} \alertNoH{ 15}{x^4 + y^4} & \alertNoH{ 15}{ = 16}. \text{ Find }y''. \\
\uncover<2->{%
\alertNoH{3}{4x^3} + \alertNoH{3}{4y^3}y'%
}%
& \uncover<2->{ = } %
\uncover<2->{%
0%
}\\%
\uncover<3->{%
\alertNoH{ 11}{y'}%
}%
& \uncover<3->{ \alertNoH{ 11}{=} } %
\uncover<3->{%
\alertNoH{3,4, 11}{-\frac{x^3}{y^3}}.%
}\\%
\uncover<4->{%
y''%
}%
& \uncover<4->{ = } %
\uncover<4->{%
\frac{\diff}{\diff x}\left(\alertNoH{4}{ -\frac{\alertNoH{5}{x^3} }{\alertNoH{6}{y^3}} } \right)%
}  \uncover<5->{ = } %
\uncover<5->{%
- \frac{\alertNoH{6}{y^3} \alertNoH{ 7-8}{\frac{\diff}{\diff x}\left(\alertNoH{5}{x^3}\right)} - \alertNoH{5}{x^3} \alertNoH{ 9-10}{\frac{\diff}{\diff x}\left(\alertNoH{6}{y^3} \right)}}{\left( \alertNoH{6}{ y^3 }\right)^2}%
}\\%
& \uncover<7->{ = } %
\uncover<7->{%
- \frac{y^3 (\alertNoH{ 7-8}{\fcAnswer{8}{3x^2}}) - x^3( \alertNoH{ 9-10}{\fcAnswerUncover{7}{10}{3y^2\alertNoH{ 11}{y'}}})}{y^6}%
} \uncover<11->{ = }%
\uncover<11->{%
- \frac{3x^2y^3  - 3x^3y^2\alertNoH{ 11}{\left( -\frac{x^3}{y^3}\right)}}{y^6}%
}\\%
& \uncover<12->{ = } %
\uncover<12->{%
- \frac{3x^2(y^3+\frac{x^4}{y})}{y^6}%
} \uncover<13->{ = }%
\uncover<13->{%
- \frac{3x^2\left( \frac{y^4+x^4}{\alertNoH{ 14}{y}}\right)}{\alertNoH{ 14}{y^6}}%
}\\%
& \uncover<14->{ = } %
\uncover<14->{%
- \frac{3x^2(\alertNoH{ 15}{y^4+x^4})}{\alertNoH{ 14}{y^7}}%
}  \uncover<15->{ = }%
\uncover<15->{%
- \frac{3x^2(\alertNoH{ 15}{16})}{y^7}%
} \uncover<16->{ = }%
\uncover<16->{%
-48 \frac{x^2}{y^7}.%
}%
\end{align*}
\end{example}
\end{frame}
% end module implicit-differentiation-ex4
