% begin module implicit-differentiation-ex3
\begin{frame}
\begin{example}
\abovedisplayskip=0pt
\belowdisplayskip=-15pt
\abovedisplayshortskip=0pt
\belowdisplayshortskip=0pt
\begin{align*}
\text{Find $y'$ if }\sin (x+y) & = y^2\cos x.\\
\uncover<2->{%
\alertNoH{ 3-4}{\frac{\diff}{\diff x} (\sin (x+y))}%
}%
& \uncover<2->{ = } %
\uncover<2->{%
\alertNoH{ 5-6}{\frac{\diff}{\diff x} (y^2\cos x)}%
}\\%
\fcAnswerUncover{3}{4}{%
\alertNoH{ 3-4}{(\cos(x+y))\alertNoH{ 7-8}{\frac{\diff}{\diff x}(x+y)}}%
}%
& \uncover<3->{ = } %
\fcAnswerUncover{3}{6}{%
\alertNoH{ 5-6}{(y^2)\alertNoH{ 9-10}{\frac{\diff}{\diff x}(\cos x)} + (\cos x) \alertNoH{ 11-12}{\frac{\diff}{\diff x}(y^2)}}%
}\\%
\uncover<7->{%
(\cos(x+y))\alertNoH{ 7-8}{\left(\fcAnswerUncover{7}{8}{1+y'}\right)}%
}%
& \uncover<7->{ = } %
\uncover<7->{%
(y^2)\alertNoH{ 9-10}{(\fcAnswerUncover{7}{10}{-\sin x})} + (\cos x) \alertNoH{ 11-12}{(\fcAnswerUncover{7}{12}{2yy'})}%
}\\%
\uncover<13->{%
\alertNoH{15}{\cos(x+y)} +\alertNoH{14}{ y'\cos(x+y)}%
}%
& \uncover<13->{ = %
\alertNoH{15}{-y^2\sin x} +\alertNoH{14}{2yy'\cos x}%
}\\%
\uncover<14->{%
\alertNoH{14}{\alertNoH{ 16}{y'}\cos(x+y) - 2y\alertNoH{ 16}{y'}\cos x}%
}%
& \uncover<14->{ = %
\alertNoH{15}{-y^2\sin x -\cos(x+y)}%
}\\%
\uncover<16->{%
\text{Factor:}\quad%
\alertNoH{ 16}{y'}(\alertNoH{17}{\cos(x+y) - 2y\cos x})%
}%
& \uncover<16->{ = %
-y^2\sin x -\cos(x+y)%
}\\%
\uncover<17->{%
y'%
}%
& \uncover<17->{ = } %
\uncover<17->{%
\frac{-y^2\sin x - \cos(x+y)}{\alertNoH{17}{\cos (x+y) - 2y\cos x}}.%
}%
\end{align*}
\end{example}
\end{frame}
% end module implicit-differentiation-ex3
