% begin module implicit-differentiation-ex3
\begin{frame}
\begin{example}[Example 3, p. 213]
\abovedisplayskip=0pt
\belowdisplayskip=-15pt
\abovedisplayshortskip=0pt
\belowdisplayshortskip=0pt
\begin{align*}
\text{Find $y'$ if } \tan xy &= x^2-y^2.\\
\uncover<2->{\alert<handout:0|3-4>{\frac{\diff}{\diff x}(\tan xy)}&= \alert<handout:0|5-6>{ \frac{\diff}{\diff x}(x^2-y^2)}}\\
\uncover<3->{\alert<handout:0|4>{\uncover<4->{(\sec^2xy)\alert<handout:0|7-8>{\frac{\diff}{\diff x}(xy)}}} & = \uncover<6->{\alert<handout:0|6>{ 2x-2yy'}}}\\
\uncover<7->{\alert<handout:0|7-8>{\left(\uncover<8->{y\alert<handout:0|9-10>{\frac{\diff}{\diff x}(x)}+x\alert<handout:0|11-12>{\frac{\diff}{\diff x}(y)}}\right)}\sec^2 xy &= 2x -2yy'}\\
\uncover<9->{\left(y\alert<handout:0|9-10>{(\uncover<10->{1})}+x\alert<handout:0|11-12>{(\uncover<12->{y'})}\right)\sec^2 xy &= 2x -2yy'}\\
\uncover<13->{y\sec^2xy+xy' \sec^2xy &= 2x -2yy'}\\
\uncover<14->{xy' \sec^2xy+2yy'&=2x-y\sec^2xy}\\
\uncover<15->{y'(x\sec^2xy+2y) &= 2x-y\sec^2xy}\\
\uncover<16->{y'&=\frac{2x-y\sec^2xy}{x\sec^2xy+2y}.}
\end{align*}
\end{example}
\end{frame}
% end module implicit-differentiation-ex3
