% begin module natural-logarithm-def-ex5
\begin{frame}
\begin{example}
Solve the equation.
\[
\renewcommand{\arraystretch}{1.7}
\begin{array}{rcll|l}
\displaystyle 3^{2x+5}&=&\displaystyle 5\cdot 2^{-x+1} &&\text{Common base}\\
\displaystyle \left( 2^{\log_2 3}\right)^{2x+5}&=&\displaystyle 5\cdot 2^{-x+1} \\
\displaystyle 2^{\left(\log_2 3\right)(2x+5)}&=&\displaystyle 5\cdot 2^{-x+1}\\
\displaystyle \frac{2^{\left(\log_2 3\right)(2x+5)}}{2^{- x+1}}&=&\displaystyle 5\\
\displaystyle 2^{\left( \log_2 3\right)(2x+5)- (-x+1)}&=& \displaystyle 5 && \text{Apply }\log_2 \\
\displaystyle (\log_2 3)(2x+5)+x-1&=&\log_2 5\\
x(2\log_2 3+1)+ 5\log_2 3&=&\displaystyle \log_2 5+1\\
\displaystyle x&=&\displaystyle \frac{\log_2 5+1-5\log_2 3}{2 \log_2 3+1}\\

\end{array}
\]
\end{example}
\end{frame}
% end module natural-logarithm-def-ex5
