% begin module natural-logarithm-def-ex5
\begin{frame}
\begin{example}
Solve the equation.

\hfil\hfil$\renewcommand{\arraystretch}{1.6}
\begin{array}{rcll|l}
\displaystyle e^{x-3}&=&\displaystyle 2 \alertNoH{2}{ e^{2x-1}} \uncover<2->{&& \text{Divide by }\alertNoH{2}{ e^{2x-1}}}\\
\uncover<2->{\displaystyle \frac{{\alertNoH{3}{e}}^{x-3}}{\alertNoH{2}{{\alertNoH{3}{e}}^{\alertNoH{4}{2x-1}}}}&=&2}\\
\uncover<3->{\displaystyle {\alertNoH{3}{e}}^{ \alertNoH{5}{x}\alertNoH{6}{-3}\alertNoH{5,6}{-}(\alertNoH{4}{\alertNoH{5}{2x}\alertNoH{6}{-1}})} &=& 2}\\
\uncover<5->{\displaystyle {\alertNoH{7}{e}}^{ \alertNoH{5}{-x}\alertNoH{6}{-2}} &=& \alertNoH{8}{2} \uncover<7->{&&\text{Apply }\alertNoH{7,8}{\ln}}}\\
\uncover<7->{-x\alertNoH{9}{-2}&=&\alertNoH{8}{ \ln 2}}\\
\uncover<9->{\alertNoH{10}{-}x&=&\ln 2+\alertNoH{9}{2}}\\
\uncover<10->{x&=& \alertNoH{10}{-(}\ln 2+2\alertNoH{10}{)}}\\
\uncover<11->{x&=&-\ln 2-2 && \text{Final answer}}\\
\uncover<12->{x&\approx& -2.693&& \text{Calculator}}
\end{array}
$
\end{example}
\end{frame}
% end module natural-logarithm-def-ex5
