% begin module exponential-equation4
\begin{frame}
\begin{example}[Solving a quadratic exponential equation]
Solve for $x$.
\abovedisplayskip=0pt
\belowdisplayskip=0pt
\begin{align*}
4^{x+1} & = 2^{x+2} + 3 \\
\uncover<2-| handout:0>{\alertNoH{ 6}{4^{x+1}} - \alertNoH{ 4}{2^{x+2}} - 3} & \uncover<2->{ = 0} \\
\intertext{\uncover<3->{Substitute $\alertNoH{ 10}{u = \uncover<3-| handout:0>{2^x}}$.  Then $\alertNoH{ 3-4}{2^{x+2} = \uncover<4-| handout:0>{4u}}$ and $\alertNoH{ 5-6}{4^{x+1} = \uncover<6-| handout:0>{4u^2.}}$ }}
\uncover<3-| handout:0>{\alertNoH{ 6}{\uncover<6->{4u^2}} - \alertNoH{ 4}{\uncover<4->{4u}} - 3} & \uncover<3->{ = 0} \\
\uncover<7->{\alertNoH{ 7-8}{(\uncover<8-| handout:0>{2u-3})(\uncover<8-| handout:0>{2u+1})}} & \uncover<7->{ = 0 }
\end{align*}
\begin{align*}
\uncover<9->{ \alertNoH{ 10}{u} } & \uncover<9->{=} \uncover<9-| handout:0>{ \frac{3}{2} } & \uncover<9->{\text{or}} & & \uncover<9->{\alertNoH{ 10}{u}} & \uncover<9->{=} \uncover<9-| handout:0>{ -\frac{1}{2}} \\
\uncover<10-| handout:0>{ \alertNoH{ 10}{2^x} } & \uncover<10-| handout:0>{ = \frac{3}{2} } & \uncover<10-| handout:0>{\text{or}} & & \uncover<10-| handout:0>{\alertNoH{ 10}{2^x}} & \uncover<10-| handout:0>{ = -\frac{1}{2}} \invisible{99999999} \\
\uncover<11-| handout:0>{ \alertNoH{ 11-12}{x} } & \uncover<11-| handout:0>{ \alertNoH{ 11-12}{ = \uncover<12->{\log_2 \Big( \frac{3}{2}\Big)} }} & & & \uncover<11-| handout:0>{\alertNoH{ 13-14}{\uncover<-13>{x}}} & \uncover<11-| handout:0>{ \alertNoH{ 13-14}{ \only<-13>{ =} \only<14->{\text{no solution}} }} \\
\uncover<15-| handout:0>{x & = \frac{\ln (3/2)}{\ln2} & & & & }
\end{align*}
\uncover<16-| handout:0>{Therefore the solution is $x = \frac{\ln (3/2)}{\ln 2} \approx  0.584962501$.}
\end{example}
\end{frame}
% end module exponential-equation4
