% begin module general-exponential-derivative
\begin{frame}
\begin{theorem}[The Derivative of $a^x$]
\[
\frac{\diff}{\diff x} (a^x) = a^x \ln a .
\]
\end{theorem}
\begin{proof}
\uncover<2->{
Use the fact that $\alert<handout:0| 4,8>{a = e^{\ln a}}$.
}
\abovedisplayskip=0pt
\belowdisplayskip=0pt
\abovedisplayshortskip=0pt
\belowdisplayshortskip=0pt
\begin{align*}
\uncover<3->{\frac{\diff}{\diff x} (\alert<handout:0| 4>{a^x})}%
& \uncover<3->{ = }  %
\uncover<4->{\frac{\diff}{\diff x} (\alert<handout:0| 4>{e^{\ln a}})^x}\\%
& \uncover<5->{ = }  %
\uncover<5->{\frac{\diff}{\diff x} e^{(\ln a)x}}\\%
& \uncover<6->{ = }  %
\uncover<6->{ e^{(\ln a)x}\frac{\diff}{\diff x}(\ln a)x }\\%
& \uncover<7->{ = }  %
\uncover<7->{ (\alert<handout:0| 8>{e^{\ln a}})^x(\ln a) }\\%
& \uncover<8->{ = }  %
\uncover<8->{ \alert<handout:0| 8>{a}^x(\ln a).}%
\end{align*}
\end{proof}
\end{frame}
% end module general-exponential-derivative
