\begin{frame}
\begin{example}
Prove that $-\ln \left(x-\sqrt{1+x^2}\right)=\ln \left( x+\sqrt{1+x^2}\right)$.

\uncover<2->{
$\begin{array}{@{}r@{}c@{}l@{}l@{}|l}
-\ln \left(x-\sqrt{1+x^2}\right)&=&\displaystyle \ln \left(\frac{1}{ \sqrt{x^2+1} - x} \right) && \text{rationalize}\\
&=&\displaystyle \ln \left(\frac{ \left( \sqrt{x^2+1}+ x\right) }{\left( \sqrt{x^2+1} - x\right) \left(\sqrt{x^2+1 }+x\right) } \right)\\
&=& \displaystyle \ln \left(\frac{\sqrt{x^2+1}+x}{x^2 +1 -x^2 }\right)\\
&=& \displaystyle \ln \left(\sqrt{x^2+1}+x\right)\quad .\\
\end{array}
$
}
\end{example}
\end{frame}