% begin module logarithm-change-base
\begin{frame}
\frametitle{General Logarithmic and Exponential Functions}
\begin{theorem}[Change of Base Formula]
For any positive number $a \neq 1$, we have
\[
\log_a x = \frac{\ln x}{\ln a} .
\]
\end{theorem}
\begin{proof}
\begin{itemize}
\item<2->  Let $\alert<handout:0| 9-10>{y = \log_a x}$.
\item<3->  Then $a^y = x$.
\item<4->  Take the natural logarithm of both sides:
\item<5->  $\only<7->{\alert<handout:0| 7>{y \ln a}}\only<handout:0| -6>{\alert<handout:0| 6>{\ln a^y}} = \ln x$.
\item<8->  $\only<-9>{\alert<handout:0| 9>{y}}\only<handout:0| 10->{\alert<handout:0| 10>{\log_a x}}=\frac{\ln x}{\ln a} $.
\end{itemize}
\end{proof}
\end{frame}
% end module logarithm-change-base
