% begin module natural-log-derivative-ex-simplify.tex
\begin{frame}
\begin{example}[Chain Rule, Natural Logarithm]
\abovedisplayskip=0pt
\belowdisplayskip=0pt
\abovedisplayshortskip=0pt
\belowdisplayshortskip=0pt
\begin{align*}
\text{Differentiate}\quad y &= \ln (e^x \sec x).\\
\uncover<2->{ y&= \alert<handout:0|3-4>{\ln e^x} + \ln \sec x}\\
\uncover<3->{ &=\uncover<4->{\alert<handout:0|4>{\alert<handout:0|5-6>{ x}}} + \ln \sec x.}\\
\uncover<5->{\frac{\diff y}{\diff x} & =\uncover<6-| handout:0>{\alert<handout:0|6>{1} }+ \uncover<7->{ \alert<handout:0|7>{\alert<handout:0|11>{\frac{\diff}{\diff x} (\ln \sec x)}}}}\\
\uncover<8->{\alert<handout:0|8-9>{\text{Let} \ \ \alert<handout:0|14-16>{u} }&  \alert<handout:0|8-9>{\alert<handout:0|14-16>{= \uncover<9-| handout:0>{ \sec x.}}}}\\
\uncover<10->{\text{Then} \ \ \ln \sec x & = \uncover<10-| handout:0>{ \ln u.}}\\
\uncover<11->{\text{Chain Rule:} \quad \frac{\diff y}{\diff x} & = 1+  \alert<handout:0|11>{\alert<handout:0|12-13>{\frac{\diff}{\diff u}(\uncover<11-| handout:0>{\ln u})} \alert<handout:0|14-15>{\frac{\diff u}{\diff x}}}}\\
\uncover<12->{& = 1+ \alert<handout:0|12-13>{\left( \uncover<13-| handout:0>{\frac{1}{\alert<handout:0|16>{u}}} \right)} \alert<handout:0|14-15>{(\uncover<15-| handout:0>{\sec x \tan x} )} }\\
\uncover<16->{& =} \uncover<16-| handout:0>{ 1+ \frac{1}{\alert<handout:0|16>{\sec x}}\sec x \tan x} \\
\uncover<17->{& =} \uncover<17-| handout:0>{ 1+ \tan x.}
\end{align*}
\end{example}
\end{frame}
% begin module natural-log-derivative-ex-simplify.tex
