% begin module power-rule-rationa-from-chain-rule
\begin{frame}
\alert<1>{You will not be tested on the material in the next slide.}
\end{frame}
\begin{frame}

\begin{example}
Derive \alert<11>{the exponent rule $\left(e^x\right)'=e^x$} \uncover<2->{using the Calc II formula below,} \uncover<3->{ \alert<3>{the infinite} {\color{gray!50} (both sides uniformly convergent)} \alert<3>{sum rule $(f_1+f_2 +f_3 +\dots)' =f_1' +f_2'  +f_3' +\dots$}}
\uncover<4->{and \alert<4>{the power rule $(x^n)'=nx^{n-1}$}. } 
\uncover<2->{\[
\alert<2,10>{e^x}=\alert<2,10>{1+x+\frac{x^2}{2!}+\frac{x^3}{3!}+\dots},
\]
}
\uncover<2->{where $n!=1\cdot2\cdot3\cdot \dots\cdot n$.} \uncover<5->{We have that $\alert<5,9>{\frac{n}{\alert<6>{ n!}}} =\uncover<6->{ \frac{\alert<7>{n} }{ \alert<6>{ 1\cdot 2\cdot \dots\cdot (n-1) \cdot  \alert<7>{n}}}=}\uncover<7->{\frac{1}{\alert<8>{1\cdot 2\cdot \dots\cdot (n-1)}}=}\uncover<8->{\alert<9>{ \frac{1}{ \alert<8>{(n-1)!} }}} $.}
\[
\begin{array}{rcl}
\uncover<2->{\alert<11>{\left(\alert<2>{e^x}\right)'} &=&\alert<3>{\left(\alert<2>{1+x+\frac{x^2}{2!}+\frac{x^3}{3!}+\dots} \right)' }} \\
\uncover<3->{&=& \alert<3>{ \alert<4>{(1)'}+\alert<4>{(x)'}+\frac{\alert<4>{(x^2)'}}{2!} +\frac{\alert<4>{(x^3)'}}{3!}+\dots + \frac{\alert<4>{(x^n)'}}{n!}+\dots}}
\\ \uncover<4->{&=&\alert<4>{0}+ \alert<4>{1}+ \frac{\alert<4>{\alert<5-9>{2}x}}{\alert<5-9>{2!}}+ \frac{\alert<4>{\alert<5-9>{3}x^3}}{\alert<5-9>{3!}}+ \dots +\frac{\alert<4>{\alert<5-9>{n}x^{n-1}}}{\alert<5-9>{n!}}+\dots }\\
\uncover<9->{&=& \alert<10>{ \phantom{ 0~ + }  \alert<9>{1}+ \frac{\phantom{2}x}{\alert<9>{1!}}+\frac{\phantom{3}x^{2}}{\alert<9>{2!}}+\dots+\frac{\phantom{n}x^{n-1}}{\alert<9>{(n-1)!}}+\dots}=}\uncover<10->{\alert<10,11>{e^x}}\\
\end{array}
\]
\uncover<11->{\alert<11>{as desired.}}
\end{example}

\end{frame}

%end module power-rule-rationa-from-chain-rule