% begin module logarithm-rule-from-exponent
\begin{frame}
\begin{example}
Derive the logarithm derivative rules
\[
\begin{array}{rcl}
\alertNoH{11,15}{(\ln x)'}&=&\alertNoH{11,15}{\frac{1}{x}}\\
\alertNoH{16}{(\log_a x)'}&=&\alertNoH{16}{\frac{1}{x\ln a}}
\end{array}
\]
\uncover<5->{using \alertNoH{5}{the chain rule},} \uncover<6->{the \alertNoH{6}{exponent derivative rule $(e^{x})'=e^x$}, } \uncover<7->{\alertNoH{7}{the rule $(x)'=1$}} \uncover<14->{and the \alertNoH{14}{constant multiple rule $(cf)'=cf'$}.}
\[
\begin{array}{rclp{0.3cm}|l}
\uncover<2->{
e^{\alertNoH{3}{\ln x}}&=&x \uncover<3->{&&  \alertNoH{3,8}{ \text{set~~~}u =\ln x }}}\\
\uncover<3->{e^{\alertNoH{3}{u}}&=&x \uncover<4->{& & \alertNoH{4}{ \frac{\diff}{\diff x}}}}\\
\uncover<5->{ \alertNoH{5}{\alertNoH{6}{\frac{\diff}{\diff u}(e^u)} u'}&=&\alertNoH{7}{(x)'}}\\
\uncover<6->{ \alertNoH{6}{e^{\alertNoH{8}{u}}} \alertNoH{8}{u}'&=&\alertNoH{7}{1}}\\
\uncover<8->{\alertNoH{9}{e^{\alertNoH{8}{\ln x}}} (\alertNoH{8}{\ln x})'&=&1}\\
\uncover<9->{\alertNoH{9}{x}(\ln x)'&=&1\uncover<10->{& &\alertNoH{10}{ \cdot \frac{1}{x}}}}\\
\uncover<10->{ \alertNoH{11}{(\ln x)'} &=& \displaystyle\alertNoH{11}{\frac{1}x} \uncover<11->{ & &\alertNoH{11}{ \text{as~desired}}}} 
\uncover<12->{\\ \hline
\alertNoH{16}{(\alertNoH{13}{\log_a x})'} & =&  \uncover<13->{ \alertNoH{14}{\left(\alertNoH{13}{\frac{\ln x}{\ln a}} \right)' }=} \uncover<14->{\alertNoH{14}{ \frac{ \alertNoH{15}{ (\ln x)'}}{\ln a}} =} \uncover<14->{\alertNoH{16}{ \frac{ \alertNoH{15}{1} }{\alertNoH{15}{x}\ln a}}}\uncover<16>{ & &  \alertNoH{16}{ \text{as~desired~}}}}
\end{array}
\]
\end{example}
\end{frame}

%end module module logarithm-rule-from-exponent
