% begin module derivatives-rules-relations

\begin{frame}
\begin{example}
Let $n$ be a positive integer. Derive the negative integer power rule
\[
(x^{-n})'=\left(\frac{1}{x^n}\right)'= -n x^{-n-1} =-\frac{n}{x^{n+1}}
\]
\uncover<4->{using \alertNoH{4}{the product rule},} \uncover<5->{\alertNoH{5}{the constant derivative rule}} \uncover<6->{and \alertNoH{6}{the power rule for positive integers}.}

\[
\begin{array}{rcl p{2cm} |r}
\uncover<2->{ x^n x^{-n} &=& 1}  \uncover<3->{&& \frac{\diff}{\diff x}}\\
\uncover<3->{\alertNoH{4}{( x^n x^{-n})'} &=&\alertNoH{5}{(1)'}  }\\

\uncover<4->{ \alertNoH{4}{ \alertNoH{6}{(x^n)'} x^{-n} + x^n (x^{-n})'}&=&\alertNoH{5}{0}}\\
\uncover<6->{ \alertNoH{7}{\alertNoH{6}{n x^{n-1}}x^{-n}}+ x^n (x^{-n})'&=&0 }\\
\uncover<7->{\alertNoH{7}{\frac{n}{x}}+ x^n (x^{-n})'&=&0 }\\
\uncover<8->{x^n (x^{-n})'&=&-\frac{n}x && \frac{1}{x^n}}\\
\uncover<9->{(x^{-n})'&=&-\frac{n}{x^{n+1}}}
\end{array}
\]

\end{example}



\end{frame}




%end module derivatives-rules-relations
