% begin module power-rule-from-exponent
\begin{frame}
\begin{example}
Derive the power rule
\[
\alertNoH{14}{\left(x^{r}\right)'=rx^{r-1}}, \quad \quad \quad \alertNoH{3}{x>0}
\]
\uncover<6->{using \alertNoH{6}{the chain rule},} \uncover<7->{the \alertNoH{7}{the rule $\left(e^{x}\right)'=e^x$},} \uncover<10->{\alertNoH{10}{the constant multiple derivative rule}} \uncover<12->{and \alertNoH{12}{the logarithm derivative rule $(\ln x)'=\frac{1}x$}.}

\[
\begin{array}{rclp{0.5cm}|l}
\uncover<2->{ \displaystyle \alertNoH{14}{ \left(\alertNoH{3} { x }^r \right)'} &= & \displaystyle \uncover<3->{ \left( \alertNoH{4}{ (\alertNoH{3}{ e^{\ln x}})^r}\right)' =}\uncover<4->{\left( \alertNoH{4}{ e^{\alertNoH{5}{r \ln x} }} \right)'}\uncover<5->{& &  \alertNoH{5,8}{ \text{Set~}u=r\ln x}}}\\ \\
\uncover<5->{&=& \displaystyle \alertNoH{6}{ (e^{\alertNoH{5}{u}})'} =\uncover<6->{ \alertNoH{6}{\alertNoH{7}{ \frac{\diff}{\diff u} \left( e^{u} \right)} u'}=} \uncover<7->{\alertNoH{7}{e^{\alertNoH{8}{u}}} \alertNoH{8}{u}' =}}\\ \\
\uncover<8->{&=&\displaystyle \alertNoH{9}{e^{\alertNoH{8}{r\ln x}}} \alertNoH{10}{(\alertNoH{8}{r\ln x})'} =} \uncover<9->{\alertNoH{9}{\left(\alertNoH{11}{e^{\ln x}}\right)^r}  \alertNoH{10}{r\alertNoH{12}{(\ln x)'}} } \\ \\\uncover<11->{&=&  \alertNoH{13}{\alertNoH{11}{x}^r } r \alertNoH{12}{ \alertNoH{13}{ \frac{1}x} } = \uncover<13->{\alertNoH{14}{r\alertNoH{13}{ x^{r-1}}}} \uncover<14->{ & & \alertNoH{14}{\text{as~desired}}}}
\end{array}
\]
\end{example}
\end{frame}

%end module power-rule-from-exponent
