% begin module power-rule-rationa-from-chain-rule
\begin{frame}
\begin{example}
Derive the power rule $\alert<13>{\left(x^{\frac{1}{q}}\right)'=\frac{1}{q} x^{\frac{1}q-1}}$ using \alert<6>{the chain rule}, \alert<4>{the rule $(x)'=1$} and the \alert<7>{integer power rule $\frac{d}{du}(u^q)=qu^{q-1} $}.

\[
\begin{array}{rclp{0.3cm}|l}
\uncover<2->{ \left(x^{\frac{1}{q}}\right)^q &=&x&& \uncover<3->{\alert<3>{\frac{d}{dx}}}}\\
\uncover<3->{ \alert<3>{\left(\left(\alert<5>{x^{\frac{1}q}} \right)^q\right)'} &=& \uncover<4->{\alert<4>{1}} \uncover<3>{\alert<3>{(x)'}} &&\uncover<5->{\alert<5,8>{\text{Set~}u=x^{\frac1q} }}}\\
\uncover<5->{ \alert<6>{\left(\alert<5>{u}^{q}\right)'}&=&1  }  \\
\uncover<6->{\alert<6>{ \alert<7>{\frac{d}{du} \left(u^q\right)} u'}&=&1}\\
\uncover<7->{\alert<7>{q (\alert<8>{u})^{q-1}} (\alert<8>{u})'&=&1 }\\
\uncover<8->{ q (\alert<8>{x^{\alert<9>{\frac{1}q}}})^{\alert<9>{q-1}} \left( \alert<8>{x^{\frac1q}}\right)'&=&1 }\\
\uncover<9->{\alert<10>{q x^{\alert<9>{\frac{q-1}q}}}\left( x^{\frac1q}\right)'&=&1}&&\uncover<10->{\alert<10>{\text{divide~by~}q x^{\frac{q-1}q}}}\\
\uncover<10->{\alert<13>{\left( x^{\frac1q}\right)'}&=&\frac{ 1}{\alert<10>{q \alert<11>{x^{\frac{q-1}q}}}}=} \uncover<11->{ \frac{\alert<11>{x^{\alert<12>{-\frac{q-1}{q}}}}}{q}=}\uncover<12->{\alert<13>{\frac{1}q x^{\alert<12>{\frac{1}q-1}}}} &&\uncover<13->{\alert<13>{\text{as~desired}}}
\end{array}
\]
\end{example}

\end{frame}

%end module power-rule-rationa-from-chain-rule