% begin module derivatives-rules-relations

\begin{frame}
\begin{example}
Let $n$-positive integer. Derive the positive integer power rules $\left( x^2\right)' =2x$, $\left( x^3\right)' =3x^2$, $\left( x^4\right)' =4x^3$, \dots from the product rule, the sum rule, and \alert<2>{the rule $(x)'=1$}.

\[
\begin{array}{rcl}
\uncover<2->{(x)'&=&1}\\
\uncover<3->{\alert<5>{(x^2)'}&=& (x*x)'=x'x +x x'= x+x=\alert<5>{2x} } \\
\uncover<4->{\alert<8>{(x^{3})'}&=& (x* x^2)'= x' x^2+x\alert<5>{(x^2)'}= \uncover<5->{x^2+ x (\alert<5>{2x})=}\uncover<6->{x^2+2x^2=\alert<8>{3x^2}}}\\
\uncover<7->{(x^{4})'&=& (x* x^3)'= x' x^3+x\alert<8>{(x^3)'}= \uncover<8->{x^3+ x (\alert<8>{3x^2})=}\uncover<9->{x^3+3x^3=4x^3}}\\
\uncover<10->{&\vdots&}\\ 
\uncover<10->{\alert<12>{(x^{n})'}&=&\dots = \alert<12>{n x^{n-1}}}\\
\uncover<11->{(x^{n+1})'&=& (x*x^n)'=x' x^n+ x\alert<12>{(x^{n})'}=}\uncover<12->{x^n+x (\alert<12>{nx^{n-1}})=}\uncover<13->{(n+1)x^n}\\
\uncover<13->{&\vdots&} 
\end{array}
\]
\end{example}


\end{frame}




%end module derivatives-rules-relations