% begin module quotient-rule-from-power-and-chain
\begin{frame}
\begin{example}
Derive the quotient rules
\[
\begin{array}{rcl}
\alertNoH{5,9}{\displaystyle\left(\frac{1}{g}\right)'}&=&\displaystyle\alertNoH{5,9}{-\frac{g'}{g^2}}
\\
\displaystyle\alertNoH{11}{\left(\frac{f}{g}\right)'}&=&\displaystyle\alertNoH{11}{\frac{f'g-fg'}{g^2}}
\end{array}
\]
\uncover<3->{using \alertNoH{3}{the chain rule},} \uncover<4->{\alertNoH{4}{the negative power rule}} \uncover<8->{and \alertNoH{8}{the product rule}.}
\[
\begin{array}{rclp{0.3cm}|l}
\displaystyle \uncover<2->{ \alertNoH{3,5}{\left(\frac{1}{g}\right)'} &=& \displaystyle \uncover<3->{\alertNoH{3}{\alertNoH{4}{\frac{\diff}{\diff g} \left( \frac1g\right)} g'} =} \uncover<4->{ \alertNoH{5 }{\alertNoH{4 }{ - \frac{1}{ g^2 }}g' }} \uncover<5->{& &\alertNoH{5 }{\text{as~desired}}}}\\
\\
\displaystyle
\uncover<6->{\alertNoH{7,11}{\left(\frac{f}{g}\right)'}\uncover<7->{&=&\displaystyle\alertNoH{7,8}{\left( f \frac{1}g\right)'} =} \uncover<8->{ \alertNoH{8}{ f' \frac{1 }{g} +f\alertNoH{9}{\left( \frac{1}{g} \right)' }} = }\uncover<9->{ \alertNoH{10}{ \frac{f'}{g} +f \alertNoH{9 }{ \left(- \frac{g' }{g^2}\right)}}}}\\
\\
\uncover<10->{&=&\displaystyle \alertNoH{10,11}{\frac{f'g-fg'}{g^2}} \uncover<11->{& & \alertNoH{11 }{\text{as~desired}}}}
\end{array}
\]
\end{example}
\end{frame}
%end module quotient-rule-from-power-and-chain
