% begin module derivatives-rules-relations

\begin{frame}
\begin{example}
Let $n$ be a positive integer. Derive the negative integer power rule 
\[
(x^{-n})'=\left(\frac{1}{x^n}\right)'= -n x^{-n-1} =-\frac{n}{x^{n+1}}
\]
using \alert<5>{the constant derivative rule}, \alert<4>{the product rule} and \alert<6>{the power rule for positive integers}.

\[
\begin{array}{rcl p{2cm} |r}
\uncover<2->{\alert<4>{\uncover<3->{(} x^n x^{-n}\uncover<3->{)'}} &=&\alert<5>{\uncover<3->{(} 1\uncover<3->{)'}}  && \uncover<2>{\frac{d}{dx}}}\\
\uncover<4->{ \alert<4>{ \alert<6>{(x^n)'} x^{-n} + x^n (x^{-n})'}&=&\alert<5>{0}}\\
\uncover<6->{ \alert<7>{\alert<6>{n x^{n-1}}x^{-n}}+ x^n (x^{-n})'&=&0 }\\
\uncover<7->{\alert<7>{\frac{n}{x}}+ x^n (x^{-n})'&=&0 }\\
\uncover<8->{x^n (x^{-n})'&=&-\frac{n}x && :x^n}\\
\uncover<9->{(x^{-n})'&=&-\frac{n}{x^{n+1}}}
\end{array}
\]

\end{example}



\end{frame}




%end module derivatives-rules-relations