\solution{\ref{problemlimxto3+sqrt(x^2/9-1)/(2x^2-3x-9)}.
We have that 
\[
\begin{array}{rcl}
\displaystyle \lim\limits_{x\to 3^+}\frac{\sqrt{\frac{x^2}9-1} }{2x^2-3x-9}&=&\displaystyle  \lim\limits_{x\to 3^+} \frac{\sqrt{(\frac{x}3-1)(\frac{x}3+1)} }{2(x+\frac{3}2)(x-3)}= \lim\limits_{x\to 3^+}
\frac{\left(\frac{1}3 (x-3)(\frac{x}3+1) \right)^{ \frac{1}2}}{ 2(x+\frac{3}2)(x-3)} \\~\\
&=&\displaystyle  \lim\limits_{x\to 3^+} \frac{\sqrt{\frac{1}3\left(\frac{x}3+1\right)} }{2\left(x+\frac{3}2\right)(x-3)^{\frac12}}= \lim\limits_{x\to 3^+} \frac{\sqrt{\underbrace{ \frac{1}3\left(\frac{x}3+1\right)}_{\to\frac23 }} }{\underbrace{2\left(x+\frac{3}2\right)}_{\to 9}\underbrace{(x-3)^{\frac12}}_{\to 0^+}}=\infty,
\end{array}
\]
where the latest term is $+\infty$ because it is of the form $\frac{(+)}{(+)(+)}$.
}