Evaluate the limit if it exists.
\begin{enumerate}
\item $\lim\limits_{x\to 3^+} \frac{\sqrt{\frac{x^2}{9}-1 }}{2x^2 -3x-9 }$. \answer{$ \infty$.}
\solution{ %   
We have that 
\[
\begin{array}{rcl}
\lim_{x\to 3^+}\frac{\sqrt{\frac{x^2}9-1} }{2x^2-3x-9}&=& \lim_{x\to 3^+} \frac{\sqrt{(\frac{x}3-1)(\frac{x}3+1)} }{2(x+\frac{3}2)(x-3)}= \lim_{x\to 3^+}
\frac{\left(\frac{1}3(x-3)(\frac{x}3+1)\right)^{\frac{1}2}}{2(x+\frac{3}2)(x-3)} \\~\\
&=& \lim_{x\to 3^+} \frac{\sqrt{\frac{1}3\left(\frac{x}3+1\right)} }{2\left(x+\frac{3}2\right)(x-3)^{\frac12}}= \lim_{x\to 3^+} \frac{\sqrt{\underbrace{ \frac{1}3\left(\frac{x}3+1\right)}_{\to\frac23 }} }{\underbrace{2\left(x+\frac{3}2\right)}_{\to 9}\underbrace{(x-3)^{\frac12}}_{\to 0^+}}=\infty,
\end{array}
\]
where the latest term is $+\infty$ because it is of the form $\frac{(+)}{(+)(+)}$.
}
\item $\lim\limits_{x\to -2^-} \frac{\sqrt{\frac{x^2}{4}-1 }}{2x^2 +3x-2 }$. \answer{$ \infty$.}
\end{enumerate}
