% begin module maclaurin-cos
\begin{frame}
\begin{example} %[Example 5, p. 776]
Find the Maclaurin series for $\cos x$.
\abovedisplayskip=0pt
\belowdisplayskip=2pt
\begin{eqnarray*}
\uncover<2->{%
\cos x%
}%
 \uncover<2->{=} %
\uncover<2->{%
\alert<handout:0| 2-3>{%
\frac{\diff}{\diff x}\left( \uncover<3->{\alert<handout:0| 4-5>{\sin x}}\right)%
}%
}%
& \uncover<4->{=} &%
\uncover<4->{%
\alert<handout:0| 6>{\frac{\diff}{\diff x}}\left( \alert<handout:0| 5>{\uncover<5->{\sum_{n=0}^\infty (-1)^n\frac{x^{2n+1}}{(2n+1)!}}}\right)%
}\\%
& \uncover<6->{=} &%
\uncover<6->{%
\sum_{n=0}^\infty\alert<handout:0| 6>{\frac{\diff}{\diff x}}\left( (-1)^n\frac{x^{2n+1}}{(2n+1)!}\right)%
}\\%
& \uncover<7->{=} &%
\uncover<7->{%
\sum_{n=0}^\infty (-1)^n\frac{(\alert<handout:0| 7-9>{2n+1})x^{\alert<handout:0| 7>{2n}}}{\alert<handout:0| 8-9>{(2n+1)!}}%
}\\%
& \uncover<8->{=} &%
\uncover<8->{%
\sum_{n=0}^\infty (-1)^n\frac{x^{2n}}{\alert<handout:0| 9>{\uncover<9->{(2n)!}}}%
}\\%
& \uncover<10->{=} &%
\uncover<10->{%
1 - \frac{x^2}{2!} + \frac{x^4}{4!} - \frac{x^6}{6!} + \cdots%
}%
\end{eqnarray*}

\end{example}
\end{frame}
% end module maclaurin-cos
