\solution{
\ref{problemTypeOfSurfacez^2+2y^2-3x^2+x+y+1=0}
We have that
\[
\begin{array}{rcl}
\displaystyle z^2+2y^2-3x^2 + x+y+1&=&0\\
\displaystyle z^2+ 2\left(y+\frac{1}{4}\right)^2 - 3\left(x-\frac{1}{6} \right)^2 -\frac{1}{8}+\frac{1}{12}+1&=&0\\
\displaystyle z^2+ 2\left(y+\frac{1}{4}\right)^2 &=&\displaystyle 3\left(x-\frac{1}{6} \right)^2-\frac{23}{24}
\end{array}
\]
This figure is given by sum of two squares equal to a square minus a positive number. That makes is a hyperboloid one sheet, as explained in the theoretical discussions.
}