% begin module derivative-tangent
\begin{frame}[t]
\begin{theorem}[The Derivative of Tangent]
\[
\frac{\diff}{\diff x}(\tan x) = \sec^2 x.
\]
\end{theorem}
\begin{proof}
\abovedisplayskip=0pt
\belowdisplayskip=-15pt
\abovedisplayshortskip=0pt
\belowdisplayshortskip=0pt
\begin{align*}
\uncover<2->{%
\text{Let}\quad y = \alert<handout:0| 2-3>{\tan x} %
}%
& \uncover<2->{\alert<handout:0| 2-3>{ = \uncover<3->{\frac{\sin x}{\cos x}.}}%
}\\%
\uncover<4->{%
\text{Quotient Rule:}%
}%
&\\%
\uncover<4->{%
\frac{\diff y}{\diff x}%
}%
& \uncover<4->{%
 = \frac%
{\left( \cos x \right) \alert<handout:0| 5-6>{\frac{\diff}{\diff x}\left( \sin x \right)} - \left( \sin x \right) \alert<handout:0| 7-8>{\frac{\diff}{\diff x}\left( \cos x \right)}}%
{\left( \cos x\right)^2}%
}\\%
& \uncover<5->{%
 = \frac%
{\left( \cos x \right) \alert<handout:0| 5-6>{\left(\uncover<6->{ \cos x }\right)} - \left( \sin x \right) \alert<handout:0| 7-8>{\left( \uncover<8->{-\sin x} \right)}}%
{ \cos^2x}%
}\\%
& \uncover<9->{%
 = \frac{\alert<handout:0| 10-11>{\cos^2 x + \sin^2 x}}{\cos^2 x}%
}%
 \uncover<10->{%
 = \frac{\alert<handout:0| 10-11>{\uncover<11->{1}}}{\cos^2 x}%
}\\%
& \uncover<12->{%
 = \sec^2 x.%
}%
\end{align*}
\end{proof}
\end{frame}
% end module derivative-tangent
