% begin module derivative-sine
\begin{frame}
\begin{align*}
\text{Let}\quad f(x) & = \sin x. \\
\text{Then}\quad f'(x) & =  %
\uncover<2->{%
\lim_{h\rightarrow 0}\frac{f(x+h)-f(x)}{h}%
}%
\uncover<3->{%
 = \lim_{h\rightarrow 0}\frac{\alert<handout:0| 4>{\sin (x+h)}-\sin x}{h}%
}\\%
& \uncover<4->{ = }  %
\uncover<4->{%
\lim_{h\rightarrow 0}\frac{\alert<handout:0| 4>{\sin x \cos h + \cos x \sin h} - \sin x}{h}%
}\\%
& \uncover<5->{ = }  %
\uncover<5->{%
\lim_{h\rightarrow 0}\left[ \frac{\sin x \cos h - \sin x}{h} + \frac{\cos x \sin h}{h}\right] %
}\\%
& \uncover<6->{ = }  %
\uncover<6->{%
\lim_{h\rightarrow 0}\left[ \sin x\left( \frac{\cos h - 1}{h}\right) + \cos x\left( \frac{\sin h}{h}\right) \right] %
}\\%
& \uncover<7->{ = }  %
\uncover<7->{%
\alert<handout:0| 8-9>{\lim_{h\rightarrow 0} \sin x}\cdot \alert<handout:0| 12>{\lim_{h\rightarrow 0} \frac{\cos h - 1}{h}} + \alert<handout:0| 10-11>{\lim_{h\rightarrow 0}\cos x}\cdot \alert<handout:0| 12>{\lim_{h\rightarrow 0}  \frac{\sin h}{h}}  %
}\\%
& \uncover<8->{ = }  %
\uncover<8->{%
\alert<handout:0| 8-9>{\uncover<9->{\sin x}}\cdot \alert<handout:0| 12>{\lim_{h\rightarrow 0} \frac{\cos h - 1}{h}} + \alert<handout:0| 10-11>{\uncover<11->{\cos x}}\cdot \alert<handout:0| 12>{\lim_{h\rightarrow 0}  \frac{\sin h}{h}}  %
}%
\end{align*}
\uncover<12->{%
We need to do more work to find the other two limits.

\uncover<13->{
From Example 3, p. 98, we think $ \lim_{h\rightarrow 0}\frac{\sin h}{h}$  is  1.}
}%
\end{frame}


\begin{frame}
\begin{columns}[c]
\column{.6\textwidth}
\[
\text{Claim:}\quad \lim_{\theta \rightarrow 0}\frac{\sin \theta }{\theta} = 1
\]
First suppose $0 < \theta < \frac{\pi}{2}$.  Then we can write $\sin \theta$ using ratios of side lengths of a triangle.
\column{.4\textwidth}
\ \only<handout:0| -3>{%
\includegraphics[width=4.5cm]{derivatives-trig/pictures/03-04-proofa.pdf}%
}%
\only<handout:0| 4-9>{%
\includegraphics[width=4.5cm]{derivatives-trig/pictures/03-04-proofb.pdf}%
}%
\only<handout:0| 10>{%
\includegraphics[width=4.5cm]{derivatives-trig/pictures/03-04-proofc.pdf}%
}%
\only<11->{%
\includegraphics[width=4.5cm]{derivatives-trig/pictures/03-04-proofd.pdf}%
}%
\end{columns}
\[
\uncover<2->{%
\alert<handout:0| 2-3>{%
\sin \theta = \uncover<3->{|BC|} %
}%
}%
\uncover<4->{%
 < |AB|%
}%
\uncover<5->{%
 < \alert<handout:0| 6-7>{\text{arc} AB \uncover<6->{ = } \uncover<7->{\theta}}%
}%
\]
\uncover<8->{%
Therefore $\alert<handout:0| 18>{\frac{\sin \theta}{\theta} < 1}$.%
}%
\abovedisplayskip=0pt
\belowdisplayskip=0pt
\begin{align*}
\uncover<9->{%
\theta = \text{arc} AB %
}%
& \uncover<10->{ < }  %
\uncover<10->{%
|AD| + \alert<handout:0| 11>{|DB|}%
}  \uncover<11->{ < }  \uncover<11->{%
|AD| + \alert<handout:0| 11>{|DE|}%
}\\%
& \uncover<12->{ = }  %
\uncover<12->{%
|AE|%
}%
\uncover<13->{%
 = |OA| \tan \theta
}  \uncover<14->{ = }  \uncover<14->{%
\tan \theta%
}%
\end{align*}
\uncover<15->{%
Therefore $\theta < \tan \theta = \frac{\sin \theta}{\cos \theta}$, so $\alert<handout:0| 17>{\cos \theta < \frac{\sin \theta}{\theta}}$.
}%

\uncover<16->{%
\abovedisplayskip=0pt
\belowdisplayskip=0pt
\[
\alert<handout:0| 17>{\cos \theta < }%
\alert<handout:0| 17-18>{\frac{\sin \theta}{\theta}}%
\alert<handout:0| 18>{ < 1}%
\]
\uncover<19->{%
\alert<handout:0| 20-21>{$\lim_{\theta\rightarrow 0}\cos \theta = \uncover<21->{1}$} and \alert<handout:0| 22-23>{$\lim_{\theta\rightarrow 0} 1 = \uncover<23->{1}$}\uncover<23->{, so by the Squeeze Theorem $\lim_{\theta \rightarrow 0^+}\frac{\sin \theta}{\theta} = 1$.}  \uncover<24->{$\frac{\sin \theta}{\theta}$ is even, so the left limit is also 1.}
}%
}%
\end{frame}

\begin{frame}
\abovedisplayskip=0pt
\belowdisplayskip=0pt
\abovedisplayshortskip=0pt
\belowdisplayshortskip=0pt
\begin{align*}
\text{Let}\quad f(x) & = \sin x. \\
\text{Then}\quad f'(x) & =  %
\uncover<1->{%
\alert<handout:0| 2-3>{\lim_{h\rightarrow 0} \sin x}\cdot \alert<handout:0| 4-5>{\lim_{h\rightarrow 0} \frac{\cos h - 1}{h}} + \alert<handout:0| 6-7>{\lim_{h\rightarrow 0}\cos x}\cdot \alert<handout:0| 8-9>{\lim_{h\rightarrow 0}  \frac{\sin h}{h}}  %
}\\%
& \uncover<2->{ = }  %
\uncover<2->{%
\uncover<3->{\alert<handout:0| 3>{ \sin x}} \uncover<5->{\cdot\alert<handout:0| 5,10>{\lim_{h\rightarrow 0} \frac{\cos h - 1}{h}}} \uncover<7->{+ \alert<handout:0| 7>{\cos x}} \uncover<9->{\cdot\alert<handout:0| 9>{1}}  %
}%
\uncover<10->{%
\intertext{We need to find}%
}%
\uncover<10->{%
\lim_{h\rightarrow 0}\frac{\cos h - 1}{h}%
}%
& \uncover<11->{ = }  %
\uncover<11->{%
\lim_{h\rightarrow 0}\left( \frac{\cos h - 1}{h} \cdot \frac{\cos h + 1}{\cos h + 1}\right)%
}  \uncover<12->{ = } \uncover<12->{%
\lim_{h\rightarrow 0} \frac{\alert<handout:0| 13>{\cos^2 h - 1}}{h(\cos  h + 1)}%
}\\%
& \uncover<13->{ = }  %
\uncover<13->{%
\lim_{h\rightarrow 0} \frac{\alert<handout:0| 13>{-\sin^2 h}}{h(\cos  h + 1)}%
}  \uncover<14->{ = } \uncover<14->{%
-\lim_{h\rightarrow 0} \left( \frac{\sin h}{h}\cdot \frac{\sin h}{\cos h + 1}\right)%
}\\%
& \uncover<15->{ = }  %
\uncover<15->{%
-\alert<handout:0| 16>{\lim_{h\rightarrow 0}  \frac{\sin h}{h}}\cdot\lim_{h\rightarrow 0} \frac{\sin h}{\cos h + 1}%
}  \uncover<16->{ = } \uncover<16->{%
-\alert<handout:0| 16>{1}\cdot \left( \frac{0}{1+1}\right)%
}  \uncover<17->{ = } \uncover<17->{%
0
}%
\end{align*}

\uncover<18->{%
\begin{theorem}[The Derivative of $\sin x$]
\[
\frac{\diff}{\diff x} \sin x = \cos x
\]
\end{theorem}
}%
\end{frame}
% end module derivative-sine
