% begin module product-rule-twice-poly-e-trig
\begin{frame}
\begin{example}[Using the Product Rule twice]
\begin{align*}
\text{Differentiate}  \quad  y &= \theta e^\theta (\tan \theta + \sec \theta) \\%
\uncover<2->{\text{Product Rule:} \quad  y' &=  \theta e^\theta \alert<handout:0|3-4>{ \frac{\diff}{\diff \theta}(\tan \theta + \sec \theta)}+ \alert<handout:0|5-6>{\frac{\diff}{\diff \theta}(\theta e^\theta )}(\tan \theta + \sec \theta)}\\%
\uncover<3->{&= \theta e^\theta \alert<handout:0|3-4>{(\uncover<4->{\sec^2 \theta + \tan \theta \sec \theta})}}\\
\uncover<3->{\uncover<6->{\text{Product Rule:} \quad \quad} & \quad + \alert<handout:0|5-6>{( \uncover<6->{\theta \alert<handout:0|7-8>{\frac{\diff}{\diff \theta}(e^\theta)} +\alert<handout:0|9-10>{\frac{\diff}{\diff \theta}(\theta)}e^\theta})}(\tan \theta + \sec \theta)}\\
\uncover<7->{&= \theta e^\theta(\sec^2 \theta + \tan \theta \sec \theta)} \\
\uncover<7->{& \quad +  (\theta \alert<handout:0|7-8>{(\uncover<8->{e^\theta})}+\alert<handout:0|9-10>{(\uncover<10->{1})}e^\theta)(\tan \theta + \sec \theta)}\\
\uncover<11->{&=  \theta e^\theta \sec \theta(\sec\theta + \tan \theta)+e^\theta( \theta +1)(\tan \theta + \sec \theta)}\\
\uncover<12->{&=(\theta\sec\theta+\theta+1)e^\theta(\tan\theta+\sec\theta).}
\end{align*}
\end{example}
\end{frame}
% end module product-rule-twice-poly-e-trig