\begin{frame}
Recall Euler substitution: $x=\frac12\left(\frac{1}{t}- t \right)$, $\alert<2>{\sqrt{x^2+1}=\frac{1}2\left(\frac 1 t +t\right)}$, $\alert<12,13,14>{ t=\sqrt{x^2+1}-x} $, $\alert<3>{ \diff x=-\frac12 \left(\frac1{t^2} +1\right)\diff t}$.
\begin{example}
$
\begin{array}{rcl}
\displaystyle \int \alert<2>{ \sqrt{x^2+1}} \alert<3>{\diff x} \vphantom{ \frac{1}{8}\left(\frac{1}{ (\sqrt{ x^2 +1} -x)^2} - (\sqrt{x^2+1}- x)^2 \right) } &=&
%vphantom below 


\displaystyle
\only<1-16>{ 
\uncover<2->{ \alert<3>{-} \int  \alert<2>{\alert<4>{\frac12} \left(\alert<5,6>{\frac1t} +\alert<7,8>{t}\right)} \alert<3>{\alert<4>{ \frac{1}{2}} \left(\alert<5,7>{ \frac 1 {t^2}} +\alert<6,8>{1} \right)\diff t}} \\
\uncover<4->{ &=&\displaystyle -\alert<4>{ \frac 1 4} \alert<9,10,11>{ \int} \left(\alert<5>{ \alert<9>{ \frac{ 1 }{ t^3}}} + \alert<6,7,10>{2\frac{1}t} + \alert<8,11>{t} \right) \alert<9,10,11>{ \diff t} } \\
\uncover<9->{&=&\displaystyle \alert<15>{-\frac{1}4} \left(\alert<9>{\alert<15>{ -}\frac{ \alert<12>{ t^{-2}}}{\alert<15>{2}}} +\alert<10>{ \alert<15>{2} \ln\alert<14>{ |t|} }+ \alert<11>{\frac{\alert<13>{ t^2}}{\alert<15>{2}}} \right)+C}\\
\uncover<12->{&=&}
}
\uncover<12->{\displaystyle \only<1-24>{  \alert<16,18,24>{ \alert<15>{\frac{1}{8}} \left(\frac{1}{\alert<12>{ (\sqrt{ x^2 +1} -x)^2}} - \alert<13>{(\sqrt{x^2+1}- x)^2} \right) } }}\only<25->{
\alert<25>{ 4x\sqrt{x^2+1}}
} {~~~~~~~~~~~~~~~~~~~~~~~~~~~~~~~~~~~~~~~~~~~~~~~~~~~~~~}  \\
\uncover<12->{ && \displaystyle \alert<16>{ \only<1-30>{\alert<15>{ -}} \only<31->{\alert<31>{+} } \alert<15>{ \frac12}  \alert<26,30>{\ln ( \alert<14>{ \sqrt{x^2+1} \only<1-30>{-}\only<31->{\alert<31>{+} } x})} +C}}
\end{array}
$

\noindent \only<17-25>{The answer is good. However, let's simplify.

\noindent 
\uncover<18->{
$
\begin{array}{l}
\phantom{=}
\displaystyle \alert<18>{ \frac{1}{(\sqrt{x^2+1}-x)^2}- (\sqrt{x^2+1 }-x)^2} \\
\uncover<19->{= \displaystyle \frac{ \alert<19>{(\sqrt{x^2+1} +x )^2} }{ ( \sqrt{x^2 +1} -x )^2  	\alert<19>{(\sqrt{x^2+1}+x)^2} } - (\sqrt{x^2+1}-x)^2} \\
\uncover<20->{ =\displaystyle \frac{(\sqrt{x^2+1}+x)^2}{ \alert<20>{ \alert<21,22>{((\sqrt{x^2 +1 } )^2 -x^2)^2}\uncover<21,22>{\alert<21,22>{=1}} } } - ( \sqrt{x^2 +1 } -x)^2} \\
= \displaystyle \uncover<22->{(\sqrt{x^2+1}+x)^2-( \sqrt{x^2 +1 } -x)^2} \uncover<23->{ = \alert<24,25>{ 4x\sqrt{x^2+1}}}
\end{array}
$
} %uncover<18->
} %only<17-25>

\only<26->{
The last expression can be transformed to:
\[
\begin{array}{rcl}
\displaystyle 
\alert<26>{\ln} \left(\frac{\alert<26,28>{(\sqrt{x^2+1}-x)} \uncover<27->{ \alert<27,28>{( \sqrt{x^2+1}+ x)}}}{\uncover<27->{ \alert<27>{ \sqrt{x^2 +1} +x}}} \right) 
&=&\displaystyle \uncover<28->{\alert<29>{ \ln \left( \frac{\alert<28>{ 1} }{ \sqrt{x^2+1}+x}\right)} }\\ \uncover<29->{&=&\alert<29,30,31>{ -\ln (\sqrt{x^2+1}+x)}}
\end{array}
\]
}
\end{example}

\vspace{8cm}
\end{frame}