%begin module Euler-substitution-case-3
\begin{frame}

\frametitle{Euler substitution to handle $\sqrt{x^2-1} $}

\begin{itemize}
\item<1-> Suppose we want to integrate 
\[
\int R(x, \sqrt{x^2-1})\diff x\quad .
\]
\only<1-14>{
\item<2-> Substitute $\alert<14>{\sqrt{x^2-1}=}(\alert<10>{x}-1)t\uncover<10->{= \left(\alert<10>{ 1+\frac{2}{t^2-1}} -1\right)t =\alert<14>{\frac{2t}{t^2-1}} .}$ 
\item<3-> How is this a substitution of $x$ via $t$? 
\[
\begin{array}{rcll|l}
\uncover<4->{\sqrt{x^2-1}&=&(x-1)t&&\text{square}}\\
\uncover<5->{(x-1)(x+1)  &=&(x-1)^2t^2&&  \text{divide by } x-1} \\
\uncover<6->{x+1 &=&(x-1)t^2}\\
\uncover<7->{x(t^2-1) &=&1+t^2}\\
\uncover<8->{\alert<10,11,14>{x}&\alert<10,11,14>{=}&\displaystyle \frac{t^2\uncover<9->{-1+1}+1}{t^2-1} \uncover<9->{=\alert<10,11, 14>{1+\frac{2}{t^2-1}}}}
\end{array}
\]
\item<11->
\[
\alert<11>{ \alert<14>{\diff x=} \alert<12,13>{\diff \left(1+\frac{2}{t^2-1} \right)}} \uncover<12->{\alert<12,13>{=}} \only<12>{\alert<12>{\textbf{?}}} \uncover<13->{\alert<13,14>{\frac{-4t}{(t^2-1)^2}\diff t} .} {~~~~~~~~~~~~~~~~~~~~~~~~~~~~~~~~~~~~~~~~~~~~~~~~}
\] 
}
\end{itemize}
\uncover<15->{
\begin{definition}
\[
\begin{array}{rcl}
\displaystyle \alert<15>{\sqrt{-x^2+1}}&\alert<15>{=}&\displaystyle \alert<15>{\frac{2t}{t^2-1} }\\
\displaystyle \alert<15>{x}&\alert<15>{=}&\displaystyle \alert<15>{ 1+\frac{2} {t^2-1} }\\
\displaystyle \alert<15>{\diff x}&\alert<15>{=}&\displaystyle \alert<15>{ \frac{-4t }{(t^2-1 )^2}dt }\quad .
\end{array}
\] 
\end{definition}
}
\vspace{5cm}
\end{frame}
%end module Euler-substitution-case-3