%end module integral-radical-x-squared-plus-one
\begin{frame}
Recall Euler substitution: $x=\frac12\left(\frac{1}{t}- t \right)$, $\alertNoH{2}{\sqrt{x^2+1}=\frac{1}2\left(\frac 1 t +t\right)}$, $\alertNoH{12,13,14}{ t=\sqrt{x^2+1}-x} $, $\alertNoH{3}{ \diff x=-\frac12 \left(\frac1{t^2} +1\right)\diff t}$.
\begin{example}
$
\begin{array}{rcl}
\displaystyle \int \alertNoH{2}{ \sqrt{x^2+1}} \alertNoH{3}{ \diff x} \vphantom{ \frac{1}{8}\left(\frac{1}{ (\sqrt{ x^2 +1} -x)^2} - (\sqrt{x^2+1}- x)^2 \right) } &=&
\displaystyle
\only<1-16>{
\uncover<2->{ \alertNoH{3}{-} \int  \alertNoH{2}{\alertNoH{4 }{ \frac12} \left(\alertNoH{5,6}{\frac1t} +\alertNoH{7,8}{t}\right)} \alertNoH{3}{\alertNoH{4}{ \frac{1}{2}} \left(\alertNoH{5,7}{ \frac 1 {t^2}} +\alertNoH{6,8}{1} \right)\diff t}} \\
\uncover<4->{ &=&\displaystyle -\alertNoH{4}{ \frac 1 4} \alertNoH{9,10,11}{ \int} \left(\alertNoH{5}{ \alertNoH{9}{ \frac{ 1 }{ t^3}}} + \alertNoH{6,7,10}{2\frac{1}t} + \alertNoH{8,11}{t} \right) \alertNoH{9,10,11}{ \diff t} } \\
\uncover<9->{&=&\displaystyle \alertNoH{15}{-\frac{1}4} \left( \alertNoH{9}{ \alertNoH{15}{ -}\frac{ \alertNoH{12}{ t^{-2}}}{\alertNoH{15}{2}}} +\alertNoH{10}{ \alertNoH{15}{2} \ln\alertNoH{14}{ |t|} }+ \alertNoH{11}{\frac{\alertNoH{13}{ t^2}}{\alertNoH{15}{2}}} \right)+C}\\
\uncover<12->{&=&}
}
\uncover<12->{\displaystyle \only<1-24>{  \alertNoH{16,17,24}{ \alertNoH{15}{\frac{1}{8}} \alertNoH{18}{\left(\frac{1}{\alertNoH{12}{ (\sqrt{ x^2 +1} -x)^2}} - \alertNoH{13}{\left(\sqrt{x^2+1}- x\right)^2} \right)} } }}\only<25->{
\alertNoH{25}{ \frac{1}{2}x\sqrt{x^2+1}}
} {~~~~~~~~~~~~~~~~~~~~~~~~~~~~~~~~~~~~~~~~~~~~~~~~~~~~~~}  \\
\uncover<12->{ && \displaystyle \alertNoH{16,17}{ \only<1-30>{ \alertNoH{15}{ -}} \only<31->{\alertNoH{31}{+} } \alertNoH{15}{ \frac12}  \alertNoH{26,30}{\ln \left( \alertNoH{ 14}{ \sqrt{x^2+1} \only<1-30>{-}\only<31->{ \alertNoH{ 31}{ +} } x} \right)} +C}}
\end{array}
$

\noindent \only<17-25>{The answer is good. However, let's simplify.

\noindent
\uncover<18->{
$
\begin{array}{l}
\phantom{=}
\displaystyle \alertNoH{18}{ \frac{1}{(\sqrt{x^2+1}-x)^2}- \left( \sqrt{ x^2+1 }-x\right)^2} \\
\uncover<19->{= \displaystyle \frac{ \alertNoH{19}{ ( \sqrt{ x^2 + 1} +x )^2} }{\alertNoH{20}{ ( \sqrt{x^2 +1} -x )}^2  	\alertNoH{19}{\alertNoH{20}{(\sqrt{x^2+1}+x)}^2} } - \left( \sqrt{ x^2+1}-x\right)^2} \\
\uncover<20->{ =\displaystyle \frac{(\sqrt{x^2+1}+x)^2}{  \alertNoH{21,22}{\alertNoH{20}{((\sqrt{x^2 +1 } )^2 -x^2 )}^2 } \uncover<21,22>{\alertNoH{21,22}{=1}}  } - \left( \sqrt{x^2 +1 } -x \right)^2} \\
\displaystyle \uncover<22->{=\left(\sqrt{x^2+1}+x\right)^2-\left( \sqrt{ x^2 + 1 } -x\right)^2} \uncover<23->{ = \alertNoH{24,25}{ 4x\sqrt{x^2+1}}}
\end{array}
$
} %uncover<18->
} %only<17-25>

\only<26->{
The last expression can be transformed to:
\[
\begin{array}{rcl}
\displaystyle
\alertNoH{26}{\ln} \left(\frac{\alertNoH{26,28}{\left(\sqrt{x^2+1}-x\right)} \uncover<27->{ \alertNoH{27,28}{\left( \sqrt{x^2+1}+ x \right)} }}{ \uncover<27->{ \alertNoH{27}{ \sqrt{x^2 +1} +x}}} \right)
&=& \displaystyle \uncover<28->{\alertNoH{29}{ \ln \left( \frac{\alertNoH{28}{ 1} }{ \sqrt{x^2+1}+x}\right)} }\\ \uncover<29->{&=&\alertNoH{29,30,31}{ -\ln \left( \sqrt{x^2 + 1} +x\right)}}
\end{array}
\]
}
\end{example}

\vspace{8cm}
\end{frame}
%end module integral-radical-x-squared-plus-one
