%begin module quadratic-radicals-linear-substitution-preparation-ex2
\begin{frame}
Recall: linear substitution is subst. of the form $u=px+q$.
\begin{example}
Use linear subst. to transform $\sqrt{-2x^2+x+1}$ to multiple of $\sqrt{-u^2+1}$. 

\noindent 
$
\begin{array}{rcl}
\sqrt{\alert<2>{ -2}x^2+x+\alert<2>{1}}&=& \uncover<2->{ \sqrt{ \alert<2>{-2}\left(x^2\alert<2>{-\frac{1}{2}}x \alert<2>{-\frac{1}{2}}\right) }} \\
&=& \sqrt{ -2\left(x^2-2\frac{1}{4}x +\frac{1}{16}-\frac{1}{16}-\frac{1}{2}\right) }\\
&=&\sqrt{-2\left(\left(x-\frac{1}{16}\right)^2-\frac{9}{16} \right)}\\
&=&\sqrt{\frac{9}{8}\left(-\frac{16}{9}\left(x-\frac{1}{16}\right)^2+1 \right)}\\
&=&\frac{3}{\sqrt{8}}\sqrt{-\left(\frac{4}{3}\left(x-\frac{1}{16}\right)\right)^2+1 }\\
&=&\frac{ 3}{\sqrt{8}} \sqrt{-u^2+1},
\end{array}
$

\noindent where $u=\frac{4}{3}\left(x-\frac{1}{16}\right)  \textbf{?}=\frac{4}{3}x-\frac{1}{12}$.
\end{example}
\end{frame}
%end module quadratic-radicals-linear-substitution-preparation-ex2