\begin{frame}

\frametitle{Trigonometric substitution $x=\cos \theta$ for $\sqrt{-x^2+1}$}
The trigonometric substitution $\alertNoH{2}{x=\cos \theta}$, $\theta\in \left[0, \pi\right] $ for $\sqrt{-x^2+1} $:
\[
\begin{array}{rclll}
\displaystyle { \sqrt{-x^2+1}}&{=}&\displaystyle \uncover<2->{ \sqrt{\alertNoH{3}{1-{\alertNoH{2}{\cos}}^2\alertNoH{2}{\theta}}}}\\
\uncover<3->{&=&\displaystyle  \sqrt{\alertNoH{3}{ \sin^2\theta} } } \uncover<4->{&&\begin{array}{|l} \text{when }\theta\in\left[0,\pi \right] \text{we have}\\
\sin \theta\geq 0 \text{ and so } \sqrt{\sin^2\theta}=\sin \theta
\end{array}} \\
\uncover<3->{&=&}
\uncover<3->{\displaystyle \sin \theta\quad .}
\end{array}
\]
\uncover<4->{
To summarize:
\begin{definition}
The trigonometric substitution $ x=\cos \theta$, $\theta\in [0,\pi]$ for $\sqrt{-x^2+1} $ is given by:
\[\begin{array}{rcl}
x&=&\cos \theta\\
\sqrt{-x^2+1}&=&\sin \theta\\
\diff x&=& -\sin \theta \diff \theta\\
\theta&=&\arccos x \quad .
\end{array}
\]
\end{definition}
}
\end{frame}
