% begin module trig-substitution-ex7
\begin{frame}
\begin{example}[Example 7, p. 507]
Evaluate $\int \frac{x}{\sqrt{3-2x-x^2}}\diff x$.
\begin{itemize}
\item<2->  Complete the square under the root sign:
\item<3-| alert@38>  $\uncover<3->{%
3 - 2x - x^2 = %
}% 
\uncover<4->{%
3 \uncover<5->{\alert<handout:0| 5>{ + 1 }} - (x^2 + 2x \uncover<5->{\alert<handout:0| 5>{ + 1}})  = %
}% 
\uncover<6->{%
4 - (x + 1)^2%
}$
\item<7->  Substitute \alert<handout:0| 8-9,17,39>{$u = \uncover<9->{x+1}$}.  Then \alert<handout:0| 10-11,16>{$\diff u = \uncover<11->{\diff x}$} and \alert<handout:0| 12-13,15>{$x = \uncover<13->{u - 1}$}.
\item<7-| alert@27>  $\int \frac{x}{\sqrt{3 - 2x - x^2}}\diff x = \int \frac{\alert<handout:0| 15>{x}}{\sqrt{4 - \alert<handout:0| 17>{(x+1)^2}}}\alert<handout:0| 16>{\diff x} = \uncover<14->{\int \frac{\alert<handout:0| 15>{u-1}}{\sqrt{4 - \alert<handout:0| 17>{u^2}}}\alert<handout:0| 16>{\diff u}}$
\item<18->  Let \alert<handout:0| 19-20,23,29,36>{$u = \uncover<20->{2\sin \theta}$}\uncover<20->{, where \alert<handout:0| 26>{$-\pi /2 \leq \theta \leq \pi / 2$}.}  Then \alert<handout:0| 21-22,30>{$\diff u = \uncover<22->{2\cos \theta\diff \theta}$}\uncover<22->{.}
\item<18->  $\uncover<18->{%
\alert<handout:0| 31,35>{%
\sqrt{4 - \alert<handout:0| 23>{u^2}} = 
}%
}%
\uncover<23->{%
\sqrt{4 - \alert<handout:0| 23>{4\sin^2 \theta}} = 
}%
\uncover<24->{%
\sqrt{4 \cos^2 \theta} = 
}%
\uncover<25->{%
2 |\cos  \theta | = 
}%
\uncover<26->{%
\alert<handout:0| 31,35>{%
2 \cos  \theta  
}%
}$%
\end{itemize}
%\abovedisplayskip=0pt
%\belowdisplayskip=0pt
\[
\begin{array}{l}
\uncover<27->{%
\ \ \int \frac{x}{\sqrt{3-2x-x^2}}\diff x%
}%
 \uncover<27->{ = }  %
\uncover<27->{%
\int\frac{\alert<handout:0| 29>{u} - 1}{\alert<handout:0| 31>{\sqrt{4-u^2}}}\alert<handout:0| 30>{ \diff u}%
}%
\uncover<28->{%
 = \int\frac{\alert<handout:0| 29>{2\sin \theta} - 1}{\alert<handout:0| 31>{2\cos \theta}}\alert<handout:0| 30>{ 2\cos \theta\diff \theta}%
}\\%
 \uncover<32->{ = }  %
\uncover<32->{%
 \int (2\sin \theta  - 1)\diff \theta
}  \uncover<33->{ = }  \uncover<33->{%
 -\alert<handout:0| 35>{2\cos \theta} - \alert<handout:0| 36>{\theta} + C
}\\
 \uncover<34->{ = } \uncover<34->{%
 -\alert<handout:0| 35>{\sqrt{\alert<handout:0| 38>{4-u^2}}} - \alert<handout:0| 36>{\sin^{-1}\left( \frac{\alert<handout:0| 39>{u}}{2}\right)} + C
}\\%
 \uncover<37->{%
 = } %
\uncover<37->{%
 -\sqrt{\alert<handout:0| 38>{3-2x-x^2}} - \alert<handout:0| 36>{\sin^{-1}\left( \frac{\alert<handout:0| 39>{x+1}}{2}\right)} + C
}%
\end{array}
\]
\end{example}
\end{frame}
% end module trig-substitution-ex7
