\solution{\ref{problemLHospital (sin (pi x) ln x )/ (cos pi x +1)}
The limit is of the form ``$\frac{0}{0}$'' so we are allowed to use L'Hospital's rule.
\[
\begin{array}{rcll|l}
\displaystyle
\lim\limits_{x\to 1} \frac{\sin \left(\pi x\right)\ln x }{\cos(\pi x)+1 } &=&\displaystyle \lim\limits_{x\to 1}  \frac{\left(\sin \left(\pi x\right)\ln x\right)' }{\left(\cos(\pi x)+1\right)' }\\
&=&\displaystyle \lim\limits_{x\to 1}  \frac{\left(\pi \cos \left(\pi x\right)\ln x+ \sin\left(\pi x\right)\frac{1}{x}\right) }{\left(-\pi\sin(\pi x)\right) } &&\text{type ``$\frac{0}{0}$'',  L'Hospital's rule}\\
&=&\displaystyle \lim\limits_{x\to 1}  \frac{\left(\pi \cos \left(\pi x\right)\ln x+ \sin\left(\pi x\right)\frac{1}{x}\right)' }{\left(-\pi\sin(\pi x)\right)' } \\
&=&\displaystyle \lim\limits_{x\to 1}  \frac{- \pi^{2} \sin{}\left(\pi x\right) \ln{}\left(x\right)+2 \pi \cos{}\left(\pi x\right) x^{-1}- \sin{}\left(\pi x\right) x^{-2} }{\left(-\pi^2\cos(\pi x)\right) } \\
&=&\displaystyle  \frac{- \pi^{2} \sin{}\left(\pi \right) \ln(1)+2 \pi \cos{}\left(\pi \right) - \sin{}\left(\pi \right)  }{\left(-\pi^2\cos(\pi )\right) } \\
&=&\displaystyle -\frac{2}{\pi}\quad .
\end{array}
\]
}