\solution{\ref{problemLHospital (sin (pi x) ln x )/ (cos pi x +1)}
The limit is of the form ``$\frac{0}{0}$'' so we are allowed to use L'Hospital's rule.
\[
\begin{array}{rcll|l}
\displaystyle
\lim\limits_{x\to 1} \frac{\sin \left(\pi x\right)\ln x }{\cos(\pi x)+1 } &=&\displaystyle \lim\limits_{x\to 1}  \frac{\left(\sin \left(\pi x\right)\ln x\right)' }{\left(\cos(\pi x)+1\right)' }\\
&=&\displaystyle \lim\limits_{x\to 1}  \frac{\left(\pi \cos \left(\pi x\right)\ln x+ \sin\left(\pi x\right)\frac{1}{x}\right) }{\left(-\pi\sin(\pi x)\right) } &&\text{type ``$\frac{0}{0}$'',  L'Hospital's rule}\\
&=&\displaystyle \lim\limits_{x\to 1}  \frac{\left(\pi \cos \left(\pi x\right)\ln x+ \sin\left(\pi x\right)\frac{1}{x}\right)' }{\left(-\pi\sin(\pi x)\right)' } \\
&=&\displaystyle \lim\limits_{x\to 1}  \frac{- \pi^{2} \sin{}\left(\pi x\right) \ln{}\left(x\right)+2 \pi \cos{}\left(\pi x\right) x^{-1}- \sin{}\left(\pi x\right) x^{-2} }{\left(-\pi^2\cos(\pi x)\right) } \\
&=&\displaystyle  \frac{- \pi^{2} \sin{}\left(\pi \right) \ln(1)+2 \pi \cos{}\left(\pi \right) - \sin{}\left(\pi \right)  }{\left(-\pi^2\cos(\pi )\right) } \\
&=&\displaystyle -\frac{2}{\pi}\quad .
\end{array}
\]
}
\solution{
\ref{problemlim x to 0 (sin x - x)/(arctan x - x)}
\noindent \textbf{Solution I.} 
\[
\begin{array}{rcll|l}
\displaystyle \lim\limits_{x\to 0}\frac{\sin x- x}{\Arctan x -x}&=&\displaystyle \lim\limits_{x\to 0} \frac{\cos x -1 }{ \frac{1}{1+x^2}-1 } &&\text{L'Hospital rule}\\
&=&\displaystyle \lim\limits_{x\to 0}\frac{-\sin x }{\frac{ -2x}{(1+x^2)^2} }&& \text{L'Hospital rule again}\\
&=&\displaystyle \lim\limits_{x\to 0} \frac{(1+x^2)^2}{2}\frac{\sin x}{x}  \\
&=&\displaystyle \lim\limits_{x\to 0} \frac{(1+x^2)^2}{2}\lim\limits_{x\to 0}\frac{\sin x}{x} \\
&=&\displaystyle \frac{1}{2}\quad .
\end{array}
\] 
}

\noindent \textbf{Solution II.}
\[
\begin{array}{rcll|l}
\displaystyle \lim\limits_{x\to 0}\frac{\sin x- x}{\Arctan x -x}&=&\displaystyle \lim\limits_{x\to 0} \frac{\left( x-\frac{x^3}{3!}+\frac{x^5}{5!}-\dots\right) -x}{\left( x-\frac{x^3}{3}+\frac{x^5}{5}-\dots\right)-x} &&\text{use the Maclaurin series of }\sin, \Arctan \\
&=&\displaystyle \lim\limits_{x\to 0}\frac{- \frac{x^3 }{6} + x^5\left(\frac{1}{5!}-\dots\right) }{- \frac{ x^3}{3} + x^5 \left(\frac{1}{5}-\dots \right)  }&& \begin{array}{rcl}
\text{The expressions in parenthesis }\\
\text{are continous functions in x }
\end{array}\\
&=&\displaystyle \lim\limits_{x\to 0} \frac{-\frac{1}{6}+ x^2 \left(\frac{1}{5!}-\dots\right) }{- \frac{1}{3} +x^2 \left( \frac{1}{5}-\dots \right)  }\\
&=&\displaystyle \frac{-\frac{1}{6}+0}{\frac{1}{3}+0}\\
&=&\displaystyle \frac{1}{2}\quad .
\end{array}
\] 

\solution{\ref{problemlimxtoinftysin(2/x)}.
\[
\begin{array}{rcll|l}
\displaystyle \lim_{x\to\infty }x\sin\left( \frac{2}{x} \right)& =&\displaystyle \lim_{x \to \infty} \frac{\sin \left(\frac{2}{x}\right) }{ \frac{ 1}{x}}
 &&\begin{array}{l}
\text{indeterminate form }\\
\text{Use L'Hospital's rule}
\end{array}\\
&=&\displaystyle \lim_{x \to \infty} \frac{\cos\left(\frac{2}{x}\right) \left (-\frac{2}{x^2}\right)}{-\frac{1}{x^2}} \\ 
&=&\displaystyle \lim_{x \to \infty} 2 \cos\left(\frac{x}{2}\right) \\
&=&\displaystyle 2\quad .
\end{array}
\]
}

