Evaluate the difference quotient and simplify your answer. 
\begin{multicols}{2}
\begin{enumerate}[ref={\fcProblemRef}]
\item $\displaystyle \frac{f(2+h)-f(2)}{h}$, where $f(x)=x^2-x-1$.

\answer{$ h+3 $}
\item $\displaystyle \frac{f(a+h)-f(a)}{h}$, where $f(x)= x^2$.

\answer{$ h+2 a  $}
\item $\displaystyle \frac{f(a+h)-f(a)}{h}$, where $f(x)= x^3$.

\answer{$h^{2}+3 a^{2}+3 a h  $}
\item $\displaystyle \frac{f(a+h)-f(a)}{h}$, where $f(x)= x^4$.

\answer{$ 6 a^{2} h+4 a h^{2}+h^{3}+4 a^{3}$}
\item $\displaystyle \frac{f(x)-f(a)}{x-a}$, where $f(x)=\frac{1}{x}$.

\answer{$-\frac{1}{ax}$.}
\item $\displaystyle \frac{f(x)-f(1)}{x-1}$, where $f(x)=\frac{x-1}{x+1}$.

\answer{$\frac{1}{x+1}$.}
\end{enumerate}
\end{multicols}
