Compute the expressions $(f\circ g)(x)$, $(g\circ f)(x)$ and simplify to a single fraction. 

\begin{enumerate}
\item $\displaystyle f{}({{x}})=\frac{x+2}{x-2},
g{}({{x}})=\frac{x-1}{x+2}$.

\answer{$(f\circ g)(x)= \frac{3+3 x}{-5- x}$, $(g\circ f)(x)=\frac{4}{-2+3 x}$  }
\item 
$\displaystyle f{}({{x}})=\frac{x+1}{3x-2},
g{}({{x}})=\frac{x-2}{x-1}
$.

\answer{
$(f\circ g)(x)= \frac{-3+2 x}{-4+x}
$, 
$(g\circ f)(x)=\frac{5-5 x}{3-2 x}
$  }
\item 
$\displaystyle f{}({{x}})=\frac{2x+1}{3x-1},
g{}({{x}})=\frac{x-2}{2x-1}
$.

\answer{
$(f\circ g)(x)=\frac{-5+4 x}{-5+x}
$, 
$(g\circ f)(x)=\frac{3-4 x}{3+x}
$  }
\item 
$\displaystyle f{}({{x}})=\frac{x+1}{x-2},
g{}({{x}})=\frac{x+2}{2x-1}
$.

\answer{
$(f\circ g)(x)= \frac{1+3 x}{4-3 x}
$, 
$(g\circ f)(x)=\frac{-3+3 x}{4+x}
$  }
\item 
$\displaystyle f{}({{x}})=\frac{5x+1}{4x-1},
g{}({{x}})=\frac{4x-1}{3x+1}
$.

\answer{
$(f\circ g)(x)= \frac{-4+23 x}{-5+13 x}
$, 
$(g\circ f)(x)=\frac{5+16 x}{2+19 x}
$  }
\item $\displaystyle  f(x)= \frac{3x-5}{x-2}$, $\displaystyle g(y)=\frac{y-2 }{y-4} $. 

\answer{ $(f\circ g)(x)=\frac{-2 x+14}{- x+6}$, $(g\circ f)(x)=\frac{x-1}{- x+3}$}
\item $\displaystyle  f(x)= \frac{x-3}{x+2}$, $\displaystyle g(y)=\frac{y+3 }{y-4} $. 

\answer{ $(f\circ g)(x)=\frac{-2 (x)+15}{3 x-5}$, $(g\circ f)(x)=\frac{4 x+3}{-3 x-11}$}
\end{enumerate}
