% begin module chain-rule-general-exponential.tex
\begin{frame}
\begin{example}[Chain Rule, general exponential function]
\abovedisplayskip=0pt
\belowdisplayskip=0pt
\abovedisplayshortskip=0pt
\belowdisplayshortskip=0pt
\begin{align*}
\text{Differentiate}\quad y & = \alert<handout:0|2-3>{2}^x.\\
\uncover<2->{y} & \uncover<2->{= \alert<handout:0|2-3>{( e^{\uncover<3->{\ln 2}} )}^x}\\
\uncover<4->{y} & \uncover<4->{= e^{x\ln 2}.}\\
\uncover<5->{\text{Let} \quad \alert<handout:0|5-6>{\alert<handout:0|13-14>{\alert<handout:0|11-12>{u}}} &\alert<handout:0|5-6>{\alert<handout:0|11-14>{=}} \uncover<6-| handout:0>{\alert<handout:0|6>{\alert<handout:0|11-12>{\alert<handout:0|13-14>{ x\ln 2.}}}}} \\
\uncover<7->{\text{Then} \quad \alert<handout:0|9-10>{y} &\alert<handout:0|9-10>{= \uncover<7-| handout:0>{e^u.}}} \\
\uncover<8->{\text{Chain Rule:}\quad \frac{\diff y}{\diff x} &= \alert<handout:0|9-10>{ \frac{\diff y}{\diff u}}\alert<handout:0|11-12>{ \frac{\diff u}{\diff x}}}\\
\uncover<9->{&= \alert<handout:0|9-10>{(\uncover<10-| handout:0>{e^{\alert<handout:0|13-14>{u}}})}\alert<handout:0|11-12>{(\uncover<12-| handout:0>{\ln 2})} }\\
\uncover<13->{ &=} \uncover<13-| handout:0>{(e^{\alert<handout:0|13-14>{(\uncover<14->{x\ln2})}})(\ln 2)}\\
\uncover<15->{& =} \uncover<15-| handout:0>{(e^{\ln 2})^x(\ln 2)}\\
\uncover<16->{& =} \uncover<16-| handout:0>{2^x\ln 2.} 
\end{align*}
\end{example}
\end{frame}
% begin module chain-rule-general-exponential.tex
